@prefix dcat: <http://www.w3.org/ns/dcat#> .
@prefix dcterms: <http://purl.org/dc/terms/> .
@prefix ns1: <https://owaspsamm.org/model/> .
@prefix owl: <http://www.w3.org/2002/07/owl#> .
@prefix rdfs: <http://www.w3.org/2000/01/rdf-schema#> .
@prefix skos: <http://www.w3.org/2004/02/skos/core#> .
@prefix xsd: <http://www.w3.org/2001/XMLSchema#> .

ns1: a owl:Ontology ;
    dcterms:creator <mailto:robipolli@gmail.com> ;
    dcterms:description "OWASP SAMM Ontology" ;
    dcterms:license <https://creativecommons.org/licenses/by-sa/4.0/> .

ns1:0082a76b1a3744d9ab0443bd2168e13d a ns1:Activity ;
    rdfs:label "Define basic security metrics" ;
    dcterms:description """Define and document metrics to evaluate the effectiveness and efficiency of the application security program. This way improvements are measurable and you can use them to secure future support and funding for the program. Considering the dynamic nature of most development environments, metrics should be comprised of measurements in the following categories

* `Effort` metrics measure the effort spent on security. For example training hours, time spent performing code reviews, and number of applications scanned for vulnerabilities.
* `Result` metrics measure the results of security efforts. Examples include number of outstanding patches with security defects and number of security incidents involving application vulnerabilities.
* `Environment` metrics measure the environment where security efforts take place. Examples include number of applications or lines of code as a measure of difficulty or complexity.

Each metric by itself is useful for a specific purpose, but a combination of two or three metrics together helps explain spikes in metrics trends. For example, a spike in a total number of vulnerabilities may be caused by the organization on-boarding several new applications that have not been previously exposed to the implemented application security mechanisms. Alternatively, an increase in the environment metrics without a corresponding increase in the effort or result could be an indicator of a mature and efficient security program.

While identifying metrics, it’s always recommended to stick to the metrics that meet several criteria

* Consistently Measured
* Inexpensive to gather
* Expressed as a cardinal number or a percentage
* Expressed as a unit of measure

Document metrics and include descriptions of best and most efficient methods for gathering data, as well as recommended methods for combining individual measures into meaningful metrics. For example, a number of applications and a total number of defects across all applications may not be useful by themselves but, when combined as a number of outstanding high-severity defects per application, they provide a more actionable metric.
""" ;
    dcterms:identifier "0082a76b1a3744d9ab0443bd2168e13d" ;
    rdfs:comment "Define metrics with insight into the effectiveness and efficiency of the Application Security Program." ;
    rdfs:seeAlso <https://owaspsamm.org/model/governance/strategy-and-metrics/stream-b> ;
    skos:altLabel "G-SM-1-B" ;
    ns1:benefit "Basic insights into your AppSec program's effectiveness and efficiency" ;
    ns1:hasPracticeLevel ns1:4e54705272fa4f1f9977b1f9011f585d ;
    ns1:hasStream ns1:2f1cac3c2e724823b3b48a7e797520b4 .

ns1:05073fb130c74143a12a6ba74a44c580 a ns1:Activity ;
    rdfs:label "Customize security training" ;
    dcterms:description """Conduct instructor-led or CBT security training specific to the organization’s roles and technologies, starting with the core development team. The organization customizes training for product managers, software developers, testers, and security auditors, based on each group’s technical needs.

- Product managers train on topics related to SAMM business functions and security practices, with emphasis on security requirements, threat modeling, and defect tracking.
- Developers train on coding standards and best practices for the technologies they work with to ensure the training directly benefits application security. They have a solid technical understanding of the OWASP Top 10 vulnerabilities, or similar weaknesses relevant to the technologies and frameworks used (e.g. mobile), and the most common remediation strategies for each issue.
- Testers train on the different testing tools and best practices for technologies used in the organization, and in tools that identify security defects.
- Security auditors train on the software development lifecycle, application security mechanisms used in the organization, and the process for submitting security defects for remediation.
- Security Champions train on security topics from various phases of the SDLC. They receive the same training as developers and testers, but also understand threat modeling and secure design, as well as security tools and technologies that can be integrated into the build environment.

Include all training content from the Maturity Level 1 activities of this stream and additional role-specific and technology-specific content. Eliminate unnecessary aspects of the training.

Ideally, identify a subject-matter expert in each technology to assist with procuring or developing the training content and updating it regularly. The training consists of demonstrations of vulnerability exploitation using intentionally weakened applications, such as WebGoat or Juice Shop. Include results of the previous penetration as examples of vulnerabilities and implemented remediation strategies. Ask a penetration tester to assist with developing examples of vulnerability exploitation demonstrations.

Training is mandatory for all employees and contractors involved with software development, and includes an auditable sign-off to demonstrate compliance.  Whenever possible, training should also include a test to ensure understanding, not just compliance.  Update and deliver training annually to include changes in the organization, technology, and trends. Poll training participants to evaluate the quality and relevance of the training. Gather suggestions of other information relevant to their work or environments.
""" ;
    dcterms:identifier "05073fb130c74143a12a6ba74a44c580" ;
    rdfs:comment "Offer technology and role-specific guidance, including security nuances of each language and platform" ;
    rdfs:seeAlso <https://owaspsamm.org/model/governance/education-and-guidance/stream-a> ;
    skos:altLabel "G-EG-2-A" ;
    ns1:benefit "Relevant employee roles trained according to their specific role" ;
    ns1:hasPracticeLevel ns1:e8de5ea176cc455bba89f0e2d1ea1f16 ;
    ns1:hasStream ns1:7344f4b153314dd8965361d23772aef1 .

ns1:05a3e75c6c654ae58a115cbf4295662b a ns1:Activity ;
    rdfs:label "Verify the integrity of deployment artifacts" ;
    dcterms:description """Take advantage of binaries being signed at the build time and include automatic verification of the integrity of software being deployed by checking their signatures against trusted certificates. This may include binaries developed and built in-house, as well as third-party artifacts. Do not deploy artifacts if their signatures cannot be verified, including those with invalid or expired certificates.

If the list of trusted certificates includes third-party developers, check them periodically, and keep them in line with the organization’s wider governance surrounding trusted third-party suppliers.

Manually approve the deployment at least once during an automated deployment. Whenever a human check is significantly more accurate than an automated one during the deployment process, go for this option.
""" ;
    dcterms:identifier "05a3e75c6c654ae58a115cbf4295662b" ;
    rdfs:comment "Automatically verify integrity of all deployed software, indenendently on whether it's internally or externally developed." ;
    rdfs:seeAlso <https://owaspsamm.org/model/implementation/secure-deployment/stream-a> ;
    skos:altLabel "I-SD-3-A" ;
    ns1:benefit "Assured integrity of artifacts being deployed to production" ;
    ns1:hasPracticeLevel ns1:fc5eb251c6ee4f3db04eb01b62d380ba ;
    ns1:hasStream ns1:9ec70d6f7ddb4cb6b37928f9994c6049 .

ns1:0721d5bd5d67479991b5b52f33dcd7b1 a ns1:Activity ;
    rdfs:label "Practice best-effort patching" ;
    dcterms:description """Identify applications and third-party components which need to be updated or patched, including underlying operating systems, application servers, and third-party code libraries.

At this level of maturity, your identification and patching activities are best-effort and _ad hoc_, without a managed process for tracking component versions, available updates, and patch status. However, high-level requirements for patching activities (e.g., testing patches before pushing to production) may exist, and product teams are achieving best-effort compliance with those requirements.

Except for critical security updates (e.g., an exploit for a third-party component has been publicly released), teams leverage maintenance windows established for other purposes to apply component patches. For software developed by the organization, component patches are delivered to customers and organization-managed solutions only as part of feature releases.

Teams share their awareness of available updates, and their experiences with patching, on an _ad hoc_ basis. Ensure teams can determine the versions of all components in use, to evaluate whether their products are affected by a security vulnerability when notified. However, the process for generating and maintaining component lists may require significant analyst effort.
""" ;
    dcterms:identifier "0721d5bd5d67479991b5b52f33dcd7b1" ;
    rdfs:comment "Perform best-effort patching of system and application components." ;
    rdfs:seeAlso <https://owaspsamm.org/model/operations/environment-management/stream-b> ;
    skos:altLabel "O-EM-1-B" ;
    ns1:benefit "Mitigation of well-known issues in third-party components" ;
    ns1:hasPracticeLevel ns1:8cb942eff46d41f38e6edc11849744a6 ;
    ns1:hasStream ns1:1a7ad26d9e48411e95a63be79e1b90ea .

ns1:09f4b814a3444b329a7c9c7f54152ffe a ns1:Activity ;
    rdfs:label "Develop test procedures" ;
    dcterms:description """To assist with the ongoing implementation and verification of compliance with policies and standards, develop application security and appropriate test scripts related to each applicable requirement. Organize these documents into libraries and make them available to all application teams in formats most conducive for inclusion into each application. Clearly label the documents and link them to the policies and standards they represent, to assist with the ongoing updates and maintenance. Version policies and standards and include detailed change logs with each iterative update to make ongoing inclusion into different products’ SDLC easier.

Write application security requirements in a format consistent with the existing requirements management processes. You may need more than one version catering to different development methodologies or technologies. The goal is to make it easy for various product teams to incorporate policies and standards into their existing development life-cycles needing minimal interpretation of requirements.

Test scripts help reinforce application security requirements through clear expectations of application functionality, and guide automated or manual testing efforts that may already be part of the development process. These efforts not only help each team establish the current state of compliance with existing policies and standards, but also ensure compliance as applications continue to change.
""" ;
    dcterms:identifier "09f4b814a3444b329a7c9c7f54152ffe" ;
    rdfs:comment "Develop security requirements applicable to all applications." ;
    rdfs:seeAlso <https://owaspsamm.org/model/governance/policy-and-compliance/stream-a> ;
    skos:altLabel "G-PC-2-A" ;
    ns1:benefit "Common understanding of how to reach compliance with security policies for product teams" ;
    ns1:hasPracticeLevel ns1:2a29c1f7d6954785b8d42d637a752f94 ;
    ns1:hasStream ns1:c404aa4f711e4f4e9e71faea22f7fb5c .

ns1:0f611af10f974da497e7f3defe0c4f12 a ns1:Activity ;
    rdfs:label "Assess application architecture" ;
    dcterms:description """Create a view of the overall architecture and examine it for the correct provision of general security mechanisms such as authentication, authorization, user and rights management, secure communication, data protection, key management and log management. Also consider the support for privacy. Do this based on project artifacts such as architecture or design documents, or interviews with business owners and technical staff. Also consider the infrastructure components - these are all the systems, components and libraries (including SDKs) that are not specific to the application, but provide direct support to use or manage the application(s) in the organisation.

Note any security-related functionality in the architecture and review its correct provision. Do this in an ad-hoc manner, from the point of view of anonymous users, authorized users, and specific application roles.
""" ;
    dcterms:identifier "0f611af10f974da497e7f3defe0c4f12" ;
    rdfs:comment "Identify application and infrastructure architecture components and review for basic security provisioning" ;
    rdfs:seeAlso <https://owaspsamm.org/model/verification/architecture-assessment/stream-a> ;
    skos:altLabel "V-AA-1-A" ;
    ns1:benefit "Understanding of high-level architecture and sensible security measures" ;
    ns1:hasPracticeLevel ns1:39bc5d271fae4ea8ba53db7de7b2712c ;
    ns1:hasStream ns1:77ca4b5e7ebc42558109829dffc2b80d .

ns1:11dd0c95f8914b6cb850a27f0557a9dd a ns1:Activity ;
    rdfs:label "Improve the incident detection process" ;
    dcterms:description """Ensure process documentation includes measures for continuous process improvement. Check the continuity of process improvement (e.g., via tracking of changes).

Ensure the checklist for suspicious event detection is correlated at least from (i) sources and knowledge bases external to the company (e.g., new vulnerability announcements affecting the used technologies), (ii) past security incidents, and (iii) threat model outcomes.

Use correlation of logs for incident detection for all reasonable incident scenarios. If the log data for incident detection is not available, document its absence as a defect, triage and handle it according to your established Defect Management process.

The quality of the incident detection does not depend on the time or day of the event. If security events are not acknowledged and resolved within a specified time (e.g., 20 minutes), ensure further notifications are generated according to an established escalation path.
""" ;
    dcterms:identifier "11dd0c95f8914b6cb850a27f0557a9dd" ;
    rdfs:comment "Use a proactively managed process for detection of incidents." ;
    rdfs:seeAlso <https://owaspsamm.org/model/operations/incident-management/stream-a> ;
    skos:altLabel "O-IM-3-A" ;
    ns1:benefit "Ability to timely detect security incidents" ;
    ns1:hasPracticeLevel ns1:6fe1973911bf4e54b018da10a5aa80a1 ;
    ns1:hasStream ns1:ff8a6a08dc684f38ab74b9db9584f0a5 .

ns1:15d73a64818c43019504c8d938ca2434 a ns1:Activity ;
    rdfs:label "Define advanced defect metrics" ;
    dcterms:description """Define, collect and calculate unified metrics across the whole organization. These might include:

* Total amount of verification activites and identified defects.
* Types and severities of identified defects.
* Time to detect and time to resolve defects.
* Windows of exposure of defects being present on live systems.
* Number of regressions / reopened vulnerabilities.
* Coverage of verification activities for particular software components.
* Amount of accepted risk.
* Ratio of security incidents caused due to unknown or undocumented security defects.

Generate a regular (e.g. monthly) report for a suitable audience. This would typically reach audience like managers and security officer and engineers. Use the information in the report as an input for your security strategy, e.g. improving trainings or security verification activities.

Share the most prominent or interesting technical details about security defects including the fixing strategy to other teams once these defects are fixed, e.g. in a regular knowledge sharing meeting. This will help scale the learning effect from defects to the whole organization and limit their occurence in the future.
""" ;
    dcterms:identifier "15d73a64818c43019504c8d938ca2434" ;
    rdfs:comment "Collect standardized defect management metrics and use these also for prioritization of centrally driven initiatives." ;
    rdfs:seeAlso <https://owaspsamm.org/model/implementation/defect-management/stream-b> ;
    skos:altLabel "I-DM-2-B" ;
    ns1:benefit "Improved learning from security defects in your organization" ;
    ns1:hasPracticeLevel ns1:b55c7a41eba747678a65651f5ccacaf2 ;
    ns1:hasStream ns1:55bf5184ff7d4b76a444e52a28c803d9 .

ns1:1a398709b9d3407dbf9db7eeff6e916c a ns1:Activity ;
    rdfs:label "Identify unused applications" ;
    dcterms:description """Identify unused applications on an _ad hoc_ basis, either by chance observation, or by occasionally performing a review. When you identify unused applications, process those findings for further action. If you have established a formal process for decommissioning unused applications, ensure teams are aware of and use it.

Manage customer/user migration from older versions of your products for each product and customer/user group. When a product version is no longer in use by any customer/user group, discontinue support for that version. However, at this level of maturity you may have a large number of product versions in active use across the customer/user base, requiring significant developer effort to back-port product fixes.
""" ;
    dcterms:identifier "1a398709b9d3407dbf9db7eeff6e916c" ;
    rdfs:comment "Decomission unused applications and services as identified. Manage customer upgrades/migrations individually." ;
    rdfs:seeAlso <https://owaspsamm.org/model/operations/operational-management/stream-b> ;
    skos:altLabel "O-OM-1-B" ;
    ns1:benefit "Identification of unused of software assets or components" ;
    ns1:hasPracticeLevel ns1:d0a99f3db27e48aa9b2d6b58a9040f49 ;
    ns1:hasStream ns1:a0d2ec4c6daa43369c07644b8745a7bd .

ns1:1cc77725cb2349f394477838668f6184 a ns1:Activity ;
    rdfs:label "Standardize and integrate security requirements" ;
    dcterms:description """Security requirements can originate from other sources including policies and legislation, known problems within the application, and intelligence from metrics and feedback. At this level, a more systematic elicitation of security requirements must be achieved by analysing different sources of such requirements. Ensure that appropriate input is received from these sources to help the elicitation of requirements. For example, organize interviews or brainstorm sessions (e.g., in the case of policy and legislation), analyze historical logs or vulnerability systems.

Use a structured notation of security requirements across applications and an appropriate formalism that integrates well with how you specify other (functional) requirements for the project. This could mean, for example, extending analysis documents, writing user stories, etc.

When requirements are specified, it is important to ensure that these requirements are taken into account during product development. Setup a mechanism to stimulate or force project teams to meet these requirements in the product. For example, annotate requirements with priorities, or influence the handling of requirements to enforce sufficient security appetite (while balancing against other non-functional requirements).
""" ;
    dcterms:identifier "1cc77725cb2349f394477838668f6184" ;
    rdfs:comment "Structured security requirements are available and utilized by developer teams." ;
    rdfs:seeAlso <https://owaspsamm.org/model/design/security-requirements/stream-a> ;
    skos:altLabel "D-SR-2-A" ;
    ns1:benefit "Alignment of security requirements with other types of requirements" ;
    ns1:hasPracticeLevel ns1:1a55b2c4666f4336a3f5c12c5bb4a1e9 ;
    ns1:hasStream ns1:7fb68bc660774b9080963c17761529a2 .

ns1:1ceadbb5a0024e2599821e7ce756f3a4 a ns1:Activity ;
    rdfs:label "Perform basic threat modeling" ;
    dcterms:description """Threat modeling is a structured activity for identifying, evaluating, and managing system threats, architectural design flaws, and recommended security mitigations. It is typically done as part of the design phase or as part of a security assessment.

Threat modeling is a team exercise, including product owners, architects, security champions, and security testers. At this maturity level, expose teams and stakeholders to threat modeling to increase security awareness and to create a shared vision on the security of the system.

At maturity level 1, you perform threat modeling ad-hoc for high-risk applications and use simple threat checklists, such as STRIDE. Avoid lengthy workshops and overly detailed lists of low-relevant threats. Perform threat modeling iteratively to align to more iterative development paradigms. If you add new functionality to an existing application, look only into the newly added functions instead of trying to cover the entire scope. A good starting point is the existing diagrams that you annotate during discussion workshops. Always make sure to persist the outcome of a threat modeling discussion for later use.

Your most important tool to start threat modeling is a whiteboard, smartboard, or a piece of paper. Aim for security awareness, a simple process, and actionable outcomes that you agree upon with your team.
""" ;
    dcterms:identifier "1ceadbb5a0024e2599821e7ce756f3a4" ;
    rdfs:comment "Perform best-effort, risk-based threat modeling using brainstorming and existing diagrams with simple threat checklists." ;
    rdfs:seeAlso <https://owaspsamm.org/model/design/threat-assessment/stream-b> ;
    skos:altLabel "D-TA-1-B" ;
    ns1:benefit "Identification of architectural design flaws in your applications" ;
    ns1:hasPracticeLevel ns1:a3d4045d5c0c4bd4a875784759539f0c ;
    ns1:hasStream ns1:ed5a9c3dd7884c88918a45dc9d231c5d .

ns1:1f3a9306778f4539a437d9f19232cda7 a ns1:Activity ;
    rdfs:label "Automate deployment and integrate security checks" ;
    dcterms:description """Automate the deployment process to cover various stages, so that no manual configuration steps are needed and the risk of isolated human errors is eliminated. Ensure and verify that the deployment is consistent over all stages.

Integrate automated security checks in your deployment process, e.g. using Dynamic Analysis Security Testing (DAST) and vulnerability scanning tools. Also, verify the integrity of the deployed artefacts where this makes sense. Log the results from these tests centrally and take any necessary actions. Ensure that in case any defects are detected, relevant personnel is notified automaticaly. In case any issues exceeding predefined criticality are identified, stop or reverse the deployment  either automatically, or introduce a separate manual approval workflow so that this decision is recorded, containing an explanation for the exception.

Account for and audit all deployments to all stages. Have a system in place to record each deployment, including information about who conducted it, the software version that was deployed, and any relevant variables specific to the deploy.
""" ;
    dcterms:identifier "1f3a9306778f4539a437d9f19232cda7" ;
    rdfs:comment "Automate the deployment process over all stages and introduce sensible security verification tests." ;
    rdfs:seeAlso <https://owaspsamm.org/model/implementation/secure-deployment/stream-a> ;
    skos:altLabel "I-SD-2-A" ;
    ns1:benefit "Efficient deployment process with integrated security tools" ;
    ns1:hasPracticeLevel ns1:3e89d1fa6cba4516a3ec446faaab5b84 ;
    ns1:hasStream ns1:9ec70d6f7ddb4cb6b37928f9994c6049 .

ns1:27bb61f3c6344359b021caeaef5ab07e a ns1:Activity ;
    rdfs:label "Adhere to basic security principles" ;
    dcterms:description """During design, technical staff on the product team use a short checklist of security principles. Typically, security principles include defense in depth, securing the weakest link, use of secure defaults, simplicity in design of security functionality, secure failure, balance of security and usability, running with least privilege, avoidance of security by obscurity, etc.

For perimeter interfaces, the team considers each principle in the context of the overall system and identify features that can be added to bolster security at each such interface. Limit these such that they only take a small amount of extra effort beyond the normal implementation cost of functional requirements. Note anything larger, and schedule it for future releases.

Train each product team with security awareness before this process, and incorporate more security-savvy staff to aid in making design decisions.
""" ;
    dcterms:identifier "27bb61f3c6344359b021caeaef5ab07e" ;
    rdfs:comment "Teams are trained on the use of basic security principles during design" ;
    rdfs:seeAlso <https://owaspsamm.org/model/design/security-architecture/stream-a> ;
    skos:altLabel "D-SA-1-A" ;
    ns1:benefit "Sets of security basic principles available to product teams" ;
    ns1:hasPracticeLevel ns1:a11b78917dec4cfdad983cf6d1d17b61 ;
    ns1:hasStream ns1:253b012094cf4e0988e08fd22609227d .

ns1:27cdd2a336a44e56a42632c7a78fcf4f a ns1:Activity ;
    rdfs:label "Identify tools and technologies" ;
    dcterms:description """People often take the path of least resistance in developing, deploying or operating a software solution. New technologies are often included when they can facilitate or speed up the effort or enable the solution to scale better. These new technologies might, however, introduce new risks to the organization that you need to manage.

Identify the most important technologies, frameworks, tools and integrations being used for each application. Use the knowledge of the architect to study the development and operating environment as well as artefacts. Then evaluate them for their security quality and raise important findings to be managed.
""" ;
    dcterms:identifier "27cdd2a336a44e56a42632c7a78fcf4f" ;
    rdfs:comment "Elicit technologies, frameworks and integrations within the overall solution to identify risk." ;
    rdfs:seeAlso <https://owaspsamm.org/model/design/security-architecture/stream-b> ;
    skos:altLabel "D-SA-1-B" ;
    ns1:benefit "Transparency of technologies that introduce security risk" ;
    ns1:hasPracticeLevel ns1:a11b78917dec4cfdad983cf6d1d17b61 ;
    ns1:hasStream ns1:79754453c74b4143b20a57d0efdaab56 .

ns1:281369f491da4d4c84b0729e344e2c93 a ns1:Activity ;
    rdfs:label "Enforce a security baseline during build" ;
    dcterms:description """Define security checks suitable to be carried out during the build process, as well as minimum criteria for passing the build - these might differ according to the risk profiles of various applications. Include the respective security checks in the build and enforce breaking the build process in case the predefined criteria are not met. Trigger warnings for issues below the threshold and log these to a centralized system to track them and take actions. If sensible, implement an exception mechanism to bypass this behavior if the risk of a particular vulnerability has been accepted or mitigated. However, ensure these cases are explicitely approved first and log their occurence together with a rationale.

If technical limitations prevent the organization from breaking the build automatically, ensure the same effect via other measures, such as a clear policy and regular audit.

Handle code signing on a separate centralized server which does not expose the certificate to the system executing the build. Where possible, use a deterministic method that outputs byte-for-byte reproducible artifacts.
""" ;
    dcterms:identifier "281369f491da4d4c84b0729e344e2c93" ;
    rdfs:comment "Define mandatory security checks in the build process and ensure that building non-compliant artifacts fails." ;
    rdfs:seeAlso <https://owaspsamm.org/model/implementation/secure-build/stream-a> ;
    skos:altLabel "I-SB-3-A" ;
    ns1:benefit "Assurance that you build software complying with a security baseline" ;
    ns1:hasPracticeLevel ns1:02e602c451d548e8a95433a46fe6b9d8 ;
    ns1:hasStream ns1:8a870a9b26724b4ba0dff177028b474a .

ns1:2b01696356ed4652accf093f6c6a47ee a ns1:Activity ;
    rdfs:label "Perform vendor assessments" ;
    dcterms:description """The security competences and habits of the external suppliers involved in the development of your software can have a significant impact on the security posture of the final product. Consequently, it is important to know and evaluate your suppliers on this front.

Carry out a vendor assessment to understand the strengths and weaknesses of your suppliers. Use a basic checklist or conduct interviews to review their typical practices and deliveries. This gives you an idea of how they organize themselves and elements to evaluate whether you need to take additional measures to mitigate potential risks. Ideally, speak to different roles in the organization, or even set up a small maturity evaluation to this end. Strong suppliers will run their own software assurance program and will be able to answer most of your questions. If suppliers have weak competences in software security, discuss with them how and to what extent they plan to work on this and evaluate whether this is enough for your organization. A software supplier might be working on a low-risk project, but this could change.

It is important that your suppliers understand and align to the risk appetite and are able to meet your requirements in that area. Make what you expect from them explicit and discuss this clearly.
""" ;
    dcterms:identifier "2b01696356ed4652accf093f6c6a47ee" ;
    rdfs:comment "Evaluate the supplier based on organizational security requirements." ;
    rdfs:seeAlso <https://owaspsamm.org/model/design/security-requirements/stream-b> ;
    skos:altLabel "D-SR-1-B" ;
    ns1:benefit "Transparency of security practices of your software suppliers" ;
    ns1:hasPracticeLevel ns1:3d035b6df77f4ee69577c9b4c9d64891 ;
    ns1:hasStream ns1:8c1dcd10821f4f2baed52fdc83d93cf6 .

ns1:2bf0e192a904444b8a2f38c33256e80a a ns1:Activity ;
    rdfs:label "Rate and track security defects" ;
    dcterms:description """Introduce and apply a well defined rating methodology for your security defects consistently across the whole organization, based on the probability and expected impact of the defect being exploited. This will allow you to identify applications which need higher attention and investments. In case you don't store the information about security defects centrally, ensure that you're still able to easily pull the information from all sources and get an overview about "hot spots" needing your attention.

Introduce SLAs for timely fixing of security defects according to their criticality rating and centrally monitor and regularly report on SLA breaches. Define a process for cases where it's not feasible or economical to fix a defect within the time defined by the SLAs. This should at least ensure that all relevant stakeholders have a solid understanding of the imposed risk. If suitable, employ compensating controls for these cases.

Even if you don't have any formal SLAs for fixing low severity defects, ensure that responsible teams still get a regular overview about issues affecting their applications and understand how particular issues affect or amplify each other.
""" ;
    dcterms:identifier "2bf0e192a904444b8a2f38c33256e80a" ;
    rdfs:comment "Rate all security defects over the whole organization consistently and define SLAs for particular severity classes." ;
    rdfs:seeAlso <https://owaspsamm.org/model/implementation/defect-management/stream-a> ;
    skos:altLabel "I-DM-2-A" ;
    ns1:benefit "Consistent classification of security defects with clear expectations of their handling" ;
    ns1:hasPracticeLevel ns1:b55c7a41eba747678a65651f5ccacaf2 ;
    ns1:hasStream ns1:a5b57fc5fa0441b7b23f599b506c5752 .

ns1:2f63f92c414546b58d035ece110d479f a ns1:Activity ;
    rdfs:label "Periodic review of risk profiles" ;
    dcterms:description """The application portfolio of an organization changes, as well as the conditions and constraints in which an application lives (e.g., driven by the company strategy). Periodically review the risk inventory to ensure correctness of the risk evaluations of the different applications.

Have a periodic review at an enterprise-wide level. Also, as your enterprise matures in software assurance, stimulate teams to continuously question which changes in conditions might impact the risk profile. For instance, an internal application might become exposed to the internet by a business decision. This should trigger the teams to rerun the risk evaluation and update the application risk profile accordingly.

In a mature implementation of this practice, train and continuously update teams on lessons learned and best practices from these risk evaluations. This leads to a better execution and a more accurate representation of the application risk profile.
""" ;
    dcterms:identifier "2f63f92c414546b58d035ece110d479f" ;
    rdfs:comment "Periodically review application risk profiles at regular intervals to ensure accuracy and reflect current state." ;
    rdfs:seeAlso <https://owaspsamm.org/model/design/threat-assessment/stream-a> ;
    skos:altLabel "D-TA-3-A" ;
    ns1:benefit "Timely update of the application classification in case of changes" ;
    ns1:hasPracticeLevel ns1:21a59897dbeb4d7fa4603a0f24362c2b ;
    ns1:hasStream ns1:17c90203f8354c3594eea22759e375a9 .

ns1:3156ab7b516e4550893427face9f86bc a ns1:Activity ;
    rdfs:label "Perform continuous configuration monitoring" ;
    dcterms:description """Actively monitor the security configurations of deployed technology stacks, performing regular checks against established baselines. Ensure results of configuration checks are readily available, through published reports and dashboards.

When you detect non-conforming configurations, treat each occurrence as a security finding, and manage corrective actions within your established Defect Management practice.

Further gains may be realized using automated measures, such as "self-healing" configurations and security information and event management (SIEM) alerts.

As part of the process for updating components (e.g., new releases, vendor patches), review corresponding baselines and configuration guides, updating them as needed to maintain their relevance and accuracy. Review other baselines and configuration guides at least annually.

Periodically review your baseline management process, incorporating feedback and lessons learned from teams applying and maintaining configuration baselines and configuration guides.
""" ;
    dcterms:identifier "3156ab7b516e4550893427face9f86bc" ;
    rdfs:comment "Actively monitor configurations for non-conformance to baselines, and handle detected occurrences as security defects." ;
    rdfs:seeAlso <https://owaspsamm.org/model/operations/environment-management/stream-a> ;
    skos:altLabel "O-EM-3-A" ;
    ns1:benefit "Clear view on component configurations to avoid non-conformities" ;
    ns1:hasPracticeLevel ns1:1cb6e197ca8245eca65b0ecbdd784720 ;
    ns1:hasStream ns1:47bff9a57f0344eeb4b083f1c2b1bb7e .

ns1:346ed576f0a94147ba2b8148abc3c73a a ns1:Activity ;
    rdfs:label "Establish a penetration testing process" ;
    dcterms:description """Using the set of security test cases identified for each project, conduct manual penetration testing to evaluate the system’s performance against each case. Generally, this happens during the testing phase prior to release and includes both static and dynamic manual penetration testing. In cases where software cannot be realistically tested outside of production, use of techniques such as blue-green deployments or A/B testing can allow ring-fenced security testing in production.

Penetration testing cases include both application-specific tests to check soundness of business logic, and common vulnerability tests to check the design and implementation. Once specified, security-savvy quality assurance or development staff can execute security test cases. The central software security group monitors first-time execution of security test cases for a project team to assist and coach the team security champions.

Many organizations offer "Bug Bunty" programmes which invite security researchers to find vulnerabilties in applications and report them responsibly in exchange for rewards. The approach allows organizations to access a bigger pool of talent, especially those lacking sufficient internal capacity or requiring the additional assurance.

Prior to release or mass deployment, stakeholders review results of security tests and accept the risks indicated by failing security tests at release time. Establish a concrete timeline to address the gaps over time. Spread the knowledge of manual security testing and the results across the development team to improve security knowledge and awareness inside the organization.
""" ;
    dcterms:identifier "346ed576f0a94147ba2b8148abc3c73a" ;
    rdfs:comment "Conduct manual penetration testing" ;
    rdfs:seeAlso <https://owaspsamm.org/model/verification/security-testing/stream-b> ;
    skos:altLabel "V-ST-2-B" ;
    ns1:benefit "Understanding of application resilience from black-box perspective" ;
    ns1:hasPracticeLevel ns1:6291462e1894467d807b913ef7da4beb ;
    ns1:hasStream ns1:8a64c7b0b35a458ea436260d5e414dfa .

ns1:38932fe4024e4ec89646a82e0b4e651e a ns1:Activity ;
    rdfs:label "Standardize policy and compliance requirements" ;
    dcterms:description """Develop a library of application requirements and test scripts to establish and verify regulatory compliance of applications. Some of these are tied to individual compliance requirements like PCI or GDPR, while others are more general in nature and address global compliance requirements such as ISO. The library is available to all application development teams. It includes guidance for determining all applicable requirements including considerations for reducing the compliance burden and scope. Implement a process to periodically re-assess each application’s compliance requirements. Re-assessment includes reviewing all application functionality and opportunities to reduce scope to lower the overall cost of compliance.

Requirements include enough information for developers to understand functional and non-functional requirements of the different compliance obligations. They include references to policies and standards, and provide explicit references to regulations. If there are questions about the implementation of a particular requirement, the original text of the regulation can help interpret the intent more accurately. Each requirement includes a set of test scripts for verifying compliance. In addition to assisting QA with compliance verification, these can help clarify compliance requirements for developers and make the compliance process transparent. Requirements have a format that allows importing them into individual requirements repositories. further clarify compliance requirements for developers and ensure the process of achieving compliance is fully transparent.
""" ;
    dcterms:identifier "38932fe4024e4ec89646a82e0b4e651e" ;
    rdfs:comment "Publish compliance-specific application requirements and test guidance." ;
    rdfs:seeAlso <https://owaspsamm.org/model/governance/policy-and-compliance/stream-b> ;
    skos:altLabel "G-PC-2-B" ;
    ns1:benefit "Common understanding how to reach compliance with external compliance drivers for product teams" ;
    ns1:hasPracticeLevel ns1:2a29c1f7d6954785b8d42d637a752f94 ;
    ns1:hasStream ns1:2919e1f19aec4f018da94a3e8733f37d .

ns1:3ae763a70854421984dfa70980e1bf68 a ns1:Activity ;
    rdfs:label "Evaluate architecture for typical threats" ;
    dcterms:description """Review the architecture for typical security threats. Security-savvy technical staff conduct this analysis with input from architects, developers, managers, and business owners as needed, to ensure the architecture addresses all common threats which development teams lacking specialised security expertise may have overlooked.

Typical threats in an architecture can relate to incorrect assumptions in, or overly reliance on, the provisioning of security mechanisms such as authentication, authorization, user and rights management, secure communication, data protection, key management and log management. Threats, on the other hand, can also relate to known limitations of, or issues in, technological components or frameworks that are part of the solution and for which insufficient mitigation has been put in place.
""" ;
    dcterms:identifier "3ae763a70854421984dfa70980e1bf68" ;
    rdfs:comment "Ad-hoc review of the architecture for unmitigated security threats." ;
    rdfs:seeAlso <https://owaspsamm.org/model/verification/architecture-assessment/stream-b> ;
    skos:altLabel "V-AA-1-B" ;
    ns1:benefit "Assures that the architecture protects against typical security threats." ;
    ns1:hasPracticeLevel ns1:39bc5d271fae4ea8ba53db7de7b2712c ;
    ns1:hasStream ns1:b7487370a07543cbb02ddb60c055d92f .

ns1:3afce608ad7c42deb37a04d6b86e5c33 a ns1:Activity ;
    rdfs:label "Enforce the use of recommended technologies" ;
    dcterms:description """For all proprietary development (in-house or acquired), impose and monitor the use of standardized technology. Depending on your organization, either implement these restrictions into build or deployment tools, by means of after-the-fact automated analysis of application artefacts (e.g., source code, configuration files or deployment artefacts), or periodically review focusing on the correct use of these frameworks.

Verify several factors with project teams. Identify use of non-recommended technologies to determine if there are gaps in recommendations versus the organization’s needs. Examine unused or incorrectly used design patterns and reference platform modules to determine if updates are needed. Additionally, implement functionality in the reference platforms as the organization evolves and project teams request it.
""" ;
    dcterms:identifier "3afce608ad7c42deb37a04d6b86e5c33" ;
    rdfs:comment "Impose the use of standard technologies on all software development." ;
    rdfs:seeAlso <https://owaspsamm.org/model/design/security-architecture/stream-b> ;
    skos:altLabel "D-SA-3-B" ;
    ns1:benefit "Limited attack surface due to usage of vetted technologies" ;
    ns1:hasPracticeLevel ns1:9d1e469966124c0fa80d1bc2fc223a0a ;
    ns1:hasStream ns1:79754453c74b4143b20a57d0efdaab56 .

ns1:43d347fd280845718f16ccc811e5d942 a ns1:Activity ;
    rdfs:label "Drive the security program through metrics" ;
    dcterms:description """Define guidelines for influencing the Application Security program based on the KPIs and other application security metrics. These guidelines  combine the maturity of the application development process and procedures  with different metrics to make the program more efficient. The following examples show a relationship between measurements and ways of evolving and improving application security

* Focus on maturity of the development lifecycle makes the relative cost per defect lower by applying security proactively.
* Monitoring the balance between effort, result, and environment metrics improves the program’s efficiency and justifies additional automation and other methods for improving the overall application security baselines.
* Individual Security Practices could provide indicators of success or failure of individual application security initiatives.
* Effort metrics helps ensure application security work is directed at the more relevant and important technologies and disciplines.

When defining the overall metrics strategy, keep the end-goal in mind and define what decisions can be made as a result of changes in KPIs and metrics as soon as possible, to help guide development of metrics.
""" ;
    dcterms:identifier "43d347fd280845718f16ccc811e5d942" ;
    rdfs:comment "Influence the strategy based on the metrics and organizational needs." ;
    rdfs:seeAlso <https://owaspsamm.org/model/governance/strategy-and-metrics/stream-b> ;
    skos:altLabel "G-SM-3-B" ;
    ns1:benefit "Continuous improvement of your program according to results" ;
    ns1:hasPracticeLevel ns1:420074f071fb4ab6b6ee6ef44c4f4f1c ;
    ns1:hasStream ns1:2f1cac3c2e724823b3b48a7e797520b4 .

ns1:4729b4bd6dca4d58a68cb854ad4409a6 a ns1:Activity ;
    rdfs:label "Include application secrets during deployment" ;
    dcterms:description """Have an automated process to add credentials and secrets to configuration files during the deployment process to respective stages. This way, developers and deployers do not see or handle those sensitive values.

Implement checks that detect the presence of secrets in code repositories and files, and run them periodically. Configure tools to look for known strings and unknown high entropy strings. In systems such as code repositories, where there is a history, include the versions in the checks. Mark potential secrets you discover as sensitive values, and remove them where appropriate. If you cannot remove them from a historic file in a code repository, for example, you may need to refresh the value on the system that consumes the secret. This way, if an attacker discovers the secret, it will not be useful to them.

Make the system used to store and process the secrets and credentials robust from a security perspective. Encrypt all secrets at rest and in transit. Users who configure this system and the secrets it contains are subject to the principle of least privilege. For example, a developer might need to manage the secrets for a development environment, but not a user acceptance test or production environment.
""" ;
    dcterms:identifier "4729b4bd6dca4d58a68cb854ad4409a6" ;
    rdfs:comment "Inject secrets dynamically during deployment process from hardened storages and audit all human access to them." ;
    rdfs:seeAlso <https://owaspsamm.org/model/implementation/secure-deployment/stream-b> ;
    skos:altLabel "I-SD-2-B" ;
    ns1:benefit "Detection of potential leakage of production secrets" ;
    ns1:hasPracticeLevel ns1:3e89d1fa6cba4516a3ec446faaab5b84 ;
    ns1:hasStream ns1:9a5f26d77f204467bdda7ffa09109d73 .

ns1:4f6a06796d0840debcc775ea1af65679 a ns1:Activity ;
    rdfs:label "Integrate security testing tools in the delivery pipeline" ;
    dcterms:description """Projects within the organization routinely run automated security tests and review results during development. Configure security testing tools to automatically run as part of the build and deploy process to make this scalable with low overhead. Inspect findings as they occur.

Conducting security tests as early as the requirements or design phases can be beneficial. While traditionally used for functional test cases, this type of test-driven development approach involves identifying and running relevant security test cases early in the development cycle. With the automatic execution of security test cases, projects enter the implementation phase with a number of failing tests for the non-existent functionality. Implementation is complete when all the tests pass. This provides a clear, upfront goal for developers early in the development cycle, lowering risk of release delays due to security concerns or forced acceptance of risk to meet project deadlines.

Make the results of automated and manual security tests visible via dashboards, and routinely present them to management and business stakeholders (e.g. before each release) for review. If there are unaddressed findings that remain as accepted risks for the release, stakeholders and development managers work together to establish a concrete timeframe for addressing them. Continuously review and improve the quality of the security tests.

Consider and implement security test correlation tools to automate the matching and merging of test results from dynamic, static, and interactive application scanners into one central dashboard, providing direct input towards Defect Management. Spread the knowledge of the created security tests and the results across the development team to improve security knowledge and awareness inside the organization.
""" ;
    dcterms:identifier "4f6a06796d0840debcc775ea1af65679" ;
    rdfs:comment "Integrate automated security testing into the build and deploy process" ;
    rdfs:seeAlso <https://owaspsamm.org/model/verification/security-testing/stream-a> ;
    skos:altLabel "V-ST-3-A" ;
    ns1:benefit "Identification of automatically identifiable vulnerabilities in earliest possible stages" ;
    ns1:hasPracticeLevel ns1:eac3184f8e2343b8b29047d023376da5 ;
    ns1:hasStream ns1:102fdab651834273abd67a3ec27aab05 .

ns1:529d528265c94447954a57f5be425f54 a ns1:Activity ;
    rdfs:label "Inventorize risk profiles" ;
    dcterms:description """The goal of this activity is to thoroughly understand the risk level of all applications within the organization, to focus the effort of your software assurance activities where it really matters.

From a risk evaluation perspective, the basic set of questions is not enough to thoroughly evaluate the risk of all applications. Create an extensive and standardized way to evaluate the risk of the application, among others via their impact on information security (confidentiality, integrity and availability of data). Next to security, you also want to evaluate the privacy risk of the application. Understand the data that the application processes and what potential privacy violations are relevant. Finally, study the impact that this application has on other applications within the organization (e.g., the application might be modifying data that was considered read-only in another context). Evaluate all applications within the organization, including all existing and legacy ones.

Leverage business impact analysis to quantify and classify application risk. A simple qualitative scheme (such as high/medium/low) is not enough to effectively manage and compare applications on an enterprise-wide level.

Based on this input, Security Officers leverage the classification to define the risk profile to build a centralized inventory of risk profiles and manage accountability. This inventory gives Product Owners, Managers, and other organizational stakeholders an aligned view of the risk level of an application in order to assign appropriate priority to security-related activities.
""" ;
    dcterms:identifier "529d528265c94447954a57f5be425f54" ;
    rdfs:comment "Understand the risk for all applications in the organization by centralizing the risk profile inventory for stakeholders." ;
    rdfs:seeAlso <https://owaspsamm.org/model/design/threat-assessment/stream-a> ;
    skos:altLabel "D-TA-2-A" ;
    ns1:benefit "Solid understanding of the risk level of your application portfolio" ;
    ns1:hasPracticeLevel ns1:e5b6dc4f907c4986b8ba7923303cd665 ;
    ns1:hasStream ns1:17c90203f8354c3594eea22759e375a9 .

ns1:5bcb52375a0f4085bb12266c9ecfa84d a ns1:Activity ;
    rdfs:label "Define an incident detection process" ;
    dcterms:description """Establish a dedicated owner for the incident detection process, make clear documentation accessible to all process stakeholders, and ensure it is regularly reviewed and updated as necessary. Ensure employees responsible for incident detection follow this process (e.g., using training).

The process typically relies on a high degree of automation, collecting and correlating log data from different sources, including application logs. You may aggregate logs in a central place, if suitable. Periodically verify the integrity of analyzed data. If you add a new application, ensure the process covers it within a reasonable period of time.

Detect possible security incidents using an available checklist. The checklist should cover expected attack vectors and known or expected kill chains. Evaluate and update it regularly.

When you determine an event is a security incident (with sufficiently high confidence), notify responsible staff immediately, even outside business hours. Perform further analysis, as appropriate, and start the escalation process.
""" ;
    dcterms:identifier "5bcb52375a0f4085bb12266c9ecfa84d" ;
    rdfs:comment "Follow an established, well-documented process for incident detection, with emphasis on automated log evaluation." ;
    rdfs:seeAlso <https://owaspsamm.org/model/operations/incident-management/stream-a> ;
    skos:altLabel "O-IM-2-A" ;
    ns1:benefit "Timely and consistent detection of expected security incidents" ;
    ns1:hasPracticeLevel ns1:439406325e6645519c149da3e05a7d9d ;
    ns1:hasStream ns1:ff8a6a08dc684f38ab74b9db9584f0a5 .

ns1:5d5e3d9beab9498ca1ce66d3a53a81c6 a ns1:Activity ;
    rdfs:label "Discuss security responsibilities with suppliers" ;
    dcterms:description """Increase your confidence in the capability of your suppliers for software security. Discuss concrete responsibilities and expectations from your suppliers and your own organization and establish a contract with the supplier. The responsibilities can be specific quality requirements or particular tasks, and minimal service can be detailed in a Service Level Agreement (SLA). A quality requirement example is that they will deliver software that is protected against the OWASP Top 10, and in case issues are detected, these will be fixed. A task example is that they have to perform continuous static code analysis, or perform an independent penetration test before a major release. The agreement stipulates liabilities and caps in case an important issue arises.

Once you have implemented this for a few suppliers, work towards a standard agreement for suppliers that forms the basis of your negotiations. You can deviate from this standard agreement on a case by case basis, but it will help you to ensure you do not overlook important topics.
""" ;
    dcterms:identifier "5d5e3d9beab9498ca1ce66d3a53a81c6" ;
    rdfs:comment "Build security into supplier agreements in order to ensure compliance with organizational requirements." ;
    rdfs:seeAlso <https://owaspsamm.org/model/design/security-requirements/stream-b> ;
    skos:altLabel "D-SR-2-B" ;
    ns1:benefit "Clearly defined security responsibilities of your software suppliers" ;
    ns1:hasPracticeLevel ns1:1a55b2c4666f4336a3f5c12c5bb4a1e9 ;
    ns1:hasStream ns1:8c1dcd10821f4f2baed52fdc83d93cf6 .

ns1:5e1dd310e28449058046c7af0fe46fce a ns1:Activity ;
    rdfs:label "Promote preferred tools and technologies" ;
    dcterms:description """Identify commonly used technologies, frameworks and tools in use across software projects in the organization, whereby you focus on capturing the high-level technologies.

Create a list and share it across the development organization as recommended technologies. When selecting them, consider incident history, track record for responding to vulnerabilities, appropriateness of functionality for the organization, excessive complexity in usage of the third-party component, and sufficient knowledge within the organization.

Senior developers and architects create this list, including input from managers and security auditors. Share this list of recommended components with the development organization. Ultimately, the goal is to provide well-known defaults for project teams. Perform a periodic review of these technologies for security and appropriateness.
""" ;
    dcterms:identifier "5e1dd310e28449058046c7af0fe46fce" ;
    rdfs:comment "Standardize technologies and frameworks to be used throughout the different applications" ;
    rdfs:seeAlso <https://owaspsamm.org/model/design/security-architecture/stream-b> ;
    skos:altLabel "D-SA-2-B" ;
    ns1:benefit "Technologies with appropriate security level available to product teams" ;
    ns1:hasPracticeLevel ns1:41c8e63716c34f1eaf09b8cad70cfbaf ;
    ns1:hasStream ns1:79754453c74b4143b20a57d0efdaab56 .

ns1:60d7a0a61dd142d5a87009bc5b93df56 a ns1:Activity ;
    rdfs:label "Formalize decommissioning process" ;
    dcterms:description """As part of decommissioning a system, application, or service, follow an established process for removing all relevant accounts, firewall rules, data, etc. from the operational environment. By removing these unused elements from configuration files, you improve the maintainability of infrastructure-as-code resources.

Follow a consistent process for timely replacement or upgrade of third-party applications, or application dependencies (e.g., operating system, utility applications, libraries), that have reached end of life.

Engage with customers and user groups for your products at or approaching end of life, to migrate them to supported versions in a timely manner.
""" ;
    dcterms:identifier "60d7a0a61dd142d5a87009bc5b93df56" ;
    rdfs:comment "Develop repeatable decommissioning processes for unused systems/services, and for migration from legacy dependencies. Manage legacy migration roadmaps for customers." ;
    rdfs:seeAlso <https://owaspsamm.org/model/operations/operational-management/stream-b> ;
    skos:altLabel "O-OM-2-B" ;
    ns1:benefit "Standardized decommisioning process decreasing the risk of forgetting components" ;
    ns1:hasPracticeLevel ns1:76f8a2e68065467ba9bd2b5ac625490b ;
    ns1:hasStream ns1:a0d2ec4c6daa43369c07644b8745a7bd .

ns1:62237ae79ab84a6687de2885b1e3d608 a ns1:Activity ;
    rdfs:label "Structurally verify the architecture for identified threats" ;
    dcterms:description """Systematically review each threat identified during the Threat Assessment activities and examine how the architecture mitigates them. Use a standardised process for analyzing system architectures and the flow of data within them. This is typically linked to the threat model used (e.g. STRIDE) in order to identify the relevant security objectives which address each type of threat. For each threat, identify the design-level features of the architecture which counter it and assess their effectiveness in doing so.

Where available, review architectural decision records to understand the architectural constraints and tradeoffs made during design. Take their impact into consideration along with any security assumptions on which the safe operation of the system relies and re-evaluate them.

Enrich your previously created threat model such that each threat and its estimated impact are linked to the corresponding counter measure. Produce a mapping document, or dashboard in a specialized tool, to make the information available and visible to the relevant stakeholders.
""" ;
    dcterms:identifier "62237ae79ab84a6687de2885b1e3d608" ;
    rdfs:comment "Analyze the architecture for known threats." ;
    rdfs:seeAlso <https://owaspsamm.org/model/verification/architecture-assessment/stream-b> ;
    skos:altLabel "V-AA-2-B" ;
    ns1:benefit "All identified threats to the application are adequately handled." ;
    ns1:hasPracticeLevel ns1:67fcd33f84364ef68fb88aba77de1a63 ;
    ns1:hasStream ns1:b7487370a07543cbb02ddb60c055d92f .

ns1:649b693315234a94928e42f3e308deac a ns1:Activity ;
    rdfs:label "Standardize and scale threat modeling" ;
    dcterms:description """Use a standardized threat modeling methodology for your organization and align this on your application risk levels. Think about ways to support the scaling of threat modeling throughout the organization.

Train your architects, security champions, and other stakeholders on how to do practical threat modeling.  Threat modeling requires understanding, clear playbooks and templates, organization-specific examples, and experience, which is hard to automate.

Your threat modeling methodology includes at least diagramming, threat identification, design flaw mitigations, and how to validate your threat model artifacts. Your threat model diagram allows a detailed understanding of the environment and the mechanics of the application. You discover threats to your application with checklists, such as STRIDE or more organization-specific threats. For identified design flaws (ranked according to risk for your organization), you add mitigating controls to support stakeholders in dealing with particular threats. Define what triggers updating a threat model, for example, a technology change or deployment of an application in a new environment.

Feed the output of threat modeling to the defect management process for adequate follow-up. Capture the threat modeling artifacts with tools that are used by your application teams.
""" ;
    dcterms:identifier "649b693315234a94928e42f3e308deac" ;
    rdfs:comment "Standardize threat modeling training, processes, and tools to scale across the organization." ;
    rdfs:seeAlso <https://owaspsamm.org/model/design/threat-assessment/stream-b> ;
    skos:altLabel "D-TA-2-B" ;
    ns1:benefit "Clear expectations of the quality of threat modeling activities" ;
    ns1:hasPracticeLevel ns1:e5b6dc4f907c4986b8ba7923303cd665 ;
    ns1:hasStream ns1:ed5a9c3dd7884c88918a45dc9d231c5d .

ns1:6e7a618abd564df5bb784ca54893bbee a ns1:Activity ;
    rdfs:label "Define policies and standards" ;
    dcterms:description """Develop a library of policies and standards to govern all aspects of software development in the organization. Policies and standards are based on existing industry standards and appropriate for the organization’s industry. Due to the full range of technology-specific limitations and best practices, review proposed standards with the various product teams. With the overarching objective of increasing security of the applications and computing infrastructure, invite product teams to offer feedback on any aspects of the standards that would not be feasible or cost-effective to implement, as well as opportunities for standards to go further with little effort on the product teams.

For policies, emphasize high-level definitions and aspects of application security that do not depend on specific technology or hosting environment. Focus on broader objectives of the organization to protect the integrity of its computing environment, safety and privacy of the data, and maturity of the software development life-cycles. For larger organizations, policies may qualify specific requirements based on data classification or application functionality, but should not be detailed enough to offer technology-specific guidance.

For standards, incorporate requirements set forth by policies, and focus on technology-specific implementation guidance intended to capture and take advantage of the security features of different programming languages and frameworks. Standards require input from senior developers and architects considered experts in various technologies in use by the organization. Create them in a format that allows for periodic updates. Label or tag individual requirements with the policy or a 3rd party requirement, to make maintenance and audits easier and more efficient.
""" ;
    dcterms:identifier "6e7a618abd564df5bb784ca54893bbee" ;
    rdfs:comment "Determine a security baseline representing organization’s policies and standards." ;
    rdfs:seeAlso <https://owaspsamm.org/model/governance/policy-and-compliance/stream-a> ;
    skos:altLabel "G-PC-1-A" ;
    ns1:benefit "Clear expectation of minimum security level in the organization" ;
    ns1:hasPracticeLevel ns1:437d447b3f11427592e938dbde53c7da ;
    ns1:hasStream ns1:c404aa4f711e4f4e9e71faea22f7fb5c .

ns1:7003146cf1a1450293001754fe74787d a ns1:Activity ;
    rdfs:label "Automate security requirements testing" ;
    dcterms:description """Write and automate regression tests for all identified (and fixed) bugs to ensure that these become a test harness preventing similar issues being introduced during later releases. Security unit tests should verify dynamically (i.e., at run time) that the components function as expected and should validate that code changes are properly implemented.

A good practice for developers is to build security test cases as a generic security test suite that is part of the existing unit testing framework. A generic security test suite might include security test cases to validate both positive and negative requirements for security controls such as Identity, Authentication & Access Control, Input Validation & Encoding, User and Session Management, Error and Exception Handling, Encryption, and Auditing and Logging. Verify the correct execution of the security tests as early as possible. If feasible for example, consider the passing of security tests as part of merge requirements before allowing new code to enter the main code base. Alternatively, consider their passing a requirement for validating a build.

For security functional tests, use unit level tests for the functionality of security controls at the software component level, such as functions, methods, or classes. For example, a test case could check input and output validation (e.g., variable sanitation) and boundary checks for variables by asserting the expected functionality of the component.
""" ;
    dcterms:identifier "7003146cf1a1450293001754fe74787d" ;
    rdfs:comment "Perform regression testing (with security unit tests)" ;
    rdfs:seeAlso <https://owaspsamm.org/model/verification/requirements-driven-testing/stream-a> ;
    skos:altLabel "V-RT-3-A" ;
    ns1:benefit "Timely and reliable detection of violations to security requirements" ;
    ns1:hasPracticeLevel ns1:812abdd0a2b54366a497919f8463911a ;
    ns1:hasStream ns1:efb5d1f275504173899da345ef5bbe8e .

ns1:77a5f467ffe140e2a2839bb522e82c4e a ns1:Activity ;
    rdfs:label "Protect application secrets in configuration and code" ;
    dcterms:description """Developers should not have access to secrets or credentials for production environments. Have a mechanism in place to adequately protect production secrets, for instance by (i) having specific persons adding them to relevant configuration files upon deployment (the separation of duty principle) or (ii) by encrypting the production secrets contained in the configuration files upfront.

Do not use production secrets in configuration files for development or testing environments, as such environments may have a significantly lower security posture. Similarly, do not keep secrets unprotected in configuration files stored in code repositories.

Store sensitive credentials and secrets for production systems with encryption-at-rest at all times. Consider using a purpose-built tool for this. Handle key management carefully so only personnel with responsibility for production deployments are able to access this data.
""" ;
    dcterms:identifier "77a5f467ffe140e2a2839bb522e82c4e" ;
    rdfs:comment "Introduce basic protection measures to limit access to your production secrets." ;
    rdfs:seeAlso <https://owaspsamm.org/model/implementation/secure-deployment/stream-b> ;
    skos:altLabel "I-SD-1-B" ;
    ns1:benefit "Defined and limited access to your production secrets" ;
    ns1:hasPracticeLevel ns1:5015427608de428cba3c324772fb4191 ;
    ns1:hasStream ns1:9a5f26d77f204467bdda7ffa09109d73 .

ns1:786b3d7b39cd49a88090554a275f04a6 a ns1:Activity ;
    rdfs:label "Use best-effort hardening" ;
    dcterms:description """Understanding the importance of securing the technology stacks you're using, apply secure configuration to stack elements, based on readily available guidance (e.g., open source projects, vendor documentation, blog articles). When your teams develop configuration guidance for their applications, based on trial-and-error and information gathered by team members, encourage them to share their learnings across the organization.

Identify key elements of common technology stacks, and establish configuration standards for those, based on teams' experiences of what works.

At this level of maturity, you don't yet have a formal process for managing configuration baselines. Configurations may not be applied consistently across applications and deployments, and monitoring of conformance is likely absent.
""" ;
    dcterms:identifier "786b3d7b39cd49a88090554a275f04a6" ;
    rdfs:comment "Perform best-effort hardening of configurations, based on readily available information." ;
    rdfs:seeAlso <https://owaspsamm.org/model/operations/environment-management/stream-a> ;
    skos:altLabel "O-EM-1-A" ;
    ns1:benefit "Hardened basic configuration settings of your components" ;
    ns1:hasPracticeLevel ns1:8cb942eff46d41f38e6edc11849744a6 ;
    ns1:hasStream ns1:47bff9a57f0344eeb4b083f1c2b1bb7e .

ns1:81ef5625583646bf8bc3fad53e4eff55 a ns1:Activity ;
    rdfs:label "Perform fuzz testing" ;
    dcterms:description """Perform fuzzing, sending random or malformed data to the test subject in an attempt to make it crash. Fuzz testing or Fuzzing is a Black Box software testing technique, which consists of finding implementation bugs using automated malformed or semi-malformed data injection. Cover at least a minimum fuzzing for vulnerabilities against the main input parameters of the application.

The advantage of fuzz testing is the simplicity of the test design, and its lack of preconceptions about system behavior. The stochastic approach results in bugs that human eyes or structured testing would often miss. It is also one of the few means of assessing the quality of a closed system (such as a SIP phone). The simplicity of fuzzing a target is offset by the difficulty in accurately detecting and triaging crashes. Favour existing fuzzing tools and frameworks to leverage their supporting tooling.
""" ;
    dcterms:identifier "81ef5625583646bf8bc3fad53e4eff55" ;
    rdfs:comment "Perform security fuzzing testing" ;
    rdfs:seeAlso <https://owaspsamm.org/model/verification/requirements-driven-testing/stream-b> ;
    skos:altLabel "V-RT-1-B" ;
    ns1:benefit "Insight into behaviour of your applications when dealing with unexpected input" ;
    ns1:hasPracticeLevel ns1:df5a0be1889a4b06835193892803dde5 ;
    ns1:hasStream ns1:27a14a265c864eb790781cd1e2bf843b .

ns1:82a962e3dcc44b1086760de517aaa3c1 a ns1:Activity ;
    rdfs:label "Establish a data catalog" ;
    dcterms:description """At this maturity level, Data Protection activities focus on actively managing your stewardship of data. Establish technical and administrative controls to protect the confidentiality of sensitive data, and the integrity and availability of all data in your care, from its initial creation/receipt through the destruction of backups at the end of their retention period.

Identify the data stored, processed, and transmitted by applications, and capture information regarding their types, sensitivity (classification) levels, and storage location(s) in your data catalog. Clearly identify records or data elements subject to specific regulation. Establishing a single source of truth regarding the data you work with supports finer-grained selection of controls for their protection. Collecting this information enhances the accuracy, timeliness, and efficiency of your responses to data-related queries (e.g., from auditors, incident response teams, or customers), and supports threat modeling and compliance activities.

Based on your Data Protection Policy, establish processes and procedures for protecting and preserving data throughout their lifetime, whether at rest, while being processed, or in transit. Pay particular attention to the handling and protection of sensitive data outside the active processing system, including, but not limited to: storage, retention, and destruction of backups; and the labeling, encryption, and physical protection of offline storage media. Your processes and procedures cover the implementation of all controls adopted to comply with regulatory, contractual, or other restrictions on storage locations, personnel access, and other factors.
""" ;
    dcterms:identifier "82a962e3dcc44b1086760de517aaa3c1" ;
    rdfs:comment "Develop data catalog and establish data protection policy." ;
    rdfs:seeAlso <https://owaspsamm.org/model/operations/operational-management/stream-a> ;
    skos:altLabel "O-OM-2-A" ;
    ns1:benefit "Standardized handling of different classes of sensitive data" ;
    ns1:hasPracticeLevel ns1:76f8a2e68065467ba9bd2b5ac625490b ;
    ns1:hasStream ns1:9c6bf45a97ae4149a44c4a5d97ea6a40 .

ns1:84dcbc954d954d95b1fb37e032f05402 a ns1:Activity ;
    rdfs:label "Establish hardening baselines" ;
    dcterms:description """Establish configuration hardening baselines for all components in each technology stack used. To assist with consistent application of the hardening baselines, develop configuration guides for the components. Require product teams to apply configuration baselines to all new systems, and to existing systems when practicable.

Place hardening baselines and configuration guides under change management, and assign an owner to each. Owners have ongoing responsibility to keep them up-to-date, based on evolving best practices or changes to the relevant components (e.g., version updates, new features).

In larger environments, derive configurations of instances from a locally maintained master, with relevant configuration baselines applied. Employ automated tools for hardening configurations.
""" ;
    dcterms:identifier "84dcbc954d954d95b1fb37e032f05402" ;
    rdfs:comment "Perform consistent hardening of configurations, following established baselines and guidance." ;
    rdfs:seeAlso <https://owaspsamm.org/model/operations/environment-management/stream-a> ;
    skos:altLabel "O-EM-2-A" ;
    ns1:benefit "Consistent hardening of technology stack components in your organization" ;
    ns1:hasPracticeLevel ns1:354292b7198b48bb8c4909e0d7e29f68 ;
    ns1:hasStream ns1:47bff9a57f0344eeb4b083f1c2b1bb7e .

ns1:852c76292e8a41de92205b31cb3f4e49 a ns1:Activity ;
    rdfs:label "Identify compliance requirements" ;
    dcterms:description """Create a comprehensive list of all compliance requirements, including any triggers that could help determine which applications are in scope. Compliance requirements may be considered in scope based on factors such as geographic location, types of data, or contractual obligations with clients or business partners. Review each identified compliance requirement with the appropriate experts and legal, to ensure the obligation is understood. Since many compliance obligations vary in applicability based on how the data is processed, stored, or transmitted across the computing environment, compliance drivers should always indicate opportunities for lowering the overall compliance burden by changing how the data is handled.

Evaluate publishing a compliance matrix to help identify which factors could put an application in scope for a specific regulatory requirement. Have the matrix indicate which compliance requirements are applicable at the organization level and do not depend on individual applications. The matrix provides at least a basic understanding of useful compliance requirements to review obligations around different applications.

Since many compliance standards are focused around security best-practices, many compliance requirements may already be a part of the Policy and Standards library published by the organization. Therefore, once you review compliance requirements, map them to any applicable existing policies and standards. Whenever there are discrepancies, update the policies and standards to include organization-wide compliance requirements. Then, begin creating compliance-specific standards only applicable to individual compliance requirements. The goal is to have a compliance matrix that indicates which policies and standards have more detailed information about compliance requirements, as well as ensure individual policies and standards reference applicable compliance requirements.
""" ;
    dcterms:identifier "852c76292e8a41de92205b31cb3f4e49" ;
    rdfs:comment "Identify 3rd-party compliance drivers and requirements and map to existing policies and standards." ;
    rdfs:seeAlso <https://owaspsamm.org/model/governance/policy-and-compliance/stream-b> ;
    skos:altLabel "G-PC-1-B" ;
    ns1:benefit "Security policies and standards aligned with external compliance drivers" ;
    ns1:hasPracticeLevel ns1:437d447b3f11427592e938dbde53c7da ;
    ns1:hasStream ns1:2919e1f19aec4f018da94a3e8733f37d .

ns1:857a43e335ba467598eca99d48ea0076 a ns1:Activity ;
    rdfs:label "Review application dependencies for security" ;
    dcterms:description """Evaluate used dependencies and establish a list of acceptable ones approved for use within a project, team, or the wider organization according to a defined set of criteria.

Introduce a central repository of dependencies that all software can be built from.

Review used dependencies regularly to ensure that&#58;

* they remain correctly licensed
* no known and significant vulnerabilities impacting your applications are present
* the dependency is still actively supported and maintained
* you are using a current version
* there is a valid reason to include the dependency

React timely and appropriately to non-conformities by handling these as defects. Consider using an automated tool to scan for vulnerable dependencies and assign the identified issues to the respective development teams.
""" ;
    dcterms:identifier "857a43e335ba467598eca99d48ea0076" ;
    rdfs:comment "Evaluate used dependencies and ensure timely reaction to situations posing risk to your applications." ;
    rdfs:seeAlso <https://owaspsamm.org/model/implementation/secure-build/stream-b> ;
    skos:altLabel "I-SB-2-B" ;
    ns1:benefit "Full transparency of known security issues in dependencies" ;
    ns1:hasPracticeLevel ns1:46f16450b23d4c29a5cf19b056c2636e ;
    ns1:hasStream ns1:2f7b501627954c6cb03342196b2065a7 .

ns1:8ab46d242edd413d99a6c1991aef2416 a ns1:Activity ;
    rdfs:label "Review application lifecycle state regularly" ;
    dcterms:description """Regularly evaluate the lifecycle state and support status of every software asset and underlying infrastructure component, and estimate their end-of-life. Follow a well-defined process for actively mitigating security risks arising as assets/components approach their end-of-life. Regularly review and update your process, to reflect lessons learned.

Establish a product support plan, providing clear timelines for ending support on older product versions. Limit product versions in active use to only a small number (e.g., N.x.x and N-1.x.x only). Establish and publicize timelines for discontinuing support on prior versions, and proactively engage with customers and user groups to prevent disruption of service or support.
""" ;
    dcterms:identifier "8ab46d242edd413d99a6c1991aef2416" ;
    rdfs:comment "Proactively manage migration roadmaps, for both unsupported end-of-life dependencies, and legacy versions of delivered software." ;
    rdfs:seeAlso <https://owaspsamm.org/model/operations/operational-management/stream-b> ;
    skos:altLabel "O-OM-3-B" ;
    ns1:benefit "Full visibility into lifecycle of all software assets" ;
    ns1:hasPracticeLevel ns1:2a059c7d07c34b9897e49e6295501608 ;
    ns1:hasStream ns1:a0d2ec4c6daa43369c07644b8745a7bd .

ns1:91086153b98b46928e36dd031b27bdc2 a ns1:Activity ;
    rdfs:label "Identify security requirements" ;
    dcterms:description """Perform a review of the functional requirements of the software project. Identify relevant security requirements (i.e. expectations) for this functionality by reasoning on the desired confidentiality, integrity or availability of the service or data offered by the software project. Requirements state the objective (e.g., “personal data for the registration process should be transferred and stored securely”), but not the actual measure to achieve the objective (e.g., “use TLSv1.2 for secure transfer”).

At the same time, review the functionality from an attacker perspective to understand how it could be misused. This way you can identify extra protective requirements for the software project at hand.

Security objectives can relate to specific security functionality you need to add to the application (e.g., “Identify the user of the application at all times”) or to the overall application quality and behavior (e.g., “Ensure personal data is properly protected in transit”), which does not necessarily lead to new functionality. Follow good practices for writing security requirements. Make them specific, measurable, actionable, relevant and time-bound (SMART). Beware of adding requirements too general-purpose to not relate to the application at hand (e.g., The application should protect against the OWASP Top 10). While they can be true, they don’t add value to the discussion.
""" ;
    dcterms:identifier "91086153b98b46928e36dd031b27bdc2" ;
    rdfs:comment "High-level application security objectives are mapped to functional requirements." ;
    rdfs:seeAlso <https://owaspsamm.org/model/design/security-requirements/stream-a> ;
    skos:altLabel "D-SR-1-A" ;
    ns1:benefit "Understanding of key security requirements during development" ;
    ns1:hasPracticeLevel ns1:3d035b6df77f4ee69577c9b4c9d64891 ;
    ns1:hasStream ns1:7fb68bc660774b9080963c17761529a2 .

ns1:921ff24f0b9f4df9a5129aa2f8a4a570 a ns1:Activity ;
    rdfs:label "Perform automated security testing" ;
    dcterms:description """Use automated static and dynamic security test tools for software, resulting in more efficient security testing and higher quality results. Progressively increase the frequency of security tests and extend code coverage.

Application security testing can be performed statically, by inspecting an application's source code without running it, or dynamically by simply observing the application's behavior in response to various input conditions. The former approach is often referred to as Static Application Security Testing (SAST), the latter as Dynamic Application Security Testing (DAST). A hybrid approach, known as Interactive Application Security Testing (IAST), combines the strengths of both approaches (at the cost of additional overhead) by dynamically testing automatically instrumented applications, allowing accurate monitoring of the application's internal state in response to external input.

Many security vulnerabilties are very hard to detect without carefully inspecting the source code. While this is ideally performed by expert or peer review, it is a slow and expensive task. Although "noisier" and frequently less accurate than expert-led reviews, automated SAST tools are cheaper, much faster, and more consistent than humans. A number of commercial and free tools are able to efficiently detect sufficiently important bugs and vulnerabilities in large code bases.

Dynamic testing does not require application source code, making it ideal for cases where source code is not available. It also identifies concrete instances of vulnerabilities. Due to its "black-box" approach , without instrumentation, it is more likely to uncover shallow bugs. Dynamic testing tools need a large source of test data whose manual test generation is prohibitive. Many tools exist which generate suitable test data automatically, leading to more efficient security testing and higher quality results.

Select appropriate tools based on several factors, including depth and accuracy of inspection, robustness and accuracy of security test cases, available integrations with other tools, usage and cost model, etc. When selecting tools, use input from security-savvy technical staff as well as developers and development managers and review results with stakeholders.
""" ;
    dcterms:identifier "921ff24f0b9f4df9a5129aa2f8a4a570" ;
    rdfs:comment "Utilize automated security testing tools" ;
    rdfs:seeAlso <https://owaspsamm.org/model/verification/security-testing/stream-a> ;
    skos:altLabel "V-ST-1-A" ;
    ns1:benefit "Detection of common easy-to-find vulnerabilities" ;
    ns1:hasPracticeLevel ns1:d6cefe3e63d149299fb088010c24778b ;
    ns1:hasStream ns1:102fdab651834273abd67a3ec27aab05 .

ns1:93ccc4cdf5d841e3986f3684467b2bf1 a ns1:Activity ;
    rdfs:label "Train all stakeholders for awareness" ;
    dcterms:description """Conduct security awareness training for all roles currently involved in the management, development, testing, or auditing of the software. The goal is to increase the awareness of application security threats and risks, security best practices, and secure software design principles. Develop training internally or procure it externally. Ideally, deliver training in person so participants can have discussions as a team, but Computer-Based Training (CBT) is also an option.

Course content should include a range of topics relevant to application security and privacy, while remaining accessible to a non-technical audience. Suitable concepts are secure design principles including Least Privilege, Defense-in-Depth, Fail Secure (Safe), Complete Mediation, Session Management, Open Design, and Psychological Acceptability. Additionally, the training should include references to any organization-wide standards, policies, and procedures defined to improve application security. The OWASP Top 10 vulnerabilities should be covered at a high level.

Training is mandatory for all employees and contractors involved with software development and includes an auditable sign-off to demonstrate compliance. Consider incorporating innovative ways of delivery (such as gamification) to maximize its effectiveness and combat desensitization.
""" ;
    dcterms:identifier "93ccc4cdf5d841e3986f3684467b2bf1" ;
    rdfs:comment "Provide security awareness training for all personnel involved in software development" ;
    rdfs:seeAlso <https://owaspsamm.org/model/governance/education-and-guidance/stream-a> ;
    skos:altLabel "G-EG-1-A" ;
    ns1:benefit "Basic security awareness for all relevant employees" ;
    ns1:hasPracticeLevel ns1:38f3a2f7633c42b98eb160f36a2c0a7b ;
    ns1:hasStream ns1:7344f4b153314dd8965361d23772aef1 .

ns1:93dff7be5f954f8d87d24f4261002508 a ns1:Activity ;
    rdfs:label "Track security defects centrally" ;
    dcterms:description """Introduce a common definition / understanding of a security defect and define the most common ways of identifying these. These typically include, but are not limited to:

* Threat assessments
* Penetration tests
* Output from static and dynamic analysis scanning tools
* Responsible disclosure processes or bug bounties

Foster a culture of transparency and avoid blaming any teams for introducing or identifying security defects. Record and track all security defects in a defined location. This location doesn't necessarily have to centralized for the whole organization, however ensure that you're able to get an overview of all defects affecting a particular application at any single point in time. Define and apply access rules for the tracked security defects to mitigate the risk of leakage and abuse of this information.

Introduce at least rudimentary qualitative classificiation of security defects so that you are able to prioritize fixing efforts accordingly. Strive for limiting duplication of information and presence of false positives to increase the trustworthiness of the process.
""" ;
    dcterms:identifier "93dff7be5f954f8d87d24f4261002508" ;
    rdfs:comment "Introduce a structured tracking of security defects and make knowledgeable decisions based on this information." ;
    rdfs:seeAlso <https://owaspsamm.org/model/implementation/defect-management/stream-a> ;
    skos:altLabel "I-DM-1-A" ;
    ns1:benefit "Transparency of known security defects impacting particular applications" ;
    ns1:hasPracticeLevel ns1:97a46a074fe849a1af2c2d2d3dd09ba5 ;
    ns1:hasStream ns1:a5b57fc5fa0441b7b23f599b506c5752 .

ns1:994bcac2bb7c4cc59a0faa365a0b58a0 a ns1:Activity ;
    rdfs:label "Use a repeatable deployment process" ;
    dcterms:description """Define the deployment process over all stages, breaking it down into a set of clear instructions to either be followed by a person or an automated tooling. The deployment process definition should describe the whole process end-to-end so that it can be consistently followed each time to produce the same result. The definition is stored centrally and accessible to all relevant personnel. Do not store or distribute multiple copies, some of which may become outdated.

Deploy applications to production either using an automated process, or manually by personnel other than the developers. Ensure that developers do not need direct access to the production environment for application deployment.

Review any deployment tools, ensuring that they are actively maintained by vendors and up to date with security patches. Harden each tool’s configuration so that it is aligned with vendor guidelines and industry best practices. Given that most of these tools require access to the production environment, their security is extremely critical. Ensure the integrity of the tools themselves and the workflows they follow, and configure access rules to these tools according to the least privilege principle.

Have personnel with access to the production environment go through at least a minimum level of training or certification to ensure their competency in this matter.
""" ;
    dcterms:identifier "994bcac2bb7c4cc59a0faa365a0b58a0" ;
    rdfs:comment "Formalize the deployment process and secure the used tooling and processes." ;
    rdfs:seeAlso <https://owaspsamm.org/model/implementation/secure-deployment/stream-a> ;
    skos:altLabel "I-SD-1-A" ;
    ns1:benefit "Limited risk of human error during deployment process minimizing security issues" ;
    ns1:hasPracticeLevel ns1:5015427608de428cba3c324772fb4191 ;
    ns1:hasStream ns1:9ec70d6f7ddb4cb6b37928f9994c6049 .

ns1:9951bda24b624cc684a2851f9d56c5d8 a ns1:Activity ;
    rdfs:label "Define and run security test cases from requirements" ;
    dcterms:description """From the security requirements, identify and implement a set of security test cases to check the software for correct functionality. To have a successful testing program, you must know the testing objectives, specified by the security requirements.

Derive security test cases for the applications in scope from the security requirements created as part of the "Security Requirements" SAMM security practice. To validate security requirements with security tests, security requirements are function-driven and highlight the expected functionality (the what) and, implicitly, the implementation (the how). These requirements are also referred to as "positive requirements", since they state the expected functionality that can be validated through security tests. Examples of positive requirements include “the application will lockout the user after six failed login attempts” or “passwords need to be a minimum of six alphanumeric characters”. The validation of positive requirements consists of asserting the expected functionality. You can do it re-creating the testing conditions and running the test according to predefined inputs. Show the results as as a fail or pass condition.

Often, it is most effective to use the project team’s time to build application-specific test cases, and publicly available resources or purchased knowledge bases to select applicable general test cases for security. Relevant development, security, and quality assurance staff review candidate test cases for applicability, efficacy, and feasibility. Derive the test cases during the requirements and/or design phase of the functionality. Testing the security requirements is part of the functional testing of the software.
""" ;
    dcterms:identifier "9951bda24b624cc684a2851f9d56c5d8" ;
    rdfs:comment "Derive test cases from known security requirements" ;
    rdfs:seeAlso <https://owaspsamm.org/model/verification/requirements-driven-testing/stream-a> ;
    skos:altLabel "V-RT-2-A" ;
    ns1:benefit "Integration of security requirements into test scenarios" ;
    ns1:hasPracticeLevel ns1:3e6e9a2b696e48018830b44fa96f98b5 ;
    ns1:hasStream ns1:efb5d1f275504173899da345ef5bbe8e .

ns1:99989f86dabc4a7a87fbe6a274c99ca3 a ns1:Activity ;
    rdfs:label "Test the effectiveness of security controls" ;
    dcterms:description """Conduct security tests to verify that the standard software security controls operate as expected. At a high level, this means testing the correct functioning of the confidentiality, integrity, and availability controls of the data as well as the service. Security tests at least include testing for authentication, access control, input validation, encoding, and escaping data and encryption controls. The test objective is to validate that the security controls are correctly implemented.

The security testing validates the relevant software security controls. Perform control-verification security tests manually or with tools, each time the application changes its use of the controls. Techniques such as feature toggles and A/B testing can be used to progressively expose features to broader audiences as they are sufficiently validated. Software control verification is mandatory for all software that is part of the SAMM program.
""" ;
    dcterms:identifier "99989f86dabc4a7a87fbe6a274c99ca3" ;
    rdfs:comment "Test for software security controls" ;
    rdfs:seeAlso <https://owaspsamm.org/model/verification/requirements-driven-testing/stream-a> ;
    skos:altLabel "V-RT-1-A" ;
    ns1:benefit "Verified effectiveness of your standard security controls" ;
    ns1:hasPracticeLevel ns1:df5a0be1889a4b06835193892803dde5 ;
    ns1:hasStream ns1:efb5d1f275504173899da345ef5bbe8e .

ns1:9b6a86278ba14a9098d3d60a9a78d6c5 a ns1:Activity ;
    rdfs:label "Provide preferred security solutions" ;
    dcterms:description """Identify shared infrastructure or services with security functionality. These typically include single-sign-on services, access control or entitlements services, logging and monitoring services or application-level firewalling. Collect and evaluate reusable systems to assemble a list of such resources and categorize them by the security mechanism they fulfill. Consider each resource in terms of why a product team would want to integrate with it, i.e. the benefits of using the shared resource.

If multiple resources exist in each category, select and standardize on one or more shared service per category. Because future software development will rely on these services, review each thoroughly to ensure understanding of the baseline security posture. For each selected service, create design guidance for product teams to understand how to integrate with the system. Make the guidance available through training, mentorship, guidelines, and standards.

Establish a set of best practices representing sound methods of implementing security functionality. You can research them or purchase them, and it is often more effective if you customize them so they are more specific to your organization. Example patterns include a single-sign-on subsystem, a cross-tier delegation model, a separation-of-duties authorization model, a centralized logging pattern, etc.

These patterns can originate from specific projects or applications, but make sure you share them between different teams across the organization for efficient and consistent application of appropriate security solutions.

To increase adoption of these patterns, link them to the shared security services, or implement them into actual component solutions that can be easily integrated into an application during development. Support the key technologies within the organization, for instance in case of different development stacks. Treat these solutions as actual applications with proper support in case of questions or issues.
""" ;
    dcterms:identifier "9b6a86278ba14a9098d3d60a9a78d6c5" ;
    rdfs:comment "Establish common design patterns and security solutions for adoption." ;
    rdfs:seeAlso <https://owaspsamm.org/model/design/security-architecture/stream-a> ;
    skos:altLabel "D-SA-2-A" ;
    ns1:benefit "Reusable security services available for product teams" ;
    ns1:hasPracticeLevel ns1:41c8e63716c34f1eaf09b8cad70cfbaf ;
    ns1:hasStream ns1:253b012094cf4e0988e08fd22609227d .

ns1:9d0433c5133c4a4c9c16ae84abe9a235 a ns1:Activity ;
    rdfs:label "Verify the effectiveness of security components" ;
    dcterms:description """Review the effectiveness of the architecture components and their provided security mechanisms in terms of alignment with the overall strategy of the organization, and scrutinize the degree of availability, scalability and enterprise-readiness of the chosen security solutions. While tactical choices for a particular application can make sense in specific contexts, it is important to keep an eye on the bigger picture and ensure future readiness of the designed solution.

Feed any findings back into defect management to trigger further improvements to the architecture.
""" ;
    dcterms:identifier "9d0433c5133c4a4c9c16ae84abe9a235" ;
    rdfs:comment "Review of the architecture components' effectiveness" ;
    rdfs:seeAlso <https://owaspsamm.org/model/verification/architecture-assessment/stream-a> ;
    skos:altLabel "V-AA-3-A" ;
    ns1:benefit "Assurance of effectiveness of architecture controls" ;
    ns1:hasPracticeLevel ns1:83ea8aaab3384b41b785107613ee4d86 ;
    ns1:hasStream ns1:77ca4b5e7ebc42558109829dffc2b80d .

ns1:a061ed8a5b1c4899bc95d9b1a10a469d a ns1:Activity ;
    rdfs:label "Standardize security guidance" ;
    dcterms:description """Implement a formal training program requiring anyone involved with the software development lifecycle to complete appropriate role and technology-specific training as part of the onboarding process. Based on the criticality of the application and user’s role, consider restricting access until the onboarding training has been completed. While the organization may source some modules externally, the program is facilitated and managed in-house and includes content specific to the organization going beyond general security best practices. The program has a defined curriculum, checks participation, and tests understanding and competence. The training consists of a combination of industry best practices and organization’s internal standards, including training on specific systems used by the organization.

In addition to issues directly related to security, the organization includes other standards to the program, such as code complexity, code documentation, naming convention, and other process-related disciplines. This training minimizes issues resulting from employees following practices incorporated outside the organization and ensures continuity in the style and competency of the code.

To facilitate progress monitoring and successful completion of each training module the organization has a learning management platform or another centralized portal with similar functionality. Employees can monitor their progress and have access to all training resources even after they complete initial training.

Review issues resulting from employees not following established standards, policies, procedures, or security best practices at least annually to gauge the effectiveness of the training and ensure it covers all issues relevant to the organization. Update the training periodically and train employees on any changes and most prevalent security deficiencies.
""" ;
    dcterms:identifier "a061ed8a5b1c4899bc95d9b1a10a469d" ;
    rdfs:comment "Standardized in-house guidance around the organization’s secure software development standards." ;
    rdfs:seeAlso <https://owaspsamm.org/model/governance/education-and-guidance/stream-a> ;
    skos:altLabel "G-EG-3-A" ;
    ns1:benefit "Adequate security knowledge of all employees ensured prior to working on critical tasks" ;
    ns1:hasPracticeLevel ns1:e3cf1d3c27b74262b9f842f27ca86333 ;
    ns1:hasStream ns1:7344f4b153314dd8965361d23772aef1 .

ns1:a11da5bb4d3c475d9e9c53b104032e65 a ns1:Activity ;
    rdfs:label "Feed review results back to improve reference architectures" ;
    dcterms:description """As an organization, you can further improve your software security posture by understanding which threats remain unaddressed in the software architectures and adapting your tactics to prevent this. Formalize a process to use recurring architecture findings as a trigger to identify the causes of gaps in the security assessment and deal with them. Feed findings back to the Design phase by creating, or updating relevant reference architectures, existing security solutions, or organisation design principles and patterns.
""" ;
    dcterms:identifier "a11da5bb4d3c475d9e9c53b104032e65" ;
    rdfs:comment "Feed the architecture review results back into the enterprise architecture, organization design principles & patterns, security solutions and reference architectures." ;
    rdfs:seeAlso <https://owaspsamm.org/model/verification/architecture-assessment/stream-b> ;
    skos:altLabel "V-AA-3-B" ;
    ns1:benefit "Continuous improvement of enterprise architecture based on architecture reviews" ;
    ns1:hasPracticeLevel ns1:83ea8aaab3384b41b785107613ee4d86 ;
    ns1:hasStream ns1:b7487370a07543cbb02ddb60c055d92f .

ns1:a3720e84d6a24a8ba235c25ce6afc5c7 a ns1:Activity ;
    rdfs:label "Establish a security community" ;
    dcterms:description """Security is the responsibility of all employees, not just the Information Security team. Deploy communication and knowledge sharing platforms to help developers build communities around different technologies, tools, and programming languages. In these communities employees share information, discuss challenges with other developers, and search the knowledge base for answers to previously discussed issues.

Form communities around roles and responsibilities and enable developers and engineers from different teams and business units to communicate freely and benefit from each other's expertise. Encourage participation, set up a program to promote those who help the most people as thought leaders, and have management recognize them. In addition to improving application security, this platform may help identify future members of the Secure Software Center of Excellence, or 'Security Champions' based on their expertise and willingness to help others.

The Secure Software Center of Excellence and Application Security teams review the information portal regularly for insights into the new and upcoming technologies, as well as opportunities to assist the development community with new initiatives, tools, programs, and training resources. Use the portal to disseminate information about new standards, tools, and resources to all developers for the continued improvement of SDLC maturity and application security.
""" ;
    dcterms:identifier "a3720e84d6a24a8ba235c25ce6afc5c7" ;
    rdfs:comment "Build a secure software community including all organization people involved in software security." ;
    rdfs:seeAlso <https://owaspsamm.org/model/governance/education-and-guidance/stream-b> ;
    skos:altLabel "G-EG-3-B" ;
    ns1:benefit "Collective development of security know-how among all product teams" ;
    ns1:hasPracticeLevel ns1:e3cf1d3c27b74262b9f842f27ca86333 ;
    ns1:hasStream ns1:0e2c4c5620e24d7d8e979020ca414182 .

ns1:a395d69917b947b28d5995738d716283 a ns1:Activity ;
    rdfs:label "Establish continuous, scalable security verification" ;
    dcterms:description """Integrate security testing in parallel to all other development activities, including requirement analysis, software design and construction.

With the multiplicity of security tools running at every phase of development, remediating security issues at a designated stage (such as pre-release testing) is no longer appropriate or desirable. Security issues must be quickly triaged and fixes planned in a tradeoff between risk and cost of remediation. Continuously striving to detect issues earlier in the development lifecycle, via specific, low-friction automated tests integrated into development tools and build processes, lowers the cost of remediation thereby increasing the likelihood of issues being quickly resolved.

Proactively improve the security testing effort integrated into the development process by adequately propagating the results of other security test activities. For example, if a security penetration test identifies issues with session management, any changes to session management should trigger explicit security tests before pushing the changes to production.

Security champions and the central secure software group continuously review results from automated and manual security tests during development, including these results as part of the security awareness trainings for the development teams. Integrate lessons learned in overall playbooks to improve security testing as part of the organization development. If there are unaddressed findings that remain as accepted risks for the release, stakeholders and development managers should work together to establish a concrete timeframe for addressing them.
""" ;
    dcterms:identifier "a395d69917b947b28d5995738d716283" ;
    rdfs:comment "Integrate security testing into development process" ;
    rdfs:seeAlso <https://owaspsamm.org/model/verification/security-testing/stream-b> ;
    skos:altLabel "V-ST-3-B" ;
    ns1:benefit "Identification of manually identifiable security issues in earliest possible stages" ;
    ns1:hasPracticeLevel ns1:eac3184f8e2343b8b29047d023376da5 ;
    ns1:hasStream ns1:8a64c7b0b35a458ea436260d5e414dfa .

ns1:a573c126b3e345fba9d1d94c8158cf60 a ns1:Activity ;
    rdfs:label "Enforce timely patch management" ;
    dcterms:description """Develop and use management dashboards/reports to track compliance with patching processes and SLAs, across the portfolio. Ensure dependency management and application packaging processes can support applying component-level patches at any time, to meet required SLAs.

Treat missed updates as security-related product defects, and manage their triage and correction in accordance with your established Defect Management practice.

Don't rely on routine notifications from component vendors to learn about vulnerabilities and associated patches. Monitor a variety of external threat intelligence sources, to learn about zero day vulnerabilities; handle those affecting your applications as risk management issues.
""" ;
    dcterms:identifier "a573c126b3e345fba9d1d94c8158cf60" ;
    rdfs:comment "Actively monitor update status and manage missing patches as security defects. Proactively obtain vulnerability and update information for components." ;
    rdfs:seeAlso <https://owaspsamm.org/model/operations/environment-management/stream-b> ;
    skos:altLabel "O-EM-3-B" ;
    ns1:benefit "Clear view on component patch state to avoid non-conformities" ;
    ns1:hasPracticeLevel ns1:1cb6e197ca8245eca65b0ecbdd784720 ;
    ns1:hasStream ns1:1a7ad26d9e48411e95a63be79e1b90ea .

ns1:a9f56795ac84426c9e45f9471e82a8d7 a ns1:Activity ;
    rdfs:label "Align security methodology with suppliers" ;
    dcterms:description """The best way to minimize the risk of issues in software is to align maximally and integrate closely between the different parties. From a process perspective, this means using similar development paradigms and introducing regular milestones to ensure proper alignment and qualitative progress. From a tools perspective, this might mean using similar build, verification and deployment environments, and sharing other supporting tools (e.g. requirements, architecture tools, or code repositories).

In case suppliers cannot meet the objectives that you have set, implement compensating controls so that, overall, you meet your objectives. Execute extra activities (e.g., threat modelling before starting the actual implementation cycle) or implement extra tooling (e.g., 3rd party library analysis at solution intake). The more suppliers deviate from your requirements, the more work will be required to compensate.
""" ;
    dcterms:identifier "a9f56795ac84426c9e45f9471e82a8d7" ;
    rdfs:comment "Ensure proper security coverage for external suppliers by providing clear objectives." ;
    rdfs:seeAlso <https://owaspsamm.org/model/design/security-requirements/stream-b> ;
    skos:altLabel "D-SR-3-B" ;
    ns1:benefit "Alignment of software development practices with suppliers to limit security risks" ;
    ns1:hasPracticeLevel ns1:f8b6eebc0662477f9286aa4f6068e364 ;
    ns1:hasStream ns1:8c1dcd10821f4f2baed52fdc83d93cf6 .

ns1:aa962032982a4d53bd34cd8771558df1 a ns1:Activity ;
    rdfs:label "Build reference architectures" ;
    dcterms:description """Build a set of reference architectures that select and combine a verified set of security components to ensure a proper design of security. Reference platforms have advantages in terms of shortening audit and security-related reviews, increasing efficiency in development, and lowering maintenance overhead. Continuously maintain and improve the reference architecture based on new insights in the organization and within the community. Have architects, senior developers and other technical stakeholders participate in design and creation of reference platforms. After creation, teams maintain ongoing support and updates.

Reference architectures may materialize into a set of software libraries and tools upon which project teams build their software. They serve as a starting point that standardizes the configuration-driven, security-by-default security approach. You can bootstrap the framework by selecting a particular project early in the lifecycle and having security-savvy staff work with them to build the security functionality in a generic way so that it can be extracted from the project and used elsewhere in the organization.

Monitor weaknesses or gaps in the set of security solutions available in your organization continuously in the context of discussions on architecture, development, or operations. This serves as an input to improve the appropriateness and effectiveness of the reference architectures that you have in place.
""" ;
    dcterms:identifier "aa962032982a4d53bd34cd8771558df1" ;
    rdfs:comment "Reference architectures are utilized and continuously evaluated for adoption and appropriateness." ;
    rdfs:seeAlso <https://owaspsamm.org/model/design/security-architecture/stream-a> ;
    skos:altLabel "D-SA-3-A" ;
    ns1:benefit "Full transparency of quality and usability of centrally provided security solutions" ;
    ns1:hasPracticeLevel ns1:9d1e469966124c0fa80d1bc2fc223a0a ;
    ns1:hasStream ns1:253b012094cf4e0988e08fd22609227d .

ns1:b082664b8815407d825b82cf23fa88ea a ns1:Activity ;
    rdfs:label "Create an incident response plan" ;
    dcterms:description """The first step is to recognize the incident response competence as such, and define a responsible owner. Provide them the time and resources they need to keep up with current state of incident handling best practices and forensic tooling.

At this level of maturity, you may not have established a dedicated incident response team, but you have defined the participants of the process (usually different roles). Assign a single point of contact for the process, known to all relevant stakeholders. Ensure that the point of contact knows how to reach each participant, and define on-call responsibilities for those who have them.

When security incidents happen, document all actions taken. Protect this information from unauthorized access.
""" ;
    dcterms:identifier "b082664b8815407d825b82cf23fa88ea" ;
    rdfs:comment "Identify roles and responsibilities for incident response." ;
    rdfs:seeAlso <https://owaspsamm.org/model/operations/incident-management/stream-b> ;
    skos:altLabel "O-IM-1-B" ;
    ns1:benefit "Ability to efficiently solve most common security incidents" ;
    ns1:hasPracticeLevel ns1:817dd6acaf85496aa005393e0e6c3e70 ;
    ns1:hasStream ns1:390bec725b8344a289d5386026925947 .

ns1:b3b20a75740c4880a21ad9aa0c1298c7 a ns1:Activity ;
    rdfs:label "Test high risk application components manually" ;
    dcterms:description """Perform selective manual security testing, possibly using a combination of static and dynamic analysis tools to guide or focus the review, in order to more thoroughly analyze parts of the application, as an attacker. Automated tools are effective at finding various types of vulnerabilities but can never replace expert manual review.

Code-level vulnerabilities in security-critical parts of software can have dramatically increased impact so project teams review high-risk modules for common vulnerabilities. Common examples of high-risk functionality include authentication modules, access control enforcement points, session management schemes, external interfaces, and input validators and data parsers. Teams can combine code-level metrics and focused automated scans to determine where best to focus their efforts. In practice, the activity can take many forms including pair programming and peer review, time-boxed security "pushes" involving the entire development team, or spontaneous independent reviews by members of a specialised security group.

During development cycles where high-risk code is changed and reviewed, development managers triage the findings and prioritize remediation appropriately with input from other project stakeholders.
""" ;
    dcterms:identifier "b3b20a75740c4880a21ad9aa0c1298c7" ;
    rdfs:comment "Perform manual security testing of high-risk components" ;
    rdfs:seeAlso <https://owaspsamm.org/model/verification/security-testing/stream-b> ;
    skos:altLabel "V-ST-1-B" ;
    ns1:benefit "Detection of manually identifiable vulnerabilities in critical components" ;
    ns1:hasPracticeLevel ns1:d6cefe3e63d149299fb088010c24778b ;
    ns1:hasStream ns1:8a64c7b0b35a458ea436260d5e414dfa .

ns1:b7f1d18fbe724a148f039ce036de98ef a ns1:Activity ;
    rdfs:label "Formalize patch management" ;
    dcterms:description """Develop and follow a well-defined process for managing patches to application components across the technology stacks in use. Ensure processes include regular schedules for applying vendor updates, aligned with vendor update calendars (e.g., Microsoft Patch Tuesday). For software developed by the organization, deliver releases to customers and organization-managed solutions on a regular basis (e.g., monthly), regardless of whether you are including new features.

Create guidance for prioritizing component patching, reflecting your risk tolerance and management objectives. Consider operational factors (e.g., criticality of the application, severity of the vulnerabilities addressed) in determining priorities for testing and applying patches.

In the event receive a notification for a critical vulnerability in a component, while no patch is yet available, triage and handle the situation as a risk management issue (e.g., implement compensating controls, obtain customer risk acceptance, or disable affected applications/features).
""" ;
    dcterms:identifier "b7f1d18fbe724a148f039ce036de98ef" ;
    rdfs:comment "Perform regular patching of system and application components, across the full stack. Ensure timely delivery of patches to customers." ;
    rdfs:seeAlso <https://owaspsamm.org/model/operations/environment-management/stream-b> ;
    skos:altLabel "O-EM-2-B" ;
    ns1:benefit "Consistent and proactive patching of technology stack components" ;
    ns1:hasPracticeLevel ns1:354292b7198b48bb8c4909e0d7e29f68 ;
    ns1:hasStream ns1:1a7ad26d9e48411e95a63be79e1b90ea .

ns1:b8dfd23d66224ac88d3ce41cf83ed15e a ns1:Activity ;
    rdfs:label "Use best-effort incident detection" ;
    dcterms:description """Analyze available log data (e.g., access logs, application logs, infrastructure logs), to detect possible security incidents in accordance with known log data retention periods.

In small setups, you can do this manually with the help of common command-line tools. With larger log volumes, employ automation techniques. Even a `cron` job, running a simple script to look for suspicious events, is a step forward!

If you send logs from different sources to a dedicated log aggregation system, analyze the logs there and employ basic log correlation principles.

Even if you don't have a 24/7 incident detection process, ensure that unavailability of the responsible person (e.g., due to vacation or illness) doesn't significantly impact detection speed or quality.

Establish and share points of contact for formal creation of security incidents.
""" ;
    dcterms:identifier "b8dfd23d66224ac88d3ce41cf83ed15e" ;
    rdfs:comment "Use available log data to perform best-effort detection of possible security incidents." ;
    rdfs:seeAlso <https://owaspsamm.org/model/operations/incident-management/stream-a> ;
    skos:altLabel "O-IM-1-A" ;
    ns1:benefit "Ability to detect the most obvious security incidents" ;
    ns1:hasPracticeLevel ns1:817dd6acaf85496aa005393e0e6c3e70 ;
    ns1:hasStream ns1:ff8a6a08dc684f38ab74b9db9584f0a5 .

ns1:bcc960e835aa4ad58a9d39a272cbf6f1 a ns1:Activity ;
    rdfs:label "Automate the build process" ;
    dcterms:description """Automate the build process so that builds can be executed consistently anytime. The build process shouldn't typically require any intervention, further reducing the likelihood of human error.

The use of an automated system increases reliance on security of the build tooling and makes hardening and maintaining the toolset even more critical. Pay particular attention to the interfaces of those tools, such as web-based portals and how they can be locked-down. The exposure of a build tool to the network could allow a malicious actor to tamper with the integrity of the process. This might, for example, allow malicious code to be built into software.

The automated process may require access to credentials and secrets required to build the software, such as the code signing certificate or access to repositories. Handle these with care. Sign generated artifacts using a certificate that identifies the organization or business unit that built it, so you can verify its integrity.

Finally, add appropriate automated security checks (e.g. using SAST tools) in the pipeline to leverage the automation for security benefit.
""" ;
    dcterms:identifier "bcc960e835aa4ad58a9d39a272cbf6f1" ;
    rdfs:comment "Automate your build pipeline and secure the used tooling. Add security checks in the build pipeline." ;
    rdfs:seeAlso <https://owaspsamm.org/model/implementation/secure-build/stream-a> ;
    skos:altLabel "I-SB-2-A" ;
    ns1:benefit "Efficient build process with integrated security tools" ;
    ns1:hasPracticeLevel ns1:46f16450b23d4c29a5cf19b056c2636e ;
    ns1:hasStream ns1:8a870a9b26724b4ba0dff177028b474a .

ns1:bed0489cae4e4401b1d44d56ad36c109 a ns1:Activity ;
    rdfs:label "Identify application dependencies" ;
    dcterms:description """Keep a record of all dependencies used throughout the target production environment. This is sometimes referred to as a Bill of Materials (BOM). Consider that different components of the application may consume entirely different dependencies. For example, if the software package is a web application, cover both the server-side application code and client-side scripts. In building these records, consider the various locations where dependencies might be specified such as configuration files, the project's directory on disk, a package management tool or the actual code (e.g. via an IDE that supports listing dependencies).

Gather the following information about each dependency&#58;

* Where it is used or referenced
* Version used
* License
* Source information (link to repository, author's name, etc.)
* Support and maintenance status of the dependency

Check the records to discover any dependencies with known vulnerabilities and update or replace them accordingly.
""" ;
    dcterms:identifier "bed0489cae4e4401b1d44d56ad36c109" ;
    rdfs:comment "Create records with Bill of Materials of your applications and opportunistically analyze these." ;
    rdfs:seeAlso <https://owaspsamm.org/model/implementation/secure-build/stream-b> ;
    skos:altLabel "I-SB-1-B" ;
    ns1:benefit "Available information on known security issues in dependencies" ;
    ns1:hasPracticeLevel ns1:b29ab542cc674901a19cf5f3c0c4be18 ;
    ns1:hasStream ns1:2f7b501627954c6cb03342196b2065a7 .

ns1:bf536a9305134a769adbd414652054ee a ns1:Activity ;
    rdfs:label "Define a consistent build process" ;
    dcterms:description """Define the build process, breaking it down into a set of clear instructions to either be followed by a person or an automated tool. The build process definition describes the whole process end-to-end so that the person or tool can follow it consistently each time and produce the same result. The definition is stored centrally and accessible to any tools or people. Avoid storing multiple copies as they may become unaligned and outdated.

The process definition does not include any secrets (specifically considering those needed during the build process).

Review any build tools, ensuring that they are actively maintained by vendors and up-to-date with security patches. Harden each tool’s configuration so that it is aligned with vendor guidelines and industry best practices.

Determine a value for each generated artifact that can be later used to verify its integrity, such as a signature or a hash. Protect this value and, if the artifact is signed, the private signing certificate.

Ensure that build tools are routinely patched and properly hardened.
""" ;
    dcterms:identifier "bf536a9305134a769adbd414652054ee" ;
    rdfs:comment "Create a formal definition of the build process so that it becomes consistent and repeatable." ;
    rdfs:seeAlso <https://owaspsamm.org/model/implementation/secure-build/stream-a> ;
    skos:altLabel "I-SB-1-A" ;
    ns1:benefit "Limited risk of human error during build process minimizing security issues" ;
    ns1:hasPracticeLevel ns1:b29ab542cc674901a19cf5f3c0c4be18 ;
    ns1:hasStream ns1:8a870a9b26724b4ba0dff177028b474a .

ns1:c16a12399dc94cc889d7e9e66e0ae2a0 a ns1:Activity ;
    rdfs:label "Organize basic data protections" ;
    dcterms:description """Understand the types and sensitivity of data stored and processed by your applications, and maintain awareness of the fate of processed data (e.g., backups, sharing with external partners). At this level of maturity, the information gathered may be captured in varying forms and different places; no organization-wide data catalog is assumed to exist. Protect and handle all data associated with a given application according to protection requirements applying to the most sensitive data stored and processed.

Implement basic controls, to prevent propagation of unsanitized sensitive data from production environments to lower environments. By ensuring unsanitized production data are never propagated to lower (non-production) environments, you can focus data protection policies and activities on production.
""" ;
    dcterms:identifier "c16a12399dc94cc889d7e9e66e0ae2a0" ;
    rdfs:comment "Implement basic data protection practices" ;
    rdfs:seeAlso <https://owaspsamm.org/model/operations/operational-management/stream-a> ;
    skos:altLabel "O-OM-1-A" ;
    ns1:benefit "Understanding of sensitivity of processed data with derived quick-win measures" ;
    ns1:hasPracticeLevel ns1:d0a99f3db27e48aa9b2d6b58a9040f49 ;
    ns1:hasStream ns1:9c6bf45a97ae4149a44c4a5d97ea6a40 .

ns1:c1778728d66e4b83b59a42405a90598a a ns1:Activity ;
    rdfs:label "Define the security strategy" ;
    dcterms:description """Based on the magnitude of assets, threats, and risk tolerance, develop a security strategic plan and budget to address business priorities around application security. The plan covers 1 to 3 years and includes milestones consistent with the organization’s business drivers and risks. It provides tactical and strategic initiatives and follows a roadmap that makes its alignment with business priorities and needs visible.

In the roadmap, you reach a balance between changes requiring financial expenditures, changes of processes and procedures, and changes impacting the organization’s culture. This balance helps accomplish multiple milestones concurrently and without overloading or exhausting available resources or development teams. The milestones are frequent enough to help monitor program success and trigger timely roadmap adjustments.

For the program to be successful, the application security team obtains buy-in from the organization’s stakeholders and application development teams. A published plan is available to anyone who is required to support or participate in its implementation.
""" ;
    dcterms:identifier "c1778728d66e4b83b59a42405a90598a" ;
    rdfs:comment "Publish a unified strategy for application security." ;
    rdfs:seeAlso <https://owaspsamm.org/model/governance/strategy-and-metrics/stream-a> ;
    skos:altLabel "G-SM-2-A" ;
    ns1:benefit "Available and agreed upon roadmap of your AppSec program" ;
    ns1:hasPracticeLevel ns1:561e85a7fb114b1d976acce95d0b41ee ;
    ns1:hasStream ns1:94bb47791e3d462cbf5f71ebb1a1327a .

ns1:c1aef0137df1400cbdd3c660b609b7b2 a ns1:Activity ;
    rdfs:label "Set strategic KPIs" ;
    dcterms:description """Once the organization has defined its application security metrics, collect enough information to establish realistic goals. Test identified metrics to ensure you can gather data consistently and efficiently over a short period. After the initial testing period, the organization should have enough information to commit to goals and objectives expressed through Key Performance Indicators (KPIs).

While several measurements are useful for monitoring the information security program and its effectiveness, KPIs are comprised of the most meaningful and effective metrics. Aim to remove volatility common in application development environments from KPIs to reduce chances of unfavorable numbers resulting from temporary or misleading individual measurements. Base KPIs on metrics considered valuable not only to Information Security professionals but also to individuals responsible for the overall success of the application, and organization’s leadership. View KPIs as definitive indicators of the success of the whole program and consider them actionable.

Fully document KPIs and distribute them to the teams contributing to the success of the program as well as organization’s leadership. Ideally, include a brief explanation of the information sources for each KPI and the meaning if the numbers are high or low. Include short and long-term goals, and ranges for unacceptable measurements requiring immediate intervention. Share action plans with application security and application development teams to ensure full transparency in understanding of the organization’s objectives and goals.
""" ;
    dcterms:identifier "c1aef0137df1400cbdd3c660b609b7b2" ;
    rdfs:comment "Set targets and KPI’s for measuring the program effectiveness." ;
    rdfs:seeAlso <https://owaspsamm.org/model/governance/strategy-and-metrics/stream-b> ;
    skos:altLabel "G-SM-2-B" ;
    ns1:benefit "Transparency on your AppSec program's performance" ;
    ns1:hasPracticeLevel ns1:561e85a7fb114b1d976acce95d0b41ee ;
    ns1:hasStream ns1:2f1cac3c2e724823b3b48a7e797520b4 .

ns1:c6da6525773644d0a18b3a927caf6dd2 a ns1:Activity ;
    rdfs:label "Perform application risk assessments" ;
    dcterms:description """Use a simple method to evaluate the application risk per application, estimating the potential business impact that it poses for the organization in case of an attack. To achieve this, evaluate the impact of a breach in the confidentiality, integrity and availability of the data or service. Consider using a set of 5-10 questions to understand important application characteristics, such as whether the application processes financial data, whether it is internet facing, or whether privacy-related data is involved. The application risk profile tells you whether these factors are applicable and if they could significatly impact the organization.

Next, use a scheme to classify applications according to this risk. A simple, qualitative scheme (e.g. high/medium/low) that translates these characteristics into a value is often effective. It is important to use these values to represent and compare the risk of different applications against each other. Mature highly risk-driven organizations might make use of more quantitative risk schemes. Don’t invent a new risk scheme if your organization already has one that works well.
""" ;
    dcterms:identifier "c6da6525773644d0a18b3a927caf6dd2" ;
    rdfs:comment "A basic assessment of the application risk is performed to understand likelihood and impact of an attack." ;
    rdfs:seeAlso <https://owaspsamm.org/model/design/threat-assessment/stream-a> ;
    skos:altLabel "D-TA-1-A" ;
    ns1:benefit "Ability to classify applications according to risk" ;
    ns1:hasPracticeLevel ns1:a3d4045d5c0c4bd4a875784759539f0c ;
    ns1:hasStream ns1:17c90203f8354c3594eea22759e375a9 .

ns1:cd80066899014962a37af7ab34c83003 a ns1:Activity ;
    rdfs:label "Respond to data breaches" ;
    dcterms:description """Activities at this maturity level are focused on automating data protection, reducing your reliance on human effort to assess and manage compliance with policies. There is a focus on feedback mechanisms and proactive reviews, to identify and act on opportunities for process improvement.

Implement technical controls to enforce compliance with your Data Protection Policy, and put monitoring in place to detect attempted or actual violations. You may use a variety of available tools for data loss prevention, access control and tracking, or anomalous behavior detection.

Regularly audit compliance with established administrative controls, and closely monitor performance and operation of automated mechanisms, including backups and record deletions. Monitoring tools quickly detect and report failures in automation, permitting you to take timely corrective action.

Reviews and update the data catalog regularly, to maintain its accurate reflection of your data landscape. Regular reviews and updates of processes and procedures maintain their alignment with your policies and priorities.
""" ;
    dcterms:identifier "cd80066899014962a37af7ab34c83003" ;
    rdfs:comment "Automate detection of policy non-compliance, and audit compliance periodically. Regularly review and update to data catalog and data protection policy." ;
    rdfs:seeAlso <https://owaspsamm.org/model/operations/operational-management/stream-a> ;
    skos:altLabel "O-OM-3-A" ;
    ns1:benefit "Technically enforced compliance with your data protection policy" ;
    ns1:hasPracticeLevel ns1:2a059c7d07c34b9897e49e6295501608 ;
    ns1:hasStream ns1:9c6bf45a97ae4149a44c4a5d97ea6a40 .

ns1:ce13df2e0dfb455588bf75135f1a718e a ns1:Activity ;
    rdfs:label "Develop a security requirements framework" ;
    dcterms:description """Setup a security requirements framework to help projects elicit an appropriate and complete requirements set for their project. This framework considers the different types of requirements and sources of requirements. It should be adapted to the organizational habits and culture, and provide effective methodology and guidance in the elicitation and formation of requirements.

The framework helps project teams increase the efficiency and effectiveness of requirements engineering. It can provide a categorisation of common requirements and a number of reusable requirements. Do remember that, while thoughtless copying is ineffective, the fact of having potential relevant requirements to reason about is often productive.

The framework also gives clear guidance on the quality of requirements and formalizes how to describe them. For user stories, for instance, concrete guidance can explain what to describe in the definition of done, definition of ready, story description, and acceptance criteria.
""" ;
    dcterms:identifier "ce13df2e0dfb455588bf75135f1a718e" ;
    rdfs:comment "Build a requirements framework for product teams to utilize." ;
    rdfs:seeAlso <https://owaspsamm.org/model/design/security-requirements/stream-a> ;
    skos:altLabel "D-SR-3-A" ;
    ns1:benefit "Efficient and effective handling of security requirements in your organization" ;
    ns1:hasPracticeLevel ns1:f8b6eebc0662477f9286aa4f6068e364 ;
    ns1:hasStream ns1:7fb68bc660774b9080963c17761529a2 .

ns1:d09a731835304ea8aeb4c21565e45c4b a ns1:Activity ;
    rdfs:label "Test application dependencies" ;
    dcterms:description """Maintain a whitelist of approved dependencies and versions, and ensure that the build process fails upon a presence of dependency not being on the list. Include a sign-off process for handling exceptions to this rule if sensible.

Perform security verification activites against dependencies on the whitelist in a comparable way to the target applications themselves (esp. using SAST and analyzing transitive dependencies). Ensure that these checks also aim to identify possible backdoors or easter eggs in the dependencies. Establish vulnerability disclosure processes with the dependency authors including SLAs for fixing issues. In case enforcing SLAs is not realistic (e.g. with open source vulnerabilities), ensure that the most probable cases are expected and you are able to implement compensating measures in a timely manner. Implement regression tests for the fixes to identified issues.

Track all identified issues and their state using your defect tracking system. Integrate your build pipeline with this system to enable failing the build whenever the included dependencies contain issues above a defined criticality level.
""" ;
    dcterms:identifier "d09a731835304ea8aeb4c21565e45c4b" ;
    rdfs:comment "Analyze used dependencies for security issues in a comparable way to your own code." ;
    rdfs:seeAlso <https://owaspsamm.org/model/implementation/secure-build/stream-b> ;
    skos:altLabel "I-SB-3-B" ;
    ns1:benefit "Handling of security issues in dependencies comparable to those in your own code" ;
    ns1:hasPracticeLevel ns1:02e602c451d548e8a95433a46fe6b9d8 ;
    ns1:hasStream ns1:2f7b501627954c6cb03342196b2065a7 .

ns1:d1cb54f1ddd3432480513df320fc0ff8 a ns1:Activity ;
    rdfs:label "Define basic defect metrics" ;
    dcterms:description """Once per defined period of time (typically at least once per year), go over your both resolved and still open recorded security defects in every team and extract basic metrics from the available data. These might include:

* The total number of defects versus total number of verification activities. This could give you an idea whether you're looking for defects with an adequate intensity and quality.
* The software components the defects reside in. This is indicative of where attention might be most required, and where security flaws might be more likely to appear in the future again.
* The type or category of the defect, which suggests areas where the development team need further training.
* The severity of the defect, which can help the team understand the software’s risk exposure.

Identify and carry out sensible quick win activities which you can derive from the newly acquired knowledge. These might include things like a knowledge sharing session about one particular vulnerability type or carrying out / automating a security scan.
""" ;
    dcterms:identifier "d1cb54f1ddd3432480513df320fc0ff8" ;
    rdfs:comment "Regularly go over previously recorded security defects and derive quick wins from basic metrics." ;
    rdfs:seeAlso <https://owaspsamm.org/model/implementation/defect-management/stream-b> ;
    skos:altLabel "I-DM-1-B" ;
    ns1:benefit "Identification of quick wins derived from available defect information" ;
    ns1:hasPracticeLevel ns1:97a46a074fe849a1af2c2d2d3dd09ba5 ;
    ns1:hasStream ns1:55bf5184ff7d4b76a444e52a28c803d9 .

ns1:d61764610f8741de894c1751f5c041ae a ns1:Activity ;
    rdfs:label "Implement centers of excellence" ;
    dcterms:description """The organization implements a formal secure coding center of excellence, with architects and senior developers representing the different business units and technology stacks. The team has an official charter and defines standards and best practices to improve software development practices. The goal is to mitigate the way velocity of change in technology, programming languages, and development frameworks and libraries makes it difficult for Information Security professionals to be fully informed of all the technical nuances that impact security. Even developers often struggle keeping up with all the changes and new tools intended to make software development faster, better, and safer.

This ensures all current programming efforts follow industry’s best practices and organization’s development and implementation standards include all critical configuration settings. It helps identify, train, and support “Product Champions”, responsible for assisting different teams with implementing tools that automate, streamline, or improve various aspects of the SDLC. It identifies development teams with higher maturity levels within their SDLC and the practices and tools that enable these achievements, with the goal of replicating them to other teams.

The group provides subject matter expertise, helping information security teams evaluate tools and solutions to improve application security, ensuring these tools are not only useful but also compatible with the way different teams develop applications. Teams looking to make significant architectural changes to their software consult with this group to avoid adversely impacting the SDLC lifecycle or established security controls.
""" ;
    dcterms:identifier "d61764610f8741de894c1751f5c041ae" ;
    rdfs:comment "Develop a secure software center of excellence promoting thought leadership among developers and architects." ;
    rdfs:seeAlso <https://owaspsamm.org/model/governance/education-and-guidance/stream-b> ;
    skos:altLabel "G-EG-2-B" ;
    ns1:benefit "Specific security best practices tailored to the organization" ;
    ns1:hasPracticeLevel ns1:e8de5ea176cc455bba89f0e2d1ea1f16 ;
    ns1:hasStream ns1:0e2c4c5620e24d7d8e979020ca414182 .

ns1:d6dd8813c5074350b5614b92f2dec60d a ns1:Activity ;
    rdfs:label "Define and incident response process" ;
    dcterms:description """Establish and document the formal security incident response process. Ensure documentation includes information like&#58;

* most probable/common scenarios of security incidents and high-level instructions for handling them; for such scenarios, also use public knowledge about possibly relevant third-party incidents
* rules for triaging each incident
* rules for involvement of different stakeholders including senior management, Public Relations, Legal, privacy, Human Resources, external (law enforcement) authorities, and customers; specify mandatory timeframe to do so, if needed
* the process for performing root-cause analysis and documentation of its results

Ensure a knowledgeable and properly trained incident response team is available both during and outside of business hours. Define timelines for action and a war room. Keep hardware and software tools up to date and ready for use anytime.
""" ;
    dcterms:identifier "d6dd8813c5074350b5614b92f2dec60d" ;
    rdfs:comment "Establish a formal incident response process and ensure staff are properly trained in performing their roles." ;
    rdfs:seeAlso <https://owaspsamm.org/model/operations/incident-management/stream-b> ;
    skos:altLabel "O-IM-2-B" ;
    ns1:benefit "Understanding and efficient handling of most security incidents" ;
    ns1:hasPracticeLevel ns1:439406325e6645519c149da3e05a7d9d ;
    ns1:hasStream ns1:390bec725b8344a289d5386026925947 .

ns1:d955a7b3fbfc4b6aa5b327af9e01c377 a ns1:Activity ;
    rdfs:label "Enforce an SLA for defect management" ;
    dcterms:description """Implement an automated alerting on security defects if the fix time breaches the defined SLAs. Ensure that these defects are automatically transfered into the risk management process and rated by a consistent quantitative methodology. Evaluate how particular defects influence / amplify each other not only on the level of separate teams, but on the level of the whole organization. Use the knowledge of the full kill chain to prioritize, introduce and track compensating controls mitigating the respective business risks.

Integrate your defect management system with the automated tooling introduced by other practices, e.g.:

* Build and Deployment: Fail the build / deployment process if security defects above certain severity affect the final artifact, unless someone explicitely signs off the exception.
* Monitoring: If possible, ensure that abuse of the security defect in production environment is recognized and alerted.
""" ;
    dcterms:identifier "d955a7b3fbfc4b6aa5b327af9e01c377" ;
    rdfs:comment "Enforce the predefined SLAs and integrate your defect management system with other relevant tooling." ;
    rdfs:seeAlso <https://owaspsamm.org/model/implementation/defect-management/stream-a> ;
    skos:altLabel "I-DM-3-A" ;
    ns1:benefit "Assurance that security defects are handled within predefined SLAs" ;
    ns1:hasPracticeLevel ns1:5a25ae9bc9134d6387128ea925c81845 ;
    ns1:hasStream ns1:a5b57fc5fa0441b7b23f599b506c5752 .

ns1:d975bb1ce1dd4d61a6039b0a4a05926e a ns1:Activity ;
    rdfs:label "Perform security stress testing" ;
    dcterms:description """Applications are particularly susceptible to denial of service attacks. Perform denial of service and security stress testing against them in controlled conditiions, preferably on application acceptance environments.

Load testing tools generate synthetic traffic, allowing you to test the application's performance under heavy load. One important test is how many requests per second an application can handle while remaining within its performance requirements. Testing from a single IP address is still useful as it gives an indication of how many requests an attacker must generate to impact the application.

Denial of service attacks typically result in application resource starvation or exhaustion. To determine if any resources can be used to create a denial of service, analyze each application resource to see how it can be exhausted. Prioritise actions unauthenticated user can do. Complement overall denial of service tests with security stress tests to perform actions or create conditions which cause delays, disruptions, or failures of the application under test.
""" ;
    dcterms:identifier "d975bb1ce1dd4d61a6039b0a4a05926e" ;
    rdfs:comment "Denial of service and security stress testing" ;
    rdfs:seeAlso <https://owaspsamm.org/model/verification/requirements-driven-testing/stream-b> ;
    skos:altLabel "V-RT-3-B" ;
    ns1:benefit "Transparency of resilience against denial of service attacks" ;
    ns1:hasPracticeLevel ns1:812abdd0a2b54366a497919f8463911a ;
    ns1:hasStream ns1:27a14a265c864eb790781cd1e2bf843b .

ns1:e092ac0ccb8c4fccb6cd662f974dc107 a ns1:Activity ;
    rdfs:label "Align security and business strategies" ;
    dcterms:description """You review the application security plan periodically for ongoing applicability and support of the organization’s evolving needs and future growth. To do this, you repeat the steps from the first two maturity levels of this Security Practice at least annually. The goal is for the plan to always support the current and future needs of the organization, which ensures the program is aligned with the business.

In addition to reviewing the business drivers, the organization closely monitors the success of the implementation of each of the roadmap milestones. You evaluate the success of the milestones based on a wide range of criteria, including completeness and efficiency of the implementation, budget considerations, and any cultural impacts or changes resulting from the initiative. You review missed or unsatisfactory milestones and evaluate possible changes to the overall program.

The organization develops dashboards and measurements for management and teams responsible for software development to monitor the implementation of the roadmap. These dashboards are detailed enough to identify individual projects and initiatives and provide a clear understanding of whether the program is successful and aligned with the organization’s needs.
""" ;
    dcterms:identifier "e092ac0ccb8c4fccb6cd662f974dc107" ;
    rdfs:comment "Align the application security program to support the organization’s growth." ;
    rdfs:seeAlso <https://owaspsamm.org/model/governance/strategy-and-metrics/stream-a> ;
    skos:altLabel "G-SM-3-A" ;
    ns1:benefit "Continuous AppSec program alignment with the organization's business goals" ;
    ns1:hasPracticeLevel ns1:420074f071fb4ab6b6ee6ef44c4f4f1c ;
    ns1:hasStream ns1:94bb47791e3d462cbf5f71ebb1a1327a .

ns1:e7ba346fabdc44beb47e2c67c14a6726 a ns1:Activity ;
    rdfs:label "Measure compliance to external requirements" ;
    dcterms:description """Develop a program for measuring and reporting on the status of compliance between different applications. Application requirements and test scripts help determine the status of compliance. Leverage testing automation to promptly detect compliance regressions in frequently updated applications and ensure compliance is maintained through the different application versions. Whenever fully automated testing is not possible, QA, Internal Audit, or Information Security teams assess compliance periodically through a combination of manual testing and interview.

While full compliance is always the ultimate goal, include tracking remediation actions and periodic updates in the program. Review compliance remediation activities periodically to check teams are making appropriate progress, and that remediation strategies will be effective in achieving compliance. To further improve the process, develop a series of standard reports and compliance scorecards. These help individual teams understand the current state of compliance, and the organization manage assistance for remediating compliance gaps more effectively.

Review compliance gaps requiring significant expenses or development with the subject-matter experts and compare them against the cost of reducing the application’s functionality, minimizing scope or eliminating the compliance requirement. longterm compliance gaps require management approval and a formal compliance risk acceptance, so they receive appropriate attention and scrutiny from the organization’s leadership.
""" ;
    dcterms:identifier "e7ba346fabdc44beb47e2c67c14a6726" ;
    rdfs:comment "Measure and report on individual application’s compliance with 3rd party requirements." ;
    rdfs:seeAlso <https://owaspsamm.org/model/governance/policy-and-compliance/stream-b> ;
    skos:altLabel "G-PC-3-B" ;
    ns1:benefit "Understanding of your organization’s compliance with external compliance drivers" ;
    ns1:hasPracticeLevel ns1:61ae1e4268b24d7986805658c89b5e54 ;
    ns1:hasStream ns1:2919e1f19aec4f018da94a3e8733f37d .

ns1:e931a744c2864bef85a3fa75ce7e214f a ns1:Activity ;
    rdfs:label "Optimize threat modeling" ;
    dcterms:description """Threat modeling is integrated into your SDLC and has become part of the developer security culture.  Reusable risk patterns, comprising of related threat libraries, design flaws, and security mitigations, are created and improved, based on the organization's threat models. You regularly (e.g., yearly) review the existing threat models to verify that no new threats are relevant for your applications.

You optimize your threat modeling methodology. You capture lessons learned from threat models and use these to improve your threat modeling methodology.  You review the threat categories relevant to your organization and update your methodology appropriately. From time to time, you evaluate the quality of your threat models independently.

You automate parts of your threat modeling process with threat modeling tools. You integrate your threat modeling tools with other security tools, such as security verification tools and risk tracking tools. You consider "threat modeling as code" practices to integrate threat modeling artifacts with application code.
""" ;
    dcterms:identifier "e931a744c2864bef85a3fa75ce7e214f" ;
    rdfs:comment "Continuously optimization and automation of your threat modeling methodology." ;
    rdfs:seeAlso <https://owaspsamm.org/model/design/threat-assessment/stream-b> ;
    skos:altLabel "D-TA-3-B" ;
    ns1:benefit "Assurance of continuous improvement of threat modeling activities" ;
    ns1:hasPracticeLevel ns1:21a59897dbeb4d7fa4603a0f24362c2b ;
    ns1:hasStream ns1:ed5a9c3dd7884c88918a45dc9d231c5d .

ns1:eba4b86963f44fa59b0b9389a1cfc59b a ns1:Activity ;
    rdfs:label "Verify the application architecture for security methodically" ;
    dcterms:description """Verify that the solution architecture addresses all identified security and compliance requirements. For each interface in the application, iterate through the list of security and compliance requirements and analyze the architecture for their provision. Also perform an interaction or data flow analysis to ensure that the requirements are adequately addressed over different components. Elaborate the analysis to show the design-level features that address each requirement.

Perform this type of analysis on both internal interfaces, e.g. between tiers, as well as external ones, e.g. those comprising the attack surface. Also identify and validate important design decisions made as part of the architecture, in particular when they deviate from the available shared security solutions in the organization. Finally, update the findings based on changes made during the development cycle, and note any requirements that are not clearly provided at the design level as assessment findings.
""" ;
    dcterms:identifier "eba4b86963f44fa59b0b9389a1cfc59b" ;
    rdfs:comment "Validate the architecture security mechanisms" ;
    rdfs:seeAlso <https://owaspsamm.org/model/verification/architecture-assessment/stream-a> ;
    skos:altLabel "V-AA-2-A" ;
    ns1:benefit "Consistent architecture review process across your organization" ;
    ns1:hasPracticeLevel ns1:67fcd33f84364ef68fb88aba77de1a63 ;
    ns1:hasStream ns1:77ca4b5e7ebc42558109829dffc2b80d .

ns1:ebd3782abc4343509981c52192904a42 a ns1:Activity ;
    rdfs:label "Identify security champions" ;
    dcterms:description """Implement a program where each software development team has a member considered a “Security Champion” who is the liaison between Information Security and developers. Depending on the size and structure of the team the “Security Champion” may be a software developer, tester, or a product manager. The “Security Champion” has a set number of hours per week for Information Security related activities. They participate in periodic briefings to increase awareness and expertise in different security disciplines. “Security Champions” have additional training to help develop these roles as Software Security subject-matter experts. You may need to customize the way you create and support “Security Champions” for cultural reasons.

The goals of the position are to increase effectiveness and efficiency of application security and compliance and to strengthen the relationship between various teams and Information Security. To achieve these objectives, “Security Champions” assist with researching, verifying, and prioritizing security and compliance related software defects. They are involved in all Risk Assessments, Threat Assessments, and Architectural Reviews to help identify opportunities to remediate security defects by making the architecture of the application more resilient and reducing the attack threat surface.

In addition to assisting Information Security, “Security Champions” provide periodic reviews of all security-related issues for the project team so everyone is aware of the problems and any current and future remediation efforts. These reviews are leveraged to help brainstorm solutions to more complex problems by engaging the entire development team.
""" ;
    dcterms:identifier "ebd3782abc4343509981c52192904a42" ;
    rdfs:comment "Identify a “Security Champion” within each development team." ;
    rdfs:seeAlso <https://owaspsamm.org/model/governance/education-and-guidance/stream-b> ;
    skos:altLabel "G-EG-1-B" ;
    ns1:benefit "Basic embedding of security in the development organization" ;
    ns1:hasPracticeLevel ns1:38f3a2f7633c42b98eb160f36a2c0a7b ;
    ns1:hasStream ns1:0e2c4c5620e24d7d8e979020ca414182 .

ns1:ef0b56870b734b13868697017a9b605e a ns1:Activity ;
    rdfs:label "Identify the organization's risk appetite" ;
    dcterms:description """Understand, based on application risk exposure, what threats exist or may exist, as well as how tolerant executive leadership is of these risks. This understanding is a key component of determining software security assurance priorities. To ascertain these threats, interview business owners and stakeholders and document drivers specific to industries where the organization operates as well as drivers specific to the organization. Gathered information includes worst-case scenarios that could impact the organization, as well as opportunities where an optimized software development lifecycle and more secure applications could provide a market-differentiator or create additional opportunities.

Gathered information provides a baseline for the organization to develop and promote its application security program. Items in the program are prioritized to address threats and opportunities most important to the organization. The baseline is split into several risk factors and drivers linked directly to the organization’s priorities and used to help build a risk profile of each custom-developed application by documenting how they can impact the organization if they are compromised.

The baseline and individual risk factors should be published and made available to application development teams to ensure a more transparent process of creating application risk profiles and incorporating the organization’s priorities into the program. Additionally, these goals should provide a set of objectives which should be used to ensure all application security program enhancements provide direct support of the organization’s current and future needs.
""" ;
    dcterms:identifier "ef0b56870b734b13868697017a9b605e" ;
    rdfs:comment "Identify organization drivers as they relate to the organization’s risk tolerance." ;
    rdfs:seeAlso <https://owaspsamm.org/model/governance/strategy-and-metrics/stream-a> ;
    skos:altLabel "G-SM-1-A" ;
    ns1:benefit "Common understanding of your organization's security posture" ;
    ns1:hasPracticeLevel ns1:4e54705272fa4f1f9977b1f9011f585d ;
    ns1:hasStream ns1:94bb47791e3d462cbf5f71ebb1a1327a .

ns1:f2a309b82fbc46cfb2f11c9cde20dc0a a ns1:Activity ;
    rdfs:label "Use metrics to improve the security strategy" ;
    dcterms:description """Regularly (at least once per year) revisit the defect management metrics you're collecting and compare the effort needed to collect and track these to the expected outcomes. Make knowledgeable decision about removing metrics which don't deliver the overall expected value. Wherever possible, include and automate verification activities for the quality of the collected data and ensure sustainable improvement if any differences are detected.

Aggregate the data with your threat intelligence and incident management metrics and use the results as input for other initiatives over the whole organization, such as:

* Planning security trainings for various personnel
* Improvement of security verification activities for both internally and externally develeoped collected
* Supply chain management, e.g. carrying out security audits of partner organizations
* Monitoring of attacks against your infrastructure and applications
* Investing in security infrastructure or compensating controls
* Staffing your security team and setting up the security budget
""" ;
    dcterms:identifier "f2a309b82fbc46cfb2f11c9cde20dc0a" ;
    rdfs:comment "Continuously improve your security defect management metrics and correlate it with other sources." ;
    rdfs:seeAlso <https://owaspsamm.org/model/implementation/defect-management/stream-b> ;
    skos:altLabel "I-DM-3-B" ;
    ns1:benefit "Optimized security strategy based on defect information" ;
    ns1:hasPracticeLevel ns1:5a25ae9bc9134d6387128ea925c81845 ;
    ns1:hasStream ns1:55bf5184ff7d4b76a444e52a28c803d9 .

ns1:f692ee8f87c1499681490cc1647c0df4 a ns1:Activity ;
    rdfs:label "Establish an incident response team" ;
    dcterms:description """Establish a dedicated incident response team, continuously available and responsible for continuous process improvement with the help of regular RCAs. For distributed organizations, define and document logistics rules for all relevant locations if sensible.

Document detailed incident response procedures and keep them up to date. Automate procedures where appropriate. Keep all resources necessary for these procedures (e.g., separate communicating infrastructure or reliable external location) ready to use. Detect and correct unavailability of these resources in a timely manner.

Carry out incident and emergency exercises are regularly. Use the results for process improvement.

Define, gather, evaluate, and act upon metrics on the incident response process, including its continuous improvement.
""" ;
    dcterms:identifier "f692ee8f87c1499681490cc1647c0df4" ;
    rdfs:comment "Employ a dedicated, well-trained incident response team." ;
    rdfs:seeAlso <https://owaspsamm.org/model/operations/incident-management/stream-b> ;
    skos:altLabel "O-IM-3-B" ;
    ns1:benefit "Efficient incident response independent of time, location, or type of incident" ;
    ns1:hasPracticeLevel ns1:6fe1973911bf4e54b018da10a5aa80a1 ;
    ns1:hasStream ns1:390bec725b8344a289d5386026925947 .

ns1:fb6f258a2e424ee9a919341758222a7a a ns1:Activity ;
    rdfs:label "Develop application-specific security test cases" ;
    dcterms:description """Increase the effectiveness of automated security testing tools by tuning and customizing them for your particular technology stacks and applications. Automated security testing tools have 2 important characteristics: Their false positive rate, i.e. the non-existent bugs and vulnerabilities they incorrectly report; their false negative rate, i.e. actual bugs and vulnerabilities which they fail to detect. As you mature in your use of automated testing tools, you strive to minimize their false positive and false negative rates. This maximizes the time development teams spend reviewing and addressing real security issues in their applications, and reduces the friction typically associated with using untuned automated security analysis tools.

Start by disabling tool support for technologies and frameworks you do not use and target specific versions where possible. This will increase execution speed and reduce the number spurious results reported. Rely on security tool champions or shared security teams to pilot the tools in coordination with a select group of motivated development teams. This will identify likely false positive findings to ignore or remove from the tools' output. Identify specific security issues and anti-patterns and favor the best tool for detecting them.

Leverage available tool features to take application-specific and organizational coding styles, as well as technical standards into account. Many automated static analysis tools allow users to write their own rules or customize default analysis rules to the specific software interfaces in the project under test for improved accuracy and depth of coverage. For example, potentially dangerous input (aka tainted) can be marked as safe after it flows through a designated custom sanitization method.

Strategically, it is better to reliably detect a limited subset of security issues via automated tooling, and incrementally extend coverage than attempting to detect all known issues immediately. Once the tools have been sufficiently tuned, they can be made available to a more development teams. It is important to continuously monitor their perceived efficacy among development teams. In more advanced forms, machine learning techniques can be adopted to identify and automatically filter out likely false positives at scale.
""" ;
    dcterms:identifier "fb6f258a2e424ee9a919341758222a7a" ;
    rdfs:comment "Employ application-specific security testing automation" ;
    rdfs:seeAlso <https://owaspsamm.org/model/verification/security-testing/stream-a> ;
    skos:altLabel "V-ST-2-A" ;
    ns1:benefit "Detection of organization-specific easy-to-find vulnerabilites" ;
    ns1:hasPracticeLevel ns1:6291462e1894467d807b913ef7da4beb ;
    ns1:hasStream ns1:102fdab651834273abd67a3ec27aab05 .

ns1:fd4d1ac720374b13a25ab1381045b731 a ns1:Activity ;
    rdfs:label "Define and run security abuse cases from requirements" ;
    dcterms:description """Misuse and abuse cases describe unintended and malicious use scenarios of the application, describing how an attacker could do this. Create misuse and abuse cases to misuse or exploit the weaknesses of controls in software features to attack an application. Use abuse-case models for an application to serve as fuel for identification of concrete security tests that directly or indirectly exploit the abuse scenarios.

Abuse of functionality, sometimes referred to as a “business logic attack”, depends on the design and implementation of application functions and features. An example is using a password reset flow to enumerate accounts. As part of business logic testing, identify the business rules that are important for the application and turn them into experiments to verify whether the application properly enforces the business rule. For example, on a stock trading application, is the attacker allowed to start a trade at the beginning of the day and lock in a price, hold the transaction open until the end of the day, then complete the sale if the stock price has risen or cancel if the price dropped?
""" ;
    dcterms:identifier "fd4d1ac720374b13a25ab1381045b731" ;
    rdfs:comment "Create and test abuse cases and business logic flaw test" ;
    rdfs:seeAlso <https://owaspsamm.org/model/verification/requirements-driven-testing/stream-b> ;
    skos:altLabel "V-RT-2-B" ;
    ns1:benefit "Detection of application business logic flaws" ;
    ns1:hasPracticeLevel ns1:3e6e9a2b696e48018830b44fa96f98b5 ;
    ns1:hasStream ns1:27a14a265c864eb790781cd1e2bf843b .

ns1:fe7afe5fc04742bcbe476d4ba37d8091 a ns1:Activity ;
    rdfs:label "Measure compliance to policies and standards" ;
    dcterms:description """Develop a program to measure each application’s compliance with existing policies and standards. Mandatory requirements should be motivated and reported consistently across all teams. Whenever possible, tie compliance status into automated testing and report with each version. Compliance reporting includes the version of policies and standards and appropriate code coverage factors.

Encourage non-compliant teams to review available resources such as security requirements and test scripts, to ensure non-compliance is not a result of inadequate guidance. Forward issues resulting from insufficient guidance to the teams responsible for publishing application requirements and test scripts, to include them in the future releases. Escalate issues resulting from the inability to meet policies and standards to teams that handle application security risks.
""" ;
    dcterms:identifier "fe7afe5fc04742bcbe476d4ba37d8091" ;
    rdfs:comment "Measure and report on the status of individual application’s adherence to policies and standards." ;
    rdfs:seeAlso <https://owaspsamm.org/model/governance/policy-and-compliance/stream-a> ;
    skos:altLabel "G-PC-3-A" ;
    ns1:benefit "Understanding of your organization’s compliance with policies and standards" ;
    ns1:hasPracticeLevel ns1:61ae1e4268b24d7986805658c89b5e54 ;
    ns1:hasStream ns1:c404aa4f711e4f4e9e71faea22f7fb5c .

ns1:fed0d75c064c4a979a5b7b98adfdedbf a ns1:Activity ;
    rdfs:label "Enforce lifecycle management of application secrets" ;
    dcterms:description """Implement lifecycle management for production secrets, and ensure the generation of new secrets as much as possible, and for every application instance. The use of secrets per application instance ensures that unexpected application behavior can be traced back and properly analyzed. Tools can help in automatically and seemlessly updating the secrets in all relevant places upon change.

Ensure that all access to secrets (both reading and writing) is logged in a central infrastructure. Review these logs regularly to identify unexpected behavior and perform proper analysis to understand why this happened. Feed issues and root causes into the defect management practice to make sure that the organization will resolve any unacceptable situations.
""" ;
    dcterms:identifier "fed0d75c064c4a979a5b7b98adfdedbf" ;
    rdfs:comment "Improve the lifecycle of application secrets by regularly generating them and by ensuring proper use." ;
    rdfs:seeAlso <https://owaspsamm.org/model/implementation/secure-deployment/stream-b> ;
    skos:altLabel "I-SD-3-B" ;
    ns1:benefit "Minimized possibility and timely detection of production secret abuse" ;
    ns1:hasPracticeLevel ns1:fc5eb251c6ee4f3db04eb01b62d380ba ;
    ns1:hasStream ns1:9a5f26d77f204467bdda7ffa09109d73 .

ns1:hasFunction a owl:ObjectProperty ;
    rdfs:domain ns1:Practice ;
    rdfs:range ns1:BusinessFunction .

ns1:hasMaturityLevel a owl:ObjectProperty ;
    rdfs:domain ns1:PracticeLevel ;
    rdfs:range ns1:MaturityLevel .

ns1:hasPractice a owl:ObjectProperty ;
    rdfs:domain ns1:PracticeLevel ;
    rdfs:range ns1:Practice .

ns1:hasPracticeLevel a owl:ObjectProperty ;
    rdfs:domain ns1:Activity ;
    rdfs:range ns1:PracticeLevel .

ns1:hasStream a owl:ObjectProperty ;
    rdfs:domain ns1:Activity ;
    rdfs:range ns1:Stream .

<https://owaspsamm.org/model/maturity/1> a ns1:MaturityLevel ;
    dcterms:identifier "0a1dc80f84964f2fa776c5d8e932353a" ;
    dcat:seeAlso ns1:0a1dc80f84964f2fa776c5d8e932353a .

<https://owaspsamm.org/model/maturity/2> a ns1:MaturityLevel ;
    dcterms:identifier "47dd82af343e4695a0385418af4398d1" ;
    dcat:seeAlso ns1:47dd82af343e4695a0385418af4398d1 .

<https://owaspsamm.org/model/maturity/3> a ns1:MaturityLevel ;
    dcterms:identifier "7bbfe31d447e48759ef0f2af25c31b43" ;
    dcat:seeAlso ns1:7bbfe31d447e48759ef0f2af25c31b43 .

ns1:02e602c451d548e8a95433a46fe6b9d8 a ns1:PracticeLevel ;
    rdfs:label "I-SB-3" ;
    dcterms:description "Build process helps prevent known defects from entering the production environment." ;
    dcterms:identifier "02e602c451d548e8a95433a46fe6b9d8" ;
    skos:altLabel "I-SB-3" ;
    ns1:hasMaturityLevel ns1:7bbfe31d447e48759ef0f2af25c31b43 ;
    ns1:hasPractice ns1:b2af112859d34cada6ce4cf44d393b94 ;
    ns1:maturitylevel 3 ;
    ns1:practice "SB" .

ns1:1a55b2c4666f4336a3f5c12c5bb4a1e9 a ns1:PracticeLevel ;
    rdfs:label "D-SR-2" ;
    dcterms:description "Increase granularity of security requirements derived from business logic and known risks." ;
    dcterms:identifier "1a55b2c4666f4336a3f5c12c5bb4a1e9" ;
    skos:altLabel "D-SR-2" ;
    ns1:hasMaturityLevel ns1:47dd82af343e4695a0385418af4398d1 ;
    ns1:hasPractice ns1:5702908efca4499e87a0239f32920d9b ;
    ns1:maturitylevel 2 ;
    ns1:practice "SR" .

ns1:1cb6e197ca8245eca65b0ecbdd784720 a ns1:PracticeLevel ;
    rdfs:label "O-EM-3" ;
    dcterms:description "Conformity with continuously improving process enforced" ;
    dcterms:identifier "1cb6e197ca8245eca65b0ecbdd784720" ;
    skos:altLabel "O-EM-3" ;
    ns1:hasMaturityLevel ns1:7bbfe31d447e48759ef0f2af25c31b43 ;
    ns1:hasPractice ns1:53a9cd5c2d3643f3b71e4e9d92b811e2 ;
    ns1:maturitylevel 3 ;
    ns1:practice "EM" .

ns1:21a59897dbeb4d7fa4603a0f24362c2b a ns1:PracticeLevel ;
    rdfs:label "D-TA-3" ;
    dcterms:description "Proactive improvement of threat coverage throughout the organization." ;
    dcterms:identifier "21a59897dbeb4d7fa4603a0f24362c2b" ;
    skos:altLabel "D-TA-3" ;
    ns1:hasMaturityLevel ns1:7bbfe31d447e48759ef0f2af25c31b43 ;
    ns1:hasPractice ns1:f9269aebfe2c4d5b9293ba42a40a93ac ;
    ns1:maturitylevel 3 ;
    ns1:practice "TA" .

ns1:2a059c7d07c34b9897e49e6295501608 a ns1:PracticeLevel ;
    rdfs:label "O-OM-3" ;
    dcterms:description "Active Monitoring and Response" ;
    dcterms:identifier "2a059c7d07c34b9897e49e6295501608" ;
    skos:altLabel "O-OM-3" ;
    ns1:hasMaturityLevel ns1:7bbfe31d447e48759ef0f2af25c31b43 ;
    ns1:hasPractice ns1:8f07145b5ea74388b2217895d5e7b5c2 ;
    ns1:maturitylevel 3 ;
    ns1:practice "OM" .

ns1:2a29c1f7d6954785b8d42d637a752f94 a ns1:PracticeLevel ;
    rdfs:label "G-PC-2" ;
    dcterms:description "Establish application-specific security and compliance baseline." ;
    dcterms:identifier "2a29c1f7d6954785b8d42d637a752f94" ;
    skos:altLabel "G-PC-2" ;
    ns1:hasMaturityLevel ns1:47dd82af343e4695a0385418af4398d1 ;
    ns1:hasPractice ns1:be9e7ddb98b84abe8b9e185b979ccf60 ;
    ns1:maturitylevel 2 ;
    ns1:practice "PC" .

ns1:354292b7198b48bb8c4909e0d7e29f68 a ns1:PracticeLevel ;
    rdfs:label "O-EM-2" ;
    dcterms:description "Formal process with baselines in place" ;
    dcterms:identifier "354292b7198b48bb8c4909e0d7e29f68" ;
    skos:altLabel "O-EM-2" ;
    ns1:hasMaturityLevel ns1:47dd82af343e4695a0385418af4398d1 ;
    ns1:hasPractice ns1:53a9cd5c2d3643f3b71e4e9d92b811e2 ;
    ns1:maturitylevel 2 ;
    ns1:practice "EM" .

ns1:38f3a2f7633c42b98eb160f36a2c0a7b a ns1:PracticeLevel ;
    rdfs:label "G-EG-1" ;
    dcterms:description "Offer staff access to resources around the topics of secure development and deployment." ;
    dcterms:identifier "38f3a2f7633c42b98eb160f36a2c0a7b" ;
    skos:altLabel "G-EG-1" ;
    ns1:hasMaturityLevel ns1:0a1dc80f84964f2fa776c5d8e932353a ;
    ns1:hasPractice ns1:483a0a1b78264cafbc470ce72d557332 ;
    ns1:maturitylevel 1 ;
    ns1:practice "EG" .

ns1:39bc5d271fae4ea8ba53db7de7b2712c a ns1:PracticeLevel ;
    rdfs:label "V-AA-1" ;
    dcterms:description "Review the architecture to ensure baseline mitigations are in place for typical risks." ;
    dcterms:identifier "39bc5d271fae4ea8ba53db7de7b2712c" ;
    skos:altLabel "V-AA-1" ;
    ns1:hasMaturityLevel ns1:0a1dc80f84964f2fa776c5d8e932353a ;
    ns1:hasPractice ns1:53f2da68c37a4ced8d5e767298fba589 ;
    ns1:maturitylevel 1 ;
    ns1:practice "AA" .

ns1:3d035b6df77f4ee69577c9b4c9d64891 a ns1:PracticeLevel ;
    rdfs:label "D-SR-1" ;
    dcterms:description "Consider security explicitly during the software requirements process." ;
    dcterms:identifier "3d035b6df77f4ee69577c9b4c9d64891" ;
    skos:altLabel "D-SR-1" ;
    ns1:hasMaturityLevel ns1:0a1dc80f84964f2fa776c5d8e932353a ;
    ns1:hasPractice ns1:5702908efca4499e87a0239f32920d9b ;
    ns1:maturitylevel 1 ;
    ns1:practice "SR" .

ns1:3e6e9a2b696e48018830b44fa96f98b5 a ns1:PracticeLevel ;
    rdfs:label "V-RT-2" ;
    dcterms:description "Perform implementation review to discover application-specific risks against the security requirements." ;
    dcterms:identifier "3e6e9a2b696e48018830b44fa96f98b5" ;
    skos:altLabel "V-RT-2" ;
    ns1:hasMaturityLevel ns1:47dd82af343e4695a0385418af4398d1 ;
    ns1:hasPractice ns1:66fb99798fe946e4979a2de98e9d6f8b ;
    ns1:maturitylevel 2 ;
    ns1:practice "RT" .

ns1:3e89d1fa6cba4516a3ec446faaab5b84 a ns1:PracticeLevel ;
    rdfs:label "I-SD-2" ;
    dcterms:description "Deployment processes include security verification milestones." ;
    dcterms:identifier "3e89d1fa6cba4516a3ec446faaab5b84" ;
    skos:altLabel "I-SD-2" ;
    ns1:hasMaturityLevel ns1:47dd82af343e4695a0385418af4398d1 ;
    ns1:hasPractice ns1:40d7879025144dbbbf34ba8ea82f060d ;
    ns1:maturitylevel 2 ;
    ns1:practice "SD" .

ns1:41c8e63716c34f1eaf09b8cad70cfbaf a ns1:PracticeLevel ;
    rdfs:label "D-SA-2" ;
    dcterms:description "Direct the software design process toward known secure services and secure-by-default designs." ;
    dcterms:identifier "41c8e63716c34f1eaf09b8cad70cfbaf" ;
    skos:altLabel "D-SA-2" ;
    ns1:hasMaturityLevel ns1:47dd82af343e4695a0385418af4398d1 ;
    ns1:hasPractice ns1:4753e55e943c4d418303bf90d599c6b1 ;
    ns1:maturitylevel 2 ;
    ns1:practice "SA" .

ns1:420074f071fb4ab6b6ee6ef44c4f4f1c a ns1:PracticeLevel ;
    rdfs:label "G-SM-3" ;
    dcterms:description "Align security efforts with the relevant organizational indicators and asset values." ;
    dcterms:identifier "420074f071fb4ab6b6ee6ef44c4f4f1c" ;
    skos:altLabel "G-SM-3" ;
    ns1:hasMaturityLevel ns1:7bbfe31d447e48759ef0f2af25c31b43 ;
    ns1:hasPractice ns1:32b3bdd85d3a4d53827960004f9d1c7e ;
    ns1:maturitylevel 3 ;
    ns1:practice "SM" .

ns1:437d447b3f11427592e938dbde53c7da a ns1:PracticeLevel ;
    rdfs:label "G-PC-1" ;
    dcterms:description "Identify and document governance and compliance drivers relevant to the organization." ;
    dcterms:identifier "437d447b3f11427592e938dbde53c7da" ;
    skos:altLabel "G-PC-1" ;
    ns1:hasMaturityLevel ns1:0a1dc80f84964f2fa776c5d8e932353a ;
    ns1:hasPractice ns1:be9e7ddb98b84abe8b9e185b979ccf60 ;
    ns1:maturitylevel 1 ;
    ns1:practice "PC" .

ns1:439406325e6645519c149da3e05a7d9d a ns1:PracticeLevel ;
    rdfs:label "O-IM-2" ;
    dcterms:description "Formal incident management process in place" ;
    dcterms:identifier "439406325e6645519c149da3e05a7d9d" ;
    skos:altLabel "O-IM-2" ;
    ns1:hasMaturityLevel ns1:47dd82af343e4695a0385418af4398d1 ;
    ns1:hasPractice ns1:c13aa12c13d04362a3ca3385a8c580ee ;
    ns1:maturitylevel 2 ;
    ns1:practice "IM" .

ns1:46f16450b23d4c29a5cf19b056c2636e a ns1:PracticeLevel ;
    rdfs:label "I-SB-2" ;
    dcterms:description "Build process is optimized and fully integrated into the workflow." ;
    dcterms:identifier "46f16450b23d4c29a5cf19b056c2636e" ;
    skos:altLabel "I-SB-2" ;
    ns1:hasMaturityLevel ns1:47dd82af343e4695a0385418af4398d1 ;
    ns1:hasPractice ns1:b2af112859d34cada6ce4cf44d393b94 ;
    ns1:maturitylevel 2 ;
    ns1:practice "SB" .

ns1:4e54705272fa4f1f9977b1f9011f585d a ns1:PracticeLevel ;
    rdfs:label "G-SM-1" ;
    dcterms:description "Identify objectives and means of measuring effectiveness of the security program." ;
    dcterms:identifier "4e54705272fa4f1f9977b1f9011f585d" ;
    skos:altLabel "G-SM-1" ;
    ns1:hasMaturityLevel ns1:0a1dc80f84964f2fa776c5d8e932353a ;
    ns1:hasPractice ns1:32b3bdd85d3a4d53827960004f9d1c7e ;
    ns1:maturitylevel 1 ;
    ns1:practice "SM" .

ns1:5015427608de428cba3c324772fb4191 a ns1:PracticeLevel ;
    rdfs:label "I-SD-1" ;
    dcterms:description "Deployment processes are fully documented." ;
    dcterms:identifier "5015427608de428cba3c324772fb4191" ;
    skos:altLabel "I-SD-1" ;
    ns1:hasMaturityLevel ns1:0a1dc80f84964f2fa776c5d8e932353a ;
    ns1:hasPractice ns1:40d7879025144dbbbf34ba8ea82f060d ;
    ns1:maturitylevel 1 ;
    ns1:practice "SD" .

ns1:561e85a7fb114b1d976acce95d0b41ee a ns1:PracticeLevel ;
    rdfs:label "G-SM-2" ;
    dcterms:description "Establish a unified strategic roadmap for software security within the organization." ;
    dcterms:identifier "561e85a7fb114b1d976acce95d0b41ee" ;
    skos:altLabel "G-SM-2" ;
    ns1:hasMaturityLevel ns1:47dd82af343e4695a0385418af4398d1 ;
    ns1:hasPractice ns1:32b3bdd85d3a4d53827960004f9d1c7e ;
    ns1:maturitylevel 2 ;
    ns1:practice "SM" .

ns1:5a25ae9bc9134d6387128ea925c81845 a ns1:PracticeLevel ;
    rdfs:label "I-DM-3" ;
    dcterms:description "Defect tracking across multiple components is used to help reduce the number of new defects." ;
    dcterms:identifier "5a25ae9bc9134d6387128ea925c81845" ;
    skos:altLabel "I-DM-3" ;
    ns1:hasMaturityLevel ns1:7bbfe31d447e48759ef0f2af25c31b43 ;
    ns1:hasPractice ns1:e17d573510904f65a1fe6040b56ad0b1 ;
    ns1:maturitylevel 3 ;
    ns1:practice "DM" .

ns1:61ae1e4268b24d7986805658c89b5e54 a ns1:PracticeLevel ;
    rdfs:label "G-PC-3" ;
    dcterms:description "Measure adherence to policies, standards, and 3rd-party requirements." ;
    dcterms:identifier "61ae1e4268b24d7986805658c89b5e54" ;
    skos:altLabel "G-PC-3" ;
    ns1:hasMaturityLevel ns1:7bbfe31d447e48759ef0f2af25c31b43 ;
    ns1:hasPractice ns1:be9e7ddb98b84abe8b9e185b979ccf60 ;
    ns1:maturitylevel 3 ;
    ns1:practice "PC" .

ns1:6291462e1894467d807b913ef7da4beb a ns1:PracticeLevel ;
    rdfs:label "V-ST-2" ;
    dcterms:description "Make security testing during development more complete and efficient through automation complemented with regular manual security penetration tests." ;
    dcterms:identifier "6291462e1894467d807b913ef7da4beb" ;
    skos:altLabel "V-ST-2" ;
    ns1:hasMaturityLevel ns1:47dd82af343e4695a0385418af4398d1 ;
    ns1:hasPractice ns1:bb5488860c124b6e8076b023485023e1 ;
    ns1:maturitylevel 2 ;
    ns1:practice "ST" .

ns1:67fcd33f84364ef68fb88aba77de1a63 a ns1:PracticeLevel ;
    rdfs:label "V-AA-2" ;
    dcterms:description "Review the complete provision of security mechanisms in the architecture." ;
    dcterms:identifier "67fcd33f84364ef68fb88aba77de1a63" ;
    skos:altLabel "V-AA-2" ;
    ns1:hasMaturityLevel ns1:47dd82af343e4695a0385418af4398d1 ;
    ns1:hasPractice ns1:53f2da68c37a4ced8d5e767298fba589 ;
    ns1:maturitylevel 2 ;
    ns1:practice "AA" .

ns1:6fe1973911bf4e54b018da10a5aa80a1 a ns1:PracticeLevel ;
    rdfs:label "O-IM-3" ;
    dcterms:description "Mature incident management" ;
    dcterms:identifier "6fe1973911bf4e54b018da10a5aa80a1" ;
    skos:altLabel "O-IM-3" ;
    ns1:hasMaturityLevel ns1:7bbfe31d447e48759ef0f2af25c31b43 ;
    ns1:hasPractice ns1:c13aa12c13d04362a3ca3385a8c580ee ;
    ns1:maturitylevel 3 ;
    ns1:practice "IM" .

ns1:76f8a2e68065467ba9bd2b5ac625490b a ns1:PracticeLevel ;
    rdfs:label "O-OM-2" ;
    dcterms:description "Managed, Responsive Processes" ;
    dcterms:identifier "76f8a2e68065467ba9bd2b5ac625490b" ;
    skos:altLabel "O-OM-2" ;
    ns1:hasMaturityLevel ns1:47dd82af343e4695a0385418af4398d1 ;
    ns1:hasPractice ns1:8f07145b5ea74388b2217895d5e7b5c2 ;
    ns1:maturitylevel 2 ;
    ns1:practice "OM" .

ns1:812abdd0a2b54366a497919f8463911a a ns1:PracticeLevel ;
    rdfs:label "V-RT-3" ;
    dcterms:description "Maintain the application security level after bug fixes, changes or during maintenance." ;
    dcterms:identifier "812abdd0a2b54366a497919f8463911a" ;
    skos:altLabel "V-RT-3" ;
    ns1:hasMaturityLevel ns1:7bbfe31d447e48759ef0f2af25c31b43 ;
    ns1:hasPractice ns1:66fb99798fe946e4979a2de98e9d6f8b ;
    ns1:maturitylevel 3 ;
    ns1:practice "RT" .

ns1:817dd6acaf85496aa005393e0e6c3e70 a ns1:PracticeLevel ;
    rdfs:label "O-IM-1" ;
    dcterms:description "Best-effort incident detection and handling" ;
    dcterms:identifier "817dd6acaf85496aa005393e0e6c3e70" ;
    skos:altLabel "O-IM-1" ;
    ns1:hasMaturityLevel ns1:0a1dc80f84964f2fa776c5d8e932353a ;
    ns1:hasPractice ns1:c13aa12c13d04362a3ca3385a8c580ee ;
    ns1:maturitylevel 1 ;
    ns1:practice "IM" .

ns1:83ea8aaab3384b41b785107613ee4d86 a ns1:PracticeLevel ;
    rdfs:label "V-AA-3" ;
    dcterms:description "Review the architecture effectiveness and feedback results to improve the security architecture." ;
    dcterms:identifier "83ea8aaab3384b41b785107613ee4d86" ;
    skos:altLabel "V-AA-3" ;
    ns1:hasMaturityLevel ns1:7bbfe31d447e48759ef0f2af25c31b43 ;
    ns1:hasPractice ns1:53f2da68c37a4ced8d5e767298fba589 ;
    ns1:maturitylevel 3 ;
    ns1:practice "AA" .

ns1:8cb942eff46d41f38e6edc11849744a6 a ns1:PracticeLevel ;
    rdfs:label "O-EM-1" ;
    dcterms:description "Best-effort patching and hardening" ;
    dcterms:identifier "8cb942eff46d41f38e6edc11849744a6" ;
    skos:altLabel "O-EM-1" ;
    ns1:hasMaturityLevel ns1:0a1dc80f84964f2fa776c5d8e932353a ;
    ns1:hasPractice ns1:53a9cd5c2d3643f3b71e4e9d92b811e2 ;
    ns1:maturitylevel 1 ;
    ns1:practice "EM" .

ns1:97a46a074fe849a1af2c2d2d3dd09ba5 a ns1:PracticeLevel ;
    rdfs:label "I-DM-1" ;
    dcterms:description "All defects are tracked within each project." ;
    dcterms:identifier "97a46a074fe849a1af2c2d2d3dd09ba5" ;
    skos:altLabel "I-DM-1" ;
    ns1:hasMaturityLevel ns1:0a1dc80f84964f2fa776c5d8e932353a ;
    ns1:hasPractice ns1:e17d573510904f65a1fe6040b56ad0b1 ;
    ns1:maturitylevel 1 ;
    ns1:practice "DM" .

ns1:9d1e469966124c0fa80d1bc2fc223a0a a ns1:PracticeLevel ;
    rdfs:label "D-SA-3" ;
    dcterms:description "Formally control the software design process and validate utilization of secure components." ;
    dcterms:identifier "9d1e469966124c0fa80d1bc2fc223a0a" ;
    skos:altLabel "D-SA-3" ;
    ns1:hasMaturityLevel ns1:7bbfe31d447e48759ef0f2af25c31b43 ;
    ns1:hasPractice ns1:4753e55e943c4d418303bf90d599c6b1 ;
    ns1:maturitylevel 3 ;
    ns1:practice "SA" .

ns1:a11b78917dec4cfdad983cf6d1d17b61 a ns1:PracticeLevel ;
    rdfs:label "D-SA-1" ;
    dcterms:description "Insert consideration of proactive security guidance into the software design process." ;
    dcterms:identifier "a11b78917dec4cfdad983cf6d1d17b61" ;
    skos:altLabel "D-SA-1" ;
    ns1:hasMaturityLevel ns1:0a1dc80f84964f2fa776c5d8e932353a ;
    ns1:hasPractice ns1:4753e55e943c4d418303bf90d599c6b1 ;
    ns1:maturitylevel 1 ;
    ns1:practice "SA" .

ns1:a3d4045d5c0c4bd4a875784759539f0c a ns1:PracticeLevel ;
    rdfs:label "D-TA-1" ;
    dcterms:description "Best-effort identification of high-level threats to the organization and individual projects." ;
    dcterms:identifier "a3d4045d5c0c4bd4a875784759539f0c" ;
    skos:altLabel "D-TA-1" ;
    ns1:hasMaturityLevel ns1:0a1dc80f84964f2fa776c5d8e932353a ;
    ns1:hasPractice ns1:f9269aebfe2c4d5b9293ba42a40a93ac ;
    ns1:maturitylevel 1 ;
    ns1:practice "TA" .

ns1:b29ab542cc674901a19cf5f3c0c4be18 a ns1:PracticeLevel ;
    rdfs:label "I-SB-1" ;
    dcterms:description "Build process is repeatable and consistent." ;
    dcterms:identifier "b29ab542cc674901a19cf5f3c0c4be18" ;
    skos:altLabel "I-SB-1" ;
    ns1:hasMaturityLevel ns1:0a1dc80f84964f2fa776c5d8e932353a ;
    ns1:hasPractice ns1:b2af112859d34cada6ce4cf44d393b94 ;
    ns1:maturitylevel 1 ;
    ns1:practice "SB" .

ns1:b55c7a41eba747678a65651f5ccacaf2 a ns1:PracticeLevel ;
    rdfs:label "I-DM-2" ;
    dcterms:description "Defect tracking used to influence the deployment process." ;
    dcterms:identifier "b55c7a41eba747678a65651f5ccacaf2" ;
    skos:altLabel "I-DM-2" ;
    ns1:hasMaturityLevel ns1:47dd82af343e4695a0385418af4398d1 ;
    ns1:hasPractice ns1:e17d573510904f65a1fe6040b56ad0b1 ;
    ns1:maturitylevel 2 ;
    ns1:practice "DM" .

ns1:d0a99f3db27e48aa9b2d6b58a9040f49 a ns1:PracticeLevel ;
    rdfs:label "O-OM-1" ;
    dcterms:description "Foundational Practices" ;
    dcterms:identifier "d0a99f3db27e48aa9b2d6b58a9040f49" ;
    skos:altLabel "O-OM-1" ;
    ns1:hasMaturityLevel ns1:0a1dc80f84964f2fa776c5d8e932353a ;
    ns1:hasPractice ns1:8f07145b5ea74388b2217895d5e7b5c2 ;
    ns1:maturitylevel 1 ;
    ns1:practice "OM" .

ns1:d6cefe3e63d149299fb088010c24778b a ns1:PracticeLevel ;
    rdfs:label "V-ST-1" ;
    dcterms:description "Perform security testing (both manual and tool based) to discover security defects." ;
    dcterms:identifier "d6cefe3e63d149299fb088010c24778b" ;
    skos:altLabel "V-ST-1" ;
    ns1:hasMaturityLevel ns1:0a1dc80f84964f2fa776c5d8e932353a ;
    ns1:hasPractice ns1:bb5488860c124b6e8076b023485023e1 ;
    ns1:maturitylevel 1 ;
    ns1:practice "ST" .

ns1:df5a0be1889a4b06835193892803dde5 a ns1:PracticeLevel ;
    rdfs:label "V-RT-1" ;
    dcterms:description "Opportunistically find basic vulnerabilities and other security issues." ;
    dcterms:identifier "df5a0be1889a4b06835193892803dde5" ;
    skos:altLabel "V-RT-1" ;
    ns1:hasMaturityLevel ns1:0a1dc80f84964f2fa776c5d8e932353a ;
    ns1:hasPractice ns1:66fb99798fe946e4979a2de98e9d6f8b ;
    ns1:maturitylevel 1 ;
    ns1:practice "RT" .

ns1:e3cf1d3c27b74262b9f842f27ca86333 a ns1:PracticeLevel ;
    rdfs:label "G-EG-3" ;
    dcterms:description "Develop in-house training programs facilitated by developers across different teams." ;
    dcterms:identifier "e3cf1d3c27b74262b9f842f27ca86333" ;
    skos:altLabel "G-EG-3" ;
    ns1:hasMaturityLevel ns1:7bbfe31d447e48759ef0f2af25c31b43 ;
    ns1:hasPractice ns1:483a0a1b78264cafbc470ce72d557332 ;
    ns1:maturitylevel 3 ;
    ns1:practice "EG" .

ns1:e5b6dc4f907c4986b8ba7923303cd665 a ns1:PracticeLevel ;
    rdfs:label "D-TA-2" ;
    dcterms:description "Standardization and enterprise-wide analysis of software-related threats within the organization." ;
    dcterms:identifier "e5b6dc4f907c4986b8ba7923303cd665" ;
    skos:altLabel "D-TA-2" ;
    ns1:hasMaturityLevel ns1:47dd82af343e4695a0385418af4398d1 ;
    ns1:hasPractice ns1:f9269aebfe2c4d5b9293ba42a40a93ac ;
    ns1:maturitylevel 2 ;
    ns1:practice "TA" .

ns1:e8de5ea176cc455bba89f0e2d1ea1f16 a ns1:PracticeLevel ;
    rdfs:label "G-EG-2" ;
    dcterms:description "Educate all personnel in the software lifecycle with technology and role-specific guidance on secure development." ;
    dcterms:identifier "e8de5ea176cc455bba89f0e2d1ea1f16" ;
    skos:altLabel "G-EG-2" ;
    ns1:hasMaturityLevel ns1:47dd82af343e4695a0385418af4398d1 ;
    ns1:hasPractice ns1:483a0a1b78264cafbc470ce72d557332 ;
    ns1:maturitylevel 2 ;
    ns1:practice "EG" .

ns1:eac3184f8e2343b8b29047d023376da5 a ns1:PracticeLevel ;
    rdfs:label "V-ST-3" ;
    dcterms:description "Embed security testing as part of the development and deployment processes." ;
    dcterms:identifier "eac3184f8e2343b8b29047d023376da5" ;
    skos:altLabel "V-ST-3" ;
    ns1:hasMaturityLevel ns1:7bbfe31d447e48759ef0f2af25c31b43 ;
    ns1:hasPractice ns1:bb5488860c124b6e8076b023485023e1 ;
    ns1:maturitylevel 3 ;
    ns1:practice "ST" .

ns1:f8b6eebc0662477f9286aa4f6068e364 a ns1:PracticeLevel ;
    rdfs:label "D-SR-3" ;
    dcterms:description "Mandate security requirements process for all software projects and third-party dependencies." ;
    dcterms:identifier "f8b6eebc0662477f9286aa4f6068e364" ;
    skos:altLabel "D-SR-3" ;
    ns1:hasMaturityLevel ns1:7bbfe31d447e48759ef0f2af25c31b43 ;
    ns1:hasPractice ns1:5702908efca4499e87a0239f32920d9b ;
    ns1:maturitylevel 3 ;
    ns1:practice "SR" .

ns1:fc5eb251c6ee4f3db04eb01b62d380ba a ns1:PracticeLevel ;
    rdfs:label "I-SD-3" ;
    dcterms:description "Deployment process is fully automated and incorporates automated verification of all critical milestones." ;
    dcterms:identifier "fc5eb251c6ee4f3db04eb01b62d380ba" ;
    skos:altLabel "I-SD-3" ;
    ns1:hasMaturityLevel ns1:7bbfe31d447e48759ef0f2af25c31b43 ;
    ns1:hasPractice ns1:40d7879025144dbbbf34ba8ea82f060d ;
    ns1:maturitylevel 3 ;
    ns1:practice "SD" .

ns1:0e2c4c5620e24d7d8e979020ca414182 a ns1:Stream ;
    rdfs:label "Organization and Culture" ;
    dcterms:description "Organization and culture focuses on promoting the culture of application security within the organization as an important success factor of an SDLC project." ;
    dcterms:identifier "0e2c4c5620e24d7d8e979020ca414182" ;
    skos:altLabel "G-EG-B" ;
    ns1:hasLetter "B" ;
    ns1:hasOrder 2 ;
    ns1:hasPractice ns1:483a0a1b78264cafbc470ce72d557332 ;
    ns1:practice "EG" .

ns1:102ad02df5dc4a8eb3837ef4ca2c1af4 a ns1:BusinessFunction ;
    rdfs:label "Governance" ;
    dcterms:description """Governance focuses on the processes and activities related to how an organization manages overall software development activities. More specifically, this includes concerns that impact cross-functional groups involved in development, as well as business processes established at the organization level.
""" ;
    dcterms:identifier "102ad02df5dc4a8eb3837ef4ca2c1af4" ;
    skos:altLabel "governance" ;
    dcat:downloadURL "https://owaspsamm.org/model/governance" ;
    ns1:hasOrder 1 ;
    ns1:model "SAMM20" .

ns1:102fdab651834273abd67a3ec27aab05 a ns1:Stream ;
    rdfs:label "Scalable Baseline" ;
    dcterms:description """Scalable baseline focuses on the use of application-specific automated testing tools that integrate security validation into the build and deploy process. The goal of this stream is to favor width (a broad spectrum of applications) over depth of testing.
""" ;
    dcterms:identifier "102fdab651834273abd67a3ec27aab05" ;
    skos:altLabel "V-ST-A" ;
    ns1:hasLetter "A" ;
    ns1:hasOrder 1 ;
    ns1:hasPractice ns1:bb5488860c124b6e8076b023485023e1 ;
    ns1:practice "ST" .

ns1:17c90203f8354c3594eea22759e375a9 a ns1:Stream ;
    rdfs:label "Application Risk Profile" ;
    dcterms:description "An application risk profile helps to identify which applications can pose a serious threat to the organization if they were attacked or breached." ;
    dcterms:identifier "17c90203f8354c3594eea22759e375a9" ;
    skos:altLabel "D-TA-A" ;
    ns1:hasLetter "A" ;
    ns1:hasOrder 1 ;
    ns1:hasPractice ns1:f9269aebfe2c4d5b9293ba42a40a93ac ;
    ns1:practice "TA" .

ns1:1a7ad26d9e48411e95a63be79e1b90ea a ns1:Stream ;
    rdfs:label "Patching and Updating" ;
    dcterms:description """The activities in this stream focus on the organization's handling of patches and updates for all elements of the technology stack. For software developed by the organization, these activities are concerned with delivering patches and updates to customers, as well as applying them to organization-managed solutions (e.g., software as a service). For third-party elements, these activities are concerned with the organization's timely application of updates and patches received.
""" ;
    dcterms:identifier "1a7ad26d9e48411e95a63be79e1b90ea" ;
    skos:altLabel "O-EM-B" ;
    ns1:hasLetter "B" ;
    ns1:hasOrder 2 ;
    ns1:hasPractice ns1:53a9cd5c2d3643f3b71e4e9d92b811e2 ;
    ns1:practice "EM" .

ns1:253b012094cf4e0988e08fd22609227d a ns1:Stream ;
    rdfs:label "Architecture Design" ;
    dcterms:description "The design of a software architecture can significantly impact the security posture of a software and the use of good security practices will improve the overall design." ;
    dcterms:identifier "253b012094cf4e0988e08fd22609227d" ;
    skos:altLabel "D-SA-A" ;
    ns1:hasLetter "A" ;
    ns1:hasOrder 1 ;
    ns1:hasPractice ns1:4753e55e943c4d418303bf90d599c6b1 ;
    ns1:practice "SA" .

ns1:27a14a265c864eb790781cd1e2bf843b a ns1:Stream ;
    rdfs:label "Misuse/Abuse Testing" ;
    dcterms:description """Misuse/Abuse Testing leverages fuzzing, misuse/abuse cases, and the identification of any functionality or resources in the software that can be abused in order to identify weaknesses in features to attack an application.
""" ;
    dcterms:identifier "27a14a265c864eb790781cd1e2bf843b" ;
    skos:altLabel "V-RT-B" ;
    ns1:hasLetter "B" ;
    ns1:hasOrder 2 ;
    ns1:hasPractice ns1:66fb99798fe946e4979a2de98e9d6f8b ;
    ns1:practice "RT" .

ns1:2919e1f19aec4f018da94a3e8733f37d a ns1:Stream ;
    rdfs:label "Compliance Management" ;
    dcterms:description "This stream focuses on identifying and providing compliance requirements to support integration into the SDLC." ;
    dcterms:identifier "2919e1f19aec4f018da94a3e8733f37d" ;
    skos:altLabel "G-PC-B" ;
    ns1:hasLetter "B" ;
    ns1:hasOrder 2 ;
    ns1:hasPractice ns1:be9e7ddb98b84abe8b9e185b979ccf60 ;
    ns1:practice "PC" .

ns1:2f1cac3c2e724823b3b48a7e797520b4 a ns1:Stream ;
    rdfs:label "Measure and Improve" ;
    dcterms:description "This stream aims to drive the validity, relevance, and improvement of the application security roadmap through measurements of performance within the organization." ;
    dcterms:identifier "2f1cac3c2e724823b3b48a7e797520b4" ;
    skos:altLabel "G-SM-B" ;
    ns1:hasLetter "B" ;
    ns1:hasOrder 2 ;
    ns1:hasPractice ns1:32b3bdd85d3a4d53827960004f9d1c7e ;
    ns1:practice "SM" .

ns1:2f7b501627954c6cb03342196b2065a7 a ns1:Stream ;
    rdfs:label "Software Dependencies" ;
    dcterms:description "External libraries are a significant part of modern software. The activities in this stream help create a view of external libraries and ensure their security strength is adequate." ;
    dcterms:identifier "2f7b501627954c6cb03342196b2065a7" ;
    skos:altLabel "I-SB-B" ;
    ns1:hasLetter "B" ;
    ns1:hasOrder 2 ;
    ns1:hasPractice ns1:b2af112859d34cada6ce4cf44d393b94 ;
    ns1:practice "SB" .

ns1:390bec725b8344a289d5386026925947 a ns1:Stream ;
    rdfs:label "Incident Response" ;
    dcterms:description """Incident Response starts the moment you acknowledge and verify the existence of a security incident. Your goal is to act in a coordinated and efficient way so that further damage is limited as much as possible. The activities in this stream focus on the organization's ability to respond appropriately and effectively to reported security incidents.
""" ;
    dcterms:identifier "390bec725b8344a289d5386026925947" ;
    skos:altLabel "O-IM-B" ;
    ns1:hasLetter "B" ;
    ns1:hasOrder 2 ;
    ns1:hasPractice ns1:c13aa12c13d04362a3ca3385a8c580ee ;
    ns1:practice "IM" .

ns1:47bff9a57f0344eeb4b083f1c2b1bb7e a ns1:Stream ;
    rdfs:label "Configuration Hardening" ;
    dcterms:description """The activities in this stream focus on the organization's management of security-related configurations in all elements of the technology stack. The emphasis is on those elements (e.g., operating systems, containers, frameworks, services, appliances, and libraries) obtained from third parties, because their architecture and design are not under the organization's control.
""" ;
    dcterms:identifier "47bff9a57f0344eeb4b083f1c2b1bb7e" ;
    skos:altLabel "O-EM-A" ;
    ns1:hasLetter "A" ;
    ns1:hasOrder 1 ;
    ns1:hasPractice ns1:53a9cd5c2d3643f3b71e4e9d92b811e2 ;
    ns1:practice "EM" .

ns1:55bf5184ff7d4b76a444e52a28c803d9 a ns1:Stream ;
    rdfs:label "Metrics and Feedback" ;
    dcterms:description "Defect tracking can drive the improvement of security activities within the organization through metrics and feedback." ;
    dcterms:identifier "55bf5184ff7d4b76a444e52a28c803d9" ;
    skos:altLabel "I-DM-B" ;
    ns1:hasLetter "B" ;
    ns1:hasOrder 2 ;
    ns1:hasPractice ns1:e17d573510904f65a1fe6040b56ad0b1 ;
    ns1:practice "DM" .

ns1:7344f4b153314dd8965361d23772aef1 a ns1:Stream ;
    rdfs:label "Training and Awareness" ;
    dcterms:description "Training and awareness focuses on increasing the overall knowledge around software security among the different stakeholders within the organization." ;
    dcterms:identifier "7344f4b153314dd8965361d23772aef1" ;
    skos:altLabel "G-EG-A" ;
    ns1:hasLetter "A" ;
    ns1:hasOrder 1 ;
    ns1:hasPractice ns1:483a0a1b78264cafbc470ce72d557332 ;
    ns1:practice "EG" .

ns1:77ca4b5e7ebc42558109829dffc2b80d a ns1:Stream ;
    rdfs:label "Architecture Validation" ;
    dcterms:description """Architecture validation confirms the security of the software and supporting architecture by identifying application and infrastructure architecture components and verifying their provision of security objectives and requirements.
""" ;
    dcterms:identifier "77ca4b5e7ebc42558109829dffc2b80d" ;
    skos:altLabel "V-AA-A" ;
    ns1:hasLetter "A" ;
    ns1:hasOrder 1 ;
    ns1:hasPractice ns1:53f2da68c37a4ced8d5e767298fba589 ;
    ns1:practice "AA" .

ns1:79754453c74b4143b20a57d0efdaab56 a ns1:Stream ;
    rdfs:label "Technology Management" ;
    dcterms:description "Technologies and frameworks are the cornerstones of any software solution. The security properties of these must be looked into to ensure an appropriate security level and to anticipate any potential issues herein." ;
    dcterms:identifier "79754453c74b4143b20a57d0efdaab56" ;
    skos:altLabel "D-SA-B" ;
    ns1:hasLetter "B" ;
    ns1:hasOrder 2 ;
    ns1:hasPractice ns1:4753e55e943c4d418303bf90d599c6b1 ;
    ns1:practice "SA" .

ns1:7fb68bc660774b9080963c17761529a2 a ns1:Stream ;
    rdfs:label "Software Requirements" ;
    dcterms:description "Software requirements specify objectives and expectations to protect the service and data at the core of the application." ;
    dcterms:identifier "7fb68bc660774b9080963c17761529a2" ;
    skos:altLabel "D-SR-A" ;
    ns1:hasLetter "A" ;
    ns1:hasOrder 1 ;
    ns1:hasPractice ns1:5702908efca4499e87a0239f32920d9b ;
    ns1:practice "SR" .

ns1:88c296acaae841a2b2fc5314bff44cb4 a ns1:BusinessFunction ;
    rdfs:label "Design" ;
    dcterms:description """Design concerns the processes and activities related to how an organization defines goals and creates software within development projects. In general, this will include requirements gathering, high-level architecture specification and detailed design.
""" ;
    dcterms:identifier "88c296acaae841a2b2fc5314bff44cb4" ;
    skos:altLabel "design" ;
    dcat:downloadURL "https://owaspsamm.org/model/design" ;
    ns1:hasOrder 2 ;
    ns1:model "SAMM20" .

ns1:8a64c7b0b35a458ea436260d5e414dfa a ns1:Stream ;
    rdfs:label "Deep Understanding" ;
    dcterms:description """Deep understanding focuses on performing manual security testing of high-risk components, using complex attack vectors with the goal of making advanced security testing an integral part of the development process. The goal of this stream is to favor testing depth (testing rigour) over testing width (the portfolio of applications).
""" ;
    dcterms:identifier "8a64c7b0b35a458ea436260d5e414dfa" ;
    skos:altLabel "V-ST-B" ;
    ns1:hasLetter "B" ;
    ns1:hasOrder 2 ;
    ns1:hasPractice ns1:bb5488860c124b6e8076b023485023e1 ;
    ns1:practice "ST" .

ns1:8a870a9b26724b4ba0dff177028b474a a ns1:Stream ;
    rdfs:label "Build Process" ;
    dcterms:description "A consistent build process ensures the software you are deploying is predictable and directly linked to the source code. Furthermore, you can take advantage of the software build process for various security activities." ;
    dcterms:identifier "8a870a9b26724b4ba0dff177028b474a" ;
    skos:altLabel "I-SB-A" ;
    ns1:hasLetter "A" ;
    ns1:hasOrder 1 ;
    ns1:hasPractice ns1:b2af112859d34cada6ce4cf44d393b94 ;
    ns1:practice "SB" .

ns1:8aa8154b83434e73b3ca8c0e9b654417 a ns1:BusinessFunction ;
    rdfs:label "Implementation" ;
    dcterms:description """Implementation is focused on the processes and activities related to how an organization builds and deploys software components and its related defects.

Activities within the Implementation function have the most impact on the daily life of developers. The joint goal is to ship reliably working software with minimum defects.
""" ;
    dcterms:identifier "8aa8154b83434e73b3ca8c0e9b654417" ;
    skos:altLabel "implementation" ;
    dcat:downloadURL "https://owaspsamm.org/model/implementation" ;
    ns1:hasOrder 3 ;
    ns1:model "SAMM20" .

ns1:8c1dcd10821f4f2baed52fdc83d93cf6 a ns1:Stream ;
    rdfs:label "Supplier Security" ;
    dcterms:description "Supplier security deals with requirements that are relative to supplier organizations within the development context of the application, in particular for outsourced development." ;
    dcterms:identifier "8c1dcd10821f4f2baed52fdc83d93cf6" ;
    skos:altLabel "D-SR-B" ;
    ns1:hasLetter "B" ;
    ns1:hasOrder 2 ;
    ns1:hasPractice ns1:5702908efca4499e87a0239f32920d9b ;
    ns1:practice "SR" .

ns1:942d679b0c9e41909f8bde728fdb1259 a ns1:BusinessFunction ;
    rdfs:label "Operations" ;
    dcterms:description """The Operations Business Function encompasses those activities necessary to ensure confidentiality, integrity, and availability are maintained throughout the operational lifetime of an application and its associated data. Increased maturity with regard to this Business Function provides greater assurance that the organization is resilient in the face of operational disruptions, and responsive to changes in the operational landscape.
""" ;
    dcterms:identifier "942d679b0c9e41909f8bde728fdb1259" ;
    skos:altLabel "operations" ;
    dcat:downloadURL "https://owaspsamm.org/model/operations" ;
    ns1:hasOrder 5 ;
    ns1:model "SAMM20" .

ns1:94bb47791e3d462cbf5f71ebb1a1327a a ns1:Stream ;
    rdfs:label "Create and Promote" ;
    dcterms:description "This stream is about creating and promoting an application security roadmap to set the objectives of the enterprise on this topic and increase alignment among stakeholders." ;
    dcterms:identifier "94bb47791e3d462cbf5f71ebb1a1327a" ;
    skos:altLabel "G-SM-A" ;
    ns1:hasLetter "A" ;
    ns1:hasOrder 1 ;
    ns1:hasPractice ns1:32b3bdd85d3a4d53827960004f9d1c7e ;
    ns1:practice "SM" .

ns1:9a5f26d77f204467bdda7ffa09109d73 a ns1:Stream ;
    rdfs:label "Secret Management" ;
    dcterms:description "As the secure execution of any software system requires credentials, this stream ensures a proper handling of these sensitive data elements within the organization's environment." ;
    dcterms:identifier "9a5f26d77f204467bdda7ffa09109d73" ;
    skos:altLabel "I-SD-B" ;
    ns1:hasLetter "B" ;
    ns1:hasOrder 2 ;
    ns1:hasPractice ns1:40d7879025144dbbbf34ba8ea82f060d ;
    ns1:practice "SD" .

ns1:9c6bf45a97ae4149a44c4a5d97ea6a40 a ns1:Stream ;
    rdfs:label "Data Protection" ;
    dcterms:description """The activities in this stream focus on ensuring the organization properly protects data in all aspects of their creation, handling, storage, and processing.
""" ;
    dcterms:identifier "9c6bf45a97ae4149a44c4a5d97ea6a40" ;
    skos:altLabel "O-OM-A" ;
    ns1:hasLetter "A" ;
    ns1:hasOrder 1 ;
    ns1:hasPractice ns1:8f07145b5ea74388b2217895d5e7b5c2 ;
    ns1:practice "OM" .

ns1:9ec70d6f7ddb4cb6b37928f9994c6049 a ns1:Stream ;
    rdfs:label "Deployment Process" ;
    dcterms:description "A repeatable and consistent deployment process ensures you only deploy correct software artifacts to production. It also paves the way for representative test environments prior to production." ;
    dcterms:identifier "9ec70d6f7ddb4cb6b37928f9994c6049" ;
    skos:altLabel "I-SD-A" ;
    ns1:hasLetter "A" ;
    ns1:hasOrder 1 ;
    ns1:hasPractice ns1:40d7879025144dbbbf34ba8ea82f060d ;
    ns1:practice "SD" .

ns1:a0d2ec4c6daa43369c07644b8745a7bd a ns1:Stream ;
    rdfs:label "System Decomissioning / Legacy Management" ;
    dcterms:description """From the perspective of the organization as a consumer of resources, the activities in this stream focus on the identification, management, and tracking of systems, applications, application dependencies, and services that are no longer used, have reached end of life, or are no longer actively developed or supported. Removal of unused systems and services improves manageability of the environment and reduces the organization's attack surface, while affording direct and indirect cost savings (e.g., reduced license count, reduced logging volume, or reduced analyst effort).
""" ;
    dcterms:identifier "a0d2ec4c6daa43369c07644b8745a7bd" ;
    skos:altLabel "O-OM-B" ;
    ns1:hasLetter "B" ;
    ns1:hasOrder 2 ;
    ns1:hasPractice ns1:8f07145b5ea74388b2217895d5e7b5c2 ;
    ns1:practice "OM" .

ns1:a5b57fc5fa0441b7b23f599b506c5752 a ns1:Stream ;
    rdfs:label "Defect Tracking" ;
    dcterms:description "Defect tracking manages the collection and follow-up of all potential issues in a piece of software, from architectural flaws to coding issues and run-time vulnerabilities." ;
    dcterms:identifier "a5b57fc5fa0441b7b23f599b506c5752" ;
    skos:altLabel "I-DM-A" ;
    ns1:hasLetter "A" ;
    ns1:hasOrder 1 ;
    ns1:hasPractice ns1:e17d573510904f65a1fe6040b56ad0b1 ;
    ns1:practice "DM" .

ns1:b7487370a07543cbb02ddb60c055d92f a ns1:Stream ;
    rdfs:label "Architecture Mitigation" ;
    dcterms:description """Architecture mitigation focuses on ensuring that all threats identified during Threat Assessment are adequately mitigated, and existing reference architectures updated to address any unhandled threats.
""" ;
    dcterms:identifier "b7487370a07543cbb02ddb60c055d92f" ;
    skos:altLabel "V-AA-B" ;
    ns1:hasLetter "B" ;
    ns1:hasOrder 2 ;
    ns1:hasPractice ns1:53f2da68c37a4ced8d5e767298fba589 ;
    ns1:practice "AA" .

ns1:c404aa4f711e4f4e9e71faea22f7fb5c a ns1:Stream ;
    rdfs:label "Policy & Standards" ;
    dcterms:description "This stream focuses on maintaining policies and standards and providing them to support integration into the SDLC." ;
    dcterms:identifier "c404aa4f711e4f4e9e71faea22f7fb5c" ;
    skos:altLabel "G-PC-A" ;
    ns1:hasLetter "A" ;
    ns1:hasOrder 1 ;
    ns1:hasPractice ns1:be9e7ddb98b84abe8b9e185b979ccf60 ;
    ns1:practice "PC" .

ns1:ed5a9c3dd7884c88918a45dc9d231c5d a ns1:Stream ;
    rdfs:label "Threat Modeling" ;
    dcterms:description "Threat modeling is intended to help software development teams understand what risks exist in what is being built, what could go wrong, and how we the risks can be mitigated or remediated." ;
    dcterms:identifier "ed5a9c3dd7884c88918a45dc9d231c5d" ;
    skos:altLabel "D-TA-B" ;
    ns1:hasLetter "B" ;
    ns1:hasOrder 2 ;
    ns1:hasPractice ns1:f9269aebfe2c4d5b9293ba42a40a93ac ;
    ns1:practice "TA" .

ns1:efb5d1f275504173899da345ef5bbe8e a ns1:Stream ;
    rdfs:label "Control Verification" ;
    dcterms:description """Control Verification validates that security controls and requirements are met through testing derived from requirements, and prevents the introduction of bugs into later releases through regression testing.
""" ;
    dcterms:identifier "efb5d1f275504173899da345ef5bbe8e" ;
    skos:altLabel "V-RT-A" ;
    ns1:hasLetter "A" ;
    ns1:hasOrder 1 ;
    ns1:hasPractice ns1:66fb99798fe946e4979a2de98e9d6f8b ;
    ns1:practice "RT" .

ns1:fa340fa1816244d79f369ae82e998368 a ns1:BusinessFunction ;
    rdfs:label "Verification" ;
    dcterms:description """Verification focuses on the processes and activities related to how an organization checks and tests artifacts produced throughout software development. This typically includes quality assurance work such as testing, but it can also include other review and evaluation activities.
""" ;
    dcterms:identifier "fa340fa1816244d79f369ae82e998368" ;
    skos:altLabel "verification" ;
    dcat:downloadURL "https://owaspsamm.org/model/verification" ;
    ns1:hasOrder 4 ;
    ns1:model "SAMM20" .

ns1:ff8a6a08dc684f38ab74b9db9584f0a5 a ns1:Stream ;
    rdfs:label "Incident Detection" ;
    dcterms:description """Incident Detection refers to the process of determining an identified security-relevant event is, in fact, a security incident. The activities in this stream focus on the organization's ability to identify security incidents when they occur, and to initiate appropriate incident response activities.
""" ;
    dcterms:identifier "ff8a6a08dc684f38ab74b9db9584f0a5" ;
    skos:altLabel "O-IM-A" ;
    ns1:hasLetter "A" ;
    ns1:hasOrder 1 ;
    ns1:hasPractice ns1:c13aa12c13d04362a3ca3385a8c580ee ;
    ns1:practice "IM" .

ns1:32b3bdd85d3a4d53827960004f9d1c7e a ns1:Practice ;
    rdfs:label "Strategy & Metrics" ;
    dcterms:description """Software assurance entails many different activities and concerns. Without an overall plan, you might be spending a lot of effort to build in security, while in fact your efforts may be unaligned, disproportional or even counterproductive. The goal of the Strategy & Metrics (SM) practice is to build an efficient and effective plan for realizing your software security objectives within your organization.

A software security program, that selects and prioritizes activities of the rest of the model, serves as the foundation for your efforts. The practice works on building the plan, maintaining and disseminating it.

At the same time, you want to keep track of your security posture and program improvements. A metrics-driven approach is included to ensure an accurate view on your activities. To measure is to know.
""" ;
    dcterms:identifier "32b3bdd85d3a4d53827960004f9d1c7e" ;
    rdfs:comment "This practice forms the basis of your secure software activities by building an overall plan." ;
    rdfs:seeAlso <https://owaspsamm.org/model/governance/strategy-and-metrics> ;
    skos:altLabel "SM" ;
    ns1:hasFunction ns1:102ad02df5dc4a8eb3837ef4ca2c1af4 ;
    ns1:hasOrder 1 .

ns1:40d7879025144dbbbf34ba8ea82f060d a ns1:Practice ;
    rdfs:label "Secure Deployment" ;
    dcterms:description """One of the final stages in delivering secure software is ensuring the security and integrity of developed applications are not compromised during deployment. The Secure Deployment (SD) practice focuses on this. To this end, the practice’s first stream focuses on removing manual error by automating the deployment process as much as possible, and making its success contingent upon the outcomes of integrated security verification checks. It also fosters Separation of Duties by making adequately trained, non-developers responsible for deployment.

The second stream goes beyond the mechanics of deployment, and focuses on protecting the privacy and integrity of sensitive data, such as passwords, tokens, and other secrets, required for applications to operate in production environments. In its simplest form, suitable production secrets are moved from repositories and configuration files into adequately managed digital vaults. In more advanced forms, secrets are dynamically generated at deployment time and routine processes detect and mitigate the presence of any unprotected secrets in the environment.
""" ;
    dcterms:identifier "40d7879025144dbbbf34ba8ea82f060d" ;
    rdfs:comment "This practice focuses on increasing the security of software deployments to the production environment and the supporting secrets." ;
    rdfs:seeAlso <https://owaspsamm.org/model/implementation/secure-deployment> ;
    skos:altLabel "SD" ;
    ns1:hasFunction ns1:8aa8154b83434e73b3ca8c0e9b654417 ;
    ns1:hasOrder 2 .

ns1:4753e55e943c4d418303bf90d599c6b1 a ns1:Practice ;
    rdfs:label "Security Architecture" ;
    dcterms:description """The Security Architecture (SA) practice focuses on the security linked to components and technology you deal with during the architectural design of your software. Secure Architecture Design looks at the selection and composition of components that form the foundation of your solution, focusing on its security properties. Technology management looks at the security of supporting technologies used during development, deployment and operations, such as development stacks and tooling, deployment tooling, and operating systems and tooling.
""" ;
    dcterms:identifier "4753e55e943c4d418303bf90d599c6b1" ;
    rdfs:comment "The security architecture practice focuses on managing architectural risks for the software solution." ;
    rdfs:seeAlso <https://owaspsamm.org/model/design/security-architecture> ;
    skos:altLabel "SA" ;
    ns1:hasFunction ns1:88c296acaae841a2b2fc5314bff44cb4 ;
    ns1:hasOrder 3 .

ns1:483a0a1b78264cafbc470ce72d557332 a ns1:Practice ;
    rdfs:label "Education & Guidance" ;
    dcterms:description """The Education & Guidance (EG) practice focuses on arming personnel involved in the software lifecycle with knowledge and resources to design, develop, and deploy secure software. With improved access to information, project teams can proactively identify and mitigate the specific security risks that apply to their organization.

One major theme for improvement across the Objectives is providing training for employees and increasing their security awareness, either through instructor-led sessions or computer-based modules. As an organization progresses, it builds a broad base of training starting with developers and moving to other roles, culminating with the addition of role-based training to ensure applicability and effectiveness.

In addition to training, this practice also requires the organization to make a significant investment in improving organizational culture to promote application security through collaboration between teams. Collaboration tools and increased transparency between technologies and tools support this approach to improve the security of the applications.
""" ;
    dcterms:identifier "483a0a1b78264cafbc470ce72d557332" ;
    rdfs:comment "This practice focuses on increasing the knowledge in the organization regarding secure software." ;
    rdfs:seeAlso <https://owaspsamm.org/model/governance/education-and-guidance> ;
    skos:altLabel "EG" ;
    ns1:hasFunction ns1:102ad02df5dc4a8eb3837ef4ca2c1af4 ;
    ns1:hasOrder 3 .

ns1:53a9cd5c2d3643f3b71e4e9d92b811e2 a ns1:Practice ;
    rdfs:label "Environment Management" ;
    dcterms:description """The organization's work on application security doesn't end once the application becomes operational. New security features and patches are regularly released for the various elements of the technology stack you're using, until they become obsolete or are no longer supported.

Most of the technologies in any application stack are not secure by default. This is frequently intentional, to enhance backwards compatibility or ease of setup. For this reason, ensuring the secure operation of the organization's technology stack requires the consistent application of secure baseline configurations to all components. The Environment Management (EM) practice focuses on keeping your environment clean and secure.

Vulnerabilities are discovered throughout the lifecycles of the technologies on which your organization relies, and new versions addressing them are released on various schedules. This makes it essential to monitor vulnerability reports and perform orderly, timely patching across all affected systems.
""" ;
    dcterms:identifier "53a9cd5c2d3643f3b71e4e9d92b811e2" ;
    rdfs:comment "This practice describes proactive activities carried out to improve and maintain the security of the environments in which the organization's applications operate." ;
    rdfs:seeAlso <https://owaspsamm.org/model/operations/environment-management> ;
    skos:altLabel "EM" ;
    ns1:hasFunction ns1:942d679b0c9e41909f8bde728fdb1259 ;
    ns1:hasOrder 2 .

ns1:53f2da68c37a4ced8d5e767298fba589 a ns1:Practice ;
    rdfs:label "Architecture Assessment" ;
    dcterms:description """The Architecture Assessment (AA) practice ensures that the application and infrastructure architecture adequately meets all relevant security and compliance requirements, and sufficiently mitigates identified security threats. The first stream focuses on verifying that the security and compliance requirements identified in the Policy & Compliance and Security Requirements practices are met, first in an ad-hoc manner, then more systematically for each interface in the system. The second stream reviews the architecture, first for mitigations against typical threats, then against the specific threats identified in the Threat Assessment practice.

In its more advanced form, the practice formalizes the security architecture review process, continuously evaluates the effectiveness of the architecture's security controls, their scalability and strategic alignment. Identified weaknesses and possible improvements are fed back to the Security Architecture practice to improve reference architectures.
""" ;
    dcterms:identifier "53f2da68c37a4ced8d5e767298fba589" ;
    rdfs:comment "This practice focuses on validating the security and compliance of the software and supporting infrastructure architecture." ;
    rdfs:seeAlso <https://owaspsamm.org/model/verification/architecture-assessment> ;
    skos:altLabel "AA" ;
    ns1:hasFunction ns1:fa340fa1816244d79f369ae82e998368 ;
    ns1:hasOrder 1 .

ns1:5702908efca4499e87a0239f32920d9b a ns1:Practice ;
    rdfs:label "Security Requirements" ;
    dcterms:description """The Security Requirements (SR) practice focuses on security requirements that are important
in the context of secure software. A first type deals with typical software-related
requirements, to specify objectives and expectations to protect the service and
data at the core of the application. A second type deals with requirements relative to supplier organizations that are part of the development context of the application, in particular for outsourced development. It is important to
streamline the expectations in terms of secure development because outsourced development
can have significant impact on the security of the application. The security of
3rd party (technical) libraries is part of the software supply chains stream (see
Secure Build), and it is not included in this practice.
""" ;
    dcterms:identifier "5702908efca4499e87a0239f32920d9b" ;
    rdfs:comment "This practice focuses on defining appropriate security requirements for your software and your software suppliers." ;
    rdfs:seeAlso <https://owaspsamm.org/model/design/security-requirements> ;
    skos:altLabel "SR" ;
    ns1:hasFunction ns1:88c296acaae841a2b2fc5314bff44cb4 ;
    ns1:hasOrder 2 .

ns1:66fb99798fe946e4979a2de98e9d6f8b a ns1:Practice ;
    rdfs:label "Requirements-driven Testing" ;
    dcterms:description """
The goal of the Requirements-driven Testing (RT) practice is to ensure that the implemented security controls operate as expected and satisfy the project's stated security requirements. It does so by incrementally building a set of security test and regression cases and executing them regularly.

A key aspect of this practice is its attention to both positive and negative testing. The former verifies that the application's security controls satisfy stated security requirements and validates their correct functioning. These requirements are typically functional in nature. Negative testing addresses the quality of the implementation of the security controls and aims to detect unexpected design flaws and implementation bugs through misuse and abuse testing. In its more advanced forms, the practice promotes security stress testing, such as denial of service, and strives to continuously improve application security by consistently automating security unit tests and creating security regression tests for all bugs identified and fixed.

Although both the Requirements-driven Testing and Security Testing practices are concerned with security testing, the former focuses on verifying the correct implementation of security requirements, while the latter aims to uncover technical implementation weaknesses in an application, irrespective of requirements.
""" ;
    dcterms:identifier "66fb99798fe946e4979a2de98e9d6f8b" ;
    rdfs:comment "This practice focuses on using both positive (control verification) and negative (misuse/abuse testing) security tests based on requirements (user stories)." ;
    rdfs:seeAlso <https://owaspsamm.org/model/verification/requirements-driven-testing> ;
    skos:altLabel "RT" ;
    ns1:hasFunction ns1:fa340fa1816244d79f369ae82e998368 ;
    ns1:hasOrder 2 .

ns1:8f07145b5ea74388b2217895d5e7b5c2 a ns1:Practice ;
    rdfs:label "Operational Management" ;
    dcterms:description """The Operational Management (OM) practice focuses on activities to ensure security is maintained throughout operational support functions. Although these functions are not performed directly by an application, the overall security of the application and its data depends on their proper performance. Deploying an application on an unsupported operating system with unpatched vulnerabilities, or failing to store backup media securely, can make the protections built into that application irrelevant.

The functions covered by this practice include, but are not limited to: system provisioning, administration, and decommissioning; database provisioning and administration; and data backup, restore, and archival.
""" ;
    dcterms:identifier "8f07145b5ea74388b2217895d5e7b5c2" ;
    rdfs:comment "This practice focuses on operational support activities required to maintain security throughout the product lifecycle." ;
    rdfs:seeAlso <https://owaspsamm.org/model/operations/operational-management> ;
    skos:altLabel "OM" ;
    ns1:hasFunction ns1:942d679b0c9e41909f8bde728fdb1259 ;
    ns1:hasOrder 3 .

ns1:b2af112859d34cada6ce4cf44d393b94 a ns1:Practice ;
    rdfs:label "Secure Build" ;
    dcterms:description """The Secure Build (SB) practice emphasises the importance of building software in a standardised, repeatable manner, and of doing so using secure components, including 3rd party software dependencies.

The first stream focuses on removing any subjectivity from the build process by striving for full automation. An automated build pipeline can include additional automated security checks such as SAST and DAST to gain further assurance and flag security regressions early by failing the build, for example.

The second stream acknowledges the prevalence of software dependencies in modern applications. It aims to identify them and track their security status in order to contain the impact of their insecurity on an otherwise secure application. In an advanced form, it applies similar security checks to software dependencies as to the application itself.
""" ;
    dcterms:identifier "b2af112859d34cada6ce4cf44d393b94" ;
    rdfs:comment "This practice focuses on creating a consistently repeatable build process and accounting for the security of application dependencies." ;
    rdfs:seeAlso <https://owaspsamm.org/model/implementation/secure-build> ;
    skos:altLabel "SB" ;
    ns1:hasFunction ns1:8aa8154b83434e73b3ca8c0e9b654417 ;
    ns1:hasOrder 1 .

ns1:bb5488860c124b6e8076b023485023e1 a ns1:Practice ;
    rdfs:label "Security Testing" ;
    dcterms:description """The Security Testing (ST) practice leverages the fact that, while automated security testing is fast and scales well to numerous applications, in-depth testing based on good knowledge of an application and its business logic is often only possible via slower, manual expert security testing. Each stream therefore has one approach at its core.

The first stream focuses on establishing a common security baseline to automatically detect so-called "low hanging fruit". Progressively customize the automated tests for each application and increase their frequency of execution to detect more bugs and regressions earlier, as close as possible to their inception. The more bugs the automated processes can detect, the more time experts have to use their knowledge and creativity to focus on more complex attack vectors and ensure in-depth application testing in the second stream. As manual review is slow and hard to scale, reviewers prioritize testing components based on their risk, recent relevant changes, or upcoming major releases. Organizations can also access external expertise by participating in bug bounty programs, for example.

Unlike the Requirements-driven testing practice which focuses on verifying that applications correctly implement their requirements, the goal of this practice is to uncover technical and business-logic weaknesses in application and make them visible to management and business stakeholders, irrespective of requirements.
""" ;
    dcterms:identifier "bb5488860c124b6e8076b023485023e1" ;
    rdfs:comment "This practice focuses on the detection and resolution of basic security issues through automation, allowing manual testing to focus on more complex attack vectors." ;
    rdfs:seeAlso <https://owaspsamm.org/model/verification/security-testing> ;
    skos:altLabel "ST" ;
    ns1:hasFunction ns1:fa340fa1816244d79f369ae82e998368 ;
    ns1:hasOrder 3 .

ns1:be9e7ddb98b84abe8b9e185b979ccf60 a ns1:Practice ;
    rdfs:label "Policy & Compliance" ;
    dcterms:description """The Policy & Compliance (PC) practice focuses on understanding and meeting external legal and regulatory requirements while driving internal security standards to ensure compliance in a way that’s aligned with the business purpose of the organization.

A driving theme for improvement within this practice is describing organization’s standards and 3rd party obligations as application requirements, enabling efficient and automated audits that may be leveraged within the SDLC and continuously demonstrate that all expectations are met.

In a sophisticated form, provision of this practice entails an organization-wide understanding of both internal standards and external compliance drivers while also maintaining low-latency checkpoints with project teams to ensure no project is operating outside expectations without visibility.
""" ;
    dcterms:identifier "be9e7ddb98b84abe8b9e185b979ccf60" ;
    rdfs:comment "This practice drives the adherence to internal and external standards and regulations." ;
    rdfs:seeAlso <https://owaspsamm.org/model/governance/policy-and-compliance> ;
    skos:altLabel "PC" ;
    ns1:hasFunction ns1:102ad02df5dc4a8eb3837ef4ca2c1af4 ;
    ns1:hasOrder 2 .

ns1:c13aa12c13d04362a3ca3385a8c580ee a ns1:Practice ;
    rdfs:label "Incident Management" ;
    dcterms:description """Once your organization has applications in operation, you're likely to face security incidents. In this model, we define a security incident as a breach, or the threat of an imminent breach, of at least one asset's security goals, whether due to malicious or negligent behavior. Examples of security incidents might include: a successful Denial of Service (DoS) attack against a cloud application, an application user accessing private data of another by abusing a security vulnerability, or an attacker modifying application source code. The Incident Management (IM) practice focuses on dealing with these in your organization.

Historically, many security incidents have been detected months, or even years, after the initial breach. During the "dwell time" before an incident is detected, significant damage can occur, increasing the difficulty of recovery. Our first activity stream, Incident Detection, focuses on decreasing that dwell time.

Once you have identified that you're suffering from a security incident, it's essential to respond in a disciplined, thorough manner to limit the damage, and return to normal operations as efficiently as possible. This is the focus of our second stream.
""" ;
    dcterms:identifier "c13aa12c13d04362a3ca3385a8c580ee" ;
    rdfs:comment "This practice addresses activities carried out improve the organization's detection of, and response to, security incidents." ;
    rdfs:seeAlso <https://owaspsamm.org/model/operations/incident-management> ;
    skos:altLabel "IM" ;
    ns1:hasFunction ns1:942d679b0c9e41909f8bde728fdb1259 ;
    ns1:hasOrder 1 .

ns1:e17d573510904f65a1fe6040b56ad0b1 a ns1:Practice ;
    rdfs:label "Defect Management" ;
    dcterms:description """The Defect Management (DM) practice focuses on collecting, recording, and analyzing software security defects and enriching them with information to drive metrics-based decisions.

The practice’s first stream deals with the process of handling and managing defects to ensure released software has a given assurance level. The second stream focuses on enriching the information about the defects and deriving metrics to guide decisions about the security of individual projects and of the security assurance program as a whole.

In a sophisticated form, the practice requires formalised, independent defect management and real-time, correlated information to detect trends and influence security strategy.
""" ;
    dcterms:identifier "e17d573510904f65a1fe6040b56ad0b1" ;
    rdfs:comment "This practice focuses on managing security defects in software and their associated metrics." ;
    rdfs:seeAlso <https://owaspsamm.org/model/implementation/defect-management> ;
    skos:altLabel "DM" ;
    ns1:hasFunction ns1:8aa8154b83434e73b3ca8c0e9b654417 ;
    ns1:hasOrder 3 .

ns1:f9269aebfe2c4d5b9293ba42a40a93ac a ns1:Practice ;
    rdfs:label "Threat Assessment" ;
    dcterms:description """The Threat Assessment (TA) practice focuses on identifying and understanding of project-level risks based on the functionality of the software being developed and characteristics of the runtime environment. From details about threats and likely attacks against each project, the organization as a whole operates more effectively through better decisions about prioritization of initiatives for security. Additionally, decisions for risk acceptance are more informed, therefore better aligned to the business.

By starting with simple threat models and building application risk profiles, an organization improves over time. Ultimately, a sophisticated organization would maintain this information in a way that is tightly coupled to the compensating factors and pass-through risks from external entities. This provides greater breadth of understanding for potential downstream impacts from security issues while keeping a close watch on the organization’s current performance against known threats.
""" ;
    dcterms:identifier "f9269aebfe2c4d5b9293ba42a40a93ac" ;
    rdfs:comment "This practice focuses on identifying potential threats in applications." ;
    rdfs:seeAlso <https://owaspsamm.org/model/design/threat-assessment> ;
    skos:altLabel "TA" ;
    ns1:hasFunction ns1:88c296acaae841a2b2fc5314bff44cb4 ;
    ns1:hasOrder 1 .

ns1:BusinessFunction a owl:Class .

ns1:MaturityLevel a owl:Class .

ns1:0a1dc80f84964f2fa776c5d8e932353a a ns1:MaturityLevel ;
    rdfs:label 1 ;
    dcterms:description "The first maturity level aims at achieving an ad-hoc, best effort implementation of a particular activity within a stream." ;
    dcterms:identifier "0a1dc80f84964f2fa776c5d8e932353a" ;
    skos:altLabel 1 .

ns1:47dd82af343e4695a0385418af4398d1 a ns1:MaturityLevel ;
    rdfs:label 2 ;
    dcterms:description "The second maturity level aims to establish a consistent, repeatable process that can be relied on." ;
    dcterms:identifier "47dd82af343e4695a0385418af4398d1" ;
    skos:altLabel 2 .

ns1:7bbfe31d447e48759ef0f2af25c31b43 a ns1:MaturityLevel ;
    rdfs:label 3 ;
    dcterms:description "The third maturity level aims to maximize effectiveness through continuous improvement, based on effective and timely feedback." ;
    dcterms:identifier "7bbfe31d447e48759ef0f2af25c31b43" ;
    skos:altLabel 3 .

ns1:Practice a owl:Class .

ns1:Stream a owl:Class .

ns1:PracticeLevel a owl:Class .

ns1:Activity a owl:Class .
