#
# Mapping iso 27001
#

@prefix dcat: <http://www.w3.org/ns/dcat#> .
@prefix dcterms: <http://purl.org/dc/terms/> .
@prefix ns1: <https://owaspsamm.org/model/> .
@prefix owl: <http://www.w3.org/2002/07/owl#> .
@prefix rdfs: <http://www.w3.org/2000/01/rdf-schema#> .
@prefix skos: <http://www.w3.org/2004/02/skos/core#> .
@prefix xsd: <http://www.w3.org/2001/XMLSchema#> .
@prefix iso: <http://par-tec.it/onto/iso/231/2017/iso27001/> .
@prefix iso27002_2013: <http://par-tec.it/onto/iso/27002/2013/> .
@prefix control: <http://par-tec.it/onto/iso/27001/control/> .
@prefix controlType: <http://par-tec.it/onto/iso/27001/control-type/> .
@prefix category: <http://par-tec.it/onto/iso/27001/category/> .

iso: a owl:Ontology ;
    dcterms:creator <mailto:robipolli@gmail.com> ;
    dcterms:description "ISO27001 Controls Ontology" ;
    dcterms:license <https://creativecommons.org/licenses/by-sa/4.0/>

.
iso:Control a owl:Class ;
    rdfs:subClassOf skos:Concept ;
    rdfs:label "Control" ;
    rdfs:comment "Controls are the basic building blocks of the ISO 27001 standard."
.

iso:ControlCategory a owl:Class;
    rdfs:subClassOf skos:Concept ;
    rdfs:label "Control Category" ;
    rdfs:comment "Control categories are the basic building blocks of the ISO 27001 standard."
.
iso:ControlType a owl:Class ;
    rdfs:subClassOf skos:Concept ;
    rdfs:label "Control Type" ;
    rdfs:comment "Control types are the different types of controls that can be used in the ISO 27001 standard."
.

iso:hasControlType a owl:ObjectProperty ;
    rdfs:label "hasControlType" ;
    rdfs:comment "The type of the control." ;
    rdfs:domain iso:Control ;
    rdfs:range controlType:ControlType .

iso:hasControlCategory a owl:ObjectProperty ;
    rdfs:label "hasControlCategory" ;
    rdfs:comment "The category of the control." ;
    rdfs:domain iso:Control ;
    rdfs:range category:ControlCategory .

iso:Preventive a iso:ControlType;
    rdfs:label "Preventive" ;
    rdfs:comment "Preventive controls are controls that prevent the occurrence of a risk." .
iso:Detective a iso:ControlType;
    rdfs:label "Detective" ;
    rdfs:comment "Detective controls are controls that detect the occurrence of a risk." .
iso:Corrective a iso:ControlType;
    rdfs:label "Corrective" ;
    rdfs:comment "Corrective controls are controls that correct a risk." .

iso:hasInformationSecurityProperty a owl:ObjectProperty ;
    rdfs:label "hasInformationSecurityProperty" ;
    rdfs:comment "The information security property of the control." ;
    rdfs:domain iso:Control ;
    rdfs:range iso:InformationSecurityProperty .

iso:InformationSecurityProperty a owl:Class;
    rdfs:subClassOf skos:Concept ;
    rdfs:label "Information Security Properties" ;
    rdfs:comment "Information security properties are the different properties that can be used in the ISO 27001 standard." .

iso:Confidentiality a iso:InformationSecurityProperty;
    rdfs:label "Confidentiality" ;
    rdfs:comment "Confidentiality properties are properties that protect the confidentiality of information."
    .
iso:Integrity a iso:InformationSecurityProperty;
    rdfs:label "Integrity" ;
    rdfs:comment "Integrity properties are properties that protect the integrity of information."
    .
iso:Availability a iso:InformationSecurityProperty;
    rdfs:label "Availability" ;
    rdfs:comment "Availability properties are properties that protect the availability of information."
    .

iso:hasCybersecurityConcet a owl:ObjectProperty ;
    rdfs:domain iso:Control ;
    rdfs:range iso:CybersecurityConcepts
.

iso:CybersecurityConcepts a owl:Class;
    rdfs:subClassOf skos:Concept ;
    rdfs:label "Cybersecurity Concepts" ;
    rdfs:comment "Cybersecurity concepts are the different concepts that can be used in the ISO 27001 standard."
    .

iso:Identify a iso:CybersecurityConcepts;
    rdfs:label "Identify" ;
    rdfs:comment "Identify concepts are concepts that identify information."
    .
iso:Protect a iso:CybersecurityConcepts;
    rdfs:label "Protect" ;
    rdfs:comment "Protect concepts are concepts that protect information."
    .
iso:Detect a iso:CybersecurityConcepts;
    rdfs:label "Detect" ;
    rdfs:comment "Detect concepts are concepts that detect information."
    .
iso:Respond a iso:CybersecurityConcepts;
    rdfs:label "Respond" ;
    rdfs:comment "Respond concepts are concepts that respond to information."
    .
iso:Recover a iso:CybersecurityConcepts;
    rdfs:label "Recover" ;
    rdfs:comment "Recover concepts are concepts that recover information."
    .

iso:OperationalCapability a owl:Class;
    rdfs:subClassOf skos:Concept ;
    rdfs:label "Operational Capabilities" ;
    rdfs:comment "Operational capabilities are the different capabilities that can be used in the ISO 27001 standard."
    .

iso:Governance a iso:OperationalCapability;
    rdfs:label "Governance" ;
    rdfs:comment "Governance capabilities are capabilities that govern the operation of information systems."
    .
iso:AssetManagement a iso:OperationalCapability;
    rdfs:label "Asset Management" ;
    rdfs:comment "Asset management capabilities are capabilities that manage information assets."
    .
iso:InformationProtection a iso:OperationalCapability;
    rdfs:label "Information Protection" ;
    rdfs:comment "Information protection capabilities are capabilities that protect information."
    .
iso:HRSecurity a iso:OperationalCapability;
    rdfs:label "Human Resources Security" ;
    rdfs:comment "Human resources security capabilities are capabilities that protect human resources."
    .
iso:PhysicalSecurity a iso:OperationalCapability;
    rdfs:label "Physical Security" ;
    rdfs:comment "Physical security capabilities are capabilities that protect physical assets."
    .
iso:SystemNetworkSecurity a iso:OperationalCapability;
    rdfs:label "System Network Security" ;
    rdfs:comment "System network security capabilities are capabilities that protect system network assets."
    .
iso:ApplicationSecurity a iso:OperationalCapability;
    rdfs:label "Application Security" ;
    rdfs:comment "Application security capabilities are capabilities that protect applications."
    .
iso:SecureConfiguration a iso:OperationalCapability;
    rdfs:label "Secure Configuration" ;
    rdfs:comment "Secure configuration capabilities are capabilities that secure configuration."
    .
iso:IAM a iso:OperationalCapability;
    rdfs:label "Identity and Access Management" ;
    rdfs:comment "Identity and access management capabilities are capabilities that manage identities and access."
    .
iso:ThreatManagement a iso:OperationalCapability;
    rdfs:label "Threat and Vulnerability Management" ;
    rdfs:comment "Threat and Vulnerability management capabilities are capabilities that manage threats."
    .
iso:Continuity a iso:OperationalCapability;
    rdfs:label "Continuity" ;
    rdfs:comment "Continuity capabilities are capabilities that manage continuity."
    .
iso:SupplierSecurity a iso:OperationalCapability;
    rdfs:label "Supplier and Relationship Security" ;
    rdfs:comment "Supplier security capabilities are capabilities that manage supplier assets."
    .
iso:Compliance a iso:OperationalCapability;
    rdfs:label "Legal andCompliance" ;
    rdfs:comment "Compliance capabilities are capabilities that manage compliance."
    .
iso:EventManangement a iso:OperationalCapability;
    rdfs:label "Event Management and Information" ;
    rdfs:comment "Event management capabilities are capabilities that manage events."
    .
#
# Security Domains
#
iso:SecurityDomain a owl:Class;
    rdfs:subClassOf skos:Concept ;
    rdfs:label "Security Domains" ;
    rdfs:comment "Security domains are the different domains that can be used in the ISO 27001 standard."
    .

iso:hasSecurityDomain a owl:ObjectProperty ;
    rdfs:label "hasInformationSecurityProperty" ;
    rdfs:comment "The information security property of the control." ;
    rdfs:domain iso:Control ;
    rdfs:range iso:SecurityDomain .


iso:GovernanceEcosystem a iso:SecurityDomain;
    rdfs:label "Governance and Ecosystem" ;
    rdfs:comment "Governance and Ecosystem domain are domains that govern the operation of information systems."
    .
iso:Protection a iso:SecurityDomain;
    rdfs:label "Protection and Risk" ;
    rdfs:comment "Protection and Risk domain are domains that protect information."
    .
iso:Defence a iso:SecurityDomain ;
    rdfs:label "Defence and Security" ;
    rdfs:comment "Defence and Security domain are domains that protect information."
    .
iso:Resilience a iso:SecurityDomain ;
    rdfs:label "Resilience and Recovery" ;
    rdfs:comment "Resilience and Recovery domain are domains that manage resilience."
    .
