@prefix dcterms: <http://purl.org/dc/terms/> .
@prefix iso: <https://par-tec.github.io/security-ontologies/onto/iso#> .
@prefix owl: <http://www.w3.org/2002/07/owl#> .
@prefix rdfs: <http://www.w3.org/2000/01/rdf-schema#> .
@prefix skos: <http://www.w3.org/2004/02/skos/core#> .
@prefix xsd: <http://www.w3.org/2001/XMLSchema#> .

iso: a owl:Ontology ;
    dcterms:creator <mailto:robipolli@gmail.com> ;
    dcterms:description "ISO27001 Controls Ontology" ;
    dcterms:license <https://creativecommons.org/licenses/by-sa/4.0/> .

<https://par-tec.github.io/security-ontologies/onto/iso#27001/2013/control-11.2.5> a iso:Control ;
    dcterms:description "Equipment, information or software shall not be taken off-site without prior authorization." ;
    dcterms:identifier "11.2.5" ;
    dcterms:title "Removal of assets" ;
    iso:controlSection <https://par-tec.github.io/security-ontologies/onto/iso#27001/2013/section-11.2> .

iso:Assurance a iso:OperationalCapability ;
    rdfs:label "Information security Assurance" ;
    rdfs:comment "Event management capabilities are capabilities that manage events." .

iso:EcosystemCybersecurityManagement a iso:GovernanceEcosystem ;
    rdfs:label "Ecosystem Cybersecurity Management" ;
    rdfs:comment "Ecosystem cybersecurity management domain is a domain that manages ecosystem cybersecurity." .

iso:ITSecurityAdministration a iso:Protection ;
    rdfs:label "IT Security Administration" ;
    rdfs:comment "IT security administration domain is a domain that manages IT security administration." .

iso:ITSecurityArchitecture a iso:Protection ;
    rdfs:label "IT Security Architecture" ;
    rdfs:comment "IT security architecture domain is a domain that manages IT security architecture." .

iso:InformationSystemSecurityGovernance_RiskManagement a iso:GovernanceEcosystem ;
    rdfs:label "Information System Security Governance and Risk Management" ;
    rdfs:comment "Information system security governance and risk management domain is a domain that manages information system security governance and risk management." .

iso:hasControlCategory a owl:ObjectProperty ;
    rdfs:label "hasControlCategory" ;
    rdfs:comment "The category of the control." ;
    rdfs:domain iso:Control ;
    rdfs:range iso:ControlCategory .

iso:hasControlType a owl:ObjectProperty ;
    rdfs:label "hasControlType" ;
    rdfs:comment "The type of the control." ;
    rdfs:domain iso:Control ;
    rdfs:range iso:ControlType .

iso:hasCybersecurityConcept a owl:ObjectProperty ;
    rdfs:comment "Associates an ISO Control to a NIST Cybersecurity Function." ;
    rdfs:domain iso:Control ;
    rdfs:range iso:CybersecurityConcept .

iso:hasInformationSecurityProperty a owl:ObjectProperty ;
    rdfs:label "hasInformationSecurityProperty" ;
    rdfs:comment "The information security property." ;
    rdfs:domain iso:Control ;
    rdfs:range iso:InformationSecurityProperty .

iso:hasOperationalCapability a owl:ObjectProperty ;
    rdfs:label "hasOperationalCapability" ;
    rdfs:comment "The operational capability." ;
    rdfs:domain iso:Control ;
    rdfs:range iso:OperationalCapability .

iso:hasSecurityDomain a owl:ObjectProperty ;
    rdfs:label "hasInformationSecurityProperty" ;
    rdfs:comment "The information security property of the control." ;
    rdfs:domain iso:Control ;
    rdfs:range iso:SecurityDomain .

<https://par-tec.github.io/security-ontologies/onto/iso#27001/2013/category-10> a iso:ControlCategory ;
    rdfs:label "Cryptography" .

<https://par-tec.github.io/security-ontologies/onto/iso#27001/2013/category-16> a iso:ControlCategory ;
    rdfs:label "Information security incident management" .

<https://par-tec.github.io/security-ontologies/onto/iso#27001/2013/category-5> a iso:ControlCategory ;
    rdfs:label "Information security policies" .

<https://par-tec.github.io/security-ontologies/onto/iso#27001/2013/control-10.1.1> a iso:Control ;
    dcterms:description "A policy on the use of cryptographic controls for protection of information shall be developed and implemented." ;
    dcterms:identifier "10.1.1" ;
    dcterms:title "Policy on the use of cryptographic controls" ;
    iso:controlSection <https://par-tec.github.io/security-ontologies/onto/iso#27001/2013/section-10.1> ;
    iso:correspondsTo <https://par-tec.github.io/security-ontologies/onto/iso#27002/2022/control-8.24> .

<https://par-tec.github.io/security-ontologies/onto/iso#27001/2013/control-10.1.2> a iso:Control ;
    dcterms:description "A policy on the use, protection and lifetime of cryptographic keys shall be developed and implemented through their whole lifecycle." ;
    dcterms:identifier "10.1.2" ;
    dcterms:title "Key management" ;
    iso:controlSection <https://par-tec.github.io/security-ontologies/onto/iso#27001/2013/section-10.1> ;
    iso:correspondsTo <https://par-tec.github.io/security-ontologies/onto/iso#27002/2022/control-8.24> .

<https://par-tec.github.io/security-ontologies/onto/iso#27001/2013/control-11.1.1> a iso:Control ;
    dcterms:description "Security perimeters shall be defined and used to protect areas that contain either sensitive or critical information and information processing facilities." ;
    dcterms:identifier "11.1.1" ;
    dcterms:title "Physical security perimeter" ;
    iso:controlSection <https://par-tec.github.io/security-ontologies/onto/iso#27001/2013/section-11.1> ;
    iso:correspondsTo <https://par-tec.github.io/security-ontologies/onto/iso#27002/2022/control-7.1> .

<https://par-tec.github.io/security-ontologies/onto/iso#27001/2013/control-11.1.2> a iso:Control ;
    dcterms:description "Secure areas shall be protected by appropriate entry controls to ensure that only authorized personnel are allowed access." ;
    dcterms:identifier "11.1.2" ;
    dcterms:title "Physical entry controls" ;
    iso:controlSection <https://par-tec.github.io/security-ontologies/onto/iso#27001/2013/section-11.1> ;
    iso:correspondsTo <https://par-tec.github.io/security-ontologies/onto/iso#27002/2022/control-7.2> .

<https://par-tec.github.io/security-ontologies/onto/iso#27001/2013/control-11.1.3> a iso:Control ;
    dcterms:description "Physical security for offices, rooms and facilities shall be designed and applied." ;
    dcterms:identifier "11.1.3" ;
    dcterms:title "Securing offices, rooms and facilities" ;
    iso:controlSection <https://par-tec.github.io/security-ontologies/onto/iso#27001/2013/section-11.1> ;
    iso:correspondsTo <https://par-tec.github.io/security-ontologies/onto/iso#27002/2022/control-7.3> .

<https://par-tec.github.io/security-ontologies/onto/iso#27001/2013/control-11.1.4> a iso:Control ;
    dcterms:description "Physical protection against natural disasters, malicious attack or accidents shall be designed and applied." ;
    dcterms:identifier "11.1.4" ;
    dcterms:title "Protecting against external and environmental threats" ;
    iso:controlSection <https://par-tec.github.io/security-ontologies/onto/iso#27001/2013/section-11.1> ;
    iso:correspondsTo <https://par-tec.github.io/security-ontologies/onto/iso#27002/2022/control-7.5> .

<https://par-tec.github.io/security-ontologies/onto/iso#27001/2013/control-11.1.5> a iso:Control ;
    dcterms:description "Procedures for working in secure areas shall be designed and applied." ;
    dcterms:identifier "11.1.5" ;
    dcterms:title "Working in secure areas" ;
    iso:controlSection <https://par-tec.github.io/security-ontologies/onto/iso#27001/2013/section-11.1> ;
    iso:correspondsTo <https://par-tec.github.io/security-ontologies/onto/iso#27002/2022/control-7.6> .

<https://par-tec.github.io/security-ontologies/onto/iso#27001/2013/control-11.1.6> a iso:Control ;
    dcterms:description "Access points such as delivery and loading areas and other points where unauthorized persons could enter the premises shall be controlled and, if possible, isolated from information processing facilities to avoid unauthorized access." ;
    dcterms:identifier "11.1.6" ;
    dcterms:title "Delivery and loading areas" ;
    iso:controlSection <https://par-tec.github.io/security-ontologies/onto/iso#27001/2013/section-11.1> ;
    iso:correspondsTo <https://par-tec.github.io/security-ontologies/onto/iso#27002/2022/control-7.2> .

<https://par-tec.github.io/security-ontologies/onto/iso#27001/2013/control-11.2.1> a iso:Control ;
    dcterms:description "Equipment shall be sited and protected to reduce the risks from environmental threats and hazards, and opportunities for unauthorized access." ;
    dcterms:identifier "11.2.1" ;
    dcterms:title "Equipment siting and protection" ;
    iso:controlSection <https://par-tec.github.io/security-ontologies/onto/iso#27001/2013/section-11.2> ;
    iso:correspondsTo <https://par-tec.github.io/security-ontologies/onto/iso#27002/2022/control-7.8> .

<https://par-tec.github.io/security-ontologies/onto/iso#27001/2013/control-11.2.2> a iso:Control ;
    dcterms:description "Equipment shall be protected from power failures and other disruptions caused by failures in supporting utilities." ;
    dcterms:identifier "11.2.2" ;
    dcterms:title "Supporting utilities" ;
    iso:controlSection <https://par-tec.github.io/security-ontologies/onto/iso#27001/2013/section-11.2> ;
    iso:correspondsTo <https://par-tec.github.io/security-ontologies/onto/iso#27002/2022/control-7.11> .

<https://par-tec.github.io/security-ontologies/onto/iso#27001/2013/control-11.2.3> a iso:Control ;
    dcterms:description "Power and telecommunications cabling carrying data or supporting information services shall be protected from interception, interference or damage." ;
    dcterms:identifier "11.2.3" ;
    dcterms:title "Cabling security" ;
    iso:controlSection <https://par-tec.github.io/security-ontologies/onto/iso#27001/2013/section-11.2> ;
    iso:correspondsTo <https://par-tec.github.io/security-ontologies/onto/iso#27002/2022/control-7.12> .

<https://par-tec.github.io/security-ontologies/onto/iso#27001/2013/control-11.2.4> a iso:Control ;
    dcterms:description "Equipment shall be correctly maintained to ensure its continued availability and integrity." ;
    dcterms:identifier "11.2.4" ;
    dcterms:title "Equipment maintenance" ;
    iso:controlSection <https://par-tec.github.io/security-ontologies/onto/iso#27001/2013/section-11.2> ;
    iso:correspondsTo <https://par-tec.github.io/security-ontologies/onto/iso#27002/2022/control-7.13> .

<https://par-tec.github.io/security-ontologies/onto/iso#27001/2013/control-11.2.6> a iso:Control ;
    dcterms:description "Security shall be applied to off-site assets taking into account the different risks of working outside the organization’s premises." ;
    dcterms:identifier "11.2.6" ;
    dcterms:title "Security of equipment and assets off-premises" ;
    iso:controlSection <https://par-tec.github.io/security-ontologies/onto/iso#27001/2013/section-11.2> ;
    iso:correspondsTo <https://par-tec.github.io/security-ontologies/onto/iso#27002/2022/control-7.9> .

<https://par-tec.github.io/security-ontologies/onto/iso#27001/2013/control-11.2.7> a iso:Control ;
    dcterms:description "All items of equipment containing storage media shall be verified to ensure that any sensitive data and licensed software has been removed or securely overwritten prior to disposal or re-use." ;
    dcterms:identifier "11.2.7" ;
    dcterms:title "Secure disposal or reuse of equipment" ;
    iso:controlSection <https://par-tec.github.io/security-ontologies/onto/iso#27001/2013/section-11.2> ;
    iso:correspondsTo <https://par-tec.github.io/security-ontologies/onto/iso#27002/2022/control-7.14> .

<https://par-tec.github.io/security-ontologies/onto/iso#27001/2013/control-11.2.8> a iso:Control ;
    dcterms:description "Users shall ensure that unattended equipment has appropriate protection." ;
    dcterms:identifier "11.2.8" ;
    dcterms:title "Unattended user equipment" ;
    iso:controlSection <https://par-tec.github.io/security-ontologies/onto/iso#27001/2013/section-11.2> ;
    iso:correspondsTo <https://par-tec.github.io/security-ontologies/onto/iso#27002/2022/control-8.1> .

<https://par-tec.github.io/security-ontologies/onto/iso#27001/2013/control-11.2.9> a iso:Control ;
    dcterms:description "A clear desk policy for papers and removable storage media and a clear screen policy for information processing facilities shall be adopted." ;
    dcterms:identifier "11.2.9" ;
    dcterms:title "Clear desk and clear screen policy" ;
    iso:controlSection <https://par-tec.github.io/security-ontologies/onto/iso#27001/2013/section-11.2> ;
    iso:correspondsTo <https://par-tec.github.io/security-ontologies/onto/iso#27002/2022/control-7.7> .

<https://par-tec.github.io/security-ontologies/onto/iso#27001/2013/control-12.1.1> a iso:Control ;
    dcterms:description "Operating procedures shall be documented and made available to all users who need them." ;
    dcterms:identifier "12.1.1" ;
    dcterms:title "Documented operating procedures" ;
    iso:controlSection <https://par-tec.github.io/security-ontologies/onto/iso#27001/2013/section-12.1> ;
    iso:correspondsTo <https://par-tec.github.io/security-ontologies/onto/iso#27002/2022/control-5.37> .

<https://par-tec.github.io/security-ontologies/onto/iso#27001/2013/control-12.1.2> a iso:Control ;
    dcterms:description "Changes to the organization, business processes, information processing facilities and systems that affect information security shall be controlled." ;
    dcterms:identifier "12.1.2" ;
    dcterms:title "Change management" ;
    iso:controlSection <https://par-tec.github.io/security-ontologies/onto/iso#27001/2013/section-12.1> ;
    iso:correspondsTo <https://par-tec.github.io/security-ontologies/onto/iso#27002/2022/control-8.32> .

<https://par-tec.github.io/security-ontologies/onto/iso#27001/2013/control-12.1.3> a iso:Control ;
    dcterms:description "The use of resources shall be monitored, tuned and projections made of future capacity requirements to ensure the required system performance." ;
    dcterms:identifier "12.1.3" ;
    dcterms:title "Capacity management" ;
    iso:controlSection <https://par-tec.github.io/security-ontologies/onto/iso#27001/2013/section-12.1> ;
    iso:correspondsTo <https://par-tec.github.io/security-ontologies/onto/iso#27002/2022/control-8.6> .

<https://par-tec.github.io/security-ontologies/onto/iso#27001/2013/control-12.1.4> a iso:Control ;
    dcterms:description "Development, testing, and operational environments shall be separated to reduce the risks of unauthorized access or changes to the operational environment." ;
    dcterms:identifier "12.1.4" ;
    dcterms:title "Separation of development, testing and operational environments" ;
    iso:controlSection <https://par-tec.github.io/security-ontologies/onto/iso#27001/2013/section-12.1> ;
    iso:correspondsTo <https://par-tec.github.io/security-ontologies/onto/iso#27002/2022/control-8.31> .

<https://par-tec.github.io/security-ontologies/onto/iso#27001/2013/control-12.2.1> a iso:Control ;
    dcterms:description "Detection, prevention and recovery controls to protect against malware shall be implemented, combined with appropriate user awareness." ;
    dcterms:identifier "12.2.1" ;
    dcterms:title "Controls against malware" ;
    iso:controlSection <https://par-tec.github.io/security-ontologies/onto/iso#27001/2013/section-12.2> ;
    iso:correspondsTo <https://par-tec.github.io/security-ontologies/onto/iso#27002/2022/control-8.7> .

<https://par-tec.github.io/security-ontologies/onto/iso#27001/2013/control-12.3.1> a iso:Control ;
    dcterms:description "Backup copies of information, software and system images shall be taken and tested regularly in accordance with an agreed backup policy." ;
    dcterms:identifier "12.3.1" ;
    dcterms:title "Information backup" ;
    iso:controlSection <https://par-tec.github.io/security-ontologies/onto/iso#27001/2013/section-12.3> ;
    iso:correspondsTo <https://par-tec.github.io/security-ontologies/onto/iso#27002/2022/control-8.13> .

<https://par-tec.github.io/security-ontologies/onto/iso#27001/2013/control-12.4.1> a iso:Control ;
    dcterms:description "Event logs recording user activities, exceptions, faults and information security events shall be produced, kept and regularly reviewed." ;
    dcterms:identifier "12.4.1" ;
    dcterms:title "Event logging" ;
    iso:controlSection <https://par-tec.github.io/security-ontologies/onto/iso#27001/2013/section-12.4> ;
    iso:correspondsTo <https://par-tec.github.io/security-ontologies/onto/iso#27002/2022/control-8.15> .

<https://par-tec.github.io/security-ontologies/onto/iso#27001/2013/control-12.4.2> a iso:Control ;
    dcterms:description "Logging facilities and log information shall be protected against tampering and unauthorized access." ;
    dcterms:identifier "12.4.2" ;
    dcterms:title "Protection of log information" ;
    iso:controlSection <https://par-tec.github.io/security-ontologies/onto/iso#27001/2013/section-12.4> ;
    iso:correspondsTo <https://par-tec.github.io/security-ontologies/onto/iso#27002/2022/control-8.15> .

<https://par-tec.github.io/security-ontologies/onto/iso#27001/2013/control-12.4.3> a iso:Control ;
    dcterms:description "System administrator and system operator activities shall be logged and the logs protected and regularly reviewed." ;
    dcterms:identifier "12.4.3" ;
    dcterms:title "Administrator and operator logs" ;
    iso:controlSection <https://par-tec.github.io/security-ontologies/onto/iso#27001/2013/section-12.4> ;
    iso:correspondsTo <https://par-tec.github.io/security-ontologies/onto/iso#27002/2022/control-8.15> .

<https://par-tec.github.io/security-ontologies/onto/iso#27001/2013/control-12.4.4> a iso:Control ;
    dcterms:description "The clocks of all relevant information processing systems within an organization or security domain shall be synchronized to a single reference time source." ;
    dcterms:identifier "12.4.4" ;
    dcterms:title "Clock synchronization" ;
    iso:controlSection <https://par-tec.github.io/security-ontologies/onto/iso#27001/2013/section-12.4> ;
    iso:correspondsTo <https://par-tec.github.io/security-ontologies/onto/iso#27002/2022/control-8.17> .

<https://par-tec.github.io/security-ontologies/onto/iso#27001/2013/control-12.5.1> a iso:Control ;
    dcterms:description "Procedures shall be implemented to control the installation of software on operational systems." ;
    dcterms:identifier "12.5.1" ;
    dcterms:title "Installation of software on operational systems" ;
    iso:controlSection <https://par-tec.github.io/security-ontologies/onto/iso#27001/2013/section-12.5> ;
    iso:correspondsTo <https://par-tec.github.io/security-ontologies/onto/iso#27002/2022/control-8.19> .

<https://par-tec.github.io/security-ontologies/onto/iso#27001/2013/control-12.6.1> a iso:Control ;
    dcterms:description "Information about technical vulnerabilities of information systems being used shall be obtained in a timely fashion, the organization’s exposure to such vulnerabilities evaluated and appropriate measures taken to address the associated risk." ;
    dcterms:identifier "12.6.1" ;
    dcterms:title "Management of technical vulnerabilities" ;
    iso:controlSection <https://par-tec.github.io/security-ontologies/onto/iso#27001/2013/section-12.6> ;
    iso:correspondsTo <https://par-tec.github.io/security-ontologies/onto/iso#27002/2022/control-8.8> .

<https://par-tec.github.io/security-ontologies/onto/iso#27001/2013/control-12.6.2> a iso:Control ;
    dcterms:description "Rules governing the installation of software by users shall be established and implemented." ;
    dcterms:identifier "12.6.2" ;
    dcterms:title "Restrictions on software installation" ;
    iso:controlSection <https://par-tec.github.io/security-ontologies/onto/iso#27001/2013/section-12.6> ;
    iso:correspondsTo <https://par-tec.github.io/security-ontologies/onto/iso#27002/2022/control-8.19> .

<https://par-tec.github.io/security-ontologies/onto/iso#27001/2013/control-12.7.1> a iso:Control ;
    dcterms:description "Audit requirements and activities involving verification of operational systems shall be carefully planned and agreed to minimize disruptions to business processes." ;
    dcterms:identifier "12.7.1" ;
    dcterms:title "Information systems audit controls" ;
    iso:controlSection <https://par-tec.github.io/security-ontologies/onto/iso#27001/2013/section-12.7> ;
    iso:correspondsTo <https://par-tec.github.io/security-ontologies/onto/iso#27002/2022/control-8.34> .

<https://par-tec.github.io/security-ontologies/onto/iso#27001/2013/control-13.1.1> a iso:Control ;
    dcterms:description "Networks shall be managed and controlled to protect information in systems and applications." ;
    dcterms:identifier "13.1.1" ;
    dcterms:title "Network controls" ;
    iso:controlSection <https://par-tec.github.io/security-ontologies/onto/iso#27001/2013/section-13.1> ;
    iso:correspondsTo <https://par-tec.github.io/security-ontologies/onto/iso#27002/2022/control-8.20> .

<https://par-tec.github.io/security-ontologies/onto/iso#27001/2013/control-13.1.2> a iso:Control ;
    dcterms:description "Security mechanisms, service levels and management requirements of all network services shall be identified and included in network services agreements, whether these services are provided in-house or outsourced." ;
    dcterms:identifier "13.1.2" ;
    dcterms:title """Security of network
services""" ;
    iso:controlSection <https://par-tec.github.io/security-ontologies/onto/iso#27001/2013/section-13.1> ;
    iso:correspondsTo <https://par-tec.github.io/security-ontologies/onto/iso#27002/2022/control-8.21> .

<https://par-tec.github.io/security-ontologies/onto/iso#27001/2013/control-13.1.3> a iso:Control ;
    dcterms:description "Groups of information services, users and information systems shall be segregated on networks." ;
    dcterms:identifier "13.1.3" ;
    dcterms:title "Segregation in networks" ;
    iso:controlSection <https://par-tec.github.io/security-ontologies/onto/iso#27001/2013/section-13.1> ;
    iso:correspondsTo <https://par-tec.github.io/security-ontologies/onto/iso#27002/2022/control-8.23> .

<https://par-tec.github.io/security-ontologies/onto/iso#27001/2013/control-13.2.1> a iso:Control ;
    dcterms:description "Formal transfer policies, procedures and controls shall be in place to protect the transfer of information through the use of all types of communication facilities." ;
    dcterms:identifier "13.2.1" ;
    dcterms:title "Information transfer policies and procedures" ;
    iso:controlSection <https://par-tec.github.io/security-ontologies/onto/iso#27001/2013/section-13.2> ;
    iso:correspondsTo <https://par-tec.github.io/security-ontologies/onto/iso#27002/2022/control-5.14> .

<https://par-tec.github.io/security-ontologies/onto/iso#27001/2013/control-13.2.2> a iso:Control ;
    dcterms:description "Agreements shall address the secure transfer of business information between the organization and external parties." ;
    dcterms:identifier "13.2.2" ;
    dcterms:title "Agreements on information transfer" ;
    iso:controlSection <https://par-tec.github.io/security-ontologies/onto/iso#27001/2013/section-13.2> ;
    iso:correspondsTo <https://par-tec.github.io/security-ontologies/onto/iso#27002/2022/control-5.14> .

<https://par-tec.github.io/security-ontologies/onto/iso#27001/2013/control-13.2.3> a iso:Control ;
    dcterms:description "Information involved in electronic messaging shall be appropriately protected." ;
    dcterms:identifier "13.2.3" ;
    dcterms:title "Electronic messaging" ;
    iso:controlSection <https://par-tec.github.io/security-ontologies/onto/iso#27001/2013/section-13.2> ;
    iso:correspondsTo <https://par-tec.github.io/security-ontologies/onto/iso#27002/2022/control-5.14> .

<https://par-tec.github.io/security-ontologies/onto/iso#27001/2013/control-13.2.4> a iso:Control ;
    dcterms:description "Requirements for confidentiality or non-disclosure agreements reflecting the organization’s needs for the protection of information shall be identified, regularly reviewed and documented." ;
    dcterms:identifier "13.2.4" ;
    dcterms:title "Confidentiality or nondisclosure agreements" ;
    iso:controlSection <https://par-tec.github.io/security-ontologies/onto/iso#27001/2013/section-13.2> ;
    iso:correspondsTo <https://par-tec.github.io/security-ontologies/onto/iso#27002/2022/control-6.6> .

<https://par-tec.github.io/security-ontologies/onto/iso#27001/2013/control-14.1.1> a iso:Control ;
    dcterms:description "The information security related requirements shall be included in the requirements for new information systems or enhancements to existing information systems." ;
    dcterms:identifier "14.1.1" ;
    dcterms:title """Information security
requirements analysis
and specification""" ;
    iso:controlSection <https://par-tec.github.io/security-ontologies/onto/iso#27001/2013/section-14.1> ;
    iso:correspondsTo <https://par-tec.github.io/security-ontologies/onto/iso#27002/2022/control-5.8> .

<https://par-tec.github.io/security-ontologies/onto/iso#27001/2013/control-14.1.2> a iso:Control ;
    dcterms:description "Information involved in application services passing over public networks shall be protected from fraudulent activity, contract dispute and unauthorized disclosure and modification." ;
    dcterms:identifier "14.1.2" ;
    dcterms:title """Securing application
services on public
networks""" ;
    iso:controlSection <https://par-tec.github.io/security-ontologies/onto/iso#27001/2013/section-14.1> ;
    iso:correspondsTo <https://par-tec.github.io/security-ontologies/onto/iso#27002/2022/control-8.26> .

<https://par-tec.github.io/security-ontologies/onto/iso#27001/2013/control-14.1.3> a iso:Control ;
    dcterms:description "Information involved in application service transactions shall be protected to prevent incomplete transmission, mis-routing, unauthorized message alteration, unauthorized disclosure, unauthorized message duplication or replay" ;
    dcterms:identifier "14.1.3" ;
    dcterms:title """Protecting application
services transactions""" ;
    iso:controlSection <https://par-tec.github.io/security-ontologies/onto/iso#27001/2013/section-14.1> ;
    iso:correspondsTo <https://par-tec.github.io/security-ontologies/onto/iso#27002/2022/control-8.26> .

<https://par-tec.github.io/security-ontologies/onto/iso#27001/2013/control-14.2.1> a iso:Control ;
    dcterms:description "Rules for the development of software and systems shall be established and applied to developments within the organization." ;
    dcterms:identifier "14.2.1" ;
    dcterms:title "Secure development policy" ;
    iso:controlSection <https://par-tec.github.io/security-ontologies/onto/iso#27001/2013/section-14.2> ;
    iso:correspondsTo <https://par-tec.github.io/security-ontologies/onto/iso#27002/2022/control-8.25> .

<https://par-tec.github.io/security-ontologies/onto/iso#27001/2013/control-14.2.2> a iso:Control ;
    dcterms:description "Changes to systems within the development lifecycle shall be controlled by the use of formal change control procedures." ;
    dcterms:identifier "14.2.2" ;
    dcterms:title "System change control procedures" ;
    iso:controlSection <https://par-tec.github.io/security-ontologies/onto/iso#27001/2013/section-14.2> ;
    iso:correspondsTo <https://par-tec.github.io/security-ontologies/onto/iso#27002/2022/control-8.32> .

<https://par-tec.github.io/security-ontologies/onto/iso#27001/2013/control-14.2.3> a iso:Control ;
    dcterms:description "When operating platforms are changed, business critical applications shall be reviewed and tested to ensure there is no adverse impact on organizational operations or security." ;
    dcterms:identifier "14.2.3" ;
    dcterms:title "Technical review of applications after operating platform changes" ;
    iso:controlSection <https://par-tec.github.io/security-ontologies/onto/iso#27001/2013/section-14.2> ;
    iso:correspondsTo <https://par-tec.github.io/security-ontologies/onto/iso#27002/2022/control-8.32> .

<https://par-tec.github.io/security-ontologies/onto/iso#27001/2013/control-14.2.4> a iso:Control ;
    dcterms:description "Modifications to software packages shall be discouraged, limited to necessary changes and all changes shall be strictly controlled." ;
    dcterms:identifier "14.2.4" ;
    dcterms:title "Restrictions on changes to software packages" ;
    iso:controlSection <https://par-tec.github.io/security-ontologies/onto/iso#27001/2013/section-14.2> ;
    iso:correspondsTo <https://par-tec.github.io/security-ontologies/onto/iso#27002/2022/control-8.32> .

<https://par-tec.github.io/security-ontologies/onto/iso#27001/2013/control-14.2.5> a iso:Control ;
    dcterms:description "Principles for engineering secure systems shall be established, documented, maintained and applied to any information system implementation efforts." ;
    dcterms:identifier "14.2.5" ;
    dcterms:title "Secure system engineering principles" ;
    iso:controlSection <https://par-tec.github.io/security-ontologies/onto/iso#27001/2013/section-14.2> ;
    iso:correspondsTo <https://par-tec.github.io/security-ontologies/onto/iso#27002/2022/control-8.27> .

<https://par-tec.github.io/security-ontologies/onto/iso#27001/2013/control-14.2.6> a iso:Control ;
    dcterms:description "Organizations shall establish and appropriately protect secure development environments for system development and integration efforts that cover the entire system development lifecycle." ;
    dcterms:identifier "14.2.6" ;
    dcterms:title "Secure development environment" ;
    iso:controlSection <https://par-tec.github.io/security-ontologies/onto/iso#27001/2013/section-14.2> ;
    iso:correspondsTo <https://par-tec.github.io/security-ontologies/onto/iso#27002/2022/control-8.31> .

<https://par-tec.github.io/security-ontologies/onto/iso#27001/2013/control-14.2.7> a iso:Control ;
    dcterms:description "The organization shall supervise and monitor the activity of outsourced system development." ;
    dcterms:identifier "14.2.7" ;
    dcterms:title "Outsourced development" ;
    iso:controlSection <https://par-tec.github.io/security-ontologies/onto/iso#27001/2013/section-14.2> ;
    iso:correspondsTo <https://par-tec.github.io/security-ontologies/onto/iso#27002/2022/control-8.30> .

<https://par-tec.github.io/security-ontologies/onto/iso#27001/2013/control-14.2.8> a iso:Control ;
    dcterms:description "Testing of security functionality shall be carried out during development." ;
    dcterms:identifier "14.2.8" ;
    dcterms:title "System security testing" ;
    iso:controlSection <https://par-tec.github.io/security-ontologies/onto/iso#27001/2013/section-14.2> ;
    iso:correspondsTo <https://par-tec.github.io/security-ontologies/onto/iso#27002/2022/control-8.29> .

<https://par-tec.github.io/security-ontologies/onto/iso#27001/2013/control-14.2.9> a iso:Control ;
    dcterms:description "Acceptance testing programs and related criteria shall be established for new information systems, upgrades and new versions." ;
    dcterms:identifier "14.2.9" ;
    dcterms:title "System acceptance testing" ;
    iso:controlSection <https://par-tec.github.io/security-ontologies/onto/iso#27001/2013/section-14.2> ;
    iso:correspondsTo <https://par-tec.github.io/security-ontologies/onto/iso#27002/2022/control-8.29> .

<https://par-tec.github.io/security-ontologies/onto/iso#27001/2013/control-14.3.1> a iso:Control ;
    dcterms:description "Test data shall be selected carefully, protected and controlled." ;
    dcterms:identifier "14.3.1" ;
    dcterms:title "Protection of test data" ;
    iso:controlSection <https://par-tec.github.io/security-ontologies/onto/iso#27001/2013/section-14.3> ;
    iso:correspondsTo <https://par-tec.github.io/security-ontologies/onto/iso#27002/2022/control-8.33> .

<https://par-tec.github.io/security-ontologies/onto/iso#27001/2013/control-15.1.1> a iso:Control ;
    dcterms:description "Information security requirements for mitigating the risks associated with supplier’s access to the organization’s assets shall be agreed with the supplier and documented." ;
    dcterms:identifier "15.1.1" ;
    dcterms:title "Information security policy for supplier relationships" ;
    iso:controlSection <https://par-tec.github.io/security-ontologies/onto/iso#27001/2013/section-15.1> ;
    iso:correspondsTo <https://par-tec.github.io/security-ontologies/onto/iso#27002/2022/control-5.19> .

<https://par-tec.github.io/security-ontologies/onto/iso#27001/2013/control-15.1.2> a iso:Control ;
    dcterms:description "All relevant information security requirements shall be established and agreed with each supplier that may access, process, store, communicate, or provide IT infrastructure components for, the organization’s information." ;
    dcterms:identifier "15.1.2" ;
    dcterms:title "Addressing security within supplier agreements" ;
    iso:controlSection <https://par-tec.github.io/security-ontologies/onto/iso#27001/2013/section-15.1> ;
    iso:correspondsTo <https://par-tec.github.io/security-ontologies/onto/iso#27002/2022/control-5.20> .

<https://par-tec.github.io/security-ontologies/onto/iso#27001/2013/control-15.1.3> a iso:Control ;
    dcterms:description "Agreements with suppliers shall include requirements to address the information security risks associated with information and communications technology services and product supply chain." ;
    dcterms:identifier "15.1.3" ;
    dcterms:title "Information and communication technology supply chain" ;
    iso:controlSection <https://par-tec.github.io/security-ontologies/onto/iso#27001/2013/section-15.1> ;
    iso:correspondsTo <https://par-tec.github.io/security-ontologies/onto/iso#27002/2022/control-5.21> .

<https://par-tec.github.io/security-ontologies/onto/iso#27001/2013/control-15.2.1> a iso:Control ;
    dcterms:description "Organizations shall regularly monitor, review and audit supplier service delivery." ;
    dcterms:identifier "15.2.1" ;
    dcterms:title "Monitoring and review of supplier services" ;
    iso:controlSection <https://par-tec.github.io/security-ontologies/onto/iso#27001/2013/section-15.2> ;
    iso:correspondsTo <https://par-tec.github.io/security-ontologies/onto/iso#27002/2022/control-5.22> .

<https://par-tec.github.io/security-ontologies/onto/iso#27001/2013/control-15.2.2> a iso:Control ;
    dcterms:description "Changes to the provision of services by suppliers, including maintaining and improving existing information security policies, procedures and controls, shall be managed, taking account of the criticality of business information, systems and processes involved and re-assessment of risks." ;
    dcterms:identifier "15.2.2" ;
    dcterms:title "Managing changes to supplier services" ;
    iso:controlSection <https://par-tec.github.io/security-ontologies/onto/iso#27001/2013/section-15.2> ;
    iso:correspondsTo <https://par-tec.github.io/security-ontologies/onto/iso#27002/2022/control-5.22> .

<https://par-tec.github.io/security-ontologies/onto/iso#27001/2013/control-16.1.1> a iso:Control ;
    dcterms:description "Management responsibilities and procedures shall be established to ensure a quick, effective and orderly response to information security incidents." ;
    dcterms:identifier "16.1.1" ;
    dcterms:title "Responsibilities and procedures" ;
    iso:controlSection <https://par-tec.github.io/security-ontologies/onto/iso#27001/2013/section-16.1> ;
    iso:correspondsTo <https://par-tec.github.io/security-ontologies/onto/iso#27002/2022/control-5.24> .

<https://par-tec.github.io/security-ontologies/onto/iso#27001/2013/control-16.1.2> a iso:Control ;
    dcterms:description "Information security events shall be reported through appropriate management channels as quickly as possible." ;
    dcterms:identifier "16.1.2" ;
    dcterms:title "Reporting information security events" ;
    iso:controlSection <https://par-tec.github.io/security-ontologies/onto/iso#27001/2013/section-16.1> ;
    iso:correspondsTo <https://par-tec.github.io/security-ontologies/onto/iso#27002/2022/control-6.8> .

<https://par-tec.github.io/security-ontologies/onto/iso#27001/2013/control-16.1.3> a iso:Control ;
    dcterms:description "Employees and contractors using the organization’s information systems and services shall be required to note and report any observed or suspected information security weaknesses in systems or services." ;
    dcterms:identifier "16.1.3" ;
    dcterms:title "Reporting information security weaknesses" ;
    iso:controlSection <https://par-tec.github.io/security-ontologies/onto/iso#27001/2013/section-16.1> ;
    iso:correspondsTo <https://par-tec.github.io/security-ontologies/onto/iso#27002/2022/control-6.8> .

<https://par-tec.github.io/security-ontologies/onto/iso#27001/2013/control-16.1.4> a iso:Control ;
    dcterms:description "Information security events shall be assessed and it shall be decided if they are to be classified as information security incidents." ;
    dcterms:identifier "16.1.4" ;
    dcterms:title "Assessment of and decision on information security events" ;
    iso:controlSection <https://par-tec.github.io/security-ontologies/onto/iso#27001/2013/section-16.1> ;
    iso:correspondsTo <https://par-tec.github.io/security-ontologies/onto/iso#27002/2022/control-5.25> .

<https://par-tec.github.io/security-ontologies/onto/iso#27001/2013/control-16.1.5> a iso:Control ;
    dcterms:description "Information security incidents shall be responded to in accordance with the documented procedures." ;
    dcterms:identifier "16.1.5" ;
    dcterms:title "Response to information security incidents" ;
    iso:controlSection <https://par-tec.github.io/security-ontologies/onto/iso#27001/2013/section-16.1> ;
    iso:correspondsTo <https://par-tec.github.io/security-ontologies/onto/iso#27002/2022/control-5.26> .

<https://par-tec.github.io/security-ontologies/onto/iso#27001/2013/control-16.1.6> a iso:Control ;
    dcterms:description "Knowledge gained from analyzing and resolving information security incidents shall be used to reduce the likelihood or impact of future incidents." ;
    dcterms:identifier "16.1.6" ;
    dcterms:title "Learning from information security incidents" ;
    iso:controlSection <https://par-tec.github.io/security-ontologies/onto/iso#27001/2013/section-16.1> ;
    iso:correspondsTo <https://par-tec.github.io/security-ontologies/onto/iso#27002/2022/control-5.27> .

<https://par-tec.github.io/security-ontologies/onto/iso#27001/2013/control-16.1.7> a iso:Control ;
    dcterms:description "The organization shall define and apply procedures for the identification, collection, acquisition and preservation of information, which can serve as evidence." ;
    dcterms:identifier "16.1.7" ;
    dcterms:title "Collection of evidence" ;
    iso:controlSection <https://par-tec.github.io/security-ontologies/onto/iso#27001/2013/section-16.1> ;
    iso:correspondsTo <https://par-tec.github.io/security-ontologies/onto/iso#27002/2022/control-5.28> .

<https://par-tec.github.io/security-ontologies/onto/iso#27001/2013/control-17.1.1> a iso:Control ;
    dcterms:description "The organization shall determine its requirements for information security and the continuity of information security management in adverse situations, e.g. during a crisis or disaster." ;
    dcterms:identifier "17.1.1" ;
    dcterms:title "Planning information security continuity" ;
    iso:controlSection <https://par-tec.github.io/security-ontologies/onto/iso#27001/2013/section-17.1> ;
    iso:correspondsTo <https://par-tec.github.io/security-ontologies/onto/iso#27002/2022/control-5.29> .

<https://par-tec.github.io/security-ontologies/onto/iso#27001/2013/control-17.1.2> a iso:Control ;
    dcterms:description "The organization shall establish, document, implement and maintain processes, procedures and controls to ensure the required level of continuity for information security during an adverse situation." ;
    dcterms:identifier "17.1.2" ;
    dcterms:title "Implementing information security continuity" ;
    iso:controlSection <https://par-tec.github.io/security-ontologies/onto/iso#27001/2013/section-17.1> ;
    iso:correspondsTo <https://par-tec.github.io/security-ontologies/onto/iso#27002/2022/control-5.29> .

<https://par-tec.github.io/security-ontologies/onto/iso#27001/2013/control-17.1.3> a iso:Control ;
    dcterms:description "The organization shall verify the established and implemented information security continuity controls at regular intervals in order to ensure that they are valid and effective during adverse situations." ;
    dcterms:identifier "17.1.3" ;
    dcterms:title "Verify, review and evaluate information security continuity" ;
    iso:controlSection <https://par-tec.github.io/security-ontologies/onto/iso#27001/2013/section-17.1> ;
    iso:correspondsTo <https://par-tec.github.io/security-ontologies/onto/iso#27002/2022/control-5.29> .

<https://par-tec.github.io/security-ontologies/onto/iso#27001/2013/control-17.2.1> a iso:Control ;
    dcterms:description "Information processing facilities shall be implemented with redundancy sufficient to meet availability requirements." ;
    dcterms:identifier "17.2.1" ;
    dcterms:title "Availability of information processing facilities" ;
    iso:controlSection <https://par-tec.github.io/security-ontologies/onto/iso#27001/2013/section-17.2> ;
    iso:correspondsTo <https://par-tec.github.io/security-ontologies/onto/iso#27002/2022/control-8.14> .

<https://par-tec.github.io/security-ontologies/onto/iso#27001/2013/control-18.1.1> a iso:Control ;
    dcterms:description "All relevant legislative statutory, regulatory, contractual requirements and the organization’s approach to meet these requirements shall be explicitly identified, documented and kept up to date for each information system and the organization." ;
    dcterms:identifier "18.1.1" ;
    dcterms:title "Identification of applicable legislation and contractual requirements" ;
    iso:controlSection <https://par-tec.github.io/security-ontologies/onto/iso#27001/2013/section-18.1> ;
    iso:correspondsTo <https://par-tec.github.io/security-ontologies/onto/iso#27002/2022/control-5.31> .

<https://par-tec.github.io/security-ontologies/onto/iso#27001/2013/control-18.1.2> a iso:Control ;
    dcterms:description "Appropriate procedures shall be implemented to ensure compliance with legislative, regulatory and contractual requirements related to intellectual property rights and use of proprietary software products." ;
    dcterms:identifier "18.1.2" ;
    dcterms:title "Intellectual property rights" ;
    iso:controlSection <https://par-tec.github.io/security-ontologies/onto/iso#27001/2013/section-18.1> ;
    iso:correspondsTo <https://par-tec.github.io/security-ontologies/onto/iso#27002/2022/control-5.32> .

<https://par-tec.github.io/security-ontologies/onto/iso#27001/2013/control-18.1.3> a iso:Control ;
    dcterms:description "Records shall be protected from loss, destruction, falsification, unauthorized access and unauthorized release, in accordance with legislative, regulatory, contractual and business requirements." ;
    dcterms:identifier "18.1.3" ;
    dcterms:title "Protection of records" ;
    iso:controlSection <https://par-tec.github.io/security-ontologies/onto/iso#27001/2013/section-18.1> ;
    iso:correspondsTo <https://par-tec.github.io/security-ontologies/onto/iso#27002/2022/control-5.33> .

<https://par-tec.github.io/security-ontologies/onto/iso#27001/2013/control-18.1.4> a iso:Control ;
    dcterms:description "Privacy and protection of personally identifiable information shall be ensured as required in relevant legislation and regulation where applicable." ;
    dcterms:identifier "18.1.4" ;
    dcterms:title "Privacy and protection of personally identifiable information" ;
    iso:controlSection <https://par-tec.github.io/security-ontologies/onto/iso#27001/2013/section-18.1> ;
    iso:correspondsTo <https://par-tec.github.io/security-ontologies/onto/iso#27002/2022/control-5.34> .

<https://par-tec.github.io/security-ontologies/onto/iso#27001/2013/control-18.1.5> a iso:Control ;
    dcterms:description "Cryptographic controls shall be used in compliance with all relevant agreements, legislation and regulations." ;
    dcterms:identifier "18.1.5" ;
    dcterms:title "Regulation of cryptographic controls" ;
    iso:controlSection <https://par-tec.github.io/security-ontologies/onto/iso#27001/2013/section-18.1> ;
    iso:correspondsTo <https://par-tec.github.io/security-ontologies/onto/iso#27002/2022/control-5.31> .

<https://par-tec.github.io/security-ontologies/onto/iso#27001/2013/control-18.2.1> a iso:Control ;
    dcterms:description "The organization’s approach to managing information security and its implementation (i.e. control objectives, controls, policies, processes and procedures for information security) shall be reviewed independently at planned intervals or when significant changes occur." ;
    dcterms:identifier "18.2.1" ;
    dcterms:title "Independent review of information security" ;
    iso:controlSection <https://par-tec.github.io/security-ontologies/onto/iso#27001/2013/section-18.2> ;
    iso:correspondsTo <https://par-tec.github.io/security-ontologies/onto/iso#27002/2022/control-5.35> .

<https://par-tec.github.io/security-ontologies/onto/iso#27001/2013/control-18.2.2> a iso:Control ;
    dcterms:description "Managers shall regularly review the compliance of information processing and procedures within their area of responsibility with the appropriate security policies, standards and any other security requirements." ;
    dcterms:identifier "18.2.2" ;
    dcterms:title "Compliance with security policies and standards" ;
    iso:controlSection <https://par-tec.github.io/security-ontologies/onto/iso#27001/2013/section-18.2> ;
    iso:correspondsTo <https://par-tec.github.io/security-ontologies/onto/iso#27002/2022/control-5.36> .

<https://par-tec.github.io/security-ontologies/onto/iso#27001/2013/control-5.1.1> a iso:Control ;
    dcterms:description "A set of policies for information security shall be defined, approved by management, published and communicated to employees and relevant external parties." ;
    dcterms:identifier "5.1.1" ;
    dcterms:title "Policies for information security" ;
    iso:controlSection <https://par-tec.github.io/security-ontologies/onto/iso#27001/2013/section-5.1> ;
    iso:correspondsTo <https://par-tec.github.io/security-ontologies/onto/iso#27002/2022/control-5.1> .

<https://par-tec.github.io/security-ontologies/onto/iso#27001/2013/control-5.1.2> a iso:Control ;
    dcterms:description "The policies for information security shall be reviewed at planned intervals or if significant changes occur to ensure their continuing suitability, adequacy and effectiveness." ;
    dcterms:identifier "5.1.2" ;
    dcterms:title "Review of the policies for information security" ;
    iso:controlSection <https://par-tec.github.io/security-ontologies/onto/iso#27001/2013/section-5.1> ;
    iso:correspondsTo <https://par-tec.github.io/security-ontologies/onto/iso#27002/2022/control-5.1> .

<https://par-tec.github.io/security-ontologies/onto/iso#27001/2013/control-6.1.1> a iso:Control ;
    dcterms:description "All information security responsibilities shall be defined and allocated." ;
    dcterms:identifier "6.1.1" ;
    dcterms:title "Information security roles and responsibilities" ;
    iso:controlSection <https://par-tec.github.io/security-ontologies/onto/iso#27001/2013/section-6.1> ;
    iso:correspondsTo <https://par-tec.github.io/security-ontologies/onto/iso#27002/2022/control-5.2> .

<https://par-tec.github.io/security-ontologies/onto/iso#27001/2013/control-6.1.2> a iso:Control ;
    dcterms:description "Conflicting duties and areas of responsibility shall be segregated to reduce opportunities for unauthorized or unintentional modification or misuse of the organization’s assets." ;
    dcterms:identifier "6.1.2" ;
    dcterms:title "Segregation of duties" ;
    iso:controlSection <https://par-tec.github.io/security-ontologies/onto/iso#27001/2013/section-6.1> ;
    iso:correspondsTo <https://par-tec.github.io/security-ontologies/onto/iso#27002/2022/control-5.3> .

<https://par-tec.github.io/security-ontologies/onto/iso#27001/2013/control-6.1.3> a iso:Control ;
    dcterms:description "Appropriate contacts with relevant authorities shall be maintained." ;
    dcterms:identifier "6.1.3" ;
    dcterms:title "Contact with authorities" ;
    iso:controlSection <https://par-tec.github.io/security-ontologies/onto/iso#27001/2013/section-6.1> ;
    iso:correspondsTo <https://par-tec.github.io/security-ontologies/onto/iso#27002/2022/control-5.5> .

<https://par-tec.github.io/security-ontologies/onto/iso#27001/2013/control-6.1.4> a iso:Control ;
    dcterms:description "Appropriate contacts with special interest groups or other specialist security forums and professional associations shall be maintained." ;
    dcterms:identifier "6.1.4" ;
    dcterms:title "Contact with special interest groups" ;
    iso:controlSection <https://par-tec.github.io/security-ontologies/onto/iso#27001/2013/section-6.1> ;
    iso:correspondsTo <https://par-tec.github.io/security-ontologies/onto/iso#27002/2022/control-5.6> .

<https://par-tec.github.io/security-ontologies/onto/iso#27001/2013/control-6.1.5> a iso:Control ;
    dcterms:description "Information security shall be addressed in project management, regardless of the type of the project." ;
    dcterms:identifier "6.1.5" ;
    dcterms:title "Information security in project management" ;
    iso:controlSection <https://par-tec.github.io/security-ontologies/onto/iso#27001/2013/section-6.1> ;
    iso:correspondsTo <https://par-tec.github.io/security-ontologies/onto/iso#27002/2022/control-5.8> .

<https://par-tec.github.io/security-ontologies/onto/iso#27001/2013/control-6.2.1> a iso:Control ;
    dcterms:description "A policy and supporting security measures shall be adopted to manage the risks introduced by using mobile devices." ;
    dcterms:identifier "6.2.1" ;
    dcterms:title "Mobile device policy" ;
    iso:controlSection <https://par-tec.github.io/security-ontologies/onto/iso#27001/2013/section-6.2> ;
    iso:correspondsTo <https://par-tec.github.io/security-ontologies/onto/iso#27002/2022/control-8.1> .

<https://par-tec.github.io/security-ontologies/onto/iso#27001/2013/control-6.2.2> a iso:Control ;
    dcterms:description "A policy and supporting security measures shall be implemented to protect information accessed, processed or stored at teleworking sites." ;
    dcterms:identifier "6.2.2" ;
    dcterms:title "Teleworking" ;
    iso:controlSection <https://par-tec.github.io/security-ontologies/onto/iso#27001/2013/section-6.2> ;
    iso:correspondsTo <https://par-tec.github.io/security-ontologies/onto/iso#27002/2022/control-6.7> .

<https://par-tec.github.io/security-ontologies/onto/iso#27001/2013/control-7.1.1> a iso:Control ;
    dcterms:description "Background verification checks on all candidates for employment shall be carried out in accordance with relevant laws, regulations and ethics and shall be proportional to the business requirements, the classification of the information to be accessed and the perceived risks." ;
    dcterms:identifier "7.1.1" ;
    dcterms:title "Screening" ;
    iso:controlSection <https://par-tec.github.io/security-ontologies/onto/iso#27001/2013/section-7.1> ;
    iso:correspondsTo <https://par-tec.github.io/security-ontologies/onto/iso#27002/2022/control-6.1> .

<https://par-tec.github.io/security-ontologies/onto/iso#27001/2013/control-7.1.2> a iso:Control ;
    dcterms:description "The contractual agreements with employees and contractors shall state their and the organization’s responsibilities for information security." ;
    dcterms:identifier "7.1.2" ;
    dcterms:title "Terms and conditions of employment" ;
    iso:controlSection <https://par-tec.github.io/security-ontologies/onto/iso#27001/2013/section-7.1> ;
    iso:correspondsTo <https://par-tec.github.io/security-ontologies/onto/iso#27002/2022/control-6.2> .

<https://par-tec.github.io/security-ontologies/onto/iso#27001/2013/control-7.2.1> a iso:Control ;
    dcterms:description "Management shall require all employees and contractors to apply information security in accordance with the established policies and procedures of the organization." ;
    dcterms:identifier "7.2.1" ;
    dcterms:title "Management responsibilities" ;
    iso:controlSection <https://par-tec.github.io/security-ontologies/onto/iso#27001/2013/section-7.2> ;
    iso:correspondsTo <https://par-tec.github.io/security-ontologies/onto/iso#27002/2022/control-5.4> .

<https://par-tec.github.io/security-ontologies/onto/iso#27001/2013/control-7.2.2> a iso:Control ;
    dcterms:description "All employees of the organization and, where relevant, contractors shall receive appropriate awareness education and training and regular updates in organizational policies and procedures, as relevant for their job function." ;
    dcterms:identifier "7.2.2" ;
    dcterms:title "Information security awareness, education and training" ;
    iso:controlSection <https://par-tec.github.io/security-ontologies/onto/iso#27001/2013/section-7.2> ;
    iso:correspondsTo <https://par-tec.github.io/security-ontologies/onto/iso#27002/2022/control-6.3> .

<https://par-tec.github.io/security-ontologies/onto/iso#27001/2013/control-7.2.3> a iso:Control ;
    dcterms:description "There shall be a formal and communicated disciplinary process in place to take action against employees who have committed an information security breach." ;
    dcterms:identifier "7.2.3" ;
    dcterms:title "Disciplinary process" ;
    iso:controlSection <https://par-tec.github.io/security-ontologies/onto/iso#27001/2013/section-7.2> ;
    iso:correspondsTo <https://par-tec.github.io/security-ontologies/onto/iso#27002/2022/control-6.4> .

<https://par-tec.github.io/security-ontologies/onto/iso#27001/2013/control-7.3.1> a iso:Control ;
    dcterms:description "Information security responsibilities and duties that remain valid after termination or change of employment shall be defined, communicated to the employee or contractor and enforced." ;
    dcterms:identifier "7.3.1" ;
    dcterms:title "Termination or change of employment responsibilities" ;
    iso:controlSection <https://par-tec.github.io/security-ontologies/onto/iso#27001/2013/section-7.3> ;
    iso:correspondsTo <https://par-tec.github.io/security-ontologies/onto/iso#27002/2022/control-6.5> .

<https://par-tec.github.io/security-ontologies/onto/iso#27001/2013/control-8.1.1> a iso:Control ;
    dcterms:description "Assets associated with information and information processing facilities shall be identified and an inventory of these assets shall be drawn up and maintained." ;
    dcterms:identifier "8.1.1" ;
    dcterms:title "Inventory of assets" ;
    iso:controlSection <https://par-tec.github.io/security-ontologies/onto/iso#27001/2013/section-8.1> ;
    iso:correspondsTo <https://par-tec.github.io/security-ontologies/onto/iso#27002/2022/control-5.9> .

<https://par-tec.github.io/security-ontologies/onto/iso#27001/2013/control-8.1.2> a iso:Control ;
    dcterms:description "Assets maintained in the inventory shall be owned." ;
    dcterms:identifier "8.1.2" ;
    dcterms:title "Ownership of assets" ;
    iso:controlSection <https://par-tec.github.io/security-ontologies/onto/iso#27001/2013/section-8.1> ;
    iso:correspondsTo <https://par-tec.github.io/security-ontologies/onto/iso#27002/2022/control-5.9> .

<https://par-tec.github.io/security-ontologies/onto/iso#27001/2013/control-8.1.3> a iso:Control ;
    dcterms:description "Rules for the acceptable use of information and of assets associated with information and information processing facilities shall be identified, documented and implemented." ;
    dcterms:identifier "8.1.3" ;
    dcterms:title "Acceptable use of assets" ;
    iso:controlSection <https://par-tec.github.io/security-ontologies/onto/iso#27001/2013/section-8.1> ;
    iso:correspondsTo <https://par-tec.github.io/security-ontologies/onto/iso#27002/2022/control-5.10> .

<https://par-tec.github.io/security-ontologies/onto/iso#27001/2013/control-8.1.4> a iso:Control ;
    dcterms:description "All employees and external party users shall return all of the organizational assets in their possession upon termination of their employment, contract or agreement." ;
    dcterms:identifier "8.1.4" ;
    dcterms:title "Return of assets" ;
    iso:controlSection <https://par-tec.github.io/security-ontologies/onto/iso#27001/2013/section-8.1> ;
    iso:correspondsTo <https://par-tec.github.io/security-ontologies/onto/iso#27002/2022/control-5.11> .

<https://par-tec.github.io/security-ontologies/onto/iso#27001/2013/control-8.2.1> a iso:Control ;
    dcterms:description "Information shall be classified in terms of legal requirements, value, criticality and sensitivity to unauthorized disclosure or modification." ;
    dcterms:identifier "8.2.1" ;
    dcterms:title "Classification of information" ;
    iso:controlSection <https://par-tec.github.io/security-ontologies/onto/iso#27001/2013/section-8.2> ;
    iso:correspondsTo <https://par-tec.github.io/security-ontologies/onto/iso#27002/2022/control-5.12> .

<https://par-tec.github.io/security-ontologies/onto/iso#27001/2013/control-8.2.2> a iso:Control ;
    dcterms:description "An appropriate set of procedures for information labeling shall be developed and implemented in accordance with the information classification scheme adopted by the organization." ;
    dcterms:identifier "8.2.2" ;
    dcterms:title "Labeling of information" ;
    iso:controlSection <https://par-tec.github.io/security-ontologies/onto/iso#27001/2013/section-8.2> ;
    iso:correspondsTo <https://par-tec.github.io/security-ontologies/onto/iso#27002/2022/control-5.13> .

<https://par-tec.github.io/security-ontologies/onto/iso#27001/2013/control-8.2.3> a iso:Control ;
    dcterms:description "Procedures for handling assets shall be developed and implemented in accordance with the information classification scheme adopted by the organization." ;
    dcterms:identifier "8.2.3" ;
    dcterms:title "Handling of assets" ;
    iso:controlSection <https://par-tec.github.io/security-ontologies/onto/iso#27001/2013/section-8.2> ;
    iso:correspondsTo <https://par-tec.github.io/security-ontologies/onto/iso#27002/2022/control-5.10> .

<https://par-tec.github.io/security-ontologies/onto/iso#27001/2013/control-8.3.1> a iso:Control ;
    dcterms:description "Procedures shall be implemented for the management of removable media in accordance with the classification scheme adopted by the organization." ;
    dcterms:identifier "8.3.1" ;
    dcterms:title "Management of removable media" ;
    iso:controlSection <https://par-tec.github.io/security-ontologies/onto/iso#27001/2013/section-8.3> ;
    iso:correspondsTo <https://par-tec.github.io/security-ontologies/onto/iso#27002/2022/control-7.10> .

<https://par-tec.github.io/security-ontologies/onto/iso#27001/2013/control-8.3.2> a iso:Control ;
    dcterms:description "Media shall be disposed of securely when no longer required, using formal procedures." ;
    dcterms:identifier "8.3.2" ;
    dcterms:title "Disposal of media" ;
    iso:controlSection <https://par-tec.github.io/security-ontologies/onto/iso#27001/2013/section-8.3> ;
    iso:correspondsTo <https://par-tec.github.io/security-ontologies/onto/iso#27002/2022/control-7.10> .

<https://par-tec.github.io/security-ontologies/onto/iso#27001/2013/control-8.3.3> a iso:Control ;
    dcterms:description "Media containing information shall be protected against unauthorized access, misuse or corruption during transportation." ;
    dcterms:identifier "8.3.3" ;
    dcterms:title "Physical media transfer" ;
    iso:controlSection <https://par-tec.github.io/security-ontologies/onto/iso#27001/2013/section-8.3> ;
    iso:correspondsTo <https://par-tec.github.io/security-ontologies/onto/iso#27002/2022/control-7.10> .

<https://par-tec.github.io/security-ontologies/onto/iso#27001/2013/control-9.1.1> a iso:Control ;
    dcterms:description "An access control policy shall be established, documented and reviewed based on business and information security requirements." ;
    dcterms:identifier "9.1.1" ;
    dcterms:title "Access control policy" ;
    iso:controlSection <https://par-tec.github.io/security-ontologies/onto/iso#27001/2013/section-9.1> ;
    iso:correspondsTo <https://par-tec.github.io/security-ontologies/onto/iso#27002/2022/control-5.15> .

<https://par-tec.github.io/security-ontologies/onto/iso#27001/2013/control-9.1.2> a iso:Control ;
    dcterms:description "Users shall only be provided with access to the network and network services that they have been specifically authorized to use." ;
    dcterms:identifier "9.1.2" ;
    dcterms:title "Access to networks and network services" ;
    iso:controlSection <https://par-tec.github.io/security-ontologies/onto/iso#27001/2013/section-9.1> ;
    iso:correspondsTo <https://par-tec.github.io/security-ontologies/onto/iso#27002/2022/control-5.15> .

<https://par-tec.github.io/security-ontologies/onto/iso#27001/2013/control-9.2.1> a iso:Control ;
    dcterms:description "A formal user registration and de-registration process shall be implemented to enable assignment of access rights." ;
    dcterms:identifier "9.2.1" ;
    dcterms:title "User registration and de-registration" ;
    iso:controlSection <https://par-tec.github.io/security-ontologies/onto/iso#27001/2013/section-9.2> ;
    iso:correspondsTo <https://par-tec.github.io/security-ontologies/onto/iso#27002/2022/control-5.16> .

<https://par-tec.github.io/security-ontologies/onto/iso#27001/2013/control-9.2.2> a iso:Control ;
    dcterms:description "A formal user access provisioning process shall be implemented to assign or revoke access rights for all user types to all systems and services." ;
    dcterms:identifier "9.2.2" ;
    dcterms:title "User access provisioning" ;
    iso:controlSection <https://par-tec.github.io/security-ontologies/onto/iso#27001/2013/section-9.2> ;
    iso:correspondsTo <https://par-tec.github.io/security-ontologies/onto/iso#27002/2022/control-5.18> .

<https://par-tec.github.io/security-ontologies/onto/iso#27001/2013/control-9.2.3> a iso:Control ;
    dcterms:description "The allocation and use of privileged access rights shall be restricted and controlled." ;
    dcterms:identifier "9.2.3" ;
    dcterms:title "Management of privileged access rights" ;
    iso:controlSection <https://par-tec.github.io/security-ontologies/onto/iso#27001/2013/section-9.2> ;
    iso:correspondsTo <https://par-tec.github.io/security-ontologies/onto/iso#27002/2022/control-8.2> .

<https://par-tec.github.io/security-ontologies/onto/iso#27001/2013/control-9.2.4> a iso:Control ;
    dcterms:description "The allocation of secret authentication information shall be controlled through a formal management process." ;
    dcterms:identifier "9.2.4" ;
    dcterms:title "Management of secret authentication information of users" ;
    iso:controlSection <https://par-tec.github.io/security-ontologies/onto/iso#27001/2013/section-9.2> ;
    iso:correspondsTo <https://par-tec.github.io/security-ontologies/onto/iso#27002/2022/control-5.17> .

<https://par-tec.github.io/security-ontologies/onto/iso#27001/2013/control-9.2.5> a iso:Control ;
    dcterms:description "Asset owners shall review users’ access rights at regular intervals." ;
    dcterms:identifier "9.2.5" ;
    dcterms:title "Review of user access rights" ;
    iso:controlSection <https://par-tec.github.io/security-ontologies/onto/iso#27001/2013/section-9.2> ;
    iso:correspondsTo <https://par-tec.github.io/security-ontologies/onto/iso#27002/2022/control-5.18> .

<https://par-tec.github.io/security-ontologies/onto/iso#27001/2013/control-9.2.6> a iso:Control ;
    dcterms:description "The access rights of all employees and external party users to information and information processing facilities shall be removed upon termination of their employment, contract or agreement, or adjusted upon change." ;
    dcterms:identifier "9.2.6" ;
    dcterms:title "Removal or adjustment of access rights" ;
    iso:controlSection <https://par-tec.github.io/security-ontologies/onto/iso#27001/2013/section-9.2> ;
    iso:correspondsTo <https://par-tec.github.io/security-ontologies/onto/iso#27002/2022/control-5.18> .

<https://par-tec.github.io/security-ontologies/onto/iso#27001/2013/control-9.3.1> a iso:Control ;
    dcterms:description "Users shall be required to follow the organization’s practices in the use of secret authentication information." ;
    dcterms:identifier "9.3.1" ;
    dcterms:title "Use of secret authentication information" ;
    iso:controlSection <https://par-tec.github.io/security-ontologies/onto/iso#27001/2013/section-9.3> ;
    iso:correspondsTo <https://par-tec.github.io/security-ontologies/onto/iso#27002/2022/control-5.17> .

<https://par-tec.github.io/security-ontologies/onto/iso#27001/2013/control-9.4.1> a iso:Control ;
    dcterms:description "Access to information and application system functions shall be restricted in accordance with the access control policy." ;
    dcterms:identifier "9.4.1" ;
    dcterms:title "Information access restriction" ;
    iso:controlSection <https://par-tec.github.io/security-ontologies/onto/iso#27001/2013/section-9.4> ;
    iso:correspondsTo <https://par-tec.github.io/security-ontologies/onto/iso#27002/2022/control-8.3> .

<https://par-tec.github.io/security-ontologies/onto/iso#27001/2013/control-9.4.2> a iso:Control ;
    dcterms:description "Where required by the access control policy, access to systems and applications shall be controlled by a secure log-on procedure." ;
    dcterms:identifier "9.4.2" ;
    dcterms:title "Secure log-on procedures" ;
    iso:controlSection <https://par-tec.github.io/security-ontologies/onto/iso#27001/2013/section-9.4> ;
    iso:correspondsTo <https://par-tec.github.io/security-ontologies/onto/iso#27002/2022/control-8.5> .

<https://par-tec.github.io/security-ontologies/onto/iso#27001/2013/control-9.4.3> a iso:Control ;
    dcterms:description "Password management systems shall be interactive and shall ensure quality passwords." ;
    dcterms:identifier "9.4.3" ;
    dcterms:title "Password management system" ;
    iso:controlSection <https://par-tec.github.io/security-ontologies/onto/iso#27001/2013/section-9.4> ;
    iso:correspondsTo <https://par-tec.github.io/security-ontologies/onto/iso#27002/2022/control-5.17> .

<https://par-tec.github.io/security-ontologies/onto/iso#27001/2013/control-9.4.4> a iso:Control ;
    dcterms:description "The use of utility programs that might be capable of overriding system and application controls shall be restricted and tightly controlled." ;
    dcterms:identifier "9.4.4" ;
    dcterms:title "Use of privileged utility programs" ;
    iso:controlSection <https://par-tec.github.io/security-ontologies/onto/iso#27001/2013/section-9.4> ;
    iso:correspondsTo <https://par-tec.github.io/security-ontologies/onto/iso#27002/2022/control-8.18> .

<https://par-tec.github.io/security-ontologies/onto/iso#27001/2013/control-9.4.5> a iso:Control ;
    dcterms:description "Access to program source code shall be restricted." ;
    dcterms:identifier "9.4.5" ;
    dcterms:title "Access control to program source code" ;
    iso:controlSection <https://par-tec.github.io/security-ontologies/onto/iso#27001/2013/section-9.4> ;
    iso:correspondsTo <https://par-tec.github.io/security-ontologies/onto/iso#27002/2022/control-8.4> .

<https://par-tec.github.io/security-ontologies/onto/iso#27001/2013/section-12.2> a iso:Section ;
    rdfs:label "Protection from malware" ;
    iso:controlCategory <https://par-tec.github.io/security-ontologies/onto/iso#27001/2013/category-12> .

<https://par-tec.github.io/security-ontologies/onto/iso#27001/2013/section-12.3> a iso:Section ;
    rdfs:label "Backup" ;
    iso:controlCategory <https://par-tec.github.io/security-ontologies/onto/iso#27001/2013/category-12> .

<https://par-tec.github.io/security-ontologies/onto/iso#27001/2013/section-12.5> a iso:Section ;
    rdfs:label "Control of operational software" ;
    iso:controlCategory <https://par-tec.github.io/security-ontologies/onto/iso#27001/2013/category-12> .

<https://par-tec.github.io/security-ontologies/onto/iso#27001/2013/section-12.7> a iso:Section ;
    rdfs:label "Information systems audit considerations" ;
    iso:controlCategory <https://par-tec.github.io/security-ontologies/onto/iso#27001/2013/category-12> .

<https://par-tec.github.io/security-ontologies/onto/iso#27001/2013/section-14.3> a iso:Section ;
    rdfs:label "Test data" ;
    iso:controlCategory <https://par-tec.github.io/security-ontologies/onto/iso#27001/2013/category-14> .

<https://par-tec.github.io/security-ontologies/onto/iso#27001/2013/section-17.2> a iso:Section ;
    rdfs:label "Redundancies" ;
    iso:controlCategory <https://par-tec.github.io/security-ontologies/onto/iso#27001/2013/category-17> .

<https://par-tec.github.io/security-ontologies/onto/iso#27001/2013/section-7.3> a iso:Section ;
    rdfs:label "Termination and change of employment" ;
    iso:controlCategory <https://par-tec.github.io/security-ontologies/onto/iso#27001/2013/category-7> .

<https://par-tec.github.io/security-ontologies/onto/iso#27001/2013/section-9.3> a iso:Section ;
    rdfs:label "User responsibilities" ;
    iso:controlCategory <https://par-tec.github.io/security-ontologies/onto/iso#27001/2013/category-9> .

<https://par-tec.github.io/security-ontologies/onto/iso#27002/2022/control-5.11> a iso:Control ;
    dcterms:description "Personnel and other interested parties as appropriate should return all the organization's assets in their possession upon change or termination of their employment, contract or agreement" ;
    dcterms:identifier "27002/2022/control-5.11" ;
    dcterms:title " Return of assets" ;
    iso:controlCategory iso:category-5 ;
    iso:correspondsTo <https://par-tec.github.io/security-ontologies/onto/iso#27001/2013/control-8.1.4> ;
    iso:hasControlType iso:Preventive ;
    iso:hasCybersecurityConcept iso:Protect ;
    iso:hasInformationSecurityProperty iso:Availability,
        iso:Confidentiality,
        iso:Integrity ;
    iso:hasOperationalCapability iso:AssetManagement ;
    iso:hasRelatedControls <https://par-tec.github.io/security-ontologies/onto/iso#27002/2022/control-7.14>,
        <https://par-tec.github.io/security-ontologies/onto/iso#27002/2022/control-8.4> ;
    iso:hasSecurityDomain iso:Protection ;
    iso:purpose "To protect the organization’s assets as part of the process of changing or terminating employment or contract" .

<https://par-tec.github.io/security-ontologies/onto/iso#27002/2022/control-5.19> a iso:Control ;
    dcterms:description "Processes and procedures should be identified and implemented to manage the information security risks associated with the use of supplier's products or services" ;
    dcterms:identifier "27002/2022/control-5.19" ;
    dcterms:title "Information security in supplier relationships" ;
    iso:controlCategory iso:category-5 ;
    iso:correspondsTo <https://par-tec.github.io/security-ontologies/onto/iso#27001/2013/control-15.1.1> ;
    iso:hasControlType iso:Preventive ;
    iso:hasCybersecurityConcept iso:Identify ;
    iso:hasInformationSecurityProperty iso:Availability,
        iso:Confidentiality,
        iso:Integrity ;
    iso:hasOperationalCapability iso:SupplierSecurity ;
    iso:hasSecurityDomain iso:GovernanceEcosystem,
        iso:Protection ;
    iso:purpose "To maintain an agreed level of information security in supplier relationships" .

<https://par-tec.github.io/security-ontologies/onto/iso#27002/2022/control-5.4> a iso:Control ;
    dcterms:description """Management should be a role model for information security and require all personnel to apply
information security in accordance with the established information security policy, topic-specific
policies and procedures of the organization""" ;
    dcterms:identifier "27002/2022/control-5.4" ;
    dcterms:title "Management responsibilities" ;
    iso:controlCategory iso:category-5 ;
    iso:correspondsTo <https://par-tec.github.io/security-ontologies/onto/iso#27001/2013/control-7.2.1> ;
    iso:hasControlType iso:Preventive ;
    iso:hasCybersecurityConcept iso:Identify ;
    iso:hasInformationSecurityProperty iso:Availability,
        iso:Confidentiality,
        iso:Integrity ;
    iso:hasOperationalCapability iso:Governance ;
    iso:hasRelatedControls <https://par-tec.github.io/security-ontologies/onto/iso#27002/2022/control-6.3> ;
    iso:hasSecurityDomain iso:GovernanceEcosystem ;
    iso:purpose """To ensure management understand their role in information security and undertake actions aiming to
ensure all personnel are aware of and fulfil their information security responsibilities""" .

<https://par-tec.github.io/security-ontologies/onto/iso#27002/2022/control-7.1> a iso:Control ;
    dcterms:description "Security perimeters should be defined and used to protect areas that contain either sensitive or critical information and other associated assets" ;
    dcterms:identifier "27002/2022/control-7.1" ;
    dcterms:title " Physical security perimeter" ;
    iso:controlCategory iso:category-7 ;
    iso:correspondsTo <https://par-tec.github.io/security-ontologies/onto/iso#27001/2013/control-11.1.1> ;
    iso:hasControlType iso:Preventive ;
    iso:hasCybersecurityConcept iso:Protect ;
    iso:hasInformationSecurityProperty iso:Availability,
        iso:Confidentiality,
        iso:Integrity ;
    iso:hasOperationalCapability iso:PhysicalSecurity ;
    iso:hasSecurityDomain iso:Protection ;
    iso:purpose "To prevent unauthorized physical access, damage and interference to the organization’s information and other associated assets" .

<https://par-tec.github.io/security-ontologies/onto/iso#27002/2022/control-7.11> a iso:Control ;
    dcterms:description "Information processing facilities should be protected from power failures and other disruptions caused by failures in supporting utilities" ;
    dcterms:identifier "27002/2022/control-7.11" ;
    dcterms:title "Supporting utilities" ;
    iso:controlCategory iso:category-7 ;
    iso:correspondsTo <https://par-tec.github.io/security-ontologies/onto/iso#27001/2013/control-11.2.2> ;
    iso:hasControlType iso:Detective,
        iso:Preventive ;
    iso:hasCybersecurityConcept iso:Detect,
        iso:Protect ;
    iso:hasInformationSecurityProperty iso:Availability ;
    iso:hasOperationalCapability iso:PhysicalSecurity ;
    iso:hasSecurityDomain iso:Protection ;
    iso:purpose "To prevent loss, damage or compromise of information and other associated assets due to the failure and disruption of supporting utilities or interruption to the organization’s operations" .

<https://par-tec.github.io/security-ontologies/onto/iso#27002/2022/control-7.12> a iso:Control ;
    dcterms:description "Cables carrying power, data or supporting information services should be protected from interception, interference or damage" ;
    dcterms:identifier "27002/2022/control-7.12" ;
    dcterms:title " Cabling security" ;
    iso:controlCategory iso:category-7 ;
    iso:correspondsTo <https://par-tec.github.io/security-ontologies/onto/iso#27001/2013/control-11.2.3> ;
    iso:hasControlType iso:Preventive ;
    iso:hasCybersecurityConcept iso:Protect ;
    iso:hasInformationSecurityProperty iso:Availability,
        iso:Confidentiality ;
    iso:hasOperationalCapability iso:PhysicalSecurity ;
    iso:hasSecurityDomain iso:Protection ;
    iso:purpose "To  prevent  loss,  damage,  theft  or  compromise  of  information  and  other  associated  assets  and interruption to the organization’s operations due to failure in power and communications cabling" .

<https://par-tec.github.io/security-ontologies/onto/iso#27002/2022/control-7.13> a iso:Control ;
    dcterms:description "Equipment should be maintained correctly" ;
    dcterms:identifier "27002/2022/control-7.13" ;
    dcterms:title " Equipment maintenance" ;
    iso:controlCategory iso:category-7 ;
    iso:correspondsTo <https://par-tec.github.io/security-ontologies/onto/iso#27001/2013/control-11.2.4> ;
    iso:hasControlType iso:Preventive ;
    iso:hasCybersecurityConcept iso:Protect ;
    iso:hasInformationSecurityProperty iso:Availability,
        iso:Confidentiality,
        iso:Integrity ;
    iso:hasOperationalCapability iso:AssetManagement,
        iso:PhysicalSecurity ;
    iso:hasRelatedControls <https://par-tec.github.io/security-ontologies/onto/iso#27002/2022/control-7.14>,
        <https://par-tec.github.io/security-ontologies/onto/iso#27002/2022/control-7.9> ;
    iso:hasSecurityDomain iso:Protection,
        iso:Resilience ;
    iso:purpose "To  prevent  loss,  damage,  theft  or  compromise  of  information  and  other  associated  assets  and interruption to the organization’s operations" .

<https://par-tec.github.io/security-ontologies/onto/iso#27002/2022/control-7.6> a iso:Control ;
    dcterms:description "Procedures for working in secure areas should be designed and implemented" ;
    dcterms:identifier "27002/2022/control-7.6" ;
    dcterms:title " Working in secure areas" ;
    iso:controlCategory iso:category-7 ;
    iso:correspondsTo <https://par-tec.github.io/security-ontologies/onto/iso#27001/2013/control-11.1.5> ;
    iso:hasControlType iso:Preventive ;
    iso:hasCybersecurityConcept iso:Protect ;
    iso:hasInformationSecurityProperty iso:Availability,
        iso:Confidentiality,
        iso:Integrity ;
    iso:hasOperationalCapability iso:PhysicalSecurity ;
    iso:hasSecurityDomain iso:Protection ;
    iso:purpose "To prevent damage and interference to the organization’s information and other associated assets in secure areas" .

<https://par-tec.github.io/security-ontologies/onto/iso#27002/2022/control-7.7> a iso:Control ;
    dcterms:description "Clear  desk  rules  for  papers  and  removable  storage  media  and  clear  screen  rules  for  information processing facilities should be defined and enforced" ;
    dcterms:identifier "27002/2022/control-7.7" ;
    dcterms:title "Clear desk and clear screen" ;
    iso:controlCategory iso:category-7 ;
    iso:correspondsTo <https://par-tec.github.io/security-ontologies/onto/iso#27001/2013/control-11.2.9> ;
    iso:hasControlType iso:Preventive ;
    iso:hasCybersecurityConcept iso:Protect ;
    iso:hasInformationSecurityProperty iso:Confidentiality ;
    iso:hasOperationalCapability iso:PhysicalSecurity ;
    iso:hasSecurityDomain iso:Protection ;
    iso:purpose "To reduce the risks of unauthorized access, loss of and damage to information on the desks, screens and in other accessible locations during and outside normal working hours" .

<https://par-tec.github.io/security-ontologies/onto/iso#27002/2022/control-8.12> a iso:Control ;
    dcterms:description "Data leakage prevention measures should be applied to systems, networks and endpoint devices that process, store or transmit sensitive information" ;
    dcterms:identifier "27002/2022/control-8.12" ;
    dcterms:title "Data leakage prevention" ;
    iso:controlCategory iso:category-8 ;
    iso:correspondsTo <https://par-tec.github.io/security-ontologies/onto/iso#27001/2013/control-New> ;
    iso:hasControlType iso:Detective,
        iso:Preventive ;
    iso:hasCybersecurityConcept iso:Detect,
        iso:Protect ;
    iso:hasInformationSecurityProperty iso:Confidentiality ;
    iso:hasOperationalCapability iso:InformationProtection ;
    iso:hasRelatedControls <https://par-tec.github.io/security-ontologies/onto/iso#27002/2022/control-5.12>,
        <https://par-tec.github.io/security-ontologies/onto/iso#27002/2022/control-5.15> ;
    iso:hasSecurityDomain iso:Defence,
        iso:Protection ;
    iso:purpose "To detect and prevent the unauthorized disclosure and extraction of information by individuals or systems" .

<https://par-tec.github.io/security-ontologies/onto/iso#27002/2022/control-8.21> a iso:Control ;
    dcterms:description "Security mechanisms, service levels, and service requirements of network services should be identified, implemented and monitored" ;
    dcterms:identifier "27002/2022/control-8.21" ;
    dcterms:title "Security of network services" ;
    iso:controlCategory iso:category-8 ;
    iso:correspondsTo <https://par-tec.github.io/security-ontologies/onto/iso#27001/2013/control-13.1.2> ;
    iso:hasControlType iso:Preventive ;
    iso:hasCybersecurityConcept iso:Protect ;
    iso:hasInformationSecurityProperty iso:Availability,
        iso:Confidentiality,
        iso:Integrity ;
    iso:hasOperationalCapability iso:SystemNetworkSecurity ;
    iso:hasSecurityDomain iso:Protection ;
    iso:purpose "To ensure security in the use of network services" .

<https://par-tec.github.io/security-ontologies/onto/iso#27002/2022/control-8.34> a iso:Control ;
    dcterms:description "Audit  tests  and  other  assurance  activities  involving  assessment  of  operational  systems  should  be planned and agreed between the tester and appropriate management" ;
    dcterms:identifier "27002/2022/control-8.34" ;
    dcterms:title "Protection of information systems during audit and testing" ;
    iso:controlCategory iso:category-8 ;
    iso:correspondsTo <https://par-tec.github.io/security-ontologies/onto/iso#27001/2013/control-12.7.1> ;
    iso:hasControlType iso:Preventive ;
    iso:hasCybersecurityConcept iso:Protect ;
    iso:hasInformationSecurityProperty iso:Availability,
        iso:Integrity ;
    iso:hasOperationalCapability iso:InformationProtection,
        iso:SystemNetworkSecurity ;
    iso:hasSecurityDomain iso:GovernanceEcosystem,
        iso:Protection ;
    iso:purpose "To minimize the impact of audit and other assurance activities on operational systems and business processes" .

<https://par-tec.github.io/security-ontologies/onto/iso#27002/2022/control-8.6> a iso:Control ;
    dcterms:description "The use of resources should be monitored and adjusted in line with current and expected capacity requirements" ;
    dcterms:identifier "27002/2022/control-8.6" ;
    dcterms:title " Capacity management" ;
    iso:controlCategory iso:category-8 ;
    iso:correspondsTo <https://par-tec.github.io/security-ontologies/onto/iso#27001/2013/control-12.1.3> ;
    iso:hasControlType iso:Detective,
        iso:Preventive ;
    iso:hasCybersecurityConcept iso:Detect,
        iso:Identify,
        iso:Protect ;
    iso:hasInformationSecurityProperty iso:Availability ;
    iso:hasOperationalCapability iso:Continuity ;
    iso:hasSecurityDomain iso:GovernanceEcosystem,
        iso:Protection ;
    iso:purpose "To ensure the required capacity of information processing facilities" .

<https://par-tec.github.io/security-ontologies/onto/iso#27001/2013/category-11> a iso:ControlCategory ;
    rdfs:label "Physical and environmental security" .

<https://par-tec.github.io/security-ontologies/onto/iso#27001/2013/category-13> a iso:ControlCategory ;
    rdfs:label "Communications security" .

<https://par-tec.github.io/security-ontologies/onto/iso#27001/2013/category-15> a iso:ControlCategory ;
    rdfs:label "Supplier relationships" .

<https://par-tec.github.io/security-ontologies/onto/iso#27001/2013/category-17> a iso:ControlCategory ;
    rdfs:label "Information security aspects of business continuity management" .

<https://par-tec.github.io/security-ontologies/onto/iso#27001/2013/category-18> a iso:ControlCategory ;
    rdfs:label "Compliance" .

<https://par-tec.github.io/security-ontologies/onto/iso#27001/2013/category-6> a iso:ControlCategory ;
    rdfs:label "Organization of information security" .

<https://par-tec.github.io/security-ontologies/onto/iso#27001/2013/control-18.2.3> a iso:Control ;
    dcterms:description "Information systems shall be regularly reviewed for compliance with the organization’s information security policies and standards." ;
    dcterms:identifier "18.2.3" ;
    dcterms:title "Technical compliance review" ;
    iso:controlSection <https://par-tec.github.io/security-ontologies/onto/iso#27001/2013/section-18.2> ;
    iso:correspondsTo <https://par-tec.github.io/security-ontologies/onto/iso#27002/2022/control-5.36>,
        <https://par-tec.github.io/security-ontologies/onto/iso#27002/2022/control-8.8> .

<https://par-tec.github.io/security-ontologies/onto/iso#27001/2013/section-10.1> a iso:Section ;
    rdfs:label "Cryptographic controls" ;
    iso:controlCategory <https://par-tec.github.io/security-ontologies/onto/iso#27001/2013/category-10> .

<https://par-tec.github.io/security-ontologies/onto/iso#27001/2013/section-12.6> a iso:Section ;
    rdfs:label "Technical vulnerability management" ;
    iso:controlCategory <https://par-tec.github.io/security-ontologies/onto/iso#27001/2013/category-12> .

<https://par-tec.github.io/security-ontologies/onto/iso#27001/2013/section-15.2> a iso:Section ;
    rdfs:label "Supplier service delivery management" ;
    iso:controlCategory <https://par-tec.github.io/security-ontologies/onto/iso#27001/2013/category-15> .

<https://par-tec.github.io/security-ontologies/onto/iso#27001/2013/section-5.1> a iso:Section ;
    rdfs:label "Management direction for information security" ;
    iso:controlCategory <https://par-tec.github.io/security-ontologies/onto/iso#27001/2013/category-5> .

<https://par-tec.github.io/security-ontologies/onto/iso#27001/2013/section-6.2> a iso:Section ;
    rdfs:label "Mobile devices and teleworking" ;
    iso:controlCategory <https://par-tec.github.io/security-ontologies/onto/iso#27001/2013/category-6> .

<https://par-tec.github.io/security-ontologies/onto/iso#27001/2013/section-7.1> a iso:Section ;
    rdfs:label "Prior to employment" ;
    iso:controlCategory <https://par-tec.github.io/security-ontologies/onto/iso#27001/2013/category-7> .

<https://par-tec.github.io/security-ontologies/onto/iso#27001/2013/section-9.1> a iso:Section ;
    rdfs:label "Business requirements of access control" ;
    iso:controlCategory <https://par-tec.github.io/security-ontologies/onto/iso#27001/2013/category-9> .

<https://par-tec.github.io/security-ontologies/onto/iso#27002/2022/control-5.2> a iso:Control ;
    dcterms:description """Information security roles and responsibilities should be defined and allocated according to the
organization needs""" ;
    dcterms:identifier "27002/2022/control-5.2" ;
    dcterms:title "Information security roles and responsibilities" ;
    iso:controlCategory iso:category-5 ;
    iso:correspondsTo <https://par-tec.github.io/security-ontologies/onto/iso#27001/2013/control-6.1.1> ;
    iso:hasControlType iso:Preventive ;
    iso:hasCybersecurityConcept iso:Identify ;
    iso:hasInformationSecurityProperty iso:Availability,
        iso:Confidentiality,
        iso:Integrity ;
    iso:hasOperationalCapability iso:Governance ;
    iso:hasRelatedControls <https://par-tec.github.io/security-ontologies/onto/iso#27002/2022/control-5.1> ;
    iso:hasSecurityDomain iso:GovernanceEcosystem,
        iso:Protection,
        iso:Resilience ;
    iso:purpose """To establish a defined, approved and understood structure for the implementation, operation and
management of information security within the organization""" .

<https://par-tec.github.io/security-ontologies/onto/iso#27002/2022/control-5.21> a iso:Control ;
    dcterms:description "Processes and procedures should be defined and implemented to address information security risks associated with ICT services and product supply chain" ;
    dcterms:identifier "27002/2022/control-5.21" ;
    dcterms:title "Managing information security in the ICT supply chain" ;
    iso:controlCategory iso:category-5 ;
    iso:correspondsTo <https://par-tec.github.io/security-ontologies/onto/iso#27001/2013/control-15.1.3> ;
    iso:hasControlType iso:Preventive ;
    iso:hasCybersecurityConcept iso:Detect,
        iso:Protect ;
    iso:hasInformationSecurityProperty iso:Availability,
        iso:Confidentiality,
        iso:Integrity ;
    iso:hasOperationalCapability iso:SupplierSecurity ;
    iso:hasSecurityDomain iso:GovernanceEcosystem,
        iso:Protection ;
    iso:purpose "To ensure information security of the organization in ICT supply chain" .

<https://par-tec.github.io/security-ontologies/onto/iso#27002/2022/control-5.23> a iso:Control ;
    dcterms:description "Processes for acquisition, use, management and exit from cloud services should be established in accordance with the organization’s information security requirements" ;
    dcterms:identifier "27002/2022/control-5.23" ;
    dcterms:title "Information security for use of cloud services" ;
    iso:controlCategory iso:category-5 ;
    iso:correspondsTo <https://par-tec.github.io/security-ontologies/onto/iso#27001/2013/control-New> ;
    iso:hasControlType iso:Preventive ;
    iso:hasCybersecurityConcept iso:Protect ;
    iso:hasInformationSecurityProperty iso:Availability,
        iso:Confidentiality,
        iso:Integrity ;
    iso:hasOperationalCapability iso:SupplierSecurity ;
    iso:hasRelatedControls <https://par-tec.github.io/security-ontologies/onto/iso#27002/2022/control-5.21>,
        <https://par-tec.github.io/security-ontologies/onto/iso#27002/2022/control-5.22> ;
    iso:hasSecurityDomain iso:GovernanceEcosystem,
        iso:Protection ;
    iso:purpose "To specify and manage information security for the use of cloud services" .

<https://par-tec.github.io/security-ontologies/onto/iso#27002/2022/control-5.37> a iso:Control ;
    dcterms:description "Operating procedures for information processing facilities should be documented and made available to personnel who need them" ;
    dcterms:identifier "27002/2022/control-5.37" ;
    dcterms:title " Documented operating procedures" ;
    iso:controlCategory iso:category-5 ;
    iso:correspondsTo <https://par-tec.github.io/security-ontologies/onto/iso#27001/2013/control-12.1.1> ;
    iso:hasControlType iso:Preventive ;
    iso:hasCybersecurityConcept iso:Protect ;
    iso:hasInformationSecurityProperty iso:Availability,
        iso:Confidentiality,
        iso:Integrity ;
    iso:hasOperationalCapability iso:AssetManagement,
        iso:Continuity,
        iso:PhysicalSecurity,
        iso:SystemNetworkSecurity ;
    iso:hasRelatedControls <https://par-tec.github.io/security-ontologies/onto/iso#27002/2022/control-7.10>,
        <https://par-tec.github.io/security-ontologies/onto/iso#27002/2022/control-7.14>,
        <https://par-tec.github.io/security-ontologies/onto/iso#27002/2022/control-7.4>,
        <https://par-tec.github.io/security-ontologies/onto/iso#27002/2022/control-8.13>,
        <https://par-tec.github.io/security-ontologies/onto/iso#27002/2022/control-8.15>,
        <https://par-tec.github.io/security-ontologies/onto/iso#27002/2022/control-8.17>,
        <https://par-tec.github.io/security-ontologies/onto/iso#27002/2022/control-8.18> ;
    iso:hasSecurityDomain iso:Defence,
        iso:GovernanceEcosystem,
        iso:Protection ;
    iso:purpose "To ensure the correct and secure operation of information processing facilities" .

<https://par-tec.github.io/security-ontologies/onto/iso#27002/2022/control-5.5> a iso:Control ;
    dcterms:description "The organization should establish and maintain contact with relevant authorities" ;
    dcterms:identifier "27002/2022/control-5.5" ;
    dcterms:title " Contact with authorities" ;
    iso:controlCategory iso:category-5 ;
    iso:correspondsTo <https://par-tec.github.io/security-ontologies/onto/iso#27001/2013/control-6.1.3> ;
    iso:hasControlType iso:Corrective,
        iso:Preventive ;
    iso:hasCybersecurityConcept iso:Protect,
        iso:Recover,
        iso:Respond ;
    iso:hasInformationSecurityProperty iso:Availability,
        iso:Confidentiality,
        iso:Integrity ;
    iso:hasOperationalCapability iso:Governance ;
    iso:hasRelatedControls <https://par-tec.github.io/security-ontologies/onto/iso#27002/2022/control-5.24>,
        <https://par-tec.github.io/security-ontologies/onto/iso#27002/2022/control-5.25>,
        <https://par-tec.github.io/security-ontologies/onto/iso#27002/2022/control-5.26>,
        <https://par-tec.github.io/security-ontologies/onto/iso#27002/2022/control-5.27>,
        <https://par-tec.github.io/security-ontologies/onto/iso#27002/2022/control-5.28>,
        <https://par-tec.github.io/security-ontologies/onto/iso#27002/2022/control-5.29>,
        <https://par-tec.github.io/security-ontologies/onto/iso#27002/2022/control-5.30> ;
    iso:hasSecurityDomain iso:Defence,
        iso:Resilience ;
    iso:purpose """To ensure appropriate flow of information takes place with respect to information security between
the organization and relevant legal, regulatory and supervisory authorities""" .

<https://par-tec.github.io/security-ontologies/onto/iso#27002/2022/control-5.6> a iso:Control ;
    dcterms:description """The organization should establish and maintain contact with special interest groups or other specialist
security forums and professional associations""" ;
    dcterms:identifier "27002/2022/control-5.6" ;
    dcterms:title "Contact with special interest groups" ;
    iso:controlCategory iso:category-5 ;
    iso:correspondsTo <https://par-tec.github.io/security-ontologies/onto/iso#27001/2013/control-6.1.4> ;
    iso:hasControlType iso:Corrective,
        iso:Preventive ;
    iso:hasCybersecurityConcept iso:Protect,
        iso:Recover,
        iso:Respond ;
    iso:hasInformationSecurityProperty iso:Availability,
        iso:Confidentiality,
        iso:Integrity ;
    iso:hasOperationalCapability iso:Governance ;
    iso:hasRelatedControls <https://par-tec.github.io/security-ontologies/onto/iso#27002/2022/control-5.24>,
        <https://par-tec.github.io/security-ontologies/onto/iso#27002/2022/control-5.25>,
        <https://par-tec.github.io/security-ontologies/onto/iso#27002/2022/control-5.26>,
        <https://par-tec.github.io/security-ontologies/onto/iso#27002/2022/control-5.27>,
        <https://par-tec.github.io/security-ontologies/onto/iso#27002/2022/control-5.28> ;
    iso:hasSecurityDomain iso:Defence ;
    iso:purpose "To ensure appropriate flow of information takes place with respect to information security" .

<https://par-tec.github.io/security-ontologies/onto/iso#27002/2022/control-6.1> a iso:Control ;
    dcterms:description "Background verification checks on all candidates to become personnel should be carried out prior to joining the organization and on an ongoing basis in accordance with applicable laws, regulations and ethics, and be proportional to the business requirements, the classification of the information to be accessed and the perceived risks" ;
    dcterms:identifier "27002/2022/control-6.1" ;
    dcterms:title " Screening" ;
    iso:controlCategory iso:category-6 ;
    iso:correspondsTo <https://par-tec.github.io/security-ontologies/onto/iso#27001/2013/control-7.1.1> ;
    iso:hasControlType iso:Preventive ;
    iso:hasCybersecurityConcept iso:Protect ;
    iso:hasInformationSecurityProperty iso:Availability,
        iso:Confidentiality,
        iso:Integrity ;
    iso:hasOperationalCapability iso:HRSecurity ;
    iso:hasSecurityDomain iso:GovernanceEcosystem ;
    iso:purpose "To ensure all personnel are eligible and suitable for the roles for which they are considered and remain eligible and suitable during their employment" .

<https://par-tec.github.io/security-ontologies/onto/iso#27002/2022/control-6.7> a iso:Control ;
    dcterms:description "Security measures should be implemented when personnel are working remotely to protect information accessed, processed or stored outside the organization's premises" ;
    dcterms:identifier "27002/2022/control-6.7" ;
    dcterms:title " Remote working" ;
    iso:controlCategory iso:category-6 ;
    iso:correspondsTo <https://par-tec.github.io/security-ontologies/onto/iso#27001/2013/control-6.2.2> ;
    iso:hasControlType iso:Preventive ;
    iso:hasCybersecurityConcept iso:Protect ;
    iso:hasInformationSecurityProperty iso:Availability,
        iso:Confidentiality,
        iso:Integrity ;
    iso:hasOperationalCapability iso:AssetManagement,
        iso:PhysicalSecurity,
        iso:SystemNetworkSecurity ;
    iso:hasSecurityDomain iso:GovernanceEcosystem,
        iso:Protection ;
    iso:purpose "To ensure the security of information when personnel are working remotely" .

<https://par-tec.github.io/security-ontologies/onto/iso#27002/2022/control-7.3> a iso:Control ;
    dcterms:description "Physical security for offices, rooms, and facilities should be designed and implemented" ;
    dcterms:identifier "27002/2022/control-7.3" ;
    dcterms:title "Securing offices, rooms and facilities" ;
    iso:controlCategory iso:category-7 ;
    iso:correspondsTo <https://par-tec.github.io/security-ontologies/onto/iso#27001/2013/control-11.1.3> ;
    iso:hasControlType iso:Preventive ;
    iso:hasCybersecurityConcept iso:Protect ;
    iso:hasInformationSecurityProperty iso:Availability,
        iso:Confidentiality,
        iso:Integrity ;
    iso:hasOperationalCapability iso:AssetManagement,
        iso:PhysicalSecurity ;
    iso:hasSecurityDomain iso:Protection ;
    iso:purpose "To prevent unauthorized physical access, damage and interference to the organization’s information and other associated assets in offices, rooms and facilities" .

<https://par-tec.github.io/security-ontologies/onto/iso#27002/2022/control-7.5> a iso:Control ;
    dcterms:description "Protection against physical and environmental threats, such as natural disasters and other intentional or unintentional physical threats to infrastructure should be designed and implemented" ;
    dcterms:identifier "27002/2022/control-7.5" ;
    dcterms:title "Protecting against physical and environmental threats" ;
    iso:controlCategory iso:category-7 ;
    iso:correspondsTo <https://par-tec.github.io/security-ontologies/onto/iso#27001/2013/control-11.1.4> ;
    iso:hasControlType iso:Preventive ;
    iso:hasCybersecurityConcept iso:Protect ;
    iso:hasInformationSecurityProperty iso:Availability,
        iso:Confidentiality,
        iso:Integrity ;
    iso:hasOperationalCapability iso:PhysicalSecurity ;
    iso:hasSecurityDomain iso:Protection ;
    iso:purpose "To prevent or reduce the impacts of events originating from physical and environmental threats" .

<https://par-tec.github.io/security-ontologies/onto/iso#27002/2022/control-7.8> a iso:Control ;
    dcterms:description "Equipment should be sited securely and protected" ;
    dcterms:identifier "27002/2022/control-7.8" ;
    dcterms:title "Equipment siting and protection" ;
    iso:controlCategory iso:category-7 ;
    iso:correspondsTo <https://par-tec.github.io/security-ontologies/onto/iso#27001/2013/control-11.2.1> ;
    iso:hasControlType iso:Preventive ;
    iso:hasCybersecurityConcept iso:Protect ;
    iso:hasInformationSecurityProperty iso:Availability,
        iso:Confidentiality,
        iso:Integrity ;
    iso:hasOperationalCapability iso:AssetManagement,
        iso:PhysicalSecurity ;
    iso:hasSecurityDomain iso:Protection ;
    iso:purpose "To reduce the risks from environmental threats and hazards, and opportunities for unauthorized access" .

<https://par-tec.github.io/security-ontologies/onto/iso#27002/2022/control-7.9> a iso:Control ;
    dcterms:description "Off-site assets should be protected taking into account the different risks" ;
    dcterms:identifier "27002/2022/control-7.9" ;
    dcterms:title "Security of assets off-premises" ;
    iso:controlCategory iso:category-7 ;
    iso:correspondsTo <https://par-tec.github.io/security-ontologies/onto/iso#27001/2013/control-11.2.6> ;
    iso:hasControlType iso:Preventive ;
    iso:hasCybersecurityConcept iso:Protect ;
    iso:hasInformationSecurityProperty iso:Availability,
        iso:Confidentiality,
        iso:Integrity ;
    iso:hasOperationalCapability iso:AssetManagement,
        iso:PhysicalSecurity ;
    iso:hasRelatedControls <https://par-tec.github.io/security-ontologies/onto/iso#27002/2022/control-6.7>,
        <https://par-tec.github.io/security-ontologies/onto/iso#27002/2022/control-7.4>,
        <https://par-tec.github.io/security-ontologies/onto/iso#27002/2022/control-7.5>,
        <https://par-tec.github.io/security-ontologies/onto/iso#27002/2022/control-8.1> ;
    iso:hasSecurityDomain iso:Protection ;
    iso:purpose "To prevent loss, damage, theft or compromise of off-site assets and interruption to the organization’s operations" .

<https://par-tec.github.io/security-ontologies/onto/iso#27002/2022/control-8.22> a iso:Control ;
    dcterms:description "Access to external websites should be managed to reduce exposure to malicious content" ;
    dcterms:identifier "27002/2022/control-8.22" ;
    dcterms:title " Web filtering" ;
    iso:controlCategory iso:category-8 ;
    iso:correspondsTo <https://par-tec.github.io/security-ontologies/onto/iso#27001/2013/control-New> ;
    iso:hasControlType iso:Preventive ;
    iso:hasCybersecurityConcept iso:Protect ;
    iso:hasInformationSecurityProperty iso:Availability,
        iso:Confidentiality,
        iso:Integrity ;
    iso:hasOperationalCapability iso:SystemNetworkSecurity ;
    iso:hasRelatedControls <https://par-tec.github.io/security-ontologies/onto/iso#27002/2022/control-5.7> ;
    iso:hasSecurityDomain iso:Protection ;
    iso:purpose "To protect systems from being compromised by malware and to prevent access to unauthorized web resources" .

<https://par-tec.github.io/security-ontologies/onto/iso#27002/2022/control-8.25> a iso:Control ;
    dcterms:description "Rules for the secure development of software and systems should be established and applied" ;
    dcterms:identifier "27002/2022/control-8.25" ;
    dcterms:title " Secure development lifecycle" ;
    iso:controlCategory iso:category-8 ;
    iso:correspondsTo <https://par-tec.github.io/security-ontologies/onto/iso#27001/2013/control-14.2.1> ;
    iso:hasControlType iso:Preventive ;
    iso:hasCybersecurityConcept iso:Protect ;
    iso:hasInformationSecurityProperty iso:Availability,
        iso:Confidentiality,
        iso:Integrity ;
    iso:hasOperationalCapability iso:ApplicationSecurity,
        iso:SystemNetworkSecurity ;
    iso:hasRelatedControls <https://par-tec.github.io/security-ontologies/onto/iso#27002/2022/control-5.32>,
        <https://par-tec.github.io/security-ontologies/onto/iso#27002/2022/control-5.8>,
        <https://par-tec.github.io/security-ontologies/onto/iso#27002/2022/control-8.27>,
        <https://par-tec.github.io/security-ontologies/onto/iso#27002/2022/control-8.28>,
        <https://par-tec.github.io/security-ontologies/onto/iso#27002/2022/control-8.29>,
        <https://par-tec.github.io/security-ontologies/onto/iso#27002/2022/control-8.30>,
        <https://par-tec.github.io/security-ontologies/onto/iso#27002/2022/control-8.31>,
        <https://par-tec.github.io/security-ontologies/onto/iso#27002/2022/control-8.32>,
        <https://par-tec.github.io/security-ontologies/onto/iso#27002/2022/control-8.4>,
        <https://par-tec.github.io/security-ontologies/onto/iso#27002/2022/control-8.9> ;
    iso:hasSecurityDomain iso:Protection ;
    iso:purpose "To ensure information security is designed and implemented within the secure development lifecycle of software and systems" .

<https://par-tec.github.io/security-ontologies/onto/iso#27002/2022/control-8.27> a iso:Control ;
    dcterms:description "Principles for engineering secure systems should be established, documented, maintained and applied to any information system development activities" ;
    dcterms:identifier "27002/2022/control-8.27" ;
    dcterms:title " Secure system architecture and engineering principles" ;
    iso:controlCategory iso:category-8 ;
    iso:correspondsTo <https://par-tec.github.io/security-ontologies/onto/iso#27001/2013/control-14.2.5> ;
    iso:hasControlType iso:Preventive ;
    iso:hasCybersecurityConcept iso:Protect ;
    iso:hasInformationSecurityProperty iso:Availability,
        iso:Confidentiality,
        iso:Integrity ;
    iso:hasOperationalCapability iso:ApplicationSecurity,
        iso:SystemNetworkSecurity ;
    iso:hasRelatedControls <https://par-tec.github.io/security-ontologies/onto/iso#27002/2022/control-5.12>,
        <https://par-tec.github.io/security-ontologies/onto/iso#27002/2022/control-5.16>,
        <https://par-tec.github.io/security-ontologies/onto/iso#27002/2022/control-5.17>,
        <https://par-tec.github.io/security-ontologies/onto/iso#27002/2022/control-5.18>,
        <https://par-tec.github.io/security-ontologies/onto/iso#27002/2022/control-8.2> ;
    iso:hasSecurityDomain iso:Protection ;
    iso:purpose "To  ensure  information  systems  are  securely  designed,  implemented  and  operated  within  the development lifecycle" .

<https://par-tec.github.io/security-ontologies/onto/iso#27002/2022/control-8.30> a iso:Control ;
    dcterms:description "The  organization  should  direct,  monitor  and  review  the  activities  related  to  outsourced  system development" ;
    dcterms:identifier "27002/2022/control-8.30" ;
    dcterms:title "  Outsourced development" ;
    iso:controlCategory iso:category-8 ;
    iso:correspondsTo <https://par-tec.github.io/security-ontologies/onto/iso#27001/2013/control-14.2.7> ;
    iso:hasControlType iso:Detective,
        iso:Preventive ;
    iso:hasCybersecurityConcept iso:Detect,
        iso:Identify,
        iso:Protect ;
    iso:hasInformationSecurityProperty iso:Availability,
        iso:Confidentiality,
        iso:Integrity ;
    iso:hasOperationalCapability iso:ApplicationSecurity,
        iso:SupplierSecurity,
        iso:SystemNetworkSecurity ;
    iso:hasRelatedControls <https://par-tec.github.io/security-ontologies/onto/iso#27002/2022/control-5.32>,
        <https://par-tec.github.io/security-ontologies/onto/iso#27002/2022/control-8.25-8.29>,
        <https://par-tec.github.io/security-ontologies/onto/iso#27002/2022/control-8.31> ;
    iso:hasSecurityDomain iso:GovernanceEcosystem,
        iso:Protection ;
    iso:purpose "To ensure information security measures required by the organization are implemented in outsourced system development" .

<https://par-tec.github.io/security-ontologies/onto/iso#27002/2022/control-8.33> a iso:Control ;
    dcterms:description "Test information should be appropriately selected, protected and managed" ;
    dcterms:identifier "27002/2022/control-8.33" ;
    dcterms:title "Test information" ;
    iso:controlCategory iso:category-8 ;
    iso:correspondsTo <https://par-tec.github.io/security-ontologies/onto/iso#27001/2013/control-14.3.1> ;
    iso:hasControlType iso:Preventive ;
    iso:hasCybersecurityConcept iso:Protect ;
    iso:hasInformationSecurityProperty iso:Confidentiality,
        iso:Integrity ;
    iso:hasOperationalCapability iso:InformationProtection ;
    iso:hasRelatedControls <https://par-tec.github.io/security-ontologies/onto/iso#27002/2022/control-8.10>,
        <https://par-tec.github.io/security-ontologies/onto/iso#27002/2022/control-8.11>,
        <https://par-tec.github.io/security-ontologies/onto/iso#27002/2022/control-8.31> ;
    iso:hasSecurityDomain iso:Protection ;
    iso:purpose "To ensure relevance of testing and protection of operational information used for testing" .

iso:ThreatManagement a iso:OperationalCapability ;
    rdfs:label "Threat and Vulnerability Management" ;
    rdfs:comment "Threat and Vulnerability management capabilities are capabilities that manage threats." .

<https://par-tec.github.io/security-ontologies/onto/iso#27001/2013/category-14> a iso:ControlCategory ;
    rdfs:label "System acquisition, development and maintenance" .

<https://par-tec.github.io/security-ontologies/onto/iso#27001/2013/category-7> a iso:ControlCategory ;
    rdfs:label "Human resources security" .

<https://par-tec.github.io/security-ontologies/onto/iso#27001/2013/category-8> a iso:ControlCategory ;
    rdfs:label "Asset management" .

<https://par-tec.github.io/security-ontologies/onto/iso#27001/2013/section-13.1> a iso:Section ;
    rdfs:label "Network security management" ;
    iso:controlCategory <https://par-tec.github.io/security-ontologies/onto/iso#27001/2013/category-13> .

<https://par-tec.github.io/security-ontologies/onto/iso#27001/2013/section-14.1> a iso:Section ;
    rdfs:label "Security requirements of information systems" ;
    iso:controlCategory <https://par-tec.github.io/security-ontologies/onto/iso#27001/2013/category-14> .

<https://par-tec.github.io/security-ontologies/onto/iso#27001/2013/section-15.1> a iso:Section ;
    rdfs:label "Information security in supplier relationships" ;
    iso:controlCategory <https://par-tec.github.io/security-ontologies/onto/iso#27001/2013/category-15> .

<https://par-tec.github.io/security-ontologies/onto/iso#27001/2013/section-17.1> a iso:Section ;
    rdfs:label "Information security continuity" ;
    iso:controlCategory <https://par-tec.github.io/security-ontologies/onto/iso#27001/2013/category-17> .

<https://par-tec.github.io/security-ontologies/onto/iso#27001/2013/section-18.2> a iso:Section ;
    rdfs:label "Information security reviews" ;
    iso:controlCategory <https://par-tec.github.io/security-ontologies/onto/iso#27001/2013/category-18> .

<https://par-tec.github.io/security-ontologies/onto/iso#27001/2013/section-7.2> a iso:Section ;
    rdfs:label "During employment" ;
    iso:controlCategory <https://par-tec.github.io/security-ontologies/onto/iso#27001/2013/category-7> .

<https://par-tec.github.io/security-ontologies/onto/iso#27001/2013/section-8.2> a iso:Section ;
    rdfs:label "Information classification" ;
    iso:controlCategory <https://par-tec.github.io/security-ontologies/onto/iso#27001/2013/category-8> .

<https://par-tec.github.io/security-ontologies/onto/iso#27001/2013/section-8.3> a iso:Section ;
    rdfs:label "Media Handling" ;
    iso:controlCategory <https://par-tec.github.io/security-ontologies/onto/iso#27001/2013/category-8> .

<https://par-tec.github.io/security-ontologies/onto/iso#27002/2022/control-5.1> a iso:Control ;
    dcterms:description """Information security policy and topic-specific policies should be defined, approved by management,
published, communicated to and acknowledged by relevant personnel and relevant interested parties,
and reviewed at planned intervals and if significant changes occur.""" ;
    dcterms:identifier "27002/2022/control-5.1" ;
    dcterms:title "Policies for information security" ;
    iso:controlCategory iso:category-5 ;
    iso:correspondsTo <https://par-tec.github.io/security-ontologies/onto/iso#27001/2013/control-5.1.1>,
        <https://par-tec.github.io/security-ontologies/onto/iso#27001/2013/control-5.1.2> ;
    iso:hasControlType iso:Preventive ;
    iso:hasCybersecurityConcept iso:Identify ;
    iso:hasInformationSecurityProperty iso:Availability,
        iso:Confidentiality,
        iso:Integrity ;
    iso:hasOperationalCapability iso:Governance ;
    iso:hasSecurityDomain iso:GovernanceEcosystem,
        iso:Resilience ;
    iso:purpose """To ensure continuing suitability, adequacy, effectiveness of management direction and support for
information security in accordance with business requirements, legal, statutory, regulatory and
contractual requirements.""" .

<https://par-tec.github.io/security-ontologies/onto/iso#27002/2022/control-5.16> a iso:Control ;
    dcterms:description "The full lifecycle of identities should be managed" ;
    dcterms:identifier "27002/2022/control-5.16" ;
    dcterms:title " Identity management" ;
    iso:controlCategory iso:category-5 ;
    iso:correspondsTo <https://par-tec.github.io/security-ontologies/onto/iso#27001/2013/control-9.2.1> ;
    iso:hasControlType iso:Preventive ;
    iso:hasCybersecurityConcept iso:Protect ;
    iso:hasInformationSecurityProperty iso:Availability,
        iso:Confidentiality,
        iso:Integrity ;
    iso:hasOperationalCapability iso:IAM ;
    iso:hasRelatedControls <https://par-tec.github.io/security-ontologies/onto/iso#27002/2022/control-5.18> ;
    iso:hasSecurityDomain iso:Protection ;
    iso:purpose "To  allow  for  the  unique  identification  of  individuals  and  systems  accessing  the  organisation's information and other associated assets, and to enable appropriate assignment of access rights" .

<https://par-tec.github.io/security-ontologies/onto/iso#27002/2022/control-5.35> a iso:Control ;
    dcterms:description "The organization’s approach to managing information security and its implementation including people process and technology should be reviewed independently at planned intervals, or when significant changes occur" ;
    dcterms:identifier "27002/2022/control-5.35" ;
    dcterms:title "Independent review of information security" ;
    iso:controlCategory iso:category-5 ;
    iso:correspondsTo <https://par-tec.github.io/security-ontologies/onto/iso#27001/2013/control-18.2.1> ;
    iso:hasControlType iso:Corrective,
        iso:Preventive ;
    iso:hasCybersecurityConcept iso:Identify ;
    iso:hasInformationSecurityProperty iso:Availability,
        iso:Confidentiality,
        iso:Integrity ;
    iso:purpose "To ensure the continuing suitability, adequacy and effectiveness of the organization’s approach to managing information security" .

<https://par-tec.github.io/security-ontologies/onto/iso#27002/2022/control-5.36> a iso:Control ;
    dcterms:description "Compliance with the organization’s information security policy, topic-specific policies and standards should be regularly reviewed" ;
    dcterms:identifier "27002/2022/control-5.36" ;
    dcterms:title "Compliance with policies and standards for information security" ;
    iso:controlCategory iso:category-5 ;
    iso:correspondsTo <https://par-tec.github.io/security-ontologies/onto/iso#27001/2013/control-18.2.2>,
        <https://par-tec.github.io/security-ontologies/onto/iso#27001/2013/control-18.2.3> ;
    iso:hasControlType iso:Preventive ;
    iso:hasCybersecurityConcept iso:Protect ;
    iso:hasInformationSecurityProperty iso:Availability,
        iso:Confidentiality,
        iso:Integrity ;
    iso:hasOperationalCapability iso:Compliance ;
    iso:hasRelatedControls <https://par-tec.github.io/security-ontologies/onto/iso#27002/2022/control-5.35>,
        <https://par-tec.github.io/security-ontologies/onto/iso#27002/2022/control-8.15>,
        <https://par-tec.github.io/security-ontologies/onto/iso#27002/2022/control-8.16>,
        <https://par-tec.github.io/security-ontologies/onto/iso#27002/2022/control-8.17> ;
    iso:hasSecurityDomain iso:GovernanceEcosystem ;
    iso:purpose "To ensure that information security is implemented and operated in accordance with the organizational policies topic-specific policies and standards" .

<https://par-tec.github.io/security-ontologies/onto/iso#27002/2022/control-5.7> a iso:Control ;
    dcterms:description """Information relating to information security threats should be collected and analysed to produce threat
intelligence""" ;
    dcterms:identifier "27002/2022/control-5.7" ;
    dcterms:title "Threat intelligence" ;
    iso:controlCategory iso:category-5 ;
    iso:correspondsTo <https://par-tec.github.io/security-ontologies/onto/iso#27001/2013/control-New> ;
    iso:hasControlType iso:Detective,
        iso:Preventive ;
    iso:hasCybersecurityConcept iso:Detect,
        iso:Identify ;
    iso:hasInformationSecurityProperty iso:Availability,
        iso:Confidentiality,
        iso:Integrity ;
    iso:hasOperationalCapability iso:ThreatManagement ;
    iso:hasRelatedControls <https://par-tec.github.io/security-ontologies/onto/iso#27002/2022/control-5.25>,
        <https://par-tec.github.io/security-ontologies/onto/iso#27002/2022/control-8.16>,
        <https://par-tec.github.io/security-ontologies/onto/iso#27002/2022/control-8.22>,
        <https://par-tec.github.io/security-ontologies/onto/iso#27002/2022/control-8.7> ;
    iso:hasSecurityDomain iso:Defence,
        iso:Resilience ;
    iso:purpose """To provide awareness of the threat environment that can impact the organization so that the
organization can take appropriate mitigation actions""" .

<https://par-tec.github.io/security-ontologies/onto/iso#27002/2022/control-6.4> a iso:Control ;
    dcterms:description "A disciplinary process should be formalized and communicated to take actions against personnel and other relevant interested parties who have committed an information security policy violation" ;
    dcterms:identifier "27002/2022/control-6.4" ;
    dcterms:title " Disciplinary process" ;
    iso:controlCategory iso:category-6 ;
    iso:correspondsTo <https://par-tec.github.io/security-ontologies/onto/iso#27001/2013/control-7.2.3> ;
    iso:hasControlType iso:Corrective,
        iso:Preventive ;
    iso:hasCybersecurityConcept iso:Protect,
        iso:Respond ;
    iso:hasInformationSecurityProperty iso:Availability,
        iso:Confidentiality,
        iso:Integrity ;
    iso:hasOperationalCapability iso:HRSecurity ;
    iso:hasRelatedControls <https://par-tec.github.io/security-ontologies/onto/iso#27002/2022/control-5.28> ;
    iso:hasSecurityDomain iso:GovernanceEcosystem ;
    iso:purpose "To ensure personnel and other relevant interested parties understand the consequences of information security breaches, and non-compliant activities are deterred" .

<https://par-tec.github.io/security-ontologies/onto/iso#27002/2022/control-6.5> a iso:Control ;
    dcterms:description "Information security responsibilities and duties that remain valid after termination or change of employment should be defined, enforced and communicated to relevant personnel and other interested parties" ;
    dcterms:identifier "27002/2022/control-6.5" ;
    dcterms:title "Responsibilities after termination or change of employment" ;
    iso:controlCategory iso:category-6 ;
    iso:correspondsTo <https://par-tec.github.io/security-ontologies/onto/iso#27001/2013/control-7.3.1> ;
    iso:hasControlType iso:Preventive ;
    iso:hasCybersecurityConcept iso:Protect ;
    iso:hasInformationSecurityProperty iso:Availability,
        iso:Confidentiality,
        iso:Integrity ;
    iso:hasOperationalCapability iso:AssetManagement,
        iso:HRSecurity ;
    iso:hasRelatedControls <https://par-tec.github.io/security-ontologies/onto/iso#27002/2022/control-6.2>,
        <https://par-tec.github.io/security-ontologies/onto/iso#27002/2022/control-6.6> ;
    iso:hasSecurityDomain iso:GovernanceEcosystem ;
    iso:purpose "To protect the organization’s interests as part of the process of changing or terminating employment or contract" .

<https://par-tec.github.io/security-ontologies/onto/iso#27002/2022/control-6.8> a iso:Control ;
    dcterms:description "The  organization  should  provide  a  mechanism  for  personnel  to  report  observed  or  suspected information security events through appropriate channels in a timely manner" ;
    dcterms:identifier "27002/2022/control-6.8" ;
    dcterms:title " Information security event reporting" ;
    iso:controlCategory iso:category-6 ;
    iso:correspondsTo <https://par-tec.github.io/security-ontologies/onto/iso#27001/2013/control-16.1.2>,
        <https://par-tec.github.io/security-ontologies/onto/iso#27001/2013/control-16.1.3> ;
    iso:hasControlType iso:Detective ;
    iso:hasCybersecurityConcept iso:Detect ;
    iso:hasInformationSecurityProperty iso:Availability,
        iso:Confidentiality,
        iso:Integrity ;
    iso:hasOperationalCapability iso:EventManangement ;
    iso:hasSecurityDomain iso:Defence ;
    iso:purpose "To  support  timely,  consistent  and  effective  reporting  of  information  security  events  that  can  be identified by personnel" .

<https://par-tec.github.io/security-ontologies/onto/iso#27002/2022/control-7.2> a iso:Control ;
    dcterms:description "Secure areas should be protected by appropriate entry controls and access points" ;
    dcterms:identifier "27002/2022/control-7.2" ;
    dcterms:title " Physical entry controls" ;
    iso:controlCategory iso:category-7 ;
    iso:correspondsTo <https://par-tec.github.io/security-ontologies/onto/iso#27001/2013/control-11.1.2>,
        <https://par-tec.github.io/security-ontologies/onto/iso#27001/2013/control-11.1.6> ;
    iso:hasControlType iso:Preventive ;
    iso:hasCybersecurityConcept iso:Protect ;
    iso:hasInformationSecurityProperty iso:Availability,
        iso:Confidentiality,
        iso:Integrity ;
    iso:hasOperationalCapability iso:PhysicalSecurity ;
    iso:hasRelatedControls <https://par-tec.github.io/security-ontologies/onto/iso#27002/2022/control-5.17>,
        <https://par-tec.github.io/security-ontologies/onto/iso#27002/2022/control-5.18>,
        <https://par-tec.github.io/security-ontologies/onto/iso#27002/2022/control-5.33>,
        <https://par-tec.github.io/security-ontologies/onto/iso#27002/2022/control-5.9>,
        <https://par-tec.github.io/security-ontologies/onto/iso#27002/2022/control-7.10> ;
    iso:hasSecurityDomain iso:Protection ;
    iso:purpose "To ensure only authorized physical access to the organization’s information and other associated assets occurs" .

<https://par-tec.github.io/security-ontologies/onto/iso#27002/2022/control-8.11> a iso:Control ;
    dcterms:description "Data masking should be used in accordance with the organization’s topic-specific policy on access control and business requirement, taking legal requirements into consideration" ;
    dcterms:identifier "27002/2022/control-8.11" ;
    dcterms:title " Data masking" ;
    iso:controlCategory iso:category-8 ;
    iso:correspondsTo <https://par-tec.github.io/security-ontologies/onto/iso#27001/2013/control-New> ;
    iso:hasControlType iso:Preventive ;
    iso:hasCybersecurityConcept iso:Protect ;
    iso:hasInformationSecurityProperty iso:Confidentiality ;
    iso:hasOperationalCapability iso:InformationProtection ;
    iso:hasSecurityDomain iso:Protection ;
    iso:purpose "To limit the exposure of sensitive data including personally identifiable information, and to comply with legal, statutory, regulatory and contractual requirements" .

<https://par-tec.github.io/security-ontologies/onto/iso#27002/2022/control-8.14> a iso:Control ;
    dcterms:description "Information processing facilities should be implemented with redundancy sufficient to meet availability requirements" ;
    dcterms:identifier "27002/2022/control-8.14" ;
    dcterms:title "Redundancy of information processing facilities" ;
    iso:controlCategory iso:category-8 ;
    iso:correspondsTo <https://par-tec.github.io/security-ontologies/onto/iso#27001/2013/control-17.2.1> ;
    iso:hasControlType iso:Preventive ;
    iso:hasCybersecurityConcept iso:Protect ;
    iso:hasInformationSecurityProperty iso:Availability ;
    iso:hasOperationalCapability iso:AssetManagement,
        iso:Continuity ;
    iso:hasRelatedControls <https://par-tec.github.io/security-ontologies/onto/iso#27002/2022/control-5.30> ;
    iso:hasSecurityDomain iso:Protection,
        iso:Resilience ;
    iso:purpose "To ensure the continuous operation of information processing facilities" .

<https://par-tec.github.io/security-ontologies/onto/iso#27002/2022/control-8.18> a iso:Control ;
    dcterms:description "The use of utility programs that might be capable of overriding system and application controls should be restricted and tightly controlled" ;
    dcterms:identifier "27002/2022/control-8.18" ;
    dcterms:title " Use of privileged utility programs" ;
    iso:controlCategory iso:category-8 ;
    iso:correspondsTo <https://par-tec.github.io/security-ontologies/onto/iso#27001/2013/control-9.4.4> ;
    iso:hasControlType iso:Preventive ;
    iso:hasCybersecurityConcept iso:Protect ;
    iso:hasInformationSecurityProperty iso:Availability,
        iso:Confidentiality,
        iso:Integrity ;
    iso:hasOperationalCapability iso:SecureConfiguration,
        iso:SystemNetworkSecurity ;
    iso:hasRelatedControls <https://par-tec.github.io/security-ontologies/onto/iso#27002/2022/control-8.2> ;
    iso:hasSecurityDomain iso:Protection ;
    iso:purpose "To ensure the use of utility programs does not harm system and application controls for information security" .

<https://par-tec.github.io/security-ontologies/onto/iso#27002/2022/control-8.23> a iso:Control ;
    dcterms:description "Groups  of  information  services,  users,  and  information  systems  should  be  segregated  in  the organization’s networks" ;
    dcterms:identifier "27002/2022/control-8.23" ;
    dcterms:title " Segregation in networks" ;
    iso:controlCategory iso:category-8 ;
    iso:correspondsTo <https://par-tec.github.io/security-ontologies/onto/iso#27001/2013/control-13.1.3> ;
    iso:hasControlType iso:Preventive ;
    iso:hasCybersecurityConcept iso:Protect ;
    iso:hasInformationSecurityProperty iso:Availability,
        iso:Confidentiality,
        iso:Integrity ;
    iso:hasOperationalCapability iso:SystemNetworkSecurity ;
    iso:hasRelatedControls <https://par-tec.github.io/security-ontologies/onto/iso#27002/2022/control-5.15>,
        <https://par-tec.github.io/security-ontologies/onto/iso#27002/2022/control-8.20> ;
    iso:hasSecurityDomain iso:Protection ;
    iso:purpose "To split the network in security boundaries and to control traffic between them based on business needs" .

<https://par-tec.github.io/security-ontologies/onto/iso#27002/2022/control-8.3> a iso:Control ;
    dcterms:description "Access  to  information  and  other  associated  assets  should  be  restricted  in  accordance  with  the established topic-specific policy on access control" ;
    dcterms:identifier "27002/2022/control-8.3" ;
    dcterms:title "Information access restriction" ;
    iso:controlCategory iso:category-8 ;
    iso:correspondsTo <https://par-tec.github.io/security-ontologies/onto/iso#27001/2013/control-9.4.1> ;
    iso:hasControlType iso:Preventive ;
    iso:hasCybersecurityConcept iso:Protect ;
    iso:hasInformationSecurityProperty iso:Availability,
        iso:Confidentiality,
        iso:Integrity ;
    iso:hasOperationalCapability iso:IAM ;
    iso:hasRelatedControls <https://par-tec.github.io/security-ontologies/onto/iso#27002/2022/control-5.15> ;
    iso:hasSecurityDomain iso:Protection ;
    iso:purpose "To  ensure  only  authorized  access  and  to  prevent  unauthorized  access  to  information  and  other associated assets" .

<https://par-tec.github.io/security-ontologies/onto/iso#27002/2022/control-8.7> a iso:Control ;
    dcterms:description "Protection against malware should be implemented, supported by appropriate user awareness" ;
    dcterms:identifier "27002/2022/control-8.7" ;
    dcterms:title "Protection against malware" ;
    iso:controlCategory iso:category-8 ;
    iso:correspondsTo <https://par-tec.github.io/security-ontologies/onto/iso#27001/2013/control-12.2.1> ;
    iso:hasControlType iso:Corrective,
        iso:Detective,
        iso:Preventive ;
    iso:hasCybersecurityConcept iso:Detect,
        iso:Protect ;
    iso:hasInformationSecurityProperty iso:Availability,
        iso:Confidentiality,
        iso:Integrity ;
    iso:hasOperationalCapability iso:SystemNetworkSecurity ;
    iso:hasRelatedControls <https://par-tec.github.io/security-ontologies/onto/iso#27002/2022/control-6.3>,
        <https://par-tec.github.io/security-ontologies/onto/iso#27002/2022/control-8.13>,
        <https://par-tec.github.io/security-ontologies/onto/iso#27002/2022/control-8.19>,
        <https://par-tec.github.io/security-ontologies/onto/iso#27002/2022/control-8.32>,
        <https://par-tec.github.io/security-ontologies/onto/iso#27002/2022/control-8.8> ;
    iso:hasSecurityDomain iso:Defence,
        iso:Protection ;
    iso:purpose "To ensure information and other associated assets are protected against malware" .

<https://par-tec.github.io/security-ontologies/onto/iso#27001/2013/category-9> a iso:ControlCategory ;
    rdfs:label "Access control" .

<https://par-tec.github.io/security-ontologies/onto/iso#27001/2013/section-12.1> a iso:Section ;
    rdfs:label "Operational procedures and responsibilities" ;
    iso:controlCategory <https://par-tec.github.io/security-ontologies/onto/iso#27001/2013/category-12> .

<https://par-tec.github.io/security-ontologies/onto/iso#27001/2013/section-12.4> a iso:Section ;
    rdfs:label "Logging and monitoring" ;
    iso:controlCategory <https://par-tec.github.io/security-ontologies/onto/iso#27001/2013/category-12> .

<https://par-tec.github.io/security-ontologies/onto/iso#27001/2013/section-13.2> a iso:Section ;
    rdfs:label "Information transfer" ;
    iso:controlCategory <https://par-tec.github.io/security-ontologies/onto/iso#27001/2013/category-13> .

<https://par-tec.github.io/security-ontologies/onto/iso#27001/2013/section-8.1> a iso:Section ;
    rdfs:label "Responsibility for assets" ;
    iso:controlCategory <https://par-tec.github.io/security-ontologies/onto/iso#27001/2013/category-8> .

<https://par-tec.github.io/security-ontologies/onto/iso#27002/2022/control-5.27> a iso:Control ;
    dcterms:description "Knowledge gained from information security incidents should be used to strengthen and improve the control environment" ;
    dcterms:identifier "27002/2022/control-5.27" ;
    dcterms:title "Learning from information security incidents" ;
    iso:controlCategory iso:category-5 ;
    iso:correspondsTo <https://par-tec.github.io/security-ontologies/onto/iso#27001/2013/control-16.1.6> ;
    iso:hasControlType iso:Corrective,
        iso:Preventive ;
    iso:hasCybersecurityConcept iso:Identify,
        iso:Protect ;
    iso:hasInformationSecurityProperty iso:Confidentiality,
        iso:Integrity ;
    iso:hasOperationalCapability iso:EventManangement ;
    iso:hasRelatedControls <https://par-tec.github.io/security-ontologies/onto/iso#27002/2022/control-5.24>,
        <https://par-tec.github.io/security-ontologies/onto/iso#27002/2022/control-6.3> ;
    iso:hasSecurityDomain iso:Defence ;
    iso:purpose "To reduce the likelihood or impact of future incidents" .

<https://par-tec.github.io/security-ontologies/onto/iso#27002/2022/control-5.3> a iso:Control ;
    dcterms:description "Conflicting duties and areas of responsibility should be segregated" ;
    dcterms:identifier "27002/2022/control-5.3" ;
    dcterms:title "Segregation of duties" ;
    iso:controlCategory iso:category-5 ;
    iso:correspondsTo <https://par-tec.github.io/security-ontologies/onto/iso#27001/2013/control-6.1.2> ;
    iso:hasControlType iso:Preventive ;
    iso:hasCybersecurityConcept iso:Protect ;
    iso:hasInformationSecurityProperty iso:Availability,
        iso:Confidentiality,
        iso:Integrity ;
    iso:hasOperationalCapability iso:Governance ;
    iso:hasSecurityDomain iso:GovernanceEcosystem ;
    iso:purpose "To reduce the risk of fraud, error and bypassing of information security controls" .

<https://par-tec.github.io/security-ontologies/onto/iso#27002/2022/control-5.8> a iso:Control ;
    dcterms:description "Information security should be integrated into the organization's project management activities" ;
    dcterms:identifier "27002/2022/control-5.8" ;
    dcterms:title "Information security in project management" ;
    iso:controlCategory iso:category-5 ;
    iso:correspondsTo <https://par-tec.github.io/security-ontologies/onto/iso#27001/2013/control-14.1.1>,
        <https://par-tec.github.io/security-ontologies/onto/iso#27001/2013/control-6.1.5> ;
    iso:hasControlType iso:Preventive ;
    iso:hasCybersecurityConcept iso:Identify,
        iso:Protect ;
    iso:hasInformationSecurityProperty iso:Availability,
        iso:Confidentiality,
        iso:Integrity ;
    iso:hasOperationalCapability iso:Governance ;
    iso:hasRelatedControls <https://par-tec.github.io/security-ontologies/onto/iso#27002/2022/control-5.10>,
        <https://par-tec.github.io/security-ontologies/onto/iso#27002/2022/control-5.12>,
        <https://par-tec.github.io/security-ontologies/onto/iso#27002/2022/control-5.13>,
        <https://par-tec.github.io/security-ontologies/onto/iso#27002/2022/control-5.32>,
        <https://par-tec.github.io/security-ontologies/onto/iso#27002/2022/control-8.26> ;
    iso:hasSecurityDomain iso:GovernanceEcosystem,
        iso:Protection ;
    iso:purpose "To ensure information security risks related to projects and deliverables are efficiently and effectively included in project management activities throughout the project lifecycle" .

<https://par-tec.github.io/security-ontologies/onto/iso#27002/2022/control-6.2> a iso:Control ;
    dcterms:description "The   employment   contractual   agreements   should   state   the   personnel’s   and   the   organization’s responsibilities for information security" ;
    dcterms:identifier "27002/2022/control-6.2" ;
    dcterms:title "Terms and conditions of employment" ;
    iso:controlCategory iso:category-6 ;
    iso:correspondsTo <https://par-tec.github.io/security-ontologies/onto/iso#27001/2013/control-7.1.2> ;
    iso:hasControlType iso:Preventive ;
    iso:hasCybersecurityConcept iso:Protect ;
    iso:hasInformationSecurityProperty iso:Availability,
        iso:Confidentiality,
        iso:Integrity ;
    iso:hasOperationalCapability iso:HRSecurity ;
    iso:hasRelatedControls <https://par-tec.github.io/security-ontologies/onto/iso#27002/2022/control-5.13>,
        <https://par-tec.github.io/security-ontologies/onto/iso#27002/2022/control-5.32>,
        <https://par-tec.github.io/security-ontologies/onto/iso#27002/2022/control-5.34>,
        <https://par-tec.github.io/security-ontologies/onto/iso#27002/2022/control-5.9>,
        <https://par-tec.github.io/security-ontologies/onto/iso#27002/2022/control-6.4>,
        <https://par-tec.github.io/security-ontologies/onto/iso#27002/2022/control-6.5>,
        <https://par-tec.github.io/security-ontologies/onto/iso#27002/2022/control-6.6> ;
    iso:hasSecurityDomain iso:GovernanceEcosystem ;
    iso:purpose "To ensure personnel understand their information security responsibilities for the roles for which they are considered" .

<https://par-tec.github.io/security-ontologies/onto/iso#27002/2022/control-6.3> a iso:Control ;
    dcterms:description "Personnel of the organization and relevant interested parties should receive appropriate information security awareness, education and training and regular updates of organizational policies and procedures, as relevant for their job function" ;
    dcterms:identifier "27002/2022/control-6.3" ;
    dcterms:title "Information security awareness, education and training" ;
    iso:controlCategory iso:category-6 ;
    iso:correspondsTo <https://par-tec.github.io/security-ontologies/onto/iso#27001/2013/control-7.2.2> ;
    iso:hasControlType iso:Preventive ;
    iso:hasCybersecurityConcept iso:Protect ;
    iso:hasInformationSecurityProperty iso:Availability,
        iso:Confidentiality,
        iso:Integrity ;
    iso:hasOperationalCapability iso:HRSecurity ;
    iso:hasSecurityDomain iso:GovernanceEcosystem ;
    iso:purpose "To ensure personnel and relevant interested parties are aware of and fulfil their information security responsibilities" .

<https://par-tec.github.io/security-ontologies/onto/iso#27002/2022/control-7.4> a iso:Control ;
    dcterms:description "Premises should be continuously monitored for unauthorized physical access" ;
    dcterms:identifier "27002/2022/control-7.4" ;
    dcterms:title "Physical security monitoring" ;
    iso:controlCategory iso:category-7 ;
    iso:correspondsTo <https://par-tec.github.io/security-ontologies/onto/iso#27001/2013/control-New> ;
    iso:hasControlType iso:Detective ;
    iso:hasCybersecurityConcept iso:Detect ;
    iso:hasInformationSecurityProperty iso:Availability,
        iso:Confidentiality,
        iso:Integrity ;
    iso:hasOperationalCapability iso:PhysicalSecurity ;
    iso:hasSecurityDomain iso:Defence,
        iso:Protection ;
    iso:purpose "To detect and deter unauthorized physical access" .

<https://par-tec.github.io/security-ontologies/onto/iso#27002/2022/control-8.1> a iso:Control ;
    dcterms:description "Information stored on, processed by or accessible via user endpoint devices should be protected" ;
    dcterms:identifier "27002/2022/control-8.1" ;
    dcterms:title " User endpoint devices" ;
    iso:controlCategory iso:category-8 ;
    iso:correspondsTo <https://par-tec.github.io/security-ontologies/onto/iso#27001/2013/control-11.2.8>,
        <https://par-tec.github.io/security-ontologies/onto/iso#27001/2013/control-6.2.1> ;
    iso:hasControlType iso:Preventive ;
    iso:hasCybersecurityConcept iso:Protect ;
    iso:hasInformationSecurityProperty iso:Availability,
        iso:Confidentiality,
        iso:Integrity ;
    iso:hasOperationalCapability iso:AssetManagement,
        iso:InformationProtection ;
    iso:hasRelatedControls <https://par-tec.github.io/security-ontologies/onto/iso#27002/2022/control-8.9> ;
    iso:hasSecurityDomain iso:Protection ;
    iso:purpose "To protect information against the risks introduced by using user endpoint devices" .

<https://par-tec.github.io/security-ontologies/onto/iso#27002/2022/control-8.13> a iso:Control ;
    dcterms:description "Backup copies of information, software and systems should be maintained and regularly tested in accordance with the agreed topic-specific policy on backup" ;
    dcterms:identifier "27002/2022/control-8.13" ;
    dcterms:title "Information backup" ;
    iso:controlCategory iso:category-8 ;
    iso:correspondsTo <https://par-tec.github.io/security-ontologies/onto/iso#27001/2013/control-12.3.1> ;
    iso:hasControlType iso:Corrective ;
    iso:hasCybersecurityConcept iso:Recover ;
    iso:hasInformationSecurityProperty iso:Availability,
        iso:Integrity ;
    iso:hasOperationalCapability iso:Continuity ;
    iso:hasRelatedControls <https://par-tec.github.io/security-ontologies/onto/iso#27002/2022/control-5.30>,
        <https://par-tec.github.io/security-ontologies/onto/iso#27002/2022/control-7>,
        <https://par-tec.github.io/security-ontologies/onto/iso#27002/2022/control-8.1>,
        <https://par-tec.github.io/security-ontologies/onto/iso#27002/2022/control-8.10>,
        <https://par-tec.github.io/security-ontologies/onto/iso#27002/2022/control-Clause> ;
    iso:hasSecurityDomain iso:Protection ;
    iso:purpose "To enable recovery from loss of data or systems" .

<https://par-tec.github.io/security-ontologies/onto/iso#27002/2022/control-8.16> a iso:Control ;
    dcterms:description "Networks, systems and applications should be monitored for anomalous behaviour and appropriate actions taken to evaluate potential information security incidents" ;
    dcterms:identifier "27002/2022/control-8.16" ;
    dcterms:title " Monitoring activities" ;
    iso:controlCategory iso:category-8 ;
    iso:correspondsTo <https://par-tec.github.io/security-ontologies/onto/iso#27001/2013/control-New> ;
    iso:hasControlType iso:Corrective,
        iso:Detective ;
    iso:hasCybersecurityConcept iso:Detect,
        iso:Respond ;
    iso:hasInformationSecurityProperty iso:Availability,
        iso:Confidentiality,
        iso:Integrity ;
    iso:hasOperationalCapability iso:EventManangement ;
    iso:hasRelatedControls <https://par-tec.github.io/security-ontologies/onto/iso#27002/2022/control-5.25>,
        <https://par-tec.github.io/security-ontologies/onto/iso#27002/2022/control-5.26>,
        <https://par-tec.github.io/security-ontologies/onto/iso#27002/2022/control-5.7> ;
    iso:hasSecurityDomain iso:Defence ;
    iso:purpose "To detect anomalous behaviour and potential information security incidents" .

<https://par-tec.github.io/security-ontologies/onto/iso#27002/2022/control-8.17> a iso:Control ;
    dcterms:description "The clocks of information processing systems used by the organization should be synchronized to approved time sources" ;
    dcterms:identifier "27002/2022/control-8.17" ;
    dcterms:title " Clock synchronization" ;
    iso:controlCategory iso:category-8 ;
    iso:correspondsTo <https://par-tec.github.io/security-ontologies/onto/iso#27001/2013/control-12.4.4> ;
    iso:hasControlType iso:Detective ;
    iso:hasCybersecurityConcept iso:Detect,
        iso:Protect ;
    iso:hasInformationSecurityProperty iso:Integrity ;
    iso:hasOperationalCapability iso:EventManangement ;
    iso:hasSecurityDomain iso:Defence,
        iso:Protection ;
    iso:purpose "To enable the correlation and analysis of security-related events and other recorded data, and to support investigations into information security incidents" .

<https://par-tec.github.io/security-ontologies/onto/iso#27002/2022/control-8.19> a iso:Control ;
    dcterms:description "Procedures  and  measures  should  be  implemented  to  securely  manage  software  installation  on operational systems" ;
    dcterms:identifier "27002/2022/control-8.19" ;
    dcterms:title "Installation of software on operational systems" ;
    iso:controlCategory iso:category-8 ;
    iso:correspondsTo <https://par-tec.github.io/security-ontologies/onto/iso#27001/2013/control-12.5.1>,
        <https://par-tec.github.io/security-ontologies/onto/iso#27001/2013/control-12.6.2> ;
    iso:hasControlType iso:Preventive ;
    iso:hasCybersecurityConcept iso:Protect ;
    iso:hasInformationSecurityProperty iso:Availability,
        iso:Confidentiality,
        iso:Integrity ;
    iso:hasOperationalCapability iso:SecureConfiguration ;
    iso:hasRelatedControls <https://par-tec.github.io/security-ontologies/onto/iso#27002/2022/control-5.22>,
        <https://par-tec.github.io/security-ontologies/onto/iso#27002/2022/control-8.19>,
        <https://par-tec.github.io/security-ontologies/onto/iso#27002/2022/control-8.29>,
        <https://par-tec.github.io/security-ontologies/onto/iso#27002/2022/control-8.31>,
        <https://par-tec.github.io/security-ontologies/onto/iso#27002/2022/control-8.5>,
        <https://par-tec.github.io/security-ontologies/onto/iso#27002/2022/control-8.8> ;
    iso:hasSecurityDomain iso:Protection ;
    iso:purpose "To ensure the integrity of operational systems and prevent exploitation of technical vulnerabilities" .

<https://par-tec.github.io/security-ontologies/onto/iso#27002/2022/control-8.20> a iso:Control ;
    dcterms:description "Networks should be managed and controlled to protect information in systems and applications" ;
    dcterms:identifier "27002/2022/control-8.20" ;
    dcterms:title " Network controls" ;
    iso:controlCategory iso:category-8 ;
    iso:correspondsTo <https://par-tec.github.io/security-ontologies/onto/iso#27001/2013/control-13.1.1> ;
    iso:hasControlType iso:Detective,
        iso:Preventive ;
    iso:hasCybersecurityConcept iso:Detect,
        iso:Protect ;
    iso:hasInformationSecurityProperty iso:Availability,
        iso:Confidentiality,
        iso:Integrity ;
    iso:hasOperationalCapability iso:SystemNetworkSecurity ;
    iso:hasRelatedControls <https://par-tec.github.io/security-ontologies/onto/iso#27002/2022/control-5.14>,
        <https://par-tec.github.io/security-ontologies/onto/iso#27002/2022/control-5.22>,
        <https://par-tec.github.io/security-ontologies/onto/iso#27002/2022/control-5.3>,
        <https://par-tec.github.io/security-ontologies/onto/iso#27002/2022/control-6.6>,
        <https://par-tec.github.io/security-ontologies/onto/iso#27002/2022/control-8.13>,
        <https://par-tec.github.io/security-ontologies/onto/iso#27002/2022/control-8.15>,
        <https://par-tec.github.io/security-ontologies/onto/iso#27002/2022/control-8.24> ;
    iso:hasSecurityDomain iso:Protection ;
    iso:purpose "To  ensure  the  protection  of  information  in  networks  and  its  supporting  information  processing facilities" .

<https://par-tec.github.io/security-ontologies/onto/iso#27002/2022/control-8.26> a iso:Control ;
    dcterms:description "Information security requirements should be identified, specified and approved when developing or acquiring applications" ;
    dcterms:identifier "27002/2022/control-8.26" ;
    dcterms:title " Application security requirements" ;
    iso:controlCategory iso:category-8 ;
    iso:correspondsTo <https://par-tec.github.io/security-ontologies/onto/iso#27001/2013/control-14.1.2>,
        <https://par-tec.github.io/security-ontologies/onto/iso#27001/2013/control-14.1.3> ;
    iso:hasControlType iso:Preventive ;
    iso:hasCybersecurityConcept iso:Protect ;
    iso:hasInformationSecurityProperty iso:Availability,
        iso:Confidentiality,
        iso:Integrity ;
    iso:hasOperationalCapability iso:ApplicationSecurity,
        iso:SystemNetworkSecurity ;
    iso:hasRelatedControls <https://par-tec.github.io/security-ontologies/onto/iso#27002/2022/control-5.17>,
        <https://par-tec.github.io/security-ontologies/onto/iso#27002/2022/control-5.31-5.36>,
        <https://par-tec.github.io/security-ontologies/onto/iso#27002/2022/control-8.2>,
        <https://par-tec.github.io/security-ontologies/onto/iso#27002/2022/control-8.24>,
        <https://par-tec.github.io/security-ontologies/onto/iso#27002/2022/control-8.5> ;
    iso:hasSecurityDomain iso:Defence,
        iso:Protection ;
    iso:purpose "To ensure all information security requirements are identified and addressed when developing or acquiring applications" .

<https://par-tec.github.io/security-ontologies/onto/iso#27002/2022/control-8.28> a iso:Control ;
    dcterms:description "Secure coding principles should be applied to software development" ;
    dcterms:identifier "27002/2022/control-8.28" ;
    dcterms:title " Secure coding" ;
    iso:controlCategory iso:category-8 ;
    iso:correspondsTo <https://par-tec.github.io/security-ontologies/onto/iso#27001/2013/control-New> ;
    iso:hasControlType iso:Preventive ;
    iso:hasCybersecurityConcept iso:Protect ;
    iso:hasInformationSecurityProperty iso:Availability,
        iso:Confidentiality,
        iso:Integrity ;
    iso:hasOperationalCapability iso:ApplicationSecurity,
        iso:SystemNetworkSecurity ;
    iso:hasRelatedControls <https://par-tec.github.io/security-ontologies/onto/iso#27002/2022/control-5.18>,
        <https://par-tec.github.io/security-ontologies/onto/iso#27002/2022/control-8.29>,
        <https://par-tec.github.io/security-ontologies/onto/iso#27002/2022/control-8.8> ;
    iso:hasSecurityDomain iso:Protection ;
    iso:purpose "To ensure software is written securely thereby reducing the number of potential information security vulnerabilities in the software" .

<https://par-tec.github.io/security-ontologies/onto/iso#27002/2022/control-8.4> a iso:Control ;
    dcterms:description "Read and write access to source code, development tools and software libraries should be appropriately managed" ;
    dcterms:identifier "27002/2022/control-8.4" ;
    dcterms:title " Access to source code" ;
    iso:controlCategory iso:category-8 ;
    iso:correspondsTo <https://par-tec.github.io/security-ontologies/onto/iso#27001/2013/control-9.4.5> ;
    iso:hasControlType iso:Preventive ;
    iso:hasCybersecurityConcept iso:Protect ;
    iso:hasInformationSecurityProperty iso:Availability,
        iso:Confidentiality,
        iso:Integrity ;
    iso:hasOperationalCapability iso:ApplicationSecurity,
        iso:IAM ;
    iso:hasRelatedControls <https://par-tec.github.io/security-ontologies/onto/iso#27002/2022/control-8.32> ;
    iso:hasSecurityDomain iso:Protection ;
    iso:purpose "To prevent the introduction of unauthorized functionality, avoid unintentional or malicious changes and to maintain the confidentiality of valuable intellectual property" .

<https://par-tec.github.io/security-ontologies/onto/iso#27002/2022/control-8.9> a iso:Control ;
    dcterms:description "Configurations, including security configurations, of hardware, software, services and networks should be established, documented, implemented, monitored and reviewed" ;
    dcterms:identifier "27002/2022/control-8.9" ;
    dcterms:title " Configuration management" ;
    iso:controlCategory iso:category-8 ;
    iso:correspondsTo <https://par-tec.github.io/security-ontologies/onto/iso#27001/2013/control-New> ;
    iso:hasControlType iso:Preventive ;
    iso:hasCybersecurityConcept iso:Protect ;
    iso:hasInformationSecurityProperty iso:Availability,
        iso:Confidentiality,
        iso:Integrity ;
    iso:hasOperationalCapability iso:SecureConfiguration ;
    iso:hasRelatedControls <https://par-tec.github.io/security-ontologies/onto/iso#27002/2022/control-5.32>,
        <https://par-tec.github.io/security-ontologies/onto/iso#27002/2022/control-8.32> ;
    iso:hasSecurityDomain iso:Protection ;
    iso:purpose "To  ensure  hardware,  software,  services  and  networks  function  correctly  with  required  security settings, and configuration is not altered by unauthorized or incorrect changes" .

iso:ControlType a owl:Class,
        skos:Concept ;
    rdfs:label "Control Type" ;
    rdfs:comment """
    Control type is an attribute to view controls from the perspective of when and how the control
    modifies the risk with regard to the occurrence of an information security incident.
    """ .

iso:InformationSecurityProperty a owl:Class,
        skos:Concept ;
    rdfs:label "Information Security Properties" ;
    rdfs:comment "Information security properties are the different properties of information." ;
    rdfs:seeAlso <https://dbpedia.org/page/Information_security> .

iso:SecureConfiguration a iso:OperationalCapability ;
    rdfs:label "Secure Configuration" ;
    rdfs:comment "Secure configuration capabilities are capabilities that secure configuration." .

<https://par-tec.github.io/security-ontologies/onto/iso#27001/2013/section-18.1> a iso:Section ;
    rdfs:label "Compliance with legal and contractual requirements" ;
    iso:controlCategory <https://par-tec.github.io/security-ontologies/onto/iso#27001/2013/category-18> .

<https://par-tec.github.io/security-ontologies/onto/iso#27001/2013/section-6.1> a iso:Section ;
    rdfs:label "Internal organization" ;
    iso:controlCategory <https://par-tec.github.io/security-ontologies/onto/iso#27001/2013/category-6> .

<https://par-tec.github.io/security-ontologies/onto/iso#27001/2013/section-9.4> a iso:Section ;
    rdfs:label "System and application access control" ;
    iso:controlCategory <https://par-tec.github.io/security-ontologies/onto/iso#27001/2013/category-9> .

<https://par-tec.github.io/security-ontologies/onto/iso#27002/2022/control-5.14> a iso:Control ;
    dcterms:description "Information transfer rules, procedures, or agreements, both within the organization and between the organization and other parties, should be in place for all types of transfer facilities" ;
    dcterms:identifier "27002/2022/control-5.14" ;
    dcterms:title " Information transfer" ;
    iso:controlCategory iso:category-5 ;
    iso:correspondsTo <https://par-tec.github.io/security-ontologies/onto/iso#27001/2013/control-13.2.1>,
        <https://par-tec.github.io/security-ontologies/onto/iso#27001/2013/control-13.2.2>,
        <https://par-tec.github.io/security-ontologies/onto/iso#27001/2013/control-13.2.3> ;
    iso:hasControlType iso:Preventive ;
    iso:hasCybersecurityConcept iso:Protect ;
    iso:hasInformationSecurityProperty iso:Availability,
        iso:Confidentiality,
        iso:Integrity ;
    iso:hasOperationalCapability iso:AssetManagement,
        iso:InformationProtection ;
    iso:hasRelatedControls <https://par-tec.github.io/security-ontologies/onto/iso#27002/2022/control-5.10>,
        <https://par-tec.github.io/security-ontologies/onto/iso#27002/2022/control-5.13>,
        <https://par-tec.github.io/security-ontologies/onto/iso#27002/2022/control-5.31>,
        <https://par-tec.github.io/security-ontologies/onto/iso#27002/2022/control-5.32>,
        <https://par-tec.github.io/security-ontologies/onto/iso#27002/2022/control-5.33>,
        <https://par-tec.github.io/security-ontologies/onto/iso#27002/2022/control-5.34>,
        <https://par-tec.github.io/security-ontologies/onto/iso#27002/2022/control-7,10>,
        <https://par-tec.github.io/security-ontologies/onto/iso#27002/2022/control-8.24>,
        <https://par-tec.github.io/security-ontologies/onto/iso#27002/2022/control-8.7> ;
    iso:hasSecurityDomain iso:Protection ;
    iso:purpose "To maintain the security of information transferred within an organization and with any external interested party" .

<https://par-tec.github.io/security-ontologies/onto/iso#27002/2022/control-5.20> a iso:Control ;
    dcterms:description "Relevant information security requirements should be established and agreed with each supplier based on the type of supplier relationship" ;
    dcterms:identifier "27002/2022/control-5.20" ;
    dcterms:title "Addressing information security within supplier agreements" ;
    iso:controlCategory iso:category-5 ;
    iso:correspondsTo <https://par-tec.github.io/security-ontologies/onto/iso#27001/2013/control-15.1.2> ;
    iso:hasControlType iso:Preventive ;
    iso:hasCybersecurityConcept iso:Identify ;
    iso:hasInformationSecurityProperty iso:Availability,
        iso:Confidentiality,
        iso:Integrity ;
    iso:hasOperationalCapability iso:SupplierSecurity ;
    iso:hasRelatedControls <https://par-tec.github.io/security-ontologies/onto/iso#27002/2022/control-5.10>,
        <https://par-tec.github.io/security-ontologies/onto/iso#27002/2022/control-5.12>,
        <https://par-tec.github.io/security-ontologies/onto/iso#27002/2022/control-5.13> ;
    iso:hasSecurityDomain iso:GovernanceEcosystem,
        iso:Protection ;
    iso:purpose "To ensure information security of the organization in supplier relationships" .

<https://par-tec.github.io/security-ontologies/onto/iso#27002/2022/control-5.24> a iso:Control ;
    dcterms:description "The organization should plan and prepare for managing information security incidents by defining, establishing and communicating information security incident management processes, roles and responsibilities" ;
    dcterms:identifier "27002/2022/control-5.24" ;
    dcterms:title "Information security incident management responsibilities and preparation" ;
    iso:controlCategory iso:category-5 ;
    iso:correspondsTo <https://par-tec.github.io/security-ontologies/onto/iso#27001/2013/control-16.1.1> ;
    iso:hasControlType iso:Corrective ;
    iso:hasCybersecurityConcept iso:Recover,
        iso:Respond ;
    iso:hasInformationSecurityProperty iso:Availability,
        iso:Confidentiality,
        iso:Integrity ;
    iso:hasOperationalCapability iso:EventManangement ;
    iso:hasRelatedControls <https://par-tec.github.io/security-ontologies/onto/iso#27002/2022/control-5.25>,
        <https://par-tec.github.io/security-ontologies/onto/iso#27002/2022/control-5.26>,
        <https://par-tec.github.io/security-ontologies/onto/iso#27002/2022/control-5.28>,
        <https://par-tec.github.io/security-ontologies/onto/iso#27002/2022/control-5.5>,
        <https://par-tec.github.io/security-ontologies/onto/iso#27002/2022/control-5.6>,
        <https://par-tec.github.io/security-ontologies/onto/iso#27002/2022/control-6.8>,
        <https://par-tec.github.io/security-ontologies/onto/iso#27002/2022/control-8.14>,
        <https://par-tec.github.io/security-ontologies/onto/iso#27002/2022/control-8.15> ;
    iso:hasSecurityDomain iso:Defence ;
    iso:purpose "To ensure quick, effective, consistent and orderly response to information security incidents, including communication on information security events" .

<https://par-tec.github.io/security-ontologies/onto/iso#27002/2022/control-5.33> a iso:Control ;
    dcterms:description "Records should be protected from loss, destruction, falsification, unauthorized access and unauthorized release, in accordance with legal, statutory, regulatory, contractual and business requirements" ;
    dcterms:identifier "27002/2022/control-5.33" ;
    dcterms:title " Protection of records" ;
    iso:controlCategory iso:category-5 ;
    iso:correspondsTo <https://par-tec.github.io/security-ontologies/onto/iso#27001/2013/control-18.1.3> ;
    iso:hasControlType iso:Preventive ;
    iso:hasCybersecurityConcept iso:Identify,
        iso:Protect ;
    iso:hasInformationSecurityProperty iso:Availability,
        iso:Confidentiality,
        iso:Integrity ;
    iso:hasOperationalCapability iso:AssetManagement,
        iso:Compliance,
        iso:InformationProtection ;
    iso:hasRelatedControls <https://par-tec.github.io/security-ontologies/onto/iso#27002/2022/control-8.24> ;
    iso:hasSecurityDomain iso:Defence ;
    iso:purpose "To ensure compliance with legal, statutory, regulatory or contractual requirements related to the protection of records" .

<https://par-tec.github.io/security-ontologies/onto/iso#27002/2022/control-6.6> a iso:Control ;
    dcterms:description "Confidentiality or non-disclosure agreements reflecting the organization’s needs for the protection of information should be identified, documented, regularly reviewed and signed by personnel and other relevant interested parties" ;
    dcterms:identifier "27002/2022/control-6.6" ;
    dcterms:title " Confidentiality or non-disclosure agreements" ;
    iso:controlCategory iso:category-6 ;
    iso:correspondsTo <https://par-tec.github.io/security-ontologies/onto/iso#27001/2013/control-13.2.4> ;
    iso:hasControlType iso:Preventive ;
    iso:hasCybersecurityConcept iso:Protect ;
    iso:hasInformationSecurityProperty iso:Confidentiality ;
    iso:hasOperationalCapability iso:HRSecurity,
        iso:InformationProtection,
        iso:SupplierSecurity ;
    iso:hasRelatedControls <https://par-tec.github.io/security-ontologies/onto/iso#27002/2022/control-5.31>,
        <https://par-tec.github.io/security-ontologies/onto/iso#27002/2022/control-5.32>,
        <https://par-tec.github.io/security-ontologies/onto/iso#27002/2022/control-5.33>,
        <https://par-tec.github.io/security-ontologies/onto/iso#27002/2022/control-5.34> ;
    iso:hasSecurityDomain iso:GovernanceEcosystem ;
    iso:purpose "To maintain confidentiality of information accessible by personnel or external parties" .

<https://par-tec.github.io/security-ontologies/onto/iso#27002/2022/control-8.10> a iso:Control ;
    dcterms:description "Information stored in information systems and devices should be deleted when no longer required" ;
    dcterms:identifier "27002/2022/control-8.10" ;
    dcterms:title "Information deletion" ;
    iso:controlCategory iso:category-8 ;
    iso:correspondsTo <https://par-tec.github.io/security-ontologies/onto/iso#27001/2013/control-New> ;
    iso:hasControlType iso:Preventive ;
    iso:hasCybersecurityConcept iso:Protect ;
    iso:hasInformationSecurityProperty iso:Confidentiality ;
    iso:hasOperationalCapability iso:InformationProtection ;
    iso:hasRelatedControls <https://par-tec.github.io/security-ontologies/onto/iso#27002/2022/control-7.14> ;
    iso:hasSecurityDomain iso:Protection ;
    iso:purpose "To  prevent  unnecessary  exposure  of  sensitive  information  and  to  comply  with  legal,  statutory, regulatory and contractual requirements for data deletion" .

<https://par-tec.github.io/security-ontologies/onto/iso#27002/2022/control-8.2> a iso:Control ;
    dcterms:description "The allocation and use of privileged access rights should be restricted and managed" ;
    dcterms:identifier "27002/2022/control-8.2" ;
    dcterms:title " Privileged access rights" ;
    iso:controlCategory iso:category-8 ;
    iso:correspondsTo <https://par-tec.github.io/security-ontologies/onto/iso#27001/2013/control-9.2.3> ;
    iso:hasControlType iso:Preventive ;
    iso:hasCybersecurityConcept iso:Protect ;
    iso:hasInformationSecurityProperty iso:Availability,
        iso:Confidentiality,
        iso:Integrity ;
    iso:hasOperationalCapability iso:IAM ;
    iso:hasRelatedControls <https://par-tec.github.io/security-ontologies/onto/iso#27002/2022/control-5.15>,
        <https://par-tec.github.io/security-ontologies/onto/iso#27002/2022/control-5.17>,
        <https://par-tec.github.io/security-ontologies/onto/iso#27002/2022/control-5.18> ;
    iso:hasSecurityDomain iso:Protection ;
    iso:purpose "To ensure only authorized users, software components and services are provided with privileged access rights" .

<https://par-tec.github.io/security-ontologies/onto/iso#27002/2022/control-8.5> a iso:Control ;
    dcterms:description "Secure  authentication  technologies  and  procedures  should  be  implemented  based  on  information access restrictions and the topic-specific policy on access control" ;
    dcterms:identifier "27002/2022/control-8.5" ;
    dcterms:title " Secure authentication" ;
    iso:controlCategory iso:category-8 ;
    iso:correspondsTo <https://par-tec.github.io/security-ontologies/onto/iso#27001/2013/control-9.4.2> ;
    iso:hasControlType iso:Preventive ;
    iso:hasCybersecurityConcept iso:Protect ;
    iso:hasInformationSecurityProperty iso:Availability,
        iso:Confidentiality,
        iso:Integrity ;
    iso:hasOperationalCapability iso:IAM ;
    iso:hasSecurityDomain iso:Protection ;
    iso:purpose "To ensure a user or an entity is securely authenticated when access to systems, applications, and services is granted" .

<https://par-tec.github.io/security-ontologies/onto/iso#27002/2022/control-8.8> a iso:Control ;
    dcterms:description "Information about technical vulnerabilities of information systems in use should be obtained, the organization’s exposure to such vulnerabilities should be evaluated and appropriate measures should be taken" ;
    dcterms:identifier "27002/2022/control-8.8" ;
    dcterms:title " Management of technical vulnerabilities" ;
    iso:controlCategory iso:category-8 ;
    iso:correspondsTo <https://par-tec.github.io/security-ontologies/onto/iso#27001/2013/control-12.6.1>,
        <https://par-tec.github.io/security-ontologies/onto/iso#27001/2013/control-18.2.3> ;
    iso:hasControlType iso:Preventive ;
    iso:hasCybersecurityConcept iso:Protect ;
    iso:hasInformationSecurityProperty iso:Availability,
        iso:Confidentiality,
        iso:Integrity ;
    iso:hasOperationalCapability iso:ThreatManagement ;
    iso:hasRelatedControls <https://par-tec.github.io/security-ontologies/onto/iso#27002/2022/control-5.14>,
        <https://par-tec.github.io/security-ontologies/onto/iso#27002/2022/control-5.20>,
        <https://par-tec.github.io/security-ontologies/onto/iso#27002/2022/control-5.23>,
        <https://par-tec.github.io/security-ontologies/onto/iso#27002/2022/control-5.26>,
        <https://par-tec.github.io/security-ontologies/onto/iso#27002/2022/control-5.9>,
        <https://par-tec.github.io/security-ontologies/onto/iso#27002/2022/control-8.20>,
        <https://par-tec.github.io/security-ontologies/onto/iso#27002/2022/control-8.23>,
        <https://par-tec.github.io/security-ontologies/onto/iso#27002/2022/control-8.25>,
        <https://par-tec.github.io/security-ontologies/onto/iso#27002/2022/control-8.28>,
        <https://par-tec.github.io/security-ontologies/onto/iso#27002/2022/control-8.29>,
        <https://par-tec.github.io/security-ontologies/onto/iso#27002/2022/control-8.32> ;
    iso:hasSecurityDomain iso:Defence,
        iso:GovernanceEcosystem,
        iso:Protection ;
    iso:purpose "To prevent exploitation of technical vulnerabilities" .

iso:Compliance a iso:OperationalCapability ;
    rdfs:label "Legal andCompliance" ;
    rdfs:comment "Compliance capabilities are capabilities that manage compliance." .

iso:Recover a iso:CybersecurityConcept ;
    rdfs:label "Recover" ;
    rdfs:comment "Recover concepts are concepts that recover information." .

iso:SecurityDomain a owl:Class,
        skos:Concept ;
    rdfs:label "Security Domains" ;
    rdfs:comment "Security domains are the different domains that can be used in the ISO 27001 standard." .

<https://par-tec.github.io/security-ontologies/onto/iso#27001/2013/section-11.1> a iso:Section ;
    rdfs:label "Secure areas" ;
    iso:controlCategory <https://par-tec.github.io/security-ontologies/onto/iso#27001/2013/category-11> .

<https://par-tec.github.io/security-ontologies/onto/iso#27001/2013/section-9.2> a iso:Section ;
    rdfs:label "User access management" ;
    iso:controlCategory <https://par-tec.github.io/security-ontologies/onto/iso#27001/2013/category-9> .

<https://par-tec.github.io/security-ontologies/onto/iso#27002/2022/control-5.22> a iso:Control ;
    dcterms:description "The organization should regularly monitor, review, evaluate and manage change in supplier information security practices and service delivery" ;
    dcterms:identifier "27002/2022/control-5.22" ;
    dcterms:title "Monitoring, review and change management of supplier services" ;
    iso:controlCategory iso:category-5 ;
    iso:correspondsTo <https://par-tec.github.io/security-ontologies/onto/iso#27001/2013/control-15.2.1>,
        <https://par-tec.github.io/security-ontologies/onto/iso#27001/2013/control-15.2.2> ;
    iso:hasControlType iso:Preventive ;
    iso:hasCybersecurityConcept iso:Identify ;
    iso:hasInformationSecurityProperty iso:Availability,
        iso:Confidentiality,
        iso:Integrity ;
    iso:hasOperationalCapability iso:SupplierSecurity ;
    iso:hasRelatedControls <https://par-tec.github.io/security-ontologies/onto/iso#27002/2022/control-5.29>,
        <https://par-tec.github.io/security-ontologies/onto/iso#27002/2022/control-5.35>,
        <https://par-tec.github.io/security-ontologies/onto/iso#27002/2022/control-5.36>,
        <https://par-tec.github.io/security-ontologies/onto/iso#27002/2022/control-8.14> ;
    iso:hasSecurityDomain iso:Defence,
        iso:GovernanceEcosystem,
        iso:Protection ;
    iso:purpose "To  maintain  an  agreed  level  of  information  security  and  service  delivery  in  line  with  supplier agreements" .

<https://par-tec.github.io/security-ontologies/onto/iso#27002/2022/control-5.26> a iso:Control ;
    dcterms:description "Information security incidents should be responded to in accordance with the documented procedures" ;
    dcterms:identifier "27002/2022/control-5.26" ;
    dcterms:title "Response to information security incidents" ;
    iso:controlCategory iso:category-5 ;
    iso:correspondsTo <https://par-tec.github.io/security-ontologies/onto/iso#27001/2013/control-16.1.5> ;
    iso:hasControlType iso:Corrective ;
    iso:hasCybersecurityConcept iso:Recover,
        iso:Respond ;
    iso:hasInformationSecurityProperty iso:Availability,
        iso:Confidentiality,
        iso:Integrity ;
    iso:hasOperationalCapability iso:EventManangement ;
    iso:hasRelatedControls <https://par-tec.github.io/security-ontologies/onto/iso#27002/2022/control-5.24>,
        <https://par-tec.github.io/security-ontologies/onto/iso#27002/2022/control-5.27>,
        <https://par-tec.github.io/security-ontologies/onto/iso#27002/2022/control-5.28>,
        <https://par-tec.github.io/security-ontologies/onto/iso#27002/2022/control-5.29>,
        <https://par-tec.github.io/security-ontologies/onto/iso#27002/2022/control-5.30> ;
    iso:hasSecurityDomain iso:Defence ;
    iso:purpose "To ensure efficient and effective response to information security incidents" .

<https://par-tec.github.io/security-ontologies/onto/iso#27002/2022/control-5.29> a iso:Control ;
    dcterms:description "The organization should plan how to maintain information security at an appropriate level during disruption" ;
    dcterms:identifier "27002/2022/control-5.29" ;
    dcterms:title "Information security during disruption" ;
    iso:controlCategory iso:category-5 ;
    iso:correspondsTo <https://par-tec.github.io/security-ontologies/onto/iso#27001/2013/control-17.1.1>,
        <https://par-tec.github.io/security-ontologies/onto/iso#27001/2013/control-17.1.2>,
        <https://par-tec.github.io/security-ontologies/onto/iso#27001/2013/control-17.1.3> ;
    iso:hasControlType iso:Preventive ;
    iso:hasCybersecurityConcept iso:Protect ;
    iso:hasInformationSecurityProperty iso:Availability,
        iso:Confidentiality,
        iso:Integrity ;
    iso:hasOperationalCapability iso:Continuity ;
    iso:hasSecurityDomain iso:Protection,
        iso:Resilience ;
    iso:purpose "To provide information and other associated asset with adequate protection during disruption" .

<https://par-tec.github.io/security-ontologies/onto/iso#27002/2022/control-5.30> a iso:Control ;
    dcterms:description "ICT readiness should be planned, implemented, maintained and tested based on business continuity objectives and ICT continuity requirements" ;
    dcterms:identifier "27002/2022/control-5.30" ;
    dcterms:title "ICT readiness for business continuity" ;
    iso:controlCategory iso:category-5 ;
    iso:correspondsTo <https://par-tec.github.io/security-ontologies/onto/iso#27001/2013/control-New> ;
    iso:hasControlType iso:Corrective ;
    iso:hasCybersecurityConcept iso:Protect,
        iso:Respond ;
    iso:hasInformationSecurityProperty iso:Availability ;
    iso:hasOperationalCapability iso:Continuity ;
    iso:hasSecurityDomain iso:Resilience ;
    iso:purpose "To ensure the availability of the organization’s information and other associated assets in the event of a disruption" .

<https://par-tec.github.io/security-ontologies/onto/iso#27002/2022/control-5.31> a iso:Control ;
    dcterms:description "Information  security  relevant  legal,  statutory,  regulatory  and  contractual  requirements  and  the organization’s approach to meet these requirements should be identified, documented and kept up to date" ;
    dcterms:identifier "27002/2022/control-5.31" ;
    dcterms:title "Identification of legal, statutory, regulatory and contractual requirements" ;
    iso:controlCategory iso:category-5 ;
    iso:correspondsTo <https://par-tec.github.io/security-ontologies/onto/iso#27001/2013/control-18.1.1>,
        <https://par-tec.github.io/security-ontologies/onto/iso#27001/2013/control-18.1.5> ;
    iso:hasControlType iso:Preventive ;
    iso:hasCybersecurityConcept iso:Identify ;
    iso:hasInformationSecurityProperty iso:Availability,
        iso:Confidentiality,
        iso:Integrity ;
    iso:hasOperationalCapability iso:Compliance ;
    iso:hasRelatedControls <https://par-tec.github.io/security-ontologies/onto/iso#27002/2022/control-5.20> ;
    iso:hasSecurityDomain iso:GovernanceEcosystem,
        iso:Protection ;
    iso:purpose "To  ensure  compliance  with  legal,  statutory,  regulatory  or  contractual  requirements  related  to information security" .

<https://par-tec.github.io/security-ontologies/onto/iso#27002/2022/control-5.34> a iso:Control ;
    dcterms:description "The organization should identify and meet the requirements regarding preservation of privacy and protection of PII according to applicable laws and regulations and contractual requirements" ;
    dcterms:identifier "27002/2022/control-5.34" ;
    dcterms:title " Privacy and protection of PII" ;
    iso:controlCategory iso:category-5 ;
    iso:correspondsTo <https://par-tec.github.io/security-ontologies/onto/iso#27001/2013/control-18.1.4> ;
    iso:hasControlType iso:Preventive ;
    iso:hasCybersecurityConcept iso:Identify,
        iso:Protect ;
    iso:hasInformationSecurityProperty iso:Availability,
        iso:Confidentiality,
        iso:Integrity ;
    iso:hasOperationalCapability iso:Compliance,
        iso:InformationProtection ;
    iso:hasSecurityDomain iso:Protection ;
    iso:purpose "To ensure compliance with legal, statutory, regulatory or contractual requirements related to the information security aspects of the protection of PII" .

<https://par-tec.github.io/security-ontologies/onto/iso#27002/2022/control-5.9> a iso:Control ;
    dcterms:description """An inventory of information and other associated assets, including owners, should be developed and
maintained
""" ;
    dcterms:identifier "27002/2022/control-5.9" ;
    dcterms:title "Inventory of information and other associated assets" ;
    iso:controlCategory iso:category-5 ;
    iso:correspondsTo <https://par-tec.github.io/security-ontologies/onto/iso#27001/2013/control-8.1.1>,
        <https://par-tec.github.io/security-ontologies/onto/iso#27001/2013/control-8.1.2> ;
    iso:hasControlType iso:Preventive ;
    iso:hasCybersecurityConcept iso:Identify ;
    iso:hasInformationSecurityProperty iso:Availability,
        iso:Confidentiality,
        iso:Integrity ;
    iso:hasOperationalCapability iso:AssetManagement ;
    iso:hasRelatedControls <https://par-tec.github.io/security-ontologies/onto/iso#27002/2022/control-5.10>,
        <https://par-tec.github.io/security-ontologies/onto/iso#27002/2022/control-5.12>,
        <https://par-tec.github.io/security-ontologies/onto/iso#27002/2022/control-5.13> ;
    iso:hasSecurityDomain iso:GovernanceEcosystem,
        iso:Protection ;
    iso:purpose "To identify the organization's information and other associated assets in order to preserve their information security and assign appropriate ownership" .

<https://par-tec.github.io/security-ontologies/onto/iso#27002/2022/control-7.14> a iso:Control ;
    dcterms:description "Items of equipment containing storage media should be verified to ensure that any sensitive data and licensed software has been removed or securely overwritten prior to disposal or re-use" ;
    dcterms:identifier "27002/2022/control-7.14" ;
    dcterms:title "Secure disposal or re-use of equipment" ;
    iso:controlCategory iso:category-7 ;
    iso:correspondsTo <https://par-tec.github.io/security-ontologies/onto/iso#27001/2013/control-11.2.7> ;
    iso:hasControlType iso:Preventive ;
    iso:hasCybersecurityConcept iso:Protect ;
    iso:hasInformationSecurityProperty iso:Confidentiality ;
    iso:hasOperationalCapability iso:AssetManagement,
        iso:PhysicalSecurity ;
    iso:hasRelatedControls <https://par-tec.github.io/security-ontologies/onto/iso#27002/2022/control-7.10>,
        <https://par-tec.github.io/security-ontologies/onto/iso#27002/2022/control-8.10>,
        <https://par-tec.github.io/security-ontologies/onto/iso#27002/2022/control-8.24> ;
    iso:hasSecurityDomain iso:Protection ;
    iso:purpose "To prevent leakage of information from equipment to be disposed or re-used" .

iso:Continuity a iso:OperationalCapability ;
    rdfs:label "Continuity" ;
    rdfs:comment "Continuity capabilities are capabilities that manage continuity." .

iso:CybersecurityConcept a owl:Class,
        skos:Concept ;
    rdfs:label "Cybersecurity Concepts" ;
    rdfs:comment """Cybersecurity frameworks based on ISO/IEC TS 27110
        provide a way to organize and communicate
        cybersecurity activities through 5 concepts:
        Identify, Protect, Detect, Respond, and Recover.""" ;
    rdfs:seeAlso <https://www.nist.gov/cyberframework> .

iso:HRSecurity a iso:OperationalCapability ;
    rdfs:label "Human Resources Security" ;
    rdfs:comment "Human resources security capabilities are capabilities that protect human resources." .

<https://par-tec.github.io/security-ontologies/onto/iso#27001/2013/category-12> a iso:ControlCategory ;
    rdfs:label "Operations security" .

<https://par-tec.github.io/security-ontologies/onto/iso#27001/2013/section-16.1> a iso:Section ;
    rdfs:label "Management of information security incidents and improvements" ;
    iso:controlCategory <https://par-tec.github.io/security-ontologies/onto/iso#27001/2013/category-16> .

<https://par-tec.github.io/security-ontologies/onto/iso#27002/2022/control-5.10> a iso:Control ;
    dcterms:description "Rules for the acceptable use and procedures for the handling of information and other associated assets should be identified, documented and implemented" ;
    dcterms:identifier "27002/2022/control-5.10" ;
    dcterms:title "Acceptable use of information and associated assets" ;
    iso:controlCategory iso:category-5 ;
    iso:correspondsTo <https://par-tec.github.io/security-ontologies/onto/iso#27001/2013/control-8.1.3>,
        <https://par-tec.github.io/security-ontologies/onto/iso#27001/2013/control-8.2.3> ;
    iso:hasControlType iso:Preventive ;
    iso:hasCybersecurityConcept iso:Protect ;
    iso:hasInformationSecurityProperty iso:Availability,
        iso:Confidentiality,
        iso:Integrity ;
    iso:hasOperationalCapability iso:AssetManagement,
        iso:InformationProtection ;
    iso:hasRelatedControls <https://par-tec.github.io/security-ontologies/onto/iso#27002/2022/control-5.12>,
        <https://par-tec.github.io/security-ontologies/onto/iso#27002/2022/control-7.10>,
        <https://par-tec.github.io/security-ontologies/onto/iso#27002/2022/control-7.8> ;
    iso:hasSecurityDomain iso:GovernanceEcosystem,
        iso:Protection ;
    iso:purpose "To ensure information and other associated assets are appropriately protected, used and handled" .

<https://par-tec.github.io/security-ontologies/onto/iso#27002/2022/control-5.13> a iso:Control ;
    dcterms:description "An appropriate set of procedures for information labelling should be developed and implemented in accordance with the information classification scheme adopted by the organization" ;
    dcterms:identifier "27002/2022/control-5.13" ;
    dcterms:title " Labelling of information" ;
    iso:controlCategory iso:category-5 ;
    iso:correspondsTo <https://par-tec.github.io/security-ontologies/onto/iso#27001/2013/control-8.2.2> ;
    iso:hasControlType iso:Preventive ;
    iso:hasCybersecurityConcept iso:Protect ;
    iso:hasInformationSecurityProperty iso:Availability,
        iso:Confidentiality,
        iso:Integrity ;
    iso:hasOperationalCapability iso:InformationProtection ;
    iso:hasRelatedControls <https://par-tec.github.io/security-ontologies/onto/iso#27002/2022/control-5.12> ;
    iso:hasSecurityDomain iso:Defence ;
    iso:purpose "To facilitate the communication of classification of information and support automation of information processing and management" .

<https://par-tec.github.io/security-ontologies/onto/iso#27002/2022/control-5.25> a iso:Control ;
    dcterms:description "The organization should assess information security events and decide if they are to be categorized as information security incidents" ;
    dcterms:identifier "27002/2022/control-5.25" ;
    dcterms:title "Assessment and decision on information security events" ;
    iso:controlCategory iso:category-5 ;
    iso:correspondsTo <https://par-tec.github.io/security-ontologies/onto/iso#27001/2013/control-16.1.4> ;
    iso:hasControlType iso:Detective ;
    iso:hasCybersecurityConcept iso:Detect,
        iso:Respond ;
    iso:hasInformationSecurityProperty iso:Availability,
        iso:Confidentiality,
        iso:Integrity ;
    iso:hasOperationalCapability iso:EventManangement ;
    iso:hasSecurityDomain iso:Defence ;
    iso:purpose "To ensure effective categorization and prioritization of information security events" .

<https://par-tec.github.io/security-ontologies/onto/iso#27002/2022/control-5.28> a iso:Control ;
    dcterms:description "The organization should establish and implement procedures for the identification, collection, acquisition and preservation of information from information security incidents" ;
    dcterms:identifier "27002/2022/control-5.28" ;
    dcterms:title " Collection of evidence" ;
    iso:controlCategory iso:category-5 ;
    iso:correspondsTo <https://par-tec.github.io/security-ontologies/onto/iso#27001/2013/control-16.1.7> ;
    iso:hasControlType iso:Corrective,
        iso:Detective ;
    iso:hasCybersecurityConcept iso:Detect,
        iso:Respond ;
    iso:hasInformationSecurityProperty iso:Availability,
        iso:Confidentiality,
        iso:Integrity ;
    iso:hasOperationalCapability iso:EventManangement ;
    iso:hasSecurityDomain iso:Defence ;
    iso:purpose "To ensure a consistent and effective management of evidence related to information security incidents for the purposes of disciplinary and legal action" .

<https://par-tec.github.io/security-ontologies/onto/iso#27002/2022/control-7.10> a iso:Control ;
    dcterms:description "Storage media should be managed through its lifecycle of acquisition, use, transportation and disposal in accordance with the organization’s classification scheme and handling requirements" ;
    dcterms:identifier "27002/2022/control-7.10" ;
    dcterms:title " Storage media" ;
    iso:controlCategory iso:category-7 ;
    iso:correspondsTo <https://par-tec.github.io/security-ontologies/onto/iso#27001/2013/control-8.3.1>,
        <https://par-tec.github.io/security-ontologies/onto/iso#27001/2013/control-8.3.2>,
        <https://par-tec.github.io/security-ontologies/onto/iso#27001/2013/control-8.3.3> ;
    iso:hasControlType iso:Preventive ;
    iso:hasCybersecurityConcept iso:Protect ;
    iso:hasInformationSecurityProperty iso:Availability,
        iso:Confidentiality,
        iso:Integrity ;
    iso:hasOperationalCapability iso:AssetManagement,
        iso:PhysicalSecurity ;
    iso:hasRelatedControls <https://par-tec.github.io/security-ontologies/onto/iso#27002/2022/control-7.14>,
        <https://par-tec.github.io/security-ontologies/onto/iso#27002/2022/control-8.10> ;
    iso:hasSecurityDomain iso:Protection ;
    iso:purpose "To ensure only authorized disclosure, modification, removal or destruction of information stored on media" .

iso:Governance a iso:OperationalCapability ;
    rdfs:label "Governance" ;
    rdfs:comment "Governance capabilities are capabilities that govern the operation of information systems." .

iso:SupplierSecurity a iso:OperationalCapability ;
    rdfs:label "Supplier and Relationship Security" ;
    rdfs:comment "Supplier security capabilities are capabilities that manage supplier assets." .

<https://par-tec.github.io/security-ontologies/onto/iso#27002/2022/control-5.15> a iso:Control ;
    dcterms:description "Rules to control physical and logical access to information and other associated assets should be established and implemented based on business and information security requirements" ;
    dcterms:identifier "27002/2022/control-5.15" ;
    dcterms:title " Access control" ;
    iso:controlCategory iso:category-5 ;
    iso:correspondsTo <https://par-tec.github.io/security-ontologies/onto/iso#27001/2013/control-9.1.1>,
        <https://par-tec.github.io/security-ontologies/onto/iso#27001/2013/control-9.1.2> ;
    iso:hasControlType iso:Preventive ;
    iso:hasCybersecurityConcept iso:Protect ;
    iso:hasInformationSecurityProperty iso:Availability,
        iso:Confidentiality,
        iso:Integrity ;
    iso:hasOperationalCapability iso:IAM ;
    iso:hasRelatedControls <https://par-tec.github.io/security-ontologies/onto/iso#27002/2022/control-5.10>,
        <https://par-tec.github.io/security-ontologies/onto/iso#27002/2022/control-5.12>,
        <https://par-tec.github.io/security-ontologies/onto/iso#27002/2022/control-5.13>,
        <https://par-tec.github.io/security-ontologies/onto/iso#27002/2022/control-5.16>,
        <https://par-tec.github.io/security-ontologies/onto/iso#27002/2022/control-5.17>,
        <https://par-tec.github.io/security-ontologies/onto/iso#27002/2022/control-5.18>,
        <https://par-tec.github.io/security-ontologies/onto/iso#27002/2022/control-5.2>,
        <https://par-tec.github.io/security-ontologies/onto/iso#27002/2022/control-5.3>,
        <https://par-tec.github.io/security-ontologies/onto/iso#27002/2022/control-5.31>,
        <https://par-tec.github.io/security-ontologies/onto/iso#27002/2022/control-5.32>,
        <https://par-tec.github.io/security-ontologies/onto/iso#27002/2022/control-5.33>,
        <https://par-tec.github.io/security-ontologies/onto/iso#27002/2022/control-5.34>,
        <https://par-tec.github.io/security-ontologies/onto/iso#27002/2022/control-7.2>,
        <https://par-tec.github.io/security-ontologies/onto/iso#27002/2022/control-7.3>,
        <https://par-tec.github.io/security-ontologies/onto/iso#27002/2022/control-7.4>,
        <https://par-tec.github.io/security-ontologies/onto/iso#27002/2022/control-8.15>,
        <https://par-tec.github.io/security-ontologies/onto/iso#27002/2022/control-8.18>,
        <https://par-tec.github.io/security-ontologies/onto/iso#27002/2022/control-8.2>,
        <https://par-tec.github.io/security-ontologies/onto/iso#27002/2022/control-8.26>,
        <https://par-tec.github.io/security-ontologies/onto/iso#27002/2022/control-8.3>,
        <https://par-tec.github.io/security-ontologies/onto/iso#27002/2022/control-8.4>,
        <https://par-tec.github.io/security-ontologies/onto/iso#27002/2022/control-8.5> ;
    iso:hasSecurityDomain iso:Protection ;
    iso:purpose "To  ensure  authorized  access  and  to  prevent  unauthorized  access  to  information  and  other associated assets" .

<https://par-tec.github.io/security-ontologies/onto/iso#27002/2022/control-8.15> a iso:Control ;
    dcterms:description "Logs that record activities, exceptions, faults and other relevant events should be produced, protected, stored and analysed" ;
    dcterms:identifier "27002/2022/control-8.15" ;
    dcterms:title " Logging" ;
    iso:controlCategory iso:category-8 ;
    iso:correspondsTo <https://par-tec.github.io/security-ontologies/onto/iso#27001/2013/control-12.4.1>,
        <https://par-tec.github.io/security-ontologies/onto/iso#27001/2013/control-12.4.2>,
        <https://par-tec.github.io/security-ontologies/onto/iso#27001/2013/control-12.4.3> ;
    iso:hasControlType iso:Detective ;
    iso:hasCybersecurityConcept iso:Detect ;
    iso:hasInformationSecurityProperty iso:Availability,
        iso:Confidentiality,
        iso:Integrity ;
    iso:hasOperationalCapability iso:EventManangement ;
    iso:hasRelatedControls <https://par-tec.github.io/security-ontologies/onto/iso#27002/2022/control-5.25>,
        <https://par-tec.github.io/security-ontologies/onto/iso#27002/2022/control-5.28>,
        <https://par-tec.github.io/security-ontologies/onto/iso#27002/2022/control-5.34>,
        <https://par-tec.github.io/security-ontologies/onto/iso#27002/2022/control-8.11>,
        <https://par-tec.github.io/security-ontologies/onto/iso#27002/2022/control-8.16>,
        <https://par-tec.github.io/security-ontologies/onto/iso#27002/2022/control-8.17> ;
    iso:hasSecurityDomain iso:Defence,
        iso:Protection ;
    iso:purpose "To record events, generate evidence, ensure the integrity of log information, prevent against unauthorized access, identify information security events that can lead to an information security incident and to support investigations" .

<https://par-tec.github.io/security-ontologies/onto/iso#27002/2022/control-8.31> a iso:Control ;
    dcterms:description "Development, testing, and production environments should be separated and secured" ;
    dcterms:identifier "27002/2022/control-8.31" ;
    dcterms:title "Separation of development, test and production environments" ;
    iso:controlCategory iso:category-8 ;
    iso:correspondsTo <https://par-tec.github.io/security-ontologies/onto/iso#27001/2013/control-12.1.4>,
        <https://par-tec.github.io/security-ontologies/onto/iso#27001/2013/control-14.2.6> ;
    iso:hasControlType iso:Preventive ;
    iso:hasCybersecurityConcept iso:Protect ;
    iso:hasInformationSecurityProperty iso:Availability,
        iso:Confidentiality,
        iso:Integrity ;
    iso:hasOperationalCapability iso:ApplicationSecurity,
        iso:SystemNetworkSecurity ;
    iso:hasRelatedControls <https://par-tec.github.io/security-ontologies/onto/iso#27002/2022/control-8.29>,
        <https://par-tec.github.io/security-ontologies/onto/iso#27002/2022/control-8.33> ;
    iso:hasSecurityDomain iso:Protection ;
    iso:purpose "To protect the production environment and data from compromise by development and test activities" .

iso:IAM a iso:OperationalCapability ;
    rdfs:label "Identity and Access Management" ;
    rdfs:comment "Identity and access management capabilities are capabilities that manage identities and access." .

iso:Resilience a iso:SecurityDomain ;
    rdfs:label "Resilience and Recovery" ;
    rdfs:comment "Resilience and Recovery domain are domains that manage resilience." .

iso:category-6 a iso:ControlCategory ;
    rdfs:label "People" .

<https://par-tec.github.io/security-ontologies/onto/iso#27001/2013/section-11.2> a iso:Section ;
    rdfs:label "Equipment" ;
    iso:controlCategory <https://par-tec.github.io/security-ontologies/onto/iso#27001/2013/category-11> .

<https://par-tec.github.io/security-ontologies/onto/iso#27001/2013/section-14.2> a iso:Section ;
    rdfs:label "Security in development and support processes" ;
    iso:controlCategory <https://par-tec.github.io/security-ontologies/onto/iso#27001/2013/category-14> .

<https://par-tec.github.io/security-ontologies/onto/iso#27002/2022/control-5.12> a iso:Control ;
    dcterms:description "Information should be classified according to the information security needs of the organization based on confidentiality, integrity, availability and relevant interested party requirements" ;
    dcterms:identifier "27002/2022/control-5.12" ;
    dcterms:title " Classification of information" ;
    iso:controlCategory iso:category-5 ;
    iso:correspondsTo <https://par-tec.github.io/security-ontologies/onto/iso#27001/2013/control-8.2.1> ;
    iso:hasControlType iso:Preventive ;
    iso:hasCybersecurityConcept iso:Identify ;
    iso:hasInformationSecurityProperty iso:Availability,
        iso:Confidentiality,
        iso:Integrity ;
    iso:hasOperationalCapability iso:InformationProtection ;
    iso:hasRelatedControls <https://par-tec.github.io/security-ontologies/onto/iso#27002/2022/control-5.15> ;
    iso:hasSecurityDomain iso:Defence,
        iso:Protection ;
    iso:purpose "To ensure identification and understanding of protection needs of information in accordance with its importance to the organization" .

<https://par-tec.github.io/security-ontologies/onto/iso#27002/2022/control-5.17> a iso:Control ;
    dcterms:description "Allocation  and  management  of  authentication  information  should  be  controlled  by  a  management process, including advising personnel of appropriate handling of authentication information" ;
    dcterms:identifier "27002/2022/control-5.17" ;
    dcterms:title " Authentication information" ;
    iso:controlCategory iso:category-5 ;
    iso:correspondsTo <https://par-tec.github.io/security-ontologies/onto/iso#27001/2013/control-9.2.4>,
        <https://par-tec.github.io/security-ontologies/onto/iso#27001/2013/control-9.3.1>,
        <https://par-tec.github.io/security-ontologies/onto/iso#27001/2013/control-9.4.3> ;
    iso:hasControlType iso:Preventive ;
    iso:hasCybersecurityConcept iso:Protect ;
    iso:hasInformationSecurityProperty iso:Availability,
        iso:Confidentiality,
        iso:Integrity ;
    iso:hasOperationalCapability iso:IAM ;
    iso:hasRelatedControls <https://par-tec.github.io/security-ontologies/onto/iso#27002/2022/control-6.2>,
        <https://par-tec.github.io/security-ontologies/onto/iso#27002/2022/control-8.24> ;
    iso:hasSecurityDomain iso:GovernanceEcosystem,
        iso:Protection ;
    iso:purpose "To ensure proper entity authentication and prevent failures of authentication processes" .

<https://par-tec.github.io/security-ontologies/onto/iso#27002/2022/control-5.18> a iso:Control ;
    dcterms:description "Access rights to information and other associated assets should be provisioned, reviewed, modified and removed in accordance with the organization’s topic-specific policy and rules on access control" ;
    dcterms:identifier "27002/2022/control-5.18" ;
    dcterms:title " Access rights" ;
    iso:controlCategory iso:category-5 ;
    iso:correspondsTo <https://par-tec.github.io/security-ontologies/onto/iso#27001/2013/control-9.2.2>,
        <https://par-tec.github.io/security-ontologies/onto/iso#27001/2013/control-9.2.5>,
        <https://par-tec.github.io/security-ontologies/onto/iso#27001/2013/control-9.2.6> ;
    iso:hasControlType iso:Preventive ;
    iso:hasInformationSecurityProperty iso:Availability,
        iso:Confidentiality,
        iso:Integrity ;
    iso:hasOperationalCapability iso:IAM ;
    iso:hasRelatedControls <https://par-tec.github.io/security-ontologies/onto/iso#27002/2022/control-5.15>,
        <https://par-tec.github.io/security-ontologies/onto/iso#27002/2022/control-5.17>,
        <https://par-tec.github.io/security-ontologies/onto/iso#27002/2022/control-5.20>,
        <https://par-tec.github.io/security-ontologies/onto/iso#27002/2022/control-5.3>,
        <https://par-tec.github.io/security-ontologies/onto/iso#27002/2022/control-5.9>,
        <https://par-tec.github.io/security-ontologies/onto/iso#27002/2022/control-6.1>,
        <https://par-tec.github.io/security-ontologies/onto/iso#27002/2022/control-6.2>,
        <https://par-tec.github.io/security-ontologies/onto/iso#27002/2022/control-6.4>,
        <https://par-tec.github.io/security-ontologies/onto/iso#27002/2022/control-6.5>,
        <https://par-tec.github.io/security-ontologies/onto/iso#27002/2022/control-6.6> ;
    iso:hasSecurityDomain iso:Protection ;
    iso:purpose "To ensure only authorized access to information and other associated assets" .

<https://par-tec.github.io/security-ontologies/onto/iso#27002/2022/control-5.32> a iso:Control ;
    dcterms:description "Organizations should implement appropriate procedures should be implemented to protect intellectual property rights" ;
    dcterms:identifier "27002/2022/control-5.32" ;
    dcterms:title "Intellectual property rights" ;
    iso:controlCategory iso:category-5 ;
    iso:correspondsTo <https://par-tec.github.io/security-ontologies/onto/iso#27001/2013/control-18.1.2> ;
    iso:hasControlType iso:Preventive ;
    iso:hasCybersecurityConcept iso:Identify ;
    iso:hasInformationSecurityProperty iso:Availability,
        iso:Confidentiality,
        iso:Integrity ;
    iso:hasOperationalCapability iso:Compliance ;
    iso:hasSecurityDomain iso:GovernanceEcosystem ;
    iso:purpose "To  ensure  compliance  with  legal,  statutory,  regulatory  and  contractual  requirements  related  to intellectual property rights and use of proprietary products" .

<https://par-tec.github.io/security-ontologies/onto/iso#27002/2022/control-8.29> a iso:Control ;
    dcterms:description "Security testing processes should be defined and implemented in the development lifecycle" ;
    dcterms:identifier "27002/2022/control-8.29" ;
    dcterms:title " Security testing in development and acceptance" ;
    iso:controlCategory iso:category-8 ;
    iso:correspondsTo <https://par-tec.github.io/security-ontologies/onto/iso#27001/2013/control-14.2.8>,
        <https://par-tec.github.io/security-ontologies/onto/iso#27001/2013/control-14.2.9> ;
    iso:hasControlType iso:Preventive ;
    iso:hasCybersecurityConcept iso:Detect ;
    iso:hasInformationSecurityProperty iso:Availability,
        iso:Confidentiality,
        iso:Integrity ;
    iso:hasOperationalCapability iso:ApplicationSecurity,
        iso:EventManangement,
        iso:SystemNetworkSecurity ;
    iso:hasRelatedControls <https://par-tec.github.io/security-ontologies/onto/iso#27002/2022/control-5.20>,
        <https://par-tec.github.io/security-ontologies/onto/iso#27002/2022/control-5.8>,
        <https://par-tec.github.io/security-ontologies/onto/iso#27002/2022/control-8.20>,
        <https://par-tec.github.io/security-ontologies/onto/iso#27002/2022/control-8.23>,
        <https://par-tec.github.io/security-ontologies/onto/iso#27002/2022/control-8.24>,
        <https://par-tec.github.io/security-ontologies/onto/iso#27002/2022/control-8.28>,
        <https://par-tec.github.io/security-ontologies/onto/iso#27002/2022/control-8.29>,
        <https://par-tec.github.io/security-ontologies/onto/iso#27002/2022/control-8.3>,
        <https://par-tec.github.io/security-ontologies/onto/iso#27002/2022/control-8.31>,
        <https://par-tec.github.io/security-ontologies/onto/iso#27002/2022/control-8.5>,
        <https://par-tec.github.io/security-ontologies/onto/iso#27002/2022/control-8.9> ;
    iso:hasSecurityDomain iso:Protection ;
    iso:purpose "To validate if information security requirements are met when deployed to the production environment" .

<https://par-tec.github.io/security-ontologies/onto/iso#27002/2022/control-8.32> a iso:Control ;
    dcterms:description "Changes to information processing facilities and information systems should be subject to change management procedures" ;
    dcterms:identifier "27002/2022/control-8.32" ;
    dcterms:title " Change management" ;
    iso:controlCategory iso:category-8 ;
    iso:correspondsTo <https://par-tec.github.io/security-ontologies/onto/iso#27001/2013/control-12.1.2>,
        <https://par-tec.github.io/security-ontologies/onto/iso#27001/2013/control-14.2.2>,
        <https://par-tec.github.io/security-ontologies/onto/iso#27001/2013/control-14.2.3>,
        <https://par-tec.github.io/security-ontologies/onto/iso#27001/2013/control-14.2.4> ;
    iso:hasControlType iso:Preventive ;
    iso:hasCybersecurityConcept iso:Protect ;
    iso:hasInformationSecurityProperty iso:Availability,
        iso:Confidentiality,
        iso:Integrity ;
    iso:hasOperationalCapability iso:ApplicationSecurity,
        iso:SystemNetworkSecurity ;
    iso:hasRelatedControls <https://par-tec.github.io/security-ontologies/onto/iso#27002/2022/control-5.30>,
        <https://par-tec.github.io/security-ontologies/onto/iso#27002/2022/control-5.37>,
        <https://par-tec.github.io/security-ontologies/onto/iso#27002/2022/control-8.29>,
        <https://par-tec.github.io/security-ontologies/onto/iso#27002/2022/control-8.31> ;
    iso:hasSecurityDomain iso:Protection ;
    iso:purpose "To preserve information security when executing changes" .

iso:ApplicationSecurity a iso:OperationalCapability ;
    rdfs:label "Application Security" ;
    rdfs:comment "Application security capabilities are capabilities that protect applications." .

iso:Respond a iso:CybersecurityConcept ;
    rdfs:label "Respond" ;
    rdfs:comment "Respond concepts are concepts that respond to information." .

<https://par-tec.github.io/security-ontologies/onto/iso#27002/2022/control-8.24> a iso:Control ;
    dcterms:description "Rules for the effective use of cryptography, including cryptographic key management, should be defined and implemented" ;
    dcterms:identifier "27002/2022/control-8.24" ;
    dcterms:title "Use of cryptography" ;
    iso:controlCategory iso:category-8 ;
    iso:correspondsTo <https://par-tec.github.io/security-ontologies/onto/iso#27001/2013/control-10.1.1>,
        <https://par-tec.github.io/security-ontologies/onto/iso#27001/2013/control-10.1.2> ;
    iso:hasControlType iso:Preventive ;
    iso:hasCybersecurityConcept iso:Protect ;
    iso:hasInformationSecurityProperty iso:Confidentiality,
        iso:Integrity ;
    iso:hasOperationalCapability iso:SecureConfiguration ;
    iso:hasRelatedControls <https://par-tec.github.io/security-ontologies/onto/iso#27002/2022/control-5.22>,
        <https://par-tec.github.io/security-ontologies/onto/iso#27002/2022/control-5.31>,
        <https://par-tec.github.io/security-ontologies/onto/iso#27002/2022/control-8.24> ;
    iso:hasSecurityDomain iso:Protection ;
    iso:purpose "To ensure proper and effective use of cryptography to protect the confidentiality, authenticity or integrity of information in compliance with legal, statutory, regulatory or contractual requirements related to cryptography" .

iso:EventManangement a iso:OperationalCapability ;
    rdfs:label "Information Security Event Management" ;
    rdfs:comment "Event management capabilities are capabilities that manage events." .

<https://par-tec.github.io/security-ontologies/onto/iso#27001/2013/control-New> iso:correspondsTo <https://par-tec.github.io/security-ontologies/onto/iso#27002/2022/control-5.23>,
        <https://par-tec.github.io/security-ontologies/onto/iso#27002/2022/control-5.30>,
        <https://par-tec.github.io/security-ontologies/onto/iso#27002/2022/control-5.7>,
        <https://par-tec.github.io/security-ontologies/onto/iso#27002/2022/control-7.4>,
        <https://par-tec.github.io/security-ontologies/onto/iso#27002/2022/control-8.10>,
        <https://par-tec.github.io/security-ontologies/onto/iso#27002/2022/control-8.11>,
        <https://par-tec.github.io/security-ontologies/onto/iso#27002/2022/control-8.12>,
        <https://par-tec.github.io/security-ontologies/onto/iso#27002/2022/control-8.16>,
        <https://par-tec.github.io/security-ontologies/onto/iso#27002/2022/control-8.22>,
        <https://par-tec.github.io/security-ontologies/onto/iso#27002/2022/control-8.28>,
        <https://par-tec.github.io/security-ontologies/onto/iso#27002/2022/control-8.9> .

iso:Corrective a iso:ControlType ;
    rdfs:label "Corrective" ;
    rdfs:comment "Corrective controls are controls after an incident." .

iso:InformationProtection a iso:OperationalCapability ;
    rdfs:label "Information Protection" ;
    rdfs:comment "Information protection capabilities are capabilities that protect information." .

iso:Detective a iso:ControlType ;
    rdfs:label "Detective" ;
    rdfs:comment "Detective controls are controls that detect an incident." .

iso:category-7 a iso:ControlCategory ;
    rdfs:label "Physical" .

iso:AssetManagement a iso:OperationalCapability ;
    rdfs:label "Asset Management" ;
    rdfs:comment "Asset management capabilities are capabilities that manage information assets." .

iso:Detect a iso:CybersecurityConcept ;
    rdfs:label "Detect" ;
    rdfs:comment "Detect concepts are concepts that detect information." .

iso:OperationalCapability a owl:Class,
        skos:Concept ;
    rdfs:label "Operational Capabilities" ;
    rdfs:comment "Operational capabilities correlate controls with the perspective of the practitioners." ;
    skos:prefLabel "Skos Operational Capabilities" .

iso:PhysicalSecurity a iso:OperationalCapability ;
    rdfs:label "Physical Security" ;
    rdfs:comment "Physical security capabilities are capabilities that protect physical assets." .

iso:SystemNetworkSecurity a iso:OperationalCapability ;
    rdfs:label "System Network Security" ;
    rdfs:comment "System network security capabilities are capabilities that protect system network assets." .

iso:Identify a iso:CybersecurityConcept ;
    rdfs:label "Identify" ;
    rdfs:comment """
    The Identify Function assists in developing an organizational understanding to managing cybersecurity risk
    to systems, people, assets, data, and capabilities.
    Understanding the business context, the resources that support critical functions,
    and the related cybersecurity risks enables an organization to focus and prioritize its efforts,
    consistent with its risk management strategy and business needs
    """ .

iso:ControlCategory a owl:Class,
        skos:Concept ;
    rdfs:label "Control Category" ;
    rdfs:comment "Control categories are the basic building blocks of the ISO 27001 standard." .

iso:Defence a iso:SecurityDomain ;
    rdfs:label "Defence and Security" ;
    rdfs:comment "Defence and Security domain are domains that protect information." .

iso:GovernanceEcosystem a iso:SecurityDomain ;
    rdfs:label "Governance and Ecosystem" ;
    rdfs:comment "Governance and Ecosystem domain are domains that govern the operation of information systems." .

iso:category-8 a iso:ControlCategory ;
    rdfs:label "Technological" .

iso:category-5 a iso:ControlCategory ;
    rdfs:label "Organizational" .

iso:Protect a iso:CybersecurityConcept ;
    rdfs:label "Protect" ;
    rdfs:comment "Protect concepts are concepts that protect information." .

iso:Protection a iso:SecurityDomain ;
    rdfs:label "Protection and Risk" ;
    rdfs:comment "Protection and Risk domain are domains that protect information." .

iso:Integrity a iso:InformationSecurityProperty ;
    rdfs:label "Integrity" ;
    rdfs:comment "Integrity of information." .

iso:Preventive a iso:ControlType ;
    rdfs:label "Preventive" ;
    rdfs:comment "Preventive controls are controls that prevent an incident." .

iso:Availability a iso:InformationSecurityProperty ;
    rdfs:label "Availability" ;
    rdfs:comment "Availability of information." .

iso:Confidentiality a iso:InformationSecurityProperty ;
    rdfs:label "Confidentiality" ;
    rdfs:comment "Confidentiality of information." .

iso:Control a owl:Class,
        skos:Concept ;
    rdfs:label "Control" ;
    rdfs:comment "Controls are the basic building blocks of the ISO 27001 standard." ;
    rdfs:subClassOf [ a owl:Restriction ;
            owl:onProperty iso:purpose ;
            owl:someValuesFrom xsd:string ] .
