@prefix d3f: <http://d3fend.mitre.org/ontologies/d3fend.owl#> .
@prefix dcterms: <http://purl.org/dc/terms/> .
@prefix iso: <http://par-tec.it/onto/iso/27001/latest/> .
@prefix iso27002_2013: <http://par-tec.it/onto/iso/27002/2013/> .
@prefix owl: <http://www.w3.org/2002/07/owl#> .
@prefix rdfs: <http://www.w3.org/2000/01/rdf-schema#> .
@prefix skos: <http://www.w3.org/2004/02/skos/core#> .
@prefix xsd: <http://www.w3.org/2001/XMLSchema#> .

iso: a owl:Ontology ;
    dcterms:creator <mailto:robipolli@gmail.com> ;
    dcterms:description "ISO27001 Controls Ontology" ;
    dcterms:license <https://creativecommons.org/licenses/by-sa/4.0/> .

iso:EcosystemCybersecurityManagement a iso:GovernanceEcosystem ;
    rdfs:label "Ecosystem Cybersecurity Management" ;
    rdfs:comment "Ecosystem cybersecurity management domain is a domain that manages ecosystem cybersecurity." .

iso:ITSecurityAdministration a iso:Protection ;
    rdfs:label "IT Security Administration" ;
    rdfs:comment "IT security administration domain is a domain that manages IT security administration." .

iso:ITSecurityArchitecture a iso:Protection ;
    rdfs:label "IT Security Architecture" ;
    rdfs:comment "IT security architecture domain is a domain that manages IT security architecture." .

iso:InformationSystemSecurityGovernance_RiskManagement a iso:GovernanceEcosystem ;
    rdfs:label "Information System Security Governance and Risk Management" ;
    rdfs:comment "Information system security governance and risk management domain is a domain that manages information system security governance and risk management." .

iso:control-5.11 a iso:Control ;
    iso:controlCategory iso:category-5 ;
    iso:correspondsTo iso27002_2013:control-08.1.4 ;
    iso:hasControlType iso:Preventive ;
    iso:hasCybersecurityConcept iso:Protect ;
    iso:hasInformationSecurityProperty iso:Availability,
        iso:Confidentiality,
        iso:Integrity ;
    iso:hasOperationalCapability iso:AssetManagement ;
    iso:hasRelatedControls iso:control-7.14,
        iso:control-8.4 ;
    iso:hasSecurityDomain iso:Protection ;
    iso:purpose "To protect the organization’s assets as part of the process of changing or terminating employment or contract" ;
    dcterms:description "Personnel and other interested parties as appropriate should return all the organization's assets in their possession upon change or termination of their employment, contract or agreement" ;
    dcterms:identifier "control-5.11" ;
    dcterms:title " Return of assets" .

iso:control-5.19 a iso:Control ;
    iso:controlCategory iso:category-5 ;
    iso:correspondsTo iso27002_2013:control-15.1.1 ;
    iso:hasControlType iso:Preventive ;
    iso:hasCybersecurityConcept iso:Identify ;
    iso:hasInformationSecurityProperty iso:Availability,
        iso:Confidentiality,
        iso:Integrity ;
    iso:hasOperationalCapability iso:SupplierSecurity ;
    iso:hasSecurityDomain iso:GovernanceEcosystem,
        iso:Protection ;
    iso:purpose "To maintain an agreed level of information security in supplier relationships" ;
    dcterms:description "Processes and procedures should be identified and implemented to manage the information security risks associated with the use of supplier's products or services" ;
    dcterms:identifier "control-5.19" ;
    dcterms:title "Information security in supplier relationships" .

iso:control-5.4 a iso:Control ;
    iso:controlCategory iso:category-5 ;
    iso:correspondsTo iso27002_2013:control-07.2.1 ;
    iso:hasControlType iso:Preventive ;
    iso:hasCybersecurityConcept iso:Identify ;
    iso:hasInformationSecurityProperty iso:Availability,
        iso:Confidentiality,
        iso:Integrity ;
    iso:hasOperationalCapability iso:Governance ;
    iso:hasRelatedControls iso:control-6.3 ;
    iso:hasSecurityDomain iso:GovernanceEcosystem ;
    iso:purpose """To ensure management understand their role in information security and undertake actions aiming to
ensure all personnel are aware of and fulfil their information security responsibilities""" ;
    dcterms:description """Management should be a role model for information security and require all personnel to apply
information security in accordance with the established information security policy, topic-specific
policies and procedures of the organization""" ;
    dcterms:identifier "control-5.4" ;
    dcterms:title "Management responsibilities" .

iso:control-7.1 a iso:Control ;
    iso:controlCategory iso:category-7 ;
    iso:correspondsTo iso27002_2013:control-11.1.1 ;
    iso:hasControlType iso:Preventive ;
    iso:hasCybersecurityConcept iso:Protect ;
    iso:hasInformationSecurityProperty iso:Availability,
        iso:Confidentiality,
        iso:Integrity ;
    iso:hasOperationalCapability iso:PhysicalSecurity ;
    iso:hasSecurityDomain iso:Protection ;
    iso:purpose "To prevent unauthorized physical access, damage and interference to the organization’s information and other associated assets" ;
    dcterms:description "Security perimeters should be defined and used to protect areas that contain either sensitive or critical information and other associated assets" ;
    dcterms:identifier "control-7.1" ;
    dcterms:title " Physical security perimeter" .

iso:control-7.11 a iso:Control ;
    iso:controlCategory iso:category-7 ;
    iso:correspondsTo iso27002_2013:control-11.2.2 ;
    iso:hasControlType iso:Detective,
        iso:Preventive ;
    iso:hasCybersecurityConcept iso:Detect,
        iso:Protect ;
    iso:hasInformationSecurityProperty iso:Availability ;
    iso:hasOperationalCapability iso:PhysicalSecurity ;
    iso:hasSecurityDomain iso:Protection ;
    iso:purpose "To prevent loss, damage or compromise of information and other associated assets due to the failure and disruption of supporting utilities or interruption to the organization’s operations" ;
    dcterms:description "Information processing facilities should be protected from power failures and other disruptions caused by failures in supporting utilities" ;
    dcterms:identifier "control-7.11" ;
    dcterms:title "Supporting utilities" .

iso:control-7.12 a iso:Control ;
    iso:controlCategory iso:category-7 ;
    iso:correspondsTo iso27002_2013:control-11.2.3 ;
    iso:hasControlType iso:Preventive ;
    iso:hasCybersecurityConcept iso:Protect ;
    iso:hasInformationSecurityProperty iso:Availability,
        iso:Confidentiality ;
    iso:hasOperationalCapability iso:PhysicalSecurity ;
    iso:hasSecurityDomain iso:Protection ;
    iso:purpose "To  prevent  loss,  damage,  theft  or  compromise  of  information  and  other  associated  assets  and interruption to the organization’s operations due to failure in power and communications cabling" ;
    dcterms:description "Cables carrying power, data or supporting information services should be protected from interception, interference or damage" ;
    dcterms:identifier "control-7.12" ;
    dcterms:title " Cabling security" .

iso:control-7.13 a iso:Control ;
    iso:controlCategory iso:category-7 ;
    iso:correspondsTo iso27002_2013:control-11.2.4 ;
    iso:hasControlType iso:Preventive ;
    iso:hasCybersecurityConcept iso:Protect ;
    iso:hasInformationSecurityProperty iso:Availability,
        iso:Confidentiality,
        iso:Integrity ;
    iso:hasOperationalCapability iso:AssetManagement,
        iso:PhysicalSecurity ;
    iso:hasRelatedControls iso:control-7.14,
        iso:control-7.9 ;
    iso:hasSecurityDomain iso:Protection,
        iso:Resilience ;
    iso:purpose "To  prevent  loss,  damage,  theft  or  compromise  of  information  and  other  associated  assets  and interruption to the organization’s operations" ;
    dcterms:description "Equipment should be maintained correctly" ;
    dcterms:identifier "control-7.13" ;
    dcterms:title " Equipment maintenance" .

iso:control-7.6 a iso:Control ;
    iso:controlCategory iso:category-7 ;
    iso:correspondsTo iso27002_2013:control-11.1.5 ;
    iso:hasControlType iso:Preventive ;
    iso:hasCybersecurityConcept iso:Protect ;
    iso:hasInformationSecurityProperty iso:Availability,
        iso:Confidentiality,
        iso:Integrity ;
    iso:hasOperationalCapability iso:PhysicalSecurity ;
    iso:hasSecurityDomain iso:Protection ;
    iso:purpose "To prevent damage and interference to the organization’s information and other associated assets in secure areas" ;
    dcterms:description "Procedures for working in secure areas should be designed and implemented" ;
    dcterms:identifier "control-7.6" ;
    dcterms:title " Working in secure areas" .

iso:control-7.7 a iso:Control ;
    iso:controlCategory iso:category-7 ;
    iso:correspondsTo iso27002_2013:control-11.2.9 ;
    iso:hasControlType iso:Preventive ;
    iso:hasCybersecurityConcept iso:Protect ;
    iso:hasInformationSecurityProperty iso:Confidentiality ;
    iso:hasOperationalCapability iso:PhysicalSecurity ;
    iso:hasSecurityDomain iso:Protection ;
    iso:purpose "To reduce the risks of unauthorized access, loss of and damage to information on the desks, screens and in other accessible locations during and outside normal working hours" ;
    dcterms:description "Clear  desk  rules  for  papers  and  removable  storage  media  and  clear  screen  rules  for  information processing facilities should be defined and enforced" ;
    dcterms:identifier "control-7.7" ;
    dcterms:title "Clear desk and clear screen" .

iso:control-8.12 a iso:Control ;
    iso:controlCategory iso:category-8 ;
    iso:correspondsTo iso27002_2013:control-New ;
    iso:hasControlType iso:Detective,
        iso:Preventive ;
    iso:hasCybersecurityConcept iso:Detect,
        iso:Protect ;
    iso:hasInformationSecurityProperty iso:Confidentiality ;
    iso:hasOperationalCapability iso:InformationProtection ;
    iso:hasRelatedControls iso:control-5.12,
        iso:control-5.15 ;
    iso:hasSecurityDomain iso:Defence,
        iso:Protection ;
    iso:purpose "To detect and prevent the unauthorized disclosure and extraction of information by individuals or systems" ;
    dcterms:description "Data leakage prevention measures should be applied to systems, networks and endpoint devices that process, store or transmit sensitive information" ;
    dcterms:identifier "control-8.12" ;
    dcterms:title "Data leakage prevention" .

iso:control-8.21 a iso:Control ;
    iso:controlCategory iso:category-8 ;
    iso:correspondsTo iso27002_2013:control-13.1.2 ;
    iso:hasControlType iso:Preventive ;
    iso:hasCybersecurityConcept iso:Protect ;
    iso:hasInformationSecurityProperty iso:Availability,
        iso:Confidentiality,
        iso:Integrity ;
    iso:hasOperationalCapability iso:SystemNetworkSecurity ;
    iso:hasSecurityDomain iso:Protection ;
    iso:purpose "To ensure security in the use of network services" ;
    dcterms:description "Security mechanisms, service levels, and service requirements of network services should be identified, implemented and monitored" ;
    dcterms:identifier "control-8.21" ;
    dcterms:title "Security of network services" .

iso:control-8.34 a iso:Control ;
    iso:controlCategory iso:category-8 ;
    iso:correspondsTo iso27002_2013:control-12.7.1 ;
    iso:hasControlType iso:Preventive ;
    iso:hasCybersecurityConcept iso:Protect ;
    iso:hasInformationSecurityProperty iso:Availability,
        iso:Integrity ;
    iso:hasOperationalCapability iso:InformationProtection,
        iso:SystemNetworkSecurity ;
    iso:hasSecurityDomain iso:GovernanceEcosystem,
        iso:Protection ;
    iso:purpose "To minimize the impact of audit and other assurance activities on operational systems and business processes" ;
    dcterms:description "Audit  tests  and  other  assurance  activities  involving  assessment  of  operational  systems  should  be planned and agreed between the tester and appropriate management" ;
    dcterms:identifier "control-8.34" ;
    dcterms:title "Protection of information systems during audit and testing" .

iso:control-8.6 a iso:Control ;
    iso:controlCategory iso:category-8 ;
    iso:correspondsTo iso27002_2013:control-12.1.3 ;
    iso:hasControlType iso:Detective,
        iso:Preventive ;
    iso:hasCybersecurityConcept iso:Detect,
        iso:Identify,
        iso:Protect ;
    iso:hasInformationSecurityProperty iso:Availability ;
    iso:hasOperationalCapability iso:Continuity ;
    iso:hasSecurityDomain iso:GovernanceEcosystem,
        iso:Protection ;
    iso:purpose "To ensure the required capacity of information processing facilities" ;
    dcterms:description "The use of resources should be monitored and adjusted in line with current and expected capacity requirements" ;
    dcterms:identifier "control-8.6" ;
    dcterms:title " Capacity management" .

iso:hasControlCategory a owl:ObjectProperty ;
    rdfs:label "hasControlCategory" ;
    rdfs:comment "The category of the control." ;
    rdfs:domain iso:Control ;
    rdfs:range iso:ControlCategory .

iso:hasControlType a owl:ObjectProperty ;
    rdfs:label "hasControlType" ;
    rdfs:comment "The type of the control." ;
    rdfs:domain iso:Control ;
    rdfs:range iso:ControlType .

iso:hasCybersecurityConcept a owl:ObjectProperty ;
    rdfs:comment "Associates an ISO Control to a NIST Cybersecurity Function." ;
    rdfs:domain iso:Control ;
    rdfs:range iso:CybersecurityConcept .

iso:hasInformationSecurityProperty a owl:ObjectProperty ;
    rdfs:label "hasInformationSecurityProperty" ;
    rdfs:comment "The information security property." ;
    rdfs:domain iso:Control ;
    rdfs:range iso:InformationSecurityProperty .

iso:hasOperationalCapability a owl:ObjectProperty ;
    rdfs:label "hasOperationalCapability" ;
    rdfs:comment "The operational capability." ;
    rdfs:domain iso:Control ;
    rdfs:range iso:OperationalCapability .

iso:hasSecurityDomain a owl:ObjectProperty ;
    rdfs:label "hasInformationSecurityProperty" ;
    rdfs:comment "The information security property of the control." ;
    rdfs:domain iso:Control ;
    rdfs:range iso:SecurityDomain .

iso:control-5.1 a iso:Control ;
    iso:controlCategory iso:category-5 ;
    iso:correspondsTo iso27002_2013:control-05.1.1,
        iso27002_2013:control-05.1.2 ;
    iso:hasControlType iso:Preventive ;
    iso:hasCybersecurityConcept iso:Identify ;
    iso:hasInformationSecurityProperty iso:Availability,
        iso:Confidentiality,
        iso:Integrity ;
    iso:hasOperationalCapability iso:Governance ;
    iso:hasSecurityDomain iso:GovernanceEcosystem,
        iso:Resilience ;
    iso:purpose """To ensure continuing suitability, adequacy, effectiveness of management direction and support for
information security in accordance with business requirements, legal, statutory, regulatory and
contractual requirements.""" ;
    dcterms:description """Information security policy and topic-specific policies should be defined, approved by management,
published, communicated to and acknowledged by relevant personnel and relevant interested parties,
and reviewed at planned intervals and if significant changes occur.""" ;
    dcterms:identifier "control-5.1" ;
    dcterms:title "Policies for information security" .

iso:control-5.2 a iso:Control ;
    iso:controlCategory iso:category-5 ;
    iso:correspondsTo iso27002_2013:control-06.1.1 ;
    iso:hasControlType iso:Preventive ;
    iso:hasCybersecurityConcept iso:Identify ;
    iso:hasInformationSecurityProperty iso:Availability,
        iso:Confidentiality,
        iso:Integrity ;
    iso:hasOperationalCapability iso:Governance ;
    iso:hasRelatedControls iso:control-5.1 ;
    iso:hasSecurityDomain iso:GovernanceEcosystem,
        iso:Protection,
        iso:Resilience ;
    iso:purpose """To establish a defined, approved and understood structure for the implementation, operation and
management of information security within the organization""" ;
    dcterms:description """Information security roles and responsibilities should be defined and allocated according to the
organization needs""" ;
    dcterms:identifier "control-5.2" ;
    dcterms:title "Information security roles and responsibilities" .

iso:control-5.21 a iso:Control ;
    iso:controlCategory iso:category-5 ;
    iso:correspondsTo iso27002_2013:control-15.1.3 ;
    iso:hasControlType iso:Preventive ;
    iso:hasCybersecurityConcept iso:Detect,
        iso:Protect ;
    iso:hasInformationSecurityProperty iso:Availability,
        iso:Confidentiality,
        iso:Integrity ;
    iso:hasOperationalCapability iso:SupplierSecurity ;
    iso:hasSecurityDomain iso:GovernanceEcosystem,
        iso:Protection ;
    iso:purpose "To ensure information security of the organization in ICT supply chain" ;
    dcterms:description "Processes and procedures should be defined and implemented to address information security risks associated with ICT services and product supply chain" ;
    dcterms:identifier "control-5.21" ;
    dcterms:title "Managing information security in the ICT supply chain" .

iso:control-5.23 a iso:Control ;
    iso:controlCategory iso:category-5 ;
    iso:correspondsTo iso27002_2013:control-New ;
    iso:hasControlType iso:Preventive ;
    iso:hasCybersecurityConcept iso:Protect ;
    iso:hasInformationSecurityProperty iso:Availability,
        iso:Confidentiality,
        iso:Integrity ;
    iso:hasOperationalCapability iso:SupplierSecurity ;
    iso:hasRelatedControls iso:control-5.21,
        iso:control-5.22 ;
    iso:hasSecurityDomain iso:GovernanceEcosystem,
        iso:Protection ;
    iso:purpose "To specify and manage information security for the use of cloud services" ;
    dcterms:description "Processes for acquisition, use, management and exit from cloud services should be established in accordance with the organization’s information security requirements" ;
    dcterms:identifier "control-5.23" ;
    dcterms:title "Information security for use of cloud services" .

iso:control-5.36 a iso:Control ;
    iso:controlCategory iso:category-5 ;
    iso:correspondsTo iso27002_2013:control-18.2.2,
        iso27002_2013:control-18.2.3 ;
    iso:hasControlType iso:Preventive ;
    iso:hasCybersecurityConcept iso:Protect ;
    iso:hasInformationSecurityProperty iso:Availability,
        iso:Confidentiality,
        iso:Integrity ;
    iso:hasOperationalCapability iso:Compliance ;
    iso:hasRelatedControls iso:control-5.35,
        iso:control-8.15,
        iso:control-8.16,
        iso:control-8.17 ;
    iso:hasSecurityDomain iso:GovernanceEcosystem ;
    iso:purpose "To ensure that information security is implemented and operated in accordance with the organizational policies topic-specific policies and standards" ;
    dcterms:description "Compliance with the organization’s information security policy, topic-specific policies and standards should be regularly reviewed" ;
    dcterms:identifier "control-5.36" ;
    dcterms:title "Compliance with policies and standards for information security" .

iso:control-5.37 a iso:Control ;
    iso:controlCategory iso:category-5 ;
    iso:correspondsTo iso27002_2013:control-12.1.1 ;
    iso:hasControlType iso:Preventive ;
    iso:hasCybersecurityConcept iso:Protect ;
    iso:hasInformationSecurityProperty iso:Availability,
        iso:Confidentiality,
        iso:Integrity ;
    iso:hasOperationalCapability iso:AssetManagement,
        iso:Continuity,
        iso:PhysicalSecurity,
        iso:SystemNetworkSecurity ;
    iso:hasRelatedControls iso:control-7.10,
        iso:control-7.14,
        iso:control-7.4,
        iso:control-8.13,
        iso:control-8.15,
        iso:control-8.17,
        iso:control-8.18 ;
    iso:hasSecurityDomain iso:Defence,
        iso:GovernanceEcosystem,
        iso:Protection ;
    iso:purpose "To ensure the correct and secure operation of information processing facilities" ;
    dcterms:description "Operating procedures for information processing facilities should be documented and made available to personnel who need them" ;
    dcterms:identifier "control-5.37" ;
    dcterms:title " Documented operating procedures" .

iso:control-5.5 a iso:Control ;
    iso:controlCategory iso:category-5 ;
    iso:correspondsTo iso27002_2013:control-06.1.3 ;
    iso:hasControlType iso:Corrective,
        iso:Preventive ;
    iso:hasCybersecurityConcept iso:Protect,
        iso:Recover,
        iso:Respond ;
    iso:hasInformationSecurityProperty iso:Availability,
        iso:Confidentiality,
        iso:Integrity ;
    iso:hasOperationalCapability iso:Governance ;
    iso:hasRelatedControls iso:control-5.24,
        iso:control-5.25,
        iso:control-5.26,
        iso:control-5.27,
        iso:control-5.28,
        iso:control-5.29,
        iso:control-5.30 ;
    iso:hasSecurityDomain iso:Defence,
        iso:Resilience ;
    iso:purpose """To ensure appropriate flow of information takes place with respect to information security between
the organization and relevant legal, regulatory and supervisory authorities""" ;
    dcterms:description "The organization should establish and maintain contact with relevant authorities" ;
    dcterms:identifier "control-5.5" ;
    dcterms:title " Contact with authorities" .

iso:control-5.6 a iso:Control ;
    iso:controlCategory iso:category-5 ;
    iso:correspondsTo iso27002_2013:control-06.1.4 ;
    iso:hasControlType iso:Corrective,
        iso:Preventive ;
    iso:hasCybersecurityConcept iso:Protect,
        iso:Recover,
        iso:Respond ;
    iso:hasInformationSecurityProperty iso:Availability,
        iso:Confidentiality,
        iso:Integrity ;
    iso:hasOperationalCapability iso:Governance ;
    iso:hasRelatedControls iso:control-5.24,
        iso:control-5.25,
        iso:control-5.26,
        iso:control-5.27,
        iso:control-5.28 ;
    iso:hasSecurityDomain iso:Defence ;
    iso:purpose "To ensure appropriate flow of information takes place with respect to information security" ;
    dcterms:description """The organization should establish and maintain contact with special interest groups or other specialist
security forums and professional associations""" ;
    dcterms:identifier "control-5.6" ;
    dcterms:title "Contact with special interest groups" .

iso:control-6.1 a iso:Control ;
    iso:controlCategory iso:category-6 ;
    iso:correspondsTo iso27002_2013:control-07.1.1 ;
    iso:hasControlType iso:Preventive ;
    iso:hasCybersecurityConcept iso:Protect ;
    iso:hasInformationSecurityProperty iso:Availability,
        iso:Confidentiality,
        iso:Integrity ;
    iso:hasOperationalCapability iso:HRSecurity ;
    iso:hasSecurityDomain iso:GovernanceEcosystem ;
    iso:purpose "To ensure all personnel are eligible and suitable for the roles for which they are considered and remain eligible and suitable during their employment" ;
    dcterms:description "Background verification checks on all candidates to become personnel should be carried out prior to joining the organization and on an ongoing basis in accordance with applicable laws, regulations and ethics, and be proportional to the business requirements, the classification of the information to be accessed and the perceived risks" ;
    dcterms:identifier "control-6.1" ;
    dcterms:title " Screening" .

iso:control-6.7 a iso:Control ;
    iso:controlCategory iso:category-6 ;
    iso:correspondsTo iso27002_2013:control-06.2.2 ;
    iso:hasControlType iso:Preventive ;
    iso:hasCybersecurityConcept iso:Protect ;
    iso:hasInformationSecurityProperty iso:Availability,
        iso:Confidentiality,
        iso:Integrity ;
    iso:hasOperationalCapability iso:AssetManagement,
        iso:PhysicalSecurity,
        iso:SystemNetworkSecurity ;
    iso:hasSecurityDomain iso:GovernanceEcosystem,
        iso:Protection ;
    iso:purpose "To ensure the security of information when personnel are working remotely" ;
    dcterms:description "Security measures should be implemented when personnel are working remotely to protect information accessed, processed or stored outside the organization's premises" ;
    dcterms:identifier "control-6.7" ;
    dcterms:title " Remote working" .

iso:control-6.8 a iso:Control ;
    iso:controlCategory iso:category-6 ;
    iso:correspondsTo iso27002_2013:control-16.1.2,
        iso27002_2013:control-16.1.3 ;
    iso:hasControlType iso:Detective ;
    iso:hasCybersecurityConcept iso:Detect ;
    iso:hasInformationSecurityProperty iso:Availability,
        iso:Confidentiality,
        iso:Integrity ;
    iso:hasOperationalCapability iso:EventManangement ;
    iso:hasSecurityDomain iso:Defence ;
    iso:purpose "To  support  timely,  consistent  and  effective  reporting  of  information  security  events  that  can  be identified by personnel" ;
    dcterms:description "The  organization  should  provide  a  mechanism  for  personnel  to  report  observed  or  suspected information security events through appropriate channels in a timely manner" ;
    dcterms:identifier "control-6.8" ;
    dcterms:title " Information security event reporting" .

iso:control-7.2 a iso:Control ;
    iso:controlCategory iso:category-7 ;
    iso:correspondsTo iso27002_2013:control-11.1.2,
        iso27002_2013:control-11.1.6 ;
    iso:hasControlType iso:Preventive ;
    iso:hasCybersecurityConcept iso:Protect ;
    iso:hasInformationSecurityProperty iso:Availability,
        iso:Confidentiality,
        iso:Integrity ;
    iso:hasOperationalCapability iso:PhysicalSecurity ;
    iso:hasRelatedControls iso:control-5.17,
        iso:control-5.18,
        iso:control-5.33,
        iso:control-5.9,
        iso:control-7.10 ;
    iso:hasSecurityDomain iso:Protection ;
    iso:purpose "To ensure only authorized physical access to the organization’s information and other associated assets occurs" ;
    dcterms:description "Secure areas should be protected by appropriate entry controls and access points" ;
    dcterms:identifier "control-7.2" ;
    dcterms:title " Physical entry controls" .

iso:control-7.3 a iso:Control ;
    iso:controlCategory iso:category-7 ;
    iso:correspondsTo iso27002_2013:control-11.1.3 ;
    iso:hasControlType iso:Preventive ;
    iso:hasCybersecurityConcept iso:Protect ;
    iso:hasInformationSecurityProperty iso:Availability,
        iso:Confidentiality,
        iso:Integrity ;
    iso:hasOperationalCapability iso:AssetManagement,
        iso:PhysicalSecurity ;
    iso:hasSecurityDomain iso:Protection ;
    iso:purpose "To prevent unauthorized physical access, damage and interference to the organization’s information and other associated assets in offices, rooms and facilities" ;
    dcterms:description "Physical security for offices, rooms, and facilities should be designed and implemented" ;
    dcterms:identifier "control-7.3" ;
    dcterms:title "Securing offices, rooms and facilities" .

iso:control-7.5 a iso:Control ;
    iso:controlCategory iso:category-7 ;
    iso:correspondsTo iso27002_2013:control-11.1.4 ;
    iso:hasControlType iso:Preventive ;
    iso:hasCybersecurityConcept iso:Protect ;
    iso:hasInformationSecurityProperty iso:Availability,
        iso:Confidentiality,
        iso:Integrity ;
    iso:hasOperationalCapability iso:PhysicalSecurity ;
    iso:hasSecurityDomain iso:Protection ;
    iso:purpose "To prevent or reduce the impacts of events originating from physical and environmental threats" ;
    dcterms:description "Protection against physical and environmental threats, such as natural disasters and other intentional or unintentional physical threats to infrastructure should be designed and implemented" ;
    dcterms:identifier "control-7.5" ;
    dcterms:title "Protecting against physical and environmental threats" .

iso:control-7.8 a iso:Control ;
    iso:controlCategory iso:category-7 ;
    iso:correspondsTo iso27002_2013:control-11.2.1 ;
    iso:hasControlType iso:Preventive ;
    iso:hasCybersecurityConcept iso:Protect ;
    iso:hasInformationSecurityProperty iso:Availability,
        iso:Confidentiality,
        iso:Integrity ;
    iso:hasOperationalCapability iso:AssetManagement,
        iso:PhysicalSecurity ;
    iso:hasSecurityDomain iso:Protection ;
    iso:purpose "To reduce the risks from environmental threats and hazards, and opportunities for unauthorized access" ;
    dcterms:description "Equipment should be sited securely and protected" ;
    dcterms:identifier "control-7.8" ;
    dcterms:title "Equipment siting and protection" .

iso:control-7.9 a iso:Control ;
    iso:controlCategory iso:category-7 ;
    iso:correspondsTo iso27002_2013:control-11.2.6 ;
    iso:hasControlType iso:Preventive ;
    iso:hasCybersecurityConcept iso:Protect ;
    iso:hasInformationSecurityProperty iso:Availability,
        iso:Confidentiality,
        iso:Integrity ;
    iso:hasOperationalCapability iso:AssetManagement,
        iso:PhysicalSecurity ;
    iso:hasRelatedControls iso:control-6.7,
        iso:control-7.4,
        iso:control-7.5,
        iso:control-8.1 ;
    iso:hasSecurityDomain iso:Protection ;
    iso:purpose "To prevent loss, damage, theft or compromise of off-site assets and interruption to the organization’s operations" ;
    dcterms:description "Off-site assets should be protected taking into account the different risks" ;
    dcterms:identifier "control-7.9" ;
    dcterms:title "Security of assets off-premises" .

iso:control-8.22 a iso:Control ;
    iso:controlCategory iso:category-8 ;
    iso:correspondsTo iso27002_2013:control-New ;
    iso:hasControlType iso:Preventive ;
    iso:hasCybersecurityConcept iso:Protect ;
    iso:hasInformationSecurityProperty iso:Availability,
        iso:Confidentiality,
        iso:Integrity ;
    iso:hasOperationalCapability iso:SystemNetworkSecurity ;
    iso:hasRelatedControls iso:control-5.7 ;
    iso:hasSecurityDomain iso:Protection ;
    iso:purpose "To protect systems from being compromised by malware and to prevent access to unauthorized web resources" ;
    dcterms:description "Access to external websites should be managed to reduce exposure to malicious content" ;
    dcterms:identifier "control-8.22" ;
    dcterms:title " Web filtering" .

iso:control-8.25 a iso:Control ;
    iso:controlCategory iso:category-8 ;
    iso:correspondsTo iso27002_2013:control-14.2.1 ;
    iso:hasControlType iso:Preventive ;
    iso:hasCybersecurityConcept iso:Protect ;
    iso:hasInformationSecurityProperty iso:Availability,
        iso:Confidentiality,
        iso:Integrity ;
    iso:hasOperationalCapability iso:ApplicationSecurity,
        iso:SystemNetworkSecurity ;
    iso:hasRelatedControls iso:control-5.32,
        iso:control-5.8,
        iso:control-8.27,
        iso:control-8.28,
        iso:control-8.29,
        iso:control-8.30,
        iso:control-8.31,
        iso:control-8.32,
        iso:control-8.4,
        iso:control-8.9 ;
    iso:hasSecurityDomain iso:Protection ;
    iso:purpose "To ensure information security is designed and implemented within the secure development lifecycle of software and systems" ;
    dcterms:description "Rules for the secure development of software and systems should be established and applied" ;
    dcterms:identifier "control-8.25" ;
    dcterms:title " Secure development lifecycle" .

iso:control-8.27 a iso:Control ;
    iso:controlCategory iso:category-8 ;
    iso:correspondsTo iso27002_2013:control-14.2.5 ;
    iso:hasControlType iso:Preventive ;
    iso:hasCybersecurityConcept iso:Protect ;
    iso:hasInformationSecurityProperty iso:Availability,
        iso:Confidentiality,
        iso:Integrity ;
    iso:hasOperationalCapability iso:ApplicationSecurity,
        iso:SystemNetworkSecurity ;
    iso:hasRelatedControls iso:control-5.12,
        iso:control-5.16,
        iso:control-5.17,
        iso:control-5.18,
        iso:control-8.2 ;
    iso:hasSecurityDomain iso:Protection ;
    iso:purpose "To  ensure  information  systems  are  securely  designed,  implemented  and  operated  within  the development lifecycle" ;
    dcterms:description "Principles for engineering secure systems should be established, documented, maintained and applied to any information system development activities" ;
    dcterms:identifier "control-8.27" ;
    dcterms:title " Secure system architecture and engineering principles" .

iso:control-8.30 a iso:Control ;
    iso:controlCategory iso:category-8 ;
    iso:correspondsTo iso27002_2013:control-14.2.7 ;
    iso:hasControlType iso:Detective,
        iso:Preventive ;
    iso:hasCybersecurityConcept iso:Detect,
        iso:Identify,
        iso:Protect ;
    iso:hasInformationSecurityProperty iso:Availability,
        iso:Confidentiality,
        iso:Integrity ;
    iso:hasOperationalCapability iso:ApplicationSecurity,
        iso:SupplierSecurity,
        iso:SystemNetworkSecurity ;
    iso:hasRelatedControls iso:control-5.32,
        iso:control-8.25-8.29,
        iso:control-8.31 ;
    iso:hasSecurityDomain iso:GovernanceEcosystem,
        iso:Protection ;
    iso:purpose "To ensure information security measures required by the organization are implemented in outsourced system development" ;
    dcterms:description "The  organization  should  direct,  monitor  and  review  the  activities  related  to  outsourced  system development" ;
    dcterms:identifier "control-8.30" ;
    dcterms:title "  Outsourced development" .

iso:control-8.33 a iso:Control ;
    iso:controlCategory iso:category-8 ;
    iso:correspondsTo iso27002_2013:control-14.3.1 ;
    iso:hasControlType iso:Preventive ;
    iso:hasCybersecurityConcept iso:Protect ;
    iso:hasInformationSecurityProperty iso:Confidentiality,
        iso:Integrity ;
    iso:hasOperationalCapability iso:InformationProtection ;
    iso:hasRelatedControls iso:control-8.10,
        iso:control-8.11,
        iso:control-8.31 ;
    iso:hasSecurityDomain iso:Protection ;
    iso:purpose "To ensure relevance of testing and protection of operational information used for testing" ;
    dcterms:description "Test information should be appropriately selected, protected and managed" ;
    dcterms:identifier "control-8.33" ;
    dcterms:title "Test information" .

iso:ThreatManagement a iso:OperationalCapability ;
    rdfs:label "Threat and Vulnerability Management" ;
    rdfs:comment "Threat and Vulnerability management capabilities are capabilities that manage threats." .

iso:control-5.14 a iso:Control ;
    iso:controlCategory iso:category-5 ;
    iso:correspondsTo iso27002_2013:control-13.2.1,
        iso27002_2013:control-13.2.2,
        iso27002_2013:control-13.2.3 ;
    iso:hasControlType iso:Preventive ;
    iso:hasCybersecurityConcept iso:Protect ;
    iso:hasInformationSecurityProperty iso:Availability,
        iso:Confidentiality,
        iso:Integrity ;
    iso:hasOperationalCapability iso:AssetManagement,
        iso:InformationProtection ;
    iso:hasRelatedControls iso:control-5.10,
        iso:control-5.13,
        iso:control-5.31,
        iso:control-5.32,
        iso:control-5.33,
        iso:control-5.34,
        <http://par-tec.it/onto/iso/27001/latest/control-7,10>,
        iso:control-8.24,
        iso:control-8.7 ;
    iso:hasSecurityDomain iso:Protection ;
    iso:purpose "To maintain the security of information transferred within an organization and with any external interested party" ;
    dcterms:description "Information transfer rules, procedures, or agreements, both within the organization and between the organization and other parties, should be in place for all types of transfer facilities" ;
    dcterms:identifier "control-5.14" ;
    dcterms:title " Information transfer" .

iso:control-5.16 a iso:Control ;
    iso:controlCategory iso:category-5 ;
    iso:correspondsTo iso27002_2013:control-09.2.1 ;
    iso:hasControlType iso:Preventive ;
    iso:hasCybersecurityConcept iso:Protect ;
    iso:hasInformationSecurityProperty iso:Availability,
        iso:Confidentiality,
        iso:Integrity ;
    iso:hasOperationalCapability iso:IAM ;
    iso:hasRelatedControls iso:control-5.18 ;
    iso:hasSecurityDomain iso:Protection ;
    iso:purpose "To  allow  for  the  unique  identification  of  individuals  and  systems  accessing  the  organisation's information and other associated assets, and to enable appropriate assignment of access rights" ;
    dcterms:description "The full lifecycle of identities should be managed" ;
    dcterms:identifier "control-5.16" ;
    dcterms:title " Identity management" .

iso:control-5.35 a iso:Control ;
    iso:controlCategory iso:category-5 ;
    iso:correspondsTo iso27002_2013:control-18.2.1 ;
    iso:hasControlType iso:Corrective,
        iso:Preventive ;
    iso:hasCybersecurityConcept iso:Identify ;
    iso:hasInformationSecurityProperty iso:Availability,
        iso:Confidentiality,
        iso:Integrity ;
    iso:purpose "To ensure the continuing suitability, adequacy and effectiveness of the organization’s approach to managing information security" ;
    dcterms:description "The organization’s approach to managing information security and its implementation including people process and technology should be reviewed independently at planned intervals, or when significant changes occur" ;
    dcterms:identifier "control-5.35" ;
    dcterms:title "Independent review of information security" .

iso:control-5.7 a iso:Control ;
    iso:controlCategory iso:category-5 ;
    iso:correspondsTo iso27002_2013:control-New ;
    iso:hasControlType iso:Detective,
        iso:Preventive ;
    iso:hasCybersecurityConcept iso:Detect,
        iso:Identify ;
    iso:hasInformationSecurityProperty iso:Availability,
        iso:Confidentiality,
        iso:Integrity ;
    iso:hasOperationalCapability iso:ThreatManagement ;
    iso:hasRelatedControls iso:control-5.25,
        iso:control-8.16,
        iso:control-8.22,
        iso:control-8.7 ;
    iso:hasSecurityDomain iso:Defence,
        iso:Resilience ;
    iso:purpose """To provide awareness of the threat environment that can impact the organization so that the
organization can take appropriate mitigation actions""" ;
    dcterms:description """Information relating to information security threats should be collected and analysed to produce threat
intelligence""" ;
    dcterms:identifier "control-5.7" ;
    dcterms:title "Threat intelligence" .

iso:control-5.8 a iso:Control ;
    iso:controlCategory iso:category-5 ;
    iso:correspondsTo iso27002_2013:control-06.1.5,
        iso27002_2013:control-14.1.1 ;
    iso:hasControlType iso:Preventive ;
    iso:hasCybersecurityConcept iso:Identify,
        iso:Protect ;
    iso:hasInformationSecurityProperty iso:Availability,
        iso:Confidentiality,
        iso:Integrity ;
    iso:hasOperationalCapability iso:Governance ;
    iso:hasRelatedControls iso:control-5.10,
        iso:control-5.12,
        iso:control-5.13,
        iso:control-5.32,
        iso:control-8.26 ;
    iso:hasSecurityDomain iso:GovernanceEcosystem,
        iso:Protection ;
    iso:purpose "To ensure information security risks related to projects and deliverables are efficiently and effectively included in project management activities throughout the project lifecycle" ;
    dcterms:description "Information security should be integrated into the organization's project management activities" ;
    dcterms:identifier "control-5.8" ;
    dcterms:title "Information security in project management" .

iso:control-6.4 a iso:Control ;
    iso:controlCategory iso:category-6 ;
    iso:correspondsTo iso27002_2013:control-07.2.3 ;
    iso:hasControlType iso:Corrective,
        iso:Preventive ;
    iso:hasCybersecurityConcept iso:Protect,
        iso:Respond ;
    iso:hasInformationSecurityProperty iso:Availability,
        iso:Confidentiality,
        iso:Integrity ;
    iso:hasOperationalCapability iso:HRSecurity ;
    iso:hasRelatedControls iso:control-5.28 ;
    iso:hasSecurityDomain iso:GovernanceEcosystem ;
    iso:purpose "To ensure personnel and other relevant interested parties understand the consequences of information security breaches, and non-compliant activities are deterred" ;
    dcterms:description "A disciplinary process should be formalized and communicated to take actions against personnel and other relevant interested parties who have committed an information security policy violation" ;
    dcterms:identifier "control-6.4" ;
    dcterms:title " Disciplinary process" .

iso:control-6.5 a iso:Control ;
    iso:controlCategory iso:category-6 ;
    iso:correspondsTo iso27002_2013:control-07.3.1 ;
    iso:hasControlType iso:Preventive ;
    iso:hasCybersecurityConcept iso:Protect ;
    iso:hasInformationSecurityProperty iso:Availability,
        iso:Confidentiality,
        iso:Integrity ;
    iso:hasOperationalCapability iso:AssetManagement,
        iso:HRSecurity ;
    iso:hasRelatedControls iso:control-6.2,
        iso:control-6.6 ;
    iso:hasSecurityDomain iso:GovernanceEcosystem ;
    iso:purpose "To protect the organization’s interests as part of the process of changing or terminating employment or contract" ;
    dcterms:description "Information security responsibilities and duties that remain valid after termination or change of employment should be defined, enforced and communicated to relevant personnel and other interested parties" ;
    dcterms:identifier "control-6.5" ;
    dcterms:title "Responsibilities after termination or change of employment" .

iso:control-8.1 a iso:Control ;
    iso:controlCategory iso:category-8 ;
    iso:correspondsTo iso27002_2013:control-06.2.1,
        iso27002_2013:control-11.2.8 ;
    iso:hasControlType iso:Preventive ;
    iso:hasCybersecurityConcept iso:Protect ;
    iso:hasInformationSecurityProperty iso:Availability,
        iso:Confidentiality,
        iso:Integrity ;
    iso:hasOperationalCapability iso:AssetManagement,
        iso:InformationProtection ;
    iso:hasRelatedControls iso:control-8.9 ;
    iso:hasSecurityDomain iso:Protection ;
    iso:purpose "To protect information against the risks introduced by using user endpoint devices" ;
    dcterms:description "Information stored on, processed by or accessible via user endpoint devices should be protected" ;
    dcterms:identifier "control-8.1" ;
    dcterms:title " User endpoint devices" .

iso:control-8.11 a iso:Control ;
    iso:controlCategory iso:category-8 ;
    iso:correspondsTo iso27002_2013:control-New ;
    iso:hasControlType iso:Preventive ;
    iso:hasCybersecurityConcept iso:Protect ;
    iso:hasInformationSecurityProperty iso:Confidentiality ;
    iso:hasOperationalCapability iso:InformationProtection ;
    iso:hasSecurityDomain iso:Protection ;
    iso:purpose "To limit the exposure of sensitive data including personally identifiable information, and to comply with legal, statutory, regulatory and contractual requirements" ;
    dcterms:description "Data masking should be used in accordance with the organization’s topic-specific policy on access control and business requirement, taking legal requirements into consideration" ;
    dcterms:identifier "control-8.11" ;
    dcterms:title " Data masking" .

iso:control-8.14 a iso:Control ;
    iso:controlCategory iso:category-8 ;
    iso:correspondsTo iso27002_2013:control-17.2.1 ;
    iso:hasControlType iso:Preventive ;
    iso:hasCybersecurityConcept iso:Protect ;
    iso:hasInformationSecurityProperty iso:Availability ;
    iso:hasOperationalCapability iso:AssetManagement,
        iso:Continuity ;
    iso:hasRelatedControls iso:control-5.30 ;
    iso:hasSecurityDomain iso:Protection,
        iso:Resilience ;
    iso:purpose "To ensure the continuous operation of information processing facilities" ;
    dcterms:description "Information processing facilities should be implemented with redundancy sufficient to meet availability requirements" ;
    dcterms:identifier "control-8.14" ;
    dcterms:title "Redundancy of information processing facilities" .

iso:control-8.18 a iso:Control ;
    iso:controlCategory iso:category-8 ;
    iso:correspondsTo iso27002_2013:control-09.4.4 ;
    iso:hasControlType iso:Preventive ;
    iso:hasCybersecurityConcept iso:Protect ;
    iso:hasInformationSecurityProperty iso:Availability,
        iso:Confidentiality,
        iso:Integrity ;
    iso:hasOperationalCapability iso:SecureConfiguration,
        iso:SystemNetworkSecurity ;
    iso:hasRelatedControls iso:control-8.2 ;
    iso:hasSecurityDomain iso:Protection ;
    iso:purpose "To ensure the use of utility programs does not harm system and application controls for information security" ;
    dcterms:description "The use of utility programs that might be capable of overriding system and application controls should be restricted and tightly controlled" ;
    dcterms:identifier "control-8.18" ;
    dcterms:title " Use of privileged utility programs" .

iso:control-8.19 a iso:Control ;
    iso:controlCategory iso:category-8 ;
    iso:correspondsTo iso27002_2013:control-12.5.1,
        iso27002_2013:control-12.6.2 ;
    iso:hasControlType iso:Preventive ;
    iso:hasCybersecurityConcept iso:Protect ;
    iso:hasInformationSecurityProperty iso:Availability,
        iso:Confidentiality,
        iso:Integrity ;
    iso:hasOperationalCapability iso:SecureConfiguration ;
    iso:hasRelatedControls iso:control-5.22,
        iso:control-8.19,
        iso:control-8.29,
        iso:control-8.31,
        iso:control-8.5,
        iso:control-8.8 ;
    iso:hasSecurityDomain iso:Protection ;
    iso:purpose "To ensure the integrity of operational systems and prevent exploitation of technical vulnerabilities" ;
    dcterms:description "Procedures  and  measures  should  be  implemented  to  securely  manage  software  installation  on operational systems" ;
    dcterms:identifier "control-8.19" ;
    dcterms:title "Installation of software on operational systems" .

iso:control-8.23 a iso:Control ;
    iso:controlCategory iso:category-8 ;
    iso:correspondsTo iso27002_2013:control-13.1.3 ;
    iso:hasControlType iso:Preventive ;
    iso:hasCybersecurityConcept iso:Protect ;
    iso:hasInformationSecurityProperty iso:Availability,
        iso:Confidentiality,
        iso:Integrity ;
    iso:hasOperationalCapability iso:SystemNetworkSecurity ;
    iso:hasRelatedControls iso:control-5.15,
        iso:control-8.20 ;
    iso:hasSecurityDomain iso:Protection ;
    iso:purpose "To split the network in security boundaries and to control traffic between them based on business needs" ;
    dcterms:description "Groups  of  information  services,  users,  and  information  systems  should  be  segregated  in  the organization’s networks" ;
    dcterms:identifier "control-8.23" ;
    dcterms:title " Segregation in networks" .

iso:control-8.26 a iso:Control ;
    iso:controlCategory iso:category-8 ;
    iso:correspondsTo iso27002_2013:control-14.1.2,
        iso27002_2013:control-14.1.3 ;
    iso:hasControlType iso:Preventive ;
    iso:hasCybersecurityConcept iso:Protect ;
    iso:hasInformationSecurityProperty iso:Availability,
        iso:Confidentiality,
        iso:Integrity ;
    iso:hasOperationalCapability iso:ApplicationSecurity,
        iso:SystemNetworkSecurity ;
    iso:hasRelatedControls iso:control-5.17,
        iso:control-5.31-5.36,
        iso:control-8.2,
        iso:control-8.24,
        iso:control-8.5 ;
    iso:hasSecurityDomain iso:Defence,
        iso:Protection ;
    iso:purpose "To ensure all information security requirements are identified and addressed when developing or acquiring applications" ;
    dcterms:description "Information security requirements should be identified, specified and approved when developing or acquiring applications" ;
    dcterms:identifier "control-8.26" ;
    dcterms:title " Application security requirements" .

iso:control-8.3 a iso:Control ;
    iso:controlCategory iso:category-8 ;
    iso:correspondsTo iso27002_2013:control-09.4.1 ;
    iso:hasControlType iso:Preventive ;
    iso:hasCybersecurityConcept iso:Protect ;
    iso:hasInformationSecurityProperty iso:Availability,
        iso:Confidentiality,
        iso:Integrity ;
    iso:hasOperationalCapability iso:IAM ;
    iso:hasRelatedControls iso:control-5.15 ;
    iso:hasSecurityDomain iso:Protection ;
    iso:purpose "To  ensure  only  authorized  access  and  to  prevent  unauthorized  access  to  information  and  other associated assets" ;
    dcterms:description "Access  to  information  and  other  associated  assets  should  be  restricted  in  accordance  with  the established topic-specific policy on access control" ;
    dcterms:identifier "control-8.3" ;
    dcterms:title "Information access restriction" .

iso:control-8.7 a iso:Control ;
    iso:controlCategory iso:category-8 ;
    iso:correspondsTo iso27002_2013:control-12.2.1 ;
    iso:hasControlType iso:Corrective,
        iso:Detective,
        iso:Preventive ;
    iso:hasCybersecurityConcept iso:Detect,
        iso:Protect ;
    iso:hasInformationSecurityProperty iso:Availability,
        iso:Confidentiality,
        iso:Integrity ;
    iso:hasOperationalCapability iso:SystemNetworkSecurity ;
    iso:hasRelatedControls iso:control-6.3,
        iso:control-8.13,
        iso:control-8.19,
        iso:control-8.32,
        iso:control-8.8 ;
    iso:hasSecurityDomain iso:Defence,
        iso:Protection ;
    iso:purpose "To ensure information and other associated assets are protected against malware" ;
    dcterms:description "Protection against malware should be implemented, supported by appropriate user awareness" ;
    dcterms:identifier "control-8.7" ;
    dcterms:title "Protection against malware" .

iso:control-5.27 a iso:Control ;
    iso:controlCategory iso:category-5 ;
    iso:correspondsTo iso27002_2013:control-16.1.6 ;
    iso:hasControlType iso:Corrective,
        iso:Preventive ;
    iso:hasCybersecurityConcept iso:Identify,
        iso:Protect ;
    iso:hasInformationSecurityProperty iso:Confidentiality,
        iso:Integrity ;
    iso:hasOperationalCapability iso:EventManangement ;
    iso:hasRelatedControls iso:control-5.24,
        iso:control-6.3 ;
    iso:hasSecurityDomain iso:Defence ;
    iso:purpose "To reduce the likelihood or impact of future incidents" ;
    dcterms:description "Knowledge gained from information security incidents should be used to strengthen and improve the control environment" ;
    dcterms:identifier "control-5.27" ;
    dcterms:title "Learning from information security incidents" .

iso:control-5.29 a iso:Control ;
    iso:controlCategory iso:category-5 ;
    iso:correspondsTo iso27002_2013:control-17.1.1,
        iso27002_2013:control-17.1.2,
        iso27002_2013:control-17.1.3 ;
    iso:hasControlType iso:Preventive ;
    iso:hasCybersecurityConcept iso:Protect ;
    iso:hasInformationSecurityProperty iso:Availability,
        iso:Confidentiality,
        iso:Integrity ;
    iso:hasOperationalCapability iso:Continuity ;
    iso:hasSecurityDomain iso:Protection,
        iso:Resilience ;
    iso:purpose "To provide information and other associated asset with adequate protection during disruption" ;
    dcterms:description "The organization should plan how to maintain information security at an appropriate level during disruption" ;
    dcterms:identifier "control-5.29" ;
    dcterms:title "Information security during disruption" .

iso:control-5.3 a iso:Control ;
    iso:controlCategory iso:category-5 ;
    iso:correspondsTo iso27002_2013:control-06.1.2 ;
    iso:hasControlType iso:Preventive ;
    iso:hasCybersecurityConcept iso:Protect ;
    iso:hasInformationSecurityProperty iso:Availability,
        iso:Confidentiality,
        iso:Integrity ;
    iso:hasOperationalCapability iso:Governance ;
    iso:hasSecurityDomain iso:GovernanceEcosystem ;
    iso:purpose "To reduce the risk of fraud, error and bypassing of information security controls" ;
    dcterms:description "Conflicting duties and areas of responsibility should be segregated" ;
    dcterms:identifier "control-5.3" ;
    dcterms:title "Segregation of duties" .

iso:control-6.2 a iso:Control ;
    iso:controlCategory iso:category-6 ;
    iso:correspondsTo iso27002_2013:control-07.1.2 ;
    iso:hasControlType iso:Preventive ;
    iso:hasCybersecurityConcept iso:Protect ;
    iso:hasInformationSecurityProperty iso:Availability,
        iso:Confidentiality,
        iso:Integrity ;
    iso:hasOperationalCapability iso:HRSecurity ;
    iso:hasRelatedControls iso:control-5.13,
        iso:control-5.32,
        iso:control-5.34,
        iso:control-5.9,
        iso:control-6.4,
        iso:control-6.5,
        iso:control-6.6 ;
    iso:hasSecurityDomain iso:GovernanceEcosystem ;
    iso:purpose "To ensure personnel understand their information security responsibilities for the roles for which they are considered" ;
    dcterms:description "The   employment   contractual   agreements   should   state   the   personnel’s   and   the   organization’s responsibilities for information security" ;
    dcterms:identifier "control-6.2" ;
    dcterms:title "Terms and conditions of employment" .

iso:control-6.3 a iso:Control ;
    iso:controlCategory iso:category-6 ;
    iso:correspondsTo iso27002_2013:control-07.2.2 ;
    iso:hasControlType iso:Preventive ;
    iso:hasCybersecurityConcept iso:Protect ;
    iso:hasInformationSecurityProperty iso:Availability,
        iso:Confidentiality,
        iso:Integrity ;
    iso:hasOperationalCapability iso:HRSecurity ;
    iso:hasSecurityDomain iso:GovernanceEcosystem ;
    iso:purpose "To ensure personnel and relevant interested parties are aware of and fulfil their information security responsibilities" ;
    dcterms:description "Personnel of the organization and relevant interested parties should receive appropriate information security awareness, education and training and regular updates of organizational policies and procedures, as relevant for their job function" ;
    dcterms:identifier "control-6.3" ;
    dcterms:title "Information security awareness, education and training" .

iso:control-7.4 a iso:Control ;
    iso:controlCategory iso:category-7 ;
    iso:correspondsTo iso27002_2013:control-New ;
    iso:hasControlType iso:Detective ;
    iso:hasCybersecurityConcept iso:Detect ;
    iso:hasInformationSecurityProperty iso:Availability,
        iso:Confidentiality,
        iso:Integrity ;
    iso:hasOperationalCapability iso:PhysicalSecurity ;
    iso:hasSecurityDomain iso:Defence,
        iso:Protection ;
    iso:purpose "To detect and deter unauthorized physical access" ;
    dcterms:description "Premises should be continuously monitored for unauthorized physical access" ;
    dcterms:identifier "control-7.4" ;
    dcterms:title "Physical security monitoring" .

iso:control-8.13 a iso:Control ;
    iso:controlCategory iso:category-8 ;
    iso:correspondsTo iso27002_2013:control-12.3.1 ;
    iso:hasControlType iso:Corrective ;
    iso:hasCybersecurityConcept iso:Recover ;
    iso:hasInformationSecurityProperty iso:Availability,
        iso:Integrity ;
    iso:hasOperationalCapability iso:Continuity ;
    iso:hasRelatedControls iso:control-5.30,
        iso:control-7,
        iso:control-8.1,
        iso:control-8.10,
        iso:control-Clause ;
    iso:hasSecurityDomain iso:Protection ;
    iso:purpose "To enable recovery from loss of data or systems" ;
    dcterms:description "Backup copies of information, software and systems should be maintained and regularly tested in accordance with the agreed topic-specific policy on backup" ;
    dcterms:identifier "control-8.13" ;
    dcterms:title "Information backup" .

iso:control-8.16 a iso:Control ;
    iso:controlCategory iso:category-8 ;
    iso:correspondsTo iso27002_2013:control-New ;
    iso:hasControlType iso:Corrective,
        iso:Detective ;
    iso:hasCybersecurityConcept iso:Detect,
        iso:Respond ;
    iso:hasInformationSecurityProperty iso:Availability,
        iso:Confidentiality,
        iso:Integrity ;
    iso:hasOperationalCapability iso:EventManangement ;
    iso:hasRelatedControls iso:control-5.25,
        iso:control-5.26,
        iso:control-5.7 ;
    iso:hasSecurityDomain iso:Defence ;
    iso:purpose "To detect anomalous behaviour and potential information security incidents" ;
    dcterms:description "Networks, systems and applications should be monitored for anomalous behaviour and appropriate actions taken to evaluate potential information security incidents" ;
    dcterms:identifier "control-8.16" ;
    dcterms:title " Monitoring activities" .

iso:control-8.17 a iso:Control ;
    iso:controlCategory iso:category-8 ;
    iso:correspondsTo iso27002_2013:control-12.4.4 ;
    iso:hasControlType iso:Detective ;
    iso:hasCybersecurityConcept iso:Detect,
        iso:Protect ;
    iso:hasInformationSecurityProperty iso:Integrity ;
    iso:hasOperationalCapability iso:EventManangement ;
    iso:hasSecurityDomain iso:Defence,
        iso:Protection ;
    iso:purpose "To enable the correlation and analysis of security-related events and other recorded data, and to support investigations into information security incidents" ;
    dcterms:description "The clocks of information processing systems used by the organization should be synchronized to approved time sources" ;
    dcterms:identifier "control-8.17" ;
    dcterms:title " Clock synchronization" .

iso:control-8.20 a iso:Control ;
    iso:controlCategory iso:category-8 ;
    iso:correspondsTo iso27002_2013:control-13.1.1 ;
    iso:hasControlType iso:Detective,
        iso:Preventive ;
    iso:hasCybersecurityConcept iso:Detect,
        iso:Protect ;
    iso:hasInformationSecurityProperty iso:Availability,
        iso:Confidentiality,
        iso:Integrity ;
    iso:hasOperationalCapability iso:SystemNetworkSecurity ;
    iso:hasRelatedControls iso:control-5.14,
        iso:control-5.22,
        iso:control-5.3,
        iso:control-6.6,
        iso:control-8.13,
        iso:control-8.15,
        iso:control-8.24 ;
    iso:hasSecurityDomain iso:Protection ;
    iso:purpose "To  ensure  the  protection  of  information  in  networks  and  its  supporting  information  processing facilities" ;
    dcterms:description "Networks should be managed and controlled to protect information in systems and applications" ;
    dcterms:identifier "control-8.20" ;
    dcterms:title " Network controls" .

iso:control-8.28 a iso:Control ;
    iso:controlCategory iso:category-8 ;
    iso:correspondsTo iso27002_2013:control-New ;
    iso:hasControlType iso:Preventive ;
    iso:hasCybersecurityConcept iso:Protect ;
    iso:hasInformationSecurityProperty iso:Availability,
        iso:Confidentiality,
        iso:Integrity ;
    iso:hasOperationalCapability iso:ApplicationSecurity,
        iso:SystemNetworkSecurity ;
    iso:hasRelatedControls iso:control-5.18,
        iso:control-8.29,
        iso:control-8.8 ;
    iso:hasSecurityDomain iso:Protection ;
    iso:purpose "To ensure software is written securely thereby reducing the number of potential information security vulnerabilities in the software" ;
    dcterms:description "Secure coding principles should be applied to software development" ;
    dcterms:identifier "control-8.28" ;
    dcterms:title " Secure coding" .

iso:control-8.4 a iso:Control ;
    iso:controlCategory iso:category-8 ;
    iso:correspondsTo iso27002_2013:control-09.4.5 ;
    iso:hasControlType iso:Preventive ;
    iso:hasCybersecurityConcept iso:Protect ;
    iso:hasInformationSecurityProperty iso:Availability,
        iso:Confidentiality,
        iso:Integrity ;
    iso:hasOperationalCapability iso:ApplicationSecurity,
        iso:IAM ;
    iso:hasRelatedControls iso:control-8.32 ;
    iso:hasSecurityDomain iso:Protection ;
    iso:purpose "To prevent the introduction of unauthorized functionality, avoid unintentional or malicious changes and to maintain the confidentiality of valuable intellectual property" ;
    dcterms:description "Read and write access to source code, development tools and software libraries should be appropriately managed" ;
    dcterms:identifier "control-8.4" ;
    dcterms:title " Access to source code" .

iso:control-8.8 a iso:Control ;
    iso:controlCategory iso:category-8 ;
    iso:correspondsTo iso27002_2013:control-12.6.1,
        iso27002_2013:control-18.2.3 ;
    iso:hasControlType iso:Preventive ;
    iso:hasCybersecurityConcept iso:Protect ;
    iso:hasInformationSecurityProperty iso:Availability,
        iso:Confidentiality,
        iso:Integrity ;
    iso:hasOperationalCapability iso:ThreatManagement ;
    iso:hasRelatedControls iso:control-5.14,
        iso:control-5.20,
        iso:control-5.23,
        iso:control-5.26,
        iso:control-5.9,
        iso:control-8.20,
        iso:control-8.23,
        iso:control-8.25,
        iso:control-8.28,
        iso:control-8.29,
        iso:control-8.32 ;
    iso:hasSecurityDomain iso:Defence,
        iso:GovernanceEcosystem,
        iso:Protection ;
    iso:purpose "To prevent exploitation of technical vulnerabilities" ;
    dcterms:description "Information about technical vulnerabilities of information systems in use should be obtained, the organization’s exposure to such vulnerabilities should be evaluated and appropriate measures should be taken" ;
    dcterms:identifier "control-8.8" ;
    dcterms:title " Management of technical vulnerabilities" .

iso:control-8.9 a iso:Control ;
    iso:controlCategory iso:category-8 ;
    iso:correspondsTo iso27002_2013:control-New ;
    iso:hasControlType iso:Preventive ;
    iso:hasCybersecurityConcept iso:Protect ;
    iso:hasInformationSecurityProperty iso:Availability,
        iso:Confidentiality,
        iso:Integrity ;
    iso:hasOperationalCapability iso:SecureConfiguration ;
    iso:hasRelatedControls iso:control-5.32,
        iso:control-8.32 ;
    iso:hasSecurityDomain iso:Protection ;
    iso:purpose "To  ensure  hardware,  software,  services  and  networks  function  correctly  with  required  security settings, and configuration is not altered by unauthorized or incorrect changes" ;
    dcterms:description "Configurations, including security configurations, of hardware, software, services and networks should be established, documented, implemented, monitored and reviewed" ;
    dcterms:identifier "control-8.9" ;
    dcterms:title " Configuration management" .

iso:ControlType a owl:Class,
        skos:Concept ;
    rdfs:label "Control Type" ;
    rdfs:comment """
    Control type is an attribute to view controls from the perspective of when and how the control
    modifies the risk with regard to the occurrence of an information security incident.
    """ .

iso:InformationSecurityProperty a owl:Class,
        skos:Concept ;
    rdfs:label "Information Security Properties" ;
    rdfs:comment "Information security properties are the different properties of information." ;
    rdfs:seeAlso <https://dbpedia.org/page/Information_security> .

iso:SecureConfiguration a iso:OperationalCapability ;
    rdfs:label "Secure Configuration" ;
    rdfs:comment "Secure configuration capabilities are capabilities that secure configuration." .

iso:control-5.20 a iso:Control ;
    iso:controlCategory iso:category-5 ;
    iso:correspondsTo iso27002_2013:control-15.1.2 ;
    iso:hasControlType iso:Preventive ;
    iso:hasCybersecurityConcept iso:Identify ;
    iso:hasInformationSecurityProperty iso:Availability,
        iso:Confidentiality,
        iso:Integrity ;
    iso:hasOperationalCapability iso:SupplierSecurity ;
    iso:hasRelatedControls iso:control-5.10,
        iso:control-5.12,
        iso:control-5.13 ;
    iso:hasSecurityDomain iso:GovernanceEcosystem,
        iso:Protection ;
    iso:purpose "To ensure information security of the organization in supplier relationships" ;
    dcterms:description "Relevant information security requirements should be established and agreed with each supplier based on the type of supplier relationship" ;
    dcterms:identifier "control-5.20" ;
    dcterms:title "Addressing information security within supplier agreements" .

iso:control-5.22 a iso:Control ;
    iso:controlCategory iso:category-5 ;
    iso:correspondsTo iso27002_2013:control-15.2.1,
        iso27002_2013:control-15.2.2 ;
    iso:hasControlType iso:Preventive ;
    iso:hasCybersecurityConcept iso:Identify ;
    iso:hasInformationSecurityProperty iso:Availability,
        iso:Confidentiality,
        iso:Integrity ;
    iso:hasOperationalCapability iso:SupplierSecurity ;
    iso:hasRelatedControls iso:control-5.29,
        iso:control-5.35,
        iso:control-5.36,
        iso:control-8.14 ;
    iso:hasSecurityDomain iso:Defence,
        iso:GovernanceEcosystem,
        iso:Protection ;
    iso:purpose "To  maintain  an  agreed  level  of  information  security  and  service  delivery  in  line  with  supplier agreements" ;
    dcterms:description "The organization should regularly monitor, review, evaluate and manage change in supplier information security practices and service delivery" ;
    dcterms:identifier "control-5.22" ;
    dcterms:title "Monitoring, review and change management of supplier services" .

iso:control-5.24 a iso:Control ;
    iso:controlCategory iso:category-5 ;
    iso:correspondsTo iso27002_2013:control-16.1.1 ;
    iso:hasControlType iso:Corrective ;
    iso:hasCybersecurityConcept iso:Recover,
        iso:Respond ;
    iso:hasInformationSecurityProperty iso:Availability,
        iso:Confidentiality,
        iso:Integrity ;
    iso:hasOperationalCapability iso:EventManangement ;
    iso:hasRelatedControls iso:control-5.25,
        iso:control-5.26,
        iso:control-5.28,
        iso:control-5.5,
        iso:control-5.6,
        iso:control-6.8,
        iso:control-8.14,
        iso:control-8.15 ;
    iso:hasSecurityDomain iso:Defence ;
    iso:purpose "To ensure quick, effective, consistent and orderly response to information security incidents, including communication on information security events" ;
    dcterms:description "The organization should plan and prepare for managing information security incidents by defining, establishing and communicating information security incident management processes, roles and responsibilities" ;
    dcterms:identifier "control-5.24" ;
    dcterms:title "Information security incident management responsibilities and preparation" .

iso:control-5.31 a iso:Control ;
    iso:controlCategory iso:category-5 ;
    iso:correspondsTo iso27002_2013:control-18.1.1,
        iso27002_2013:control-18.1.5 ;
    iso:hasControlType iso:Preventive ;
    iso:hasCybersecurityConcept iso:Identify ;
    iso:hasInformationSecurityProperty iso:Availability,
        iso:Confidentiality,
        iso:Integrity ;
    iso:hasOperationalCapability iso:Compliance ;
    iso:hasRelatedControls iso:control-5.20 ;
    iso:hasSecurityDomain iso:GovernanceEcosystem,
        iso:Protection ;
    iso:purpose "To  ensure  compliance  with  legal,  statutory,  regulatory  or  contractual  requirements  related  to information security" ;
    dcterms:description "Information  security  relevant  legal,  statutory,  regulatory  and  contractual  requirements  and  the organization’s approach to meet these requirements should be identified, documented and kept up to date" ;
    dcterms:identifier "control-5.31" ;
    dcterms:title "Identification of legal, statutory, regulatory and contractual requirements" .

iso:control-5.33 a iso:Control ;
    iso:controlCategory iso:category-5 ;
    iso:correspondsTo iso27002_2013:control-18.1.3 ;
    iso:hasControlType iso:Preventive ;
    iso:hasCybersecurityConcept iso:Identify,
        iso:Protect ;
    iso:hasInformationSecurityProperty iso:Availability,
        iso:Confidentiality,
        iso:Integrity ;
    iso:hasOperationalCapability iso:AssetManagement,
        iso:Compliance,
        iso:InformationProtection ;
    iso:hasRelatedControls iso:control-8.24 ;
    iso:hasSecurityDomain iso:Defence ;
    iso:purpose "To ensure compliance with legal, statutory, regulatory or contractual requirements related to the protection of records" ;
    dcterms:description "Records should be protected from loss, destruction, falsification, unauthorized access and unauthorized release, in accordance with legal, statutory, regulatory, contractual and business requirements" ;
    dcterms:identifier "control-5.33" ;
    dcterms:title " Protection of records" .

iso:control-5.9 a iso:Control ;
    iso:controlCategory iso:category-5 ;
    iso:correspondsTo iso27002_2013:control-08.1.1,
        iso27002_2013:control-08.1.2 ;
    iso:hasControlType iso:Preventive ;
    iso:hasCybersecurityConcept iso:Identify ;
    iso:hasInformationSecurityProperty iso:Availability,
        iso:Confidentiality,
        iso:Integrity ;
    iso:hasOperationalCapability iso:AssetManagement ;
    iso:hasRelatedControls iso:control-5.10,
        iso:control-5.12,
        iso:control-5.13 ;
    iso:hasSecurityDomain iso:GovernanceEcosystem,
        iso:Protection ;
    iso:purpose "To identify the organization's information and other associated assets in order to preserve their information security and assign appropriate ownership" ;
    dcterms:description """An inventory of information and other associated assets, including owners, should be developed and
maintained
""" ;
    dcterms:identifier "control-5.9" ;
    dcterms:title "Inventory of information and other associated assets" .

iso:control-6.6 a iso:Control ;
    iso:controlCategory iso:category-6 ;
    iso:correspondsTo iso27002_2013:control-13.2.4 ;
    iso:hasControlType iso:Preventive ;
    iso:hasCybersecurityConcept iso:Protect ;
    iso:hasInformationSecurityProperty iso:Confidentiality ;
    iso:hasOperationalCapability iso:HRSecurity,
        iso:InformationProtection,
        iso:SupplierSecurity ;
    iso:hasRelatedControls iso:control-5.31,
        iso:control-5.32,
        iso:control-5.33,
        iso:control-5.34 ;
    iso:hasSecurityDomain iso:GovernanceEcosystem ;
    iso:purpose "To maintain confidentiality of information accessible by personnel or external parties" ;
    dcterms:description "Confidentiality or non-disclosure agreements reflecting the organization’s needs for the protection of information should be identified, documented, regularly reviewed and signed by personnel and other relevant interested parties" ;
    dcterms:identifier "control-6.6" ;
    dcterms:title " Confidentiality or non-disclosure agreements" .

iso:control-7.10 a iso:Control ;
    iso:controlCategory iso:category-7 ;
    iso:correspondsTo iso27002_2013:control-08.3.1,
        iso27002_2013:control-08.3.2,
        iso27002_2013:control-08.3.3 ;
    iso:hasControlType iso:Preventive ;
    iso:hasCybersecurityConcept iso:Protect ;
    iso:hasInformationSecurityProperty iso:Availability,
        iso:Confidentiality,
        iso:Integrity ;
    iso:hasOperationalCapability iso:AssetManagement,
        iso:PhysicalSecurity ;
    iso:hasRelatedControls iso:control-7.14,
        iso:control-8.10 ;
    iso:hasSecurityDomain iso:Protection ;
    iso:purpose "To ensure only authorized disclosure, modification, removal or destruction of information stored on media" ;
    dcterms:description "Storage media should be managed through its lifecycle of acquisition, use, transportation and disposal in accordance with the organization’s classification scheme and handling requirements" ;
    dcterms:identifier "control-7.10" ;
    dcterms:title " Storage media" .

iso:control-8.10 a iso:Control ;
    iso:controlCategory iso:category-8 ;
    iso:correspondsTo iso27002_2013:control-New ;
    iso:hasControlType iso:Preventive ;
    iso:hasCybersecurityConcept iso:Protect ;
    iso:hasInformationSecurityProperty iso:Confidentiality ;
    iso:hasOperationalCapability iso:InformationProtection ;
    iso:hasRelatedControls iso:control-7.14 ;
    iso:hasSecurityDomain iso:Protection ;
    iso:purpose "To  prevent  unnecessary  exposure  of  sensitive  information  and  to  comply  with  legal,  statutory, regulatory and contractual requirements for data deletion" ;
    dcterms:description "Information stored in information systems and devices should be deleted when no longer required" ;
    dcterms:identifier "control-8.10" ;
    dcterms:title "Information deletion" .

iso:control-8.2 a iso:Control ;
    iso:controlCategory iso:category-8 ;
    iso:correspondsTo iso27002_2013:control-09.2.3 ;
    iso:hasControlType iso:Preventive ;
    iso:hasCybersecurityConcept iso:Protect ;
    iso:hasInformationSecurityProperty iso:Availability,
        iso:Confidentiality,
        iso:Integrity ;
    iso:hasOperationalCapability iso:IAM ;
    iso:hasRelatedControls iso:control-5.15,
        iso:control-5.17,
        iso:control-5.18 ;
    iso:hasSecurityDomain iso:Protection ;
    iso:purpose "To ensure only authorized users, software components and services are provided with privileged access rights" ;
    dcterms:description "The allocation and use of privileged access rights should be restricted and managed" ;
    dcterms:identifier "control-8.2" ;
    dcterms:title " Privileged access rights" .

iso:control-8.5 a iso:Control ;
    iso:controlCategory iso:category-8 ;
    iso:correspondsTo iso27002_2013:control-09.4.2 ;
    iso:hasControlType iso:Preventive ;
    iso:hasCybersecurityConcept iso:Protect ;
    iso:hasInformationSecurityProperty iso:Availability,
        iso:Confidentiality,
        iso:Integrity ;
    iso:hasOperationalCapability iso:IAM ;
    iso:hasSecurityDomain iso:Protection ;
    iso:purpose "To ensure a user or an entity is securely authenticated when access to systems, applications, and services is granted" ;
    dcterms:description "Secure  authentication  technologies  and  procedures  should  be  implemented  based  on  information access restrictions and the topic-specific policy on access control" ;
    dcterms:identifier "control-8.5" ;
    dcterms:title " Secure authentication" .

iso:Compliance a iso:OperationalCapability ;
    rdfs:label "Legal andCompliance" ;
    rdfs:comment "Compliance capabilities are capabilities that manage compliance." .

iso:ControlCategory a owl:Class,
        skos:Concept ;
    rdfs:label "Control Category" ;
    rdfs:comment "Control categories are the basic building blocks of the ISO 27001 standard." .

iso:Recover a iso:CybersecurityConcept ;
    rdfs:label "Recover" ;
    rdfs:comment "Recover concepts are concepts that recover information." .

iso:SecurityDomain a owl:Class,
        skos:Concept ;
    rdfs:label "Security Domains" ;
    rdfs:comment "Security domains are the different domains that can be used in the ISO 27001 standard." .

iso:control-5.10 a iso:Control ;
    iso:controlCategory iso:category-5 ;
    iso:correspondsTo iso27002_2013:control-08.1.3,
        iso27002_2013:control-08.2.3 ;
    iso:hasControlType iso:Preventive ;
    iso:hasCybersecurityConcept iso:Protect ;
    iso:hasInformationSecurityProperty iso:Availability,
        iso:Confidentiality,
        iso:Integrity ;
    iso:hasOperationalCapability iso:AssetManagement,
        iso:InformationProtection ;
    iso:hasRelatedControls iso:control-5.12,
        iso:control-7.10,
        iso:control-7.8 ;
    iso:hasSecurityDomain iso:GovernanceEcosystem,
        iso:Protection ;
    iso:purpose "To ensure information and other associated assets are appropriately protected, used and handled" ;
    dcterms:description "Rules for the acceptable use and procedures for the handling of information and other associated assets should be identified, documented and implemented" ;
    dcterms:identifier "control-5.10" ;
    dcterms:title "Acceptable use of information and associated assets" .

iso:control-5.26 a iso:Control ;
    iso:controlCategory iso:category-5 ;
    iso:correspondsTo iso27002_2013:control-16.1.5 ;
    iso:hasControlType iso:Corrective ;
    iso:hasCybersecurityConcept iso:Recover,
        iso:Respond ;
    iso:hasInformationSecurityProperty iso:Availability,
        iso:Confidentiality,
        iso:Integrity ;
    iso:hasOperationalCapability iso:EventManangement ;
    iso:hasRelatedControls iso:control-5.24,
        iso:control-5.27,
        iso:control-5.28,
        iso:control-5.29,
        iso:control-5.30 ;
    iso:hasSecurityDomain iso:Defence ;
    iso:purpose "To ensure efficient and effective response to information security incidents" ;
    dcterms:description "Information security incidents should be responded to in accordance with the documented procedures" ;
    dcterms:identifier "control-5.26" ;
    dcterms:title "Response to information security incidents" .

iso:control-5.30 a iso:Control ;
    iso:controlCategory iso:category-5 ;
    iso:correspondsTo iso27002_2013:control-New ;
    iso:hasControlType iso:Corrective ;
    iso:hasCybersecurityConcept iso:Protect,
        iso:Respond ;
    iso:hasInformationSecurityProperty iso:Availability ;
    iso:hasOperationalCapability iso:Continuity ;
    iso:hasSecurityDomain iso:Resilience ;
    iso:purpose "To ensure the availability of the organization’s information and other associated assets in the event of a disruption" ;
    dcterms:description "ICT readiness should be planned, implemented, maintained and tested based on business continuity objectives and ICT continuity requirements" ;
    dcterms:identifier "control-5.30" ;
    dcterms:title "ICT readiness for business continuity" .

iso:control-5.34 a iso:Control ;
    iso:controlCategory iso:category-5 ;
    iso:correspondsTo iso27002_2013:control-18.1.4 ;
    iso:hasControlType iso:Preventive ;
    iso:hasCybersecurityConcept iso:Identify,
        iso:Protect ;
    iso:hasInformationSecurityProperty iso:Availability,
        iso:Confidentiality,
        iso:Integrity ;
    iso:hasOperationalCapability iso:Compliance,
        iso:InformationProtection ;
    iso:hasSecurityDomain iso:Protection ;
    iso:purpose "To ensure compliance with legal, statutory, regulatory or contractual requirements related to the information security aspects of the protection of PII" ;
    dcterms:description "The organization should identify and meet the requirements regarding preservation of privacy and protection of PII according to applicable laws and regulations and contractual requirements" ;
    dcterms:identifier "control-5.34" ;
    dcterms:title " Privacy and protection of PII" .

iso:control-7.14 a iso:Control ;
    iso:controlCategory iso:category-7 ;
    iso:correspondsTo iso27002_2013:control-11.2.7 ;
    iso:hasControlType iso:Preventive ;
    iso:hasCybersecurityConcept iso:Protect ;
    iso:hasInformationSecurityProperty iso:Confidentiality ;
    iso:hasOperationalCapability iso:AssetManagement,
        iso:PhysicalSecurity ;
    iso:hasRelatedControls iso:control-7.10,
        iso:control-8.10,
        iso:control-8.24 ;
    iso:hasSecurityDomain iso:Protection ;
    iso:purpose "To prevent leakage of information from equipment to be disposed or re-used" ;
    dcterms:description "Items of equipment containing storage media should be verified to ensure that any sensitive data and licensed software has been removed or securely overwritten prior to disposal or re-use" ;
    dcterms:identifier "control-7.14" ;
    dcterms:title "Secure disposal or re-use of equipment" .

iso:control-8.15 a iso:Control ;
    iso:controlCategory iso:category-8 ;
    iso:correspondsTo iso27002_2013:control-12.4.1,
        iso27002_2013:control-12.4.2,
        iso27002_2013:control-12.4.3 ;
    iso:hasControlType iso:Detective ;
    iso:hasCybersecurityConcept iso:Detect ;
    iso:hasInformationSecurityProperty iso:Availability,
        iso:Confidentiality,
        iso:Integrity ;
    iso:hasOperationalCapability iso:EventManangement ;
    iso:hasRelatedControls iso:control-5.25,
        iso:control-5.28,
        iso:control-5.34,
        iso:control-8.11,
        iso:control-8.16,
        iso:control-8.17 ;
    iso:hasSecurityDomain iso:Defence,
        iso:Protection ;
    iso:purpose "To record events, generate evidence, ensure the integrity of log information, prevent against unauthorized access, identify information security events that can lead to an information security incident and to support investigations" ;
    dcterms:description "Logs that record activities, exceptions, faults and other relevant events should be produced, protected, stored and analysed" ;
    dcterms:identifier "control-8.15" ;
    dcterms:title " Logging" .

iso:control-8.32 a iso:Control ;
    iso:controlCategory iso:category-8 ;
    iso:correspondsTo iso27002_2013:control-12.1.2,
        iso27002_2013:control-14.2.2,
        iso27002_2013:control-14.2.3,
        iso27002_2013:control-14.2.4 ;
    iso:hasControlType iso:Preventive ;
    iso:hasCybersecurityConcept iso:Protect ;
    iso:hasInformationSecurityProperty iso:Availability,
        iso:Confidentiality,
        iso:Integrity ;
    iso:hasOperationalCapability iso:ApplicationSecurity,
        iso:SystemNetworkSecurity ;
    iso:hasRelatedControls iso:control-5.30,
        iso:control-5.37,
        iso:control-8.29,
        iso:control-8.31 ;
    iso:hasSecurityDomain iso:Protection ;
    iso:purpose "To preserve information security when executing changes" ;
    dcterms:description "Changes to information processing facilities and information systems should be subject to change management procedures" ;
    dcterms:identifier "control-8.32" ;
    dcterms:title " Change management" .

iso:Continuity a iso:OperationalCapability ;
    rdfs:label "Continuity" ;
    rdfs:comment "Continuity capabilities are capabilities that manage continuity." .

iso:CybersecurityConcept a owl:Class,
        skos:Concept ;
    rdfs:label "Cybersecurity Concepts" ;
    rdfs:comment """Cybersecurity frameworks based on ISO/IEC TS 27110
        provide a way to organize and communicate
        cybersecurity activities through 5 concepts:
        Identify, Protect, Detect, Respond, and Recover.""" ;
    rdfs:seeAlso <https://www.nist.gov/cyberframework> .

iso:HRSecurity a iso:OperationalCapability ;
    rdfs:label "Human Resources Security" ;
    rdfs:comment "Human resources security capabilities are capabilities that protect human resources." .

iso:control-5.13 a iso:Control ;
    iso:controlCategory iso:category-5 ;
    iso:correspondsTo iso27002_2013:control-08.2.2 ;
    iso:hasControlType iso:Preventive ;
    iso:hasCybersecurityConcept iso:Protect ;
    iso:hasInformationSecurityProperty iso:Availability,
        iso:Confidentiality,
        iso:Integrity ;
    iso:hasOperationalCapability iso:InformationProtection ;
    iso:hasRelatedControls iso:control-5.12 ;
    iso:hasSecurityDomain iso:Defence ;
    iso:purpose "To facilitate the communication of classification of information and support automation of information processing and management" ;
    dcterms:description "An appropriate set of procedures for information labelling should be developed and implemented in accordance with the information classification scheme adopted by the organization" ;
    dcterms:identifier "control-5.13" ;
    dcterms:title " Labelling of information" .

iso:control-5.15 a iso:Control ;
    iso:controlCategory iso:category-5 ;
    iso:correspondsTo iso27002_2013:control-09.1.1,
        iso27002_2013:control-09.1.2 ;
    iso:hasControlType iso:Preventive ;
    iso:hasCybersecurityConcept iso:Protect ;
    iso:hasInformationSecurityProperty iso:Availability,
        iso:Confidentiality,
        iso:Integrity ;
    iso:hasOperationalCapability iso:IAM ;
    iso:hasRelatedControls iso:control-5.10,
        iso:control-5.12,
        iso:control-5.13,
        iso:control-5.16,
        iso:control-5.17,
        iso:control-5.18,
        iso:control-5.2,
        iso:control-5.3,
        iso:control-5.31,
        iso:control-5.32,
        iso:control-5.33,
        iso:control-5.34,
        iso:control-7.2,
        iso:control-7.3,
        iso:control-7.4,
        iso:control-8.15,
        iso:control-8.18,
        iso:control-8.2,
        iso:control-8.26,
        iso:control-8.3,
        iso:control-8.4,
        iso:control-8.5 ;
    iso:hasSecurityDomain iso:Protection ;
    iso:purpose "To  ensure  authorized  access  and  to  prevent  unauthorized  access  to  information  and  other associated assets" ;
    dcterms:description "Rules to control physical and logical access to information and other associated assets should be established and implemented based on business and information security requirements" ;
    dcterms:identifier "control-5.15" ;
    dcterms:title " Access control" .

iso:control-5.17 a iso:Control ;
    iso:controlCategory iso:category-5 ;
    iso:correspondsTo iso27002_2013:control-09.2.4,
        iso27002_2013:control-09.3.1,
        iso27002_2013:control-09.4.3 ;
    iso:hasControlType iso:Preventive ;
    iso:hasCybersecurityConcept iso:Protect ;
    iso:hasInformationSecurityProperty iso:Availability,
        iso:Confidentiality,
        iso:Integrity ;
    iso:hasOperationalCapability iso:IAM ;
    iso:hasRelatedControls iso:control-6.2,
        iso:control-8.24 ;
    iso:hasSecurityDomain iso:GovernanceEcosystem,
        iso:Protection ;
    iso:purpose "To ensure proper entity authentication and prevent failures of authentication processes" ;
    dcterms:description "Allocation  and  management  of  authentication  information  should  be  controlled  by  a  management process, including advising personnel of appropriate handling of authentication information" ;
    dcterms:identifier "control-5.17" ;
    dcterms:title " Authentication information" .

iso:control-5.18 a iso:Control ;
    iso:controlCategory iso:category-5 ;
    iso:correspondsTo iso27002_2013:control-09.2.2,
        iso27002_2013:control-09.2.5,
        iso27002_2013:control-09.2.6 ;
    iso:hasControlType iso:Preventive ;
    iso:hasInformationSecurityProperty iso:Availability,
        iso:Confidentiality,
        iso:Integrity ;
    iso:hasOperationalCapability iso:IAM ;
    iso:hasRelatedControls iso:control-5.15,
        iso:control-5.17,
        iso:control-5.20,
        iso:control-5.3,
        iso:control-5.9,
        iso:control-6.1,
        iso:control-6.2,
        iso:control-6.4,
        iso:control-6.5,
        iso:control-6.6 ;
    iso:hasSecurityDomain iso:Protection ;
    iso:purpose "To ensure only authorized access to information and other associated assets" ;
    dcterms:description "Access rights to information and other associated assets should be provisioned, reviewed, modified and removed in accordance with the organization’s topic-specific policy and rules on access control" ;
    dcterms:identifier "control-5.18" ;
    dcterms:title " Access rights" .

iso:control-5.25 a iso:Control ;
    iso:controlCategory iso:category-5 ;
    iso:correspondsTo iso27002_2013:control-16.1.4 ;
    iso:hasControlType iso:Detective ;
    iso:hasCybersecurityConcept iso:Detect,
        iso:Respond ;
    iso:hasInformationSecurityProperty iso:Availability,
        iso:Confidentiality,
        iso:Integrity ;
    iso:hasOperationalCapability iso:EventManangement ;
    iso:hasSecurityDomain iso:Defence ;
    iso:purpose "To ensure effective categorization and prioritization of information security events" ;
    dcterms:description "The organization should assess information security events and decide if they are to be categorized as information security incidents" ;
    dcterms:identifier "control-5.25" ;
    dcterms:title "Assessment and decision on information security events" .

iso:control-5.28 a iso:Control ;
    iso:controlCategory iso:category-5 ;
    iso:correspondsTo iso27002_2013:control-16.1.7 ;
    iso:hasControlType iso:Corrective,
        iso:Detective ;
    iso:hasCybersecurityConcept iso:Detect,
        iso:Respond ;
    iso:hasInformationSecurityProperty iso:Availability,
        iso:Confidentiality,
        iso:Integrity ;
    iso:hasOperationalCapability iso:EventManangement ;
    iso:hasSecurityDomain iso:Defence ;
    iso:purpose "To ensure a consistent and effective management of evidence related to information security incidents for the purposes of disciplinary and legal action" ;
    dcterms:description "The organization should establish and implement procedures for the identification, collection, acquisition and preservation of information from information security incidents" ;
    dcterms:identifier "control-5.28" ;
    dcterms:title " Collection of evidence" .

iso:control-8.31 a iso:Control ;
    iso:controlCategory iso:category-8 ;
    iso:correspondsTo iso27002_2013:control-12.1.4,
        iso27002_2013:control-14.2.6 ;
    iso:hasControlType iso:Preventive ;
    iso:hasCybersecurityConcept iso:Protect ;
    iso:hasInformationSecurityProperty iso:Availability,
        iso:Confidentiality,
        iso:Integrity ;
    iso:hasOperationalCapability iso:ApplicationSecurity,
        iso:SystemNetworkSecurity ;
    iso:hasRelatedControls iso:control-8.29,
        iso:control-8.33 ;
    iso:hasSecurityDomain iso:Protection ;
    iso:purpose "To protect the production environment and data from compromise by development and test activities" ;
    dcterms:description "Development, testing, and production environments should be separated and secured" ;
    dcterms:identifier "control-8.31" ;
    dcterms:title "Separation of development, test and production environments" .

iso:Governance a iso:OperationalCapability ;
    rdfs:label "Governance" ;
    rdfs:comment "Governance capabilities are capabilities that govern the operation of information systems." .

iso:SupplierSecurity a iso:OperationalCapability ;
    rdfs:label "Supplier and Relationship Security" ;
    rdfs:comment "Supplier security capabilities are capabilities that manage supplier assets." .

iso:control-8.29 a iso:Control ;
    iso:controlCategory iso:category-8 ;
    iso:correspondsTo iso27002_2013:control-14.2.8,
        iso27002_2013:control-14.2.9 ;
    iso:hasControlType iso:Preventive ;
    iso:hasCybersecurityConcept iso:Detect ;
    iso:hasInformationSecurityProperty iso:Availability,
        iso:Confidentiality,
        iso:Integrity ;
    iso:hasOperationalCapability iso:ApplicationSecurity,
        iso:EventManangement,
        iso:SystemNetworkSecurity ;
    iso:hasRelatedControls iso:control-5.20,
        iso:control-5.8,
        iso:control-8.20,
        iso:control-8.23,
        iso:control-8.24,
        iso:control-8.28,
        iso:control-8.29,
        iso:control-8.3,
        iso:control-8.31,
        iso:control-8.5,
        iso:control-8.9 ;
    iso:hasSecurityDomain iso:Protection ;
    iso:purpose "To validate if information security requirements are met when deployed to the production environment" ;
    dcterms:description "Security testing processes should be defined and implemented in the development lifecycle" ;
    dcterms:identifier "control-8.29" ;
    dcterms:title " Security testing in development and acceptance" .

iso:IAM a iso:OperationalCapability ;
    rdfs:label "Identity and Access Management" ;
    rdfs:comment "Identity and access management capabilities are capabilities that manage identities and access." .

iso:Resilience a iso:SecurityDomain ;
    rdfs:label "Resilience and Recovery" ;
    rdfs:comment "Resilience and Recovery domain are domains that manage resilience." .

iso:category-6 a iso:ControlCategory ;
    rdfs:label "People" .

iso:control-5.12 a iso:Control ;
    iso:controlCategory iso:category-5 ;
    iso:correspondsTo iso27002_2013:control-08.2.1 ;
    iso:hasControlType iso:Preventive ;
    iso:hasCybersecurityConcept iso:Identify ;
    iso:hasInformationSecurityProperty iso:Availability,
        iso:Confidentiality,
        iso:Integrity ;
    iso:hasOperationalCapability iso:InformationProtection ;
    iso:hasRelatedControls iso:control-5.15 ;
    iso:hasSecurityDomain iso:Defence,
        iso:Protection ;
    iso:purpose "To ensure identification and understanding of protection needs of information in accordance with its importance to the organization" ;
    dcterms:description "Information should be classified according to the information security needs of the organization based on confidentiality, integrity, availability and relevant interested party requirements" ;
    dcterms:identifier "control-5.12" ;
    dcterms:title " Classification of information" .

iso:control-5.32 a iso:Control ;
    iso:controlCategory iso:category-5 ;
    iso:correspondsTo iso27002_2013:control-18.1.2 ;
    iso:hasControlType iso:Preventive ;
    iso:hasCybersecurityConcept iso:Identify ;
    iso:hasInformationSecurityProperty iso:Availability,
        iso:Confidentiality,
        iso:Integrity ;
    iso:hasOperationalCapability iso:Compliance ;
    iso:hasSecurityDomain iso:GovernanceEcosystem ;
    iso:purpose "To  ensure  compliance  with  legal,  statutory,  regulatory  and  contractual  requirements  related  to intellectual property rights and use of proprietary products" ;
    dcterms:description "Organizations should implement appropriate procedures should be implemented to protect intellectual property rights" ;
    dcterms:identifier "control-5.32" ;
    dcterms:title "Intellectual property rights" .

iso:control-8.24 a iso:Control ;
    iso:controlCategory iso:category-8 ;
    iso:correspondsTo iso27002_2013:control-10.1.1,
        iso27002_2013:control-10.1.2 ;
    iso:hasControlType iso:Preventive ;
    iso:hasCybersecurityConcept iso:Protect ;
    iso:hasInformationSecurityProperty iso:Confidentiality,
        iso:Integrity ;
    iso:hasOperationalCapability iso:SecureConfiguration ;
    iso:hasRelatedControls iso:control-5.22,
        iso:control-5.31,
        iso:control-8.24 ;
    iso:hasSecurityDomain iso:Protection ;
    iso:purpose "To ensure proper and effective use of cryptography to protect the confidentiality, authenticity or integrity of information in compliance with legal, statutory, regulatory or contractual requirements related to cryptography" ;
    dcterms:description "Rules for the effective use of cryptography, including cryptographic key management, should be defined and implemented" ;
    dcterms:identifier "control-8.24" ;
    dcterms:title "Use of cryptography" .

iso:ApplicationSecurity a iso:OperationalCapability ;
    rdfs:label "Application Security" ;
    rdfs:comment "Application security capabilities are capabilities that protect applications." .

iso:Respond a iso:CybersecurityConcept ;
    rdfs:label "Respond" ;
    iso:related d3f:Evict ;
    rdfs:comment "Respond concepts are concepts that respond to information." .

iso:EventManangement a iso:OperationalCapability ;
    rdfs:label "Event Management and Information" ;
    rdfs:comment "Event management capabilities are capabilities that manage events." .

iso:Corrective a iso:ControlType ;
    rdfs:label "Corrective" ;
    rdfs:comment "Corrective controls are controls after an incident." .

iso:InformationProtection a iso:OperationalCapability ;
    rdfs:label "Information Protection" ;
    rdfs:comment "Information protection capabilities are capabilities that protect information." .

iso:Detective a iso:ControlType ;
    rdfs:label "Detective" ;
    rdfs:comment "Detective controls are controls that detect an incident." .

iso:category-7 a iso:ControlCategory ;
    rdfs:label "Physical" .

iso:OperationalCapability a owl:Class,
        skos:Concept ;
    rdfs:label "Operational Capabilities" ;
    rdfs:comment "Operational capabilities correlate controls with the perspective of the practitioners." ;
    skos:prefLabel "Skos Operational Capabilities" .

iso:AssetManagement a iso:OperationalCapability ;
    rdfs:label "Asset Management" ;
    rdfs:comment "Asset management capabilities are capabilities that manage information assets." .

iso:Detect a iso:CybersecurityConcept ;
    rdfs:label "Detect" ;
    iso:related d3f:Detect ;
    rdfs:comment "Detect concepts are concepts that detect information." .

iso:PhysicalSecurity a iso:OperationalCapability ;
    rdfs:label "Physical Security" ;
    rdfs:comment "Physical security capabilities are capabilities that protect physical assets." .

iso:SystemNetworkSecurity a iso:OperationalCapability ;
    rdfs:label "System Network Security" ;
    rdfs:comment "System network security capabilities are capabilities that protect system network assets." .

iso:Identify a iso:CybersecurityConcept ;
    rdfs:label "Identify" ;
    rdfs:comment """
    The Identify Function assists in developing an organizational understanding to managing cybersecurity risk
    to systems, people, assets, data, and capabilities.
    Understanding the business context, the resources that support critical functions,
    and the related cybersecurity risks enables an organization to focus and prioritize its efforts,
    consistent with its risk management strategy and business needs
    """ .

iso:Defence a iso:SecurityDomain ;
    rdfs:label "Defence and Security" ;
    rdfs:comment "Defence and Security domain are domains that protect information." .

iso:GovernanceEcosystem a iso:SecurityDomain ;
    rdfs:label "Governance and Ecosystem" ;
    rdfs:comment "Governance and Ecosystem domain are domains that govern the operation of information systems." .

iso:category-8 a iso:ControlCategory ;
    rdfs:label "Technological" .

iso:category-5 a iso:ControlCategory ;
    rdfs:label "Organizational" .

iso:Protect a iso:CybersecurityConcept ;
    rdfs:label "Protect" ;
    iso:related d3f:Harden,
        d3f:Isolate ;
    rdfs:comment "Protect concepts are concepts that protect information." .

iso:Protection a iso:SecurityDomain ;
    rdfs:label "Protection and Risk" ;
    rdfs:comment "Protection and Risk domain are domains that protect information." .

iso:Integrity a iso:InformationSecurityProperty ;
    rdfs:label "Integrity" ;
    rdfs:comment "Integrity of information." .

iso:Preventive a iso:ControlType ;
    rdfs:label "Preventive" ;
    rdfs:comment "Preventive controls are controls that prevent an incident." .

iso:Availability a iso:InformationSecurityProperty ;
    rdfs:label "Availability" ;
    rdfs:comment "Availability of information." .

iso:Confidentiality a iso:InformationSecurityProperty ;
    rdfs:label "Confidentiality" ;
    rdfs:comment "Confidentiality of information." .

iso:Control a owl:Class,
        skos:Concept ;
    rdfs:label "Control" ;
    rdfs:comment "Controls are the basic building blocks of the ISO 27001 standard." ;
    rdfs:subClassOf [ a owl:Restriction ;
            owl:onProperty iso:purpose ;
            owl:someValuesFrom xsd:string ] .
